format-version: 1.0
date: 27:04:2005 11:00
version: $Revision: 1.3 $
saved-by: pj37
auto-generated-by: DAG-Edit 1.419 rev 3
default-namespace: plant_ontology
remark: This version is based on merging the po_anatomy.obo (ver 1.3 ) and temporal.obo (ver 1.16).

[Term]
id: PO:0000001
name: embryo proper
namespace: plant_structure
def: "The body of the developing embryo attached to the maternal tissue in the ovule by filamentous suspensor." [TAIR:ki]
relationship: part_of PO:0009009

[Term]
id: PO:0000002
name: anther wall
namespace: plant_structure
def: "A multicellular layer with outer epidermis and an inner endothecium." [GR:pj]
relationship: part_of PO:0009070

[Term]
id: PO:0000003
name: whole plant
namespace: plant_structure
def: "The entire plant\, including roots\, shoots and leaves\, at any stage of its life cycle." [TAIR:ki]
comment: This term is so general that it should be avoided whenever possible.
is_a: PO:0009011

[Term]
id: PO:0000004
name: in vitro cell, tissue and organ culture
namespace: plant_structure
def: "Isolated and grown plant protoplast\, cell\, tissue and organ\, involving\, as a common factor\, growth of microbe-free plant material in sterile environment\, such as sterilized nutrient medium in a test tube or petri dish." [TAIR:ki]
is_a: PO:0009011

[Term]
id: PO:0000005
name: cultured cell
namespace: plant_structure
def: "In vitro grown isolated cells and small cell aggregates that proliferate while suspended in liquid sterile medium or spread on a solid agar medium." [TAIR:ki]
comment: In cell cultures\, the cells are no longer organized into tissues.
synonym: "cell suspension" []
is_a: PO:0000004

[Term]
id: PO:0000006
name: cultured protoplast
namespace: plant_structure
def: "In vitro isolated cells from which the entire cell wall has been enzymatically removed." [TAIR:ki]
is_a: PO:0000005

[Term]
id: PO:0000007
name: cultured leaf cell
namespace: plant_structure
def: "In vitro grown isolated cells and small cell aggregates that originated from isolated leaf protoplasts (after they re-established cell wall\, or from callus that was induced from leaf tissue)." [TAIR:ki]
is_a: PO:0000005

[Term]
id: PO:0000008
name: cultured root cell
namespace: plant_structure
def: "In vitro grown isolated cells and small cell aggregates that originated from isolated protoplasts after they re-established cell wall\, or from callus that was induced from segment of root." [TAIR:ki]
is_a: PO:0000005

[Term]
id: PO:0000009
name: cultured callus
namespace: plant_structure
def: "In vitro grown cell aggregates that originated from isolated protoplasts\, cell suspensions\, or from callus that was induced in sterile medium the supplemented by plant growth regulators." [TAIR:ki]
is_a: PO:0000004

[Term]
id: PO:0000010
name: cultured embryo
namespace: plant_structure
def: "In vitro isolated and maintained mature or immature zygotic embryos\, somatic embryos or haploid embryos (derived from male gametophyte)." [TAIR:ki]
is_a: PO:0000004

[Term]
id: PO:0000011
name: somatic embryo
namespace: plant_structure
def: "An embryo arising from previously differentiated somatic cells in vitro\, rather than from fused haploid gametes\, i.e.\, zygote." [TAIR:ki]
is_a: PO:0000010

[Term]
id: PO:0000012
name: apical hook
namespace: plant_structure
def: "Hook-like structure which develops at the apical part of the hypocotyl in dark-grown seedlings in dicots. " [TAIR:ki]
synonym: "hypocotyl hook" []
relationship: part_of PO:0006341

[Term]
id: PO:0000013
name: cauline leaf
namespace: plant_structure
def: "Leaf or pairs/whorls of leaves borne on the stem. " [TAIR:ki]
comment: In Arabidopsis\, refers to the leaves that are borne on the elongated inflorescence branches.
is_a: PO:0009025

[Term]
id: PO:0000014
name: rosette leaf
namespace: plant_structure
def: "One of multiple leaves borne in a rosette - a group of leaves\, generally borne at the base of the plant\, that are separated by very short internodes." [TAIR:ki]
comment: n Arabidopsis\, vegetative development is characterized by the production of the rosette leaves.
is_a: PO:0009025

[Term]
id: PO:0000015
name: cotyledon primordium
namespace: plant_structure
def: "An organized group of cells that will differentiate into a cotyledon. " [TAIR:ki]
is_a: PO:0020030

[Term]
id: PO:0000016
name: lateral root primordium
namespace: plant_structure
def: "An organized group of cells derived from the root pericycle that will differentiate into a new root. " [TAIR:ki]
is_a: PO:0020121

[Term]
id: PO:0000017
name: leaf primordium
namespace: plant_structure
def: "An organized group of cells that will differentiate into leaf that are emerging as an outgrowth in the shoot apex (flanking the meristem). " [TAIR:ki]
is_a: PO:0009025
relationship: part_of PO:0000037

[Term]
id: PO:0000018
name: ovule primordium
namespace: plant_structure
def: "An organized group of cells that will differentiate into ovule. " [TAIR:ki]
is_a: PO:0020003

[Term]
id: PO:0000019
name: gynoecium primordium
namespace: plant_structure
def: "The very first appearance of gynoecium. " [TAIR:ki]
is_a: PO:0009062

[Term]
id: PO:0000020
name: starch sheath cell
namespace: plant_structure
def: "OBSOLETE. Cells characterized by conspicuous and rather stable accumulation of starch." [ISBN:044174520]
comment: Uninformative definition
is_obsolete: true

[Term]
id: PO:0000021
name: petal primordium
namespace: plant_structure
def: "The very first appearance of a petal. " [TAIR:ki]
is_a: PO:0009032

[Term]
id: PO:0000022
name: cuticle
namespace: plant_structure
def: "A layer of fatty material\, cutin\, rather impervious to water\, located on the outer walls of epidermal cells." [ISBN:0471245208]
is_a: PO:0004013

[Term]
id: PO:0000023
name: casparian strip
namespace: plant_structure
def: "A band-like wall formation within primary walls that contains suberin and lignin; typical of endodermal cells in roots\, in which it occurs in radial and transverse anticlinal walls." [ISBN:0471245208]
relationship: part_of PO:0005059

[Term]
id: PO:0000024
name: filiform apparatus
namespace: plant_structure
def: "A complex of cell wall invaginations in a synergid cell similar to those in transfer cells." [ISBN:0471245208]
relationship: part_of PO:0000191

[Term]
id: PO:0000025
name: root tip
namespace: plant_structure
def: "The portion of the root including the meristem and root cap." [ISBN:ki]
relationship: part_of PO:0009005

[Term]
id: PO:0000026
name: primary root tip
namespace: plant_structure
def: "The portion of the primary root including the meristem and root cap." [TAIR:ki]
is_a: PO:0000025
relationship: part_of PO:0020127

[Term]
id: PO:0000027
name: lateral root tip
namespace: plant_structure
def: "The portion of the lateral root including the meristem and root cap." [TAIR:ki]
is_a: PO:0000025
relationship: part_of PO:0020121

[Term]
id: PO:0000028
name: pollen tube tip
namespace: plant_structure
def: "Tip portion of the pollen tube that is rapidly growing." [TAIR:ki]
is_a: PO:0006345

[Term]
id: PO:0000029
name: root hair tip
namespace: plant_structure
def: "Tip portion of an outgrowth of a root epidermal cell." [TAIR:ki]
relationship: part_of PO:0000256

[Term]
id: PO:0000030
name: septum
namespace: plant_structure
def: "A thin partition or membrane that divides a cavity or a mass of tissue\, e.g.\, in anther\, ovary or fruit." [APWeb:Glossary]
relationship: part_of PO:0009001
relationship: part_of PO:0009030
relationship: part_of PO:0009066

[Term]
id: PO:0000031
name: lenticel
namespace: plant_structure
def: "Loosely-packed mass of cork cells occurring especially in the young stem\, bark or even leaf of a plant\, visible on the surface as a raised\, often powdery-appearing spot\, through which gaseous exchange occurs." [ISBN: 0471245208]
relationship: part_of PO:0009047

[Term]
id: PO:0000032
name: tetrad of microspores
namespace: plant_structure
def: "A group of four haploid cells that remained joined together shortly after meiosis. Each cell will give rise to the male gametophyte." [TAIR:ki]
relationship: develops_from PO:0020047

[Term]
id: PO:0000033
name: valve
namespace: plant_structure
def: " Portion of an organ that is fragmented; in capsule\, theportions into which the pericarp splits at maturity." [APWeb:Glossary]
relationship: part_of PO:0009001

[Term]
id: PO:0000034
name: vascular system
namespace: plant_structure
def: "Total of the vascular tissues in their specific arrangement in a plant or plant organ." [ISBN:0471245208]
is_a: PO:0009007

[Term]
id: PO:0000035
name: cotyledon vascular system
namespace: plant_structure
def: "Vascular system of the leaf." [ISBN:ki]
is_a: PO:0000034
relationship: part_of PO:0020030

[Term]
id: PO:0000036
name: leaf vascular system
namespace: plant_structure
def: "Vascular system of the leaf." [ISBN:ki]
is_a: PO:0000034
relationship: part_of PO:0009025

[Term]
id: PO:0000037
name: shoot apex
namespace: plant_structure
def: "The topmost part of the shoot\, situated at the distal extremity of the shoot axis\, consists of apical meristem the youngest leaf primordia." [TAIR:ki]
relationship: part_of PO:0009006

[Term]
id: PO:0000066
name: epithem cell
namespace: plant_structure
def: "Cell of the mesophyll of a hydathode found between the xylem endings and the epidermis." [PMID:12662305, ISBN:0471245208]
comment: Proposed to be involved in the retrieval of solutes from the xylem sap.
is_a: PO:0009002
relationship: part_of PO:0005660

[Term]
id: PO:0000070
name: meristemoid
namespace: plant_structure
def: "A cell or a group of cells constituting an active locus of meristematic activity in a tissue composed of somewhat older\, differentiating cells." [PO:syr, ISBN:0471245208]
is_a: PO:0009002

[Term]
id: PO:0000071
name: companion cell
namespace: plant_structure
def: "A specialized parenchyma cell associated with a sieve-tube member in angiosperm phloem and arising from the same mother cell as the sieve-tube member." [ISBN:0879015322]
relationship: part_of PO:0005043
relationship: part_of PO:0006075

[Term]
id: PO:0000074
name: parenchyma cell
namespace: plant_structure
def: "A relatively unspecialized cell with a nucleate protoplast." [ISBN:0471245208]
is_a: PO:0009002
relationship: part_of PO:0005421

[Term]
id: PO:0000075
name: collenchyma cell
namespace: plant_structure
def: "Elongated living cells with unevenly thickened nonlignified primary walls." [ISBN:0471245208]
is_a: PO:0009002
relationship: part_of PO:0005423

[Term]
id: PO:0000076
name: chlorenchyma cell
namespace: plant_structure
def: "Parenchyma cell containing chloroplasts; a component of leaf mesophyll and other green parenchyma tissue." [ISBN:0471245208]
is_a: PO:0000074
relationship: part_of PO:0005426

[Term]
id: PO:0000077
name: sclerenchyma cell
namespace: plant_structure
def: "Usually dead cell variable in form and size\, with more or less thick\, often lignified\, secondary walls." [ISBN:0471245208]
is_a: PO:0009002
relationship: part_of PO:0005427

[Term]
id: PO:0000078
name: transfer cell
namespace: plant_structure
def: "A cell with wall ingrowths (or invaginations) that increase the surface of the plasmalemma. " [ISBN:0471245208]
comment: Appears to be specialized for short-distance transfer of solutes.
is_a: PO:0009002

[Term]
id: PO:0000079
name: fusiform initial
alt_id: PO:0000275
namespace: plant_structure
def: "An elongated cell with approximately wedge-shaped ends\, found in the vascular cambium\, which gives rise to the elements of the axial system in the secondary vascular tissues." [ISBN:0471245208]
synonym: "xylem initial" []
synonym: "xylem mother cell" []
is_a: PO:0000295

[Term]
id: PO:0000081
name: axial cell
namespace: plant_structure
def: "A vascular cell derived from the fusiform cambial initial and oriented with its longest diameter parallel with the main axis of stem or root." [ISBN:0471245208]
comment: These cells make up the axial system\, also known as vertical or longitudinal system.
is_a: PO:0009002
relationship: develops_from PO:0000079

[Term]
id: PO:0000082
name: ray initial
namespace: plant_structure
def: "A cell in the vascular cambium that gives rise to ray cells of the secondary xylem and secondary phloem." [ISBN:0471245208]
is_a: PO:0000295

[Term]
id: PO:0000084
name: sperm cell
alt_id: PO:0020098
namespace: plant_structure
def: "A haploid male reproductive cell (usually two in number); during double fertilization\, one fuses with the female gamete (egg cell) to produce a zygote while another fusses with the two polar nuclei of the central cell to give rise to endosperm." [TAIR:ki]
synonym: "sperm nucleus" []
is_a: PO:0009002
relationship: develops_from PO:0020097
relationship: part_of PO:0020091

[Term]
id: PO:0000112
name: stem epidermis
namespace: plant_structure
def: "Epidermal layer of the stem." [TAIR:lr]
synonym: "culm epidermis" []
is_a: PO:0006035
relationship: part_of PO:0009047

[Term]
id: PO:0000115
name: socket cell
namespace: plant_structure
def: "Cell that surrounds a trichome and provides its support." [ISBN:0471245208]
is_a: PO:0004013
relationship: develops_from PO:0000349

[Term]
id: PO:0000146
name: abscission zone
namespace: plant_structure
def: "Zone at base of leaf\, flower\, fruit\, or other plant part that contains an abscission (or separation) layer and a protective layer\, both involved in the abscission of the plant part." [ISBN:047124529]
synonym: "abscission layer" []
is_a: PO:0009007

[Term]
id: PO:0000191
name: synergid
namespace: plant_structure
def: "Cell\, usually two in number\, in the micropylar end of the embryo sac of angiosperms associated with the egg in the egg apparatus." [ISBN:047125208, TAIR:ki]
is_a: PO:0009002
relationship: part_of PO:0020096

[Term]
id: PO:0000198
name: free nuclear endosperm
namespace: plant_structure
def: "Endosperm in which at least the first karyokinesis is not followed by cytokinesis." [ISBN:0080374913, ISBN:0471245194]
synonym: "cenocytic endosperm" []
synonym: "coenocytic endosperm" []
synonym: "nuclear endosperm" []
is_a: PO:0009089

[Term]
id: PO:0000199
name: cellular endosperm
namespace: plant_structure
def: "Endosperm in which the first karyokinesis event is accompanied by cytokinesis." [ISBN:0080374913, ISBN:0471245194]
is_a: PO:0009089

[Term]
id: PO:0000200
name: micropylar endosperm
namespace: plant_structure
def: "The region of the endosperm closest to the micropyle of the seed." [TAIR:lr]
synonym: "micropylar region" []
relationship: part_of PO:0009089

[Term]
id: PO:0000201
name: chalazal cyst
namespace: plant_structure
def: "The part of the endosperm nearest the chalazal region of the ovule and forming a cyst-like structure." [TAIR:lr, ISBN:047124529]
comment: Not in current literature. More like an attribute.
synonym: "chalazal endosperm cyst" []
relationship: part_of PO:0009089

[Term]
id: PO:0000207
name: nectary epidermis
namespace: plant_structure
def: "The epidermal layer of the nectary." [TAIR:lr]
is_a: PO:0006035
relationship: part_of PO:0009035

[Term]
id: PO:0000223
name: stem cortex
namespace: plant_structure
def: "The primary tissue located between the vascular system and the epidermis of the root." [GR:pj, ISBN:047124529]
is_a: PO:0005708
relationship: part_of PO:0009047

[Term]
id: PO:0000224
name: central zone
namespace: plant_structure
def: "An area of densely packed cells in the shoot apex that divide infrequently." [TAIR:lr, ISBN:0521288959]
comment: Functions as a population of stem cells that replenishes the meristem.
synonym: "central initiation zone" []
relationship: part_of PO:0020148

[Term]
id: PO:0000225
name: peripheral zone
namespace: plant_structure
def: "Organogenic region of the meristem\,  characterized by higher rates of cell division." [TAIR:lr, ISBN:0521288959]
synonym: "peripheral meristem" []
relationship: part_of PO:0020148

[Term]
id: PO:0000226
name: rib zone
namespace: plant_structure
def: "The region of the meristem that lies below the central zone and is flanked by the peripheral zone" [ISBN:0521288959, TAIR:lr]
synonym: "file meristem" []
relationship: part_of PO:0020148

[Term]
id: PO:0000229
name: floral meristem
namespace: plant_structure
def: "Meristem that gives rise to the floral organs." [GR:pj]
synonym: "floral apical meristem" []
is_a: PO:0020148
relationship: part_of PO:0009049

[Term]
id: PO:0000230
name: inflorescence meristem
namespace: plant_structure
def: "Meristem that gives rise to the inflorescence." [GR:pj]
is_a: PO:0020148
relationship: part_of PO:0009049

[Term]
id: PO:0000232
name: axillary bud meristem
namespace: plant_structure
def: "Meristems formed in the axil of the leaf." [TAIR:lr]
synonym: "axillary meristem" []
is_a: PO:0006079

[Term]
id: PO:0000244
name: functional megaspore
namespace: plant_structure
def: "The megaspore(s) that forms the embryo sac." [TAIR:lr]
is_a: PO:0020019

[Term]
id: PO:0000245
name: degenerate megaspore
namespace: plant_structure
def: "In monosporic and bisporic megasporogenesis\: the megaspore(s) that would not participate in megagametogenesis." [TAIR:lr]
is_a: PO:0020019

[Term]
id: PO:0000252
name: endodermis
alt_id: PO:0006064
namespace: plant_structure
def: "The innermost layer of the cortex in roots and stems of seed plants. The layer of tissue forming a sheath around the vascular region and often having a casparian strip in its anticlinal walls; it may have secondary walls later." [ISBN:047124529]
synonym: "endodermoid" []
relationship: part_of PO:0005708

[Term]
id: PO:0000256
name: root hair
namespace: plant_structure
def: "A root epidermal cell with a simple extension that is concerned with absorption of soil solution." [ISBN:0471245208]
is_a: PO:0004013
relationship: develops_from PO:0000262
relationship: part_of PO:0006036

[Term]
id: PO:0000258
name: root cortex
alt_id: PO:0003010
namespace: plant_structure
def: "The primary tissue located between the vascular system and the epidermis of the root." [ISBN:047125208, GR:pj]
comment: In dicots and gymnosperms\, the cortex consists of mainly parenchyma cells. In monocots sclerenchyma develops in addition to parenchyma.
is_a: PO:0005708
relationship: part_of PO:0009005

[Term]
id: PO:0000262
name: trichoblast
namespace: plant_structure
def: "The smaller cell produced by the asymmetric division of a root epidermal cell that gives rise to a root hair." [ISBN:0471245208]
synonym: "hair cell" []
is_a: PO:0004013
relationship: develops_from PO:0000349
relationship: part_of PO:0006036

[Term]
id: PO:0000263
name: atrichoblast
namespace: plant_structure
def: "A cell formed after asymmetric division of root epidermal cell that does not give rise to a root hair." [ISBN:0387987819]
synonym: "non-hair cell" []
is_a: PO:0004013
relationship: develops_from PO:0000349
relationship: part_of PO:0006036

[Term]
id: PO:0000272
name: protoxylem
namespace: plant_structure
def: "The first formed elements of the primary xylem." [ISBN:047125208]
relationship: part_of PO:0005849

[Term]
id: PO:0000273
name: xylem element
namespace: plant_structure
def: "A cell making up xylem tissue." [ISBN:0471245208]
is_a: PO:0000081
is_a: PO:0009002

[Term]
id: PO:0000274
name: xylem fiber cell
namespace: plant_structure
def: "A fiber in xylem." [ISBN:0471245208]
comment: Two types are recognized in the secondary xylem\: fiber tracheids and libriform fibers.
is_a: PO:0000273
relationship: part_of PO:0005848

[Term]
id: PO:0000282
name: trichome
namespace: plant_structure
def: "An outgrowth from the epidermis varying in size and complexity and including hairs\, scales\, and other structures; may be glandular." [ISBN:0471245208, TAIR:ki]
comment: In Arabidopsis\, patterning of trichome development is not random but does not appear to be lineage-based like stomata.
is_a: PO:0004013

[Term]
id: PO:0000283
name: idioblast
namespace: plant_structure
def: "OBSOLETE. A cell in a tissue that markedly differs in form\, size\, or contents from other cells in the same tissue." [ISBN:0471245208]
comment: This term was made obsolete because its a kind of attribute for a cell type.
is_obsolete: true

[Term]
id: PO:0000284
name: subsidiary cell
alt_id: PO:0000296
namespace: plant_structure
def: "An epidermal cell associated with a stoma and at least morphologically distinguishable from the other epidermal cells." [ISBN:047124520]
synonym: "accessory cell" []
is_a: PO:0004013
relationship: part_of PO:0002000

[Term]
id: PO:0000289
name: sieve tube member
alt_id: PO:0000286
namespace: plant_structure
def: "One of the series of cells that make up a sieve tube; it shows a more or less pronounced differentiation between sieve plates (wide pores) and lateral sieve areas (narrow pores)." [ISBN:0471245208]
comment: Also sieve tube element and the obsolete sieve tube segment.
synonym: "sieve element" []
synonym: "sieve tube element" []
is_a: PO:0009002
relationship: part_of PO:0005043
relationship: part_of PO:0006075

[Term]
id: PO:0000290
name: tracheary element
namespace: plant_structure
def: "General term for any water conducting cell\, tracheid or vessel member." [ISBN:0471245208]
is_a: PO:0000273
is_a: PO:0009002
relationship: part_of PO:0005848
relationship: part_of PO:0005849

[Term]
id: PO:0000293
name: guard cell
namespace: plant_structure
def: "One of a pair of cells flanking the stomatal pore." [ISBN:0471245208]
comment: They cause the opening and closing of the pore by changes in turgor.
is_a: PO:0004013
relationship: develops_from PO:0000351
relationship: part_of PO:0002000

[Term]
id: PO:0000295
name: cambial initial
alt_id: PO:0000080
namespace: plant_structure
def: "Cell localized in the vascular cambium or phellogen that their periclinal divisions can contribute cells either to the outside or to the inside of the axis; in vascular cambium\, classified into fusiform initials (source of axial cells of xylem and phloem) and ray initials (source of the ray cells)." [ISBN:0471245208]
synonym: "cambial cell" []
is_a: PO:0004011
relationship: part_of PO:0005598

[Term]
id: PO:0000301
name: tracheid
namespace: plant_structure
def: "In the xylem\, a dead elongated water-conducting cell in which at least the middle lamella of the end walls remains intact." [APWeb:Glossary]
is_a: PO:0000290

[Term]
id: PO:0000309
name: nectary parenchyma
namespace: plant_structure
def: "Relatively unspecialized tissue present in the nectary." [TAIR:lr]
is_a: PO:0005421

[Term]
id: PO:0000332
name: pavement cell
namespace: plant_structure
def: "Epidermal cell with characteristic sinuous anticlinal cell walls that overall give a jigsaw like appearance to the leaf epidermis." [ISBN:087694289]
is_a: PO:0004013
relationship: develops_from PO:0000349
relationship: part_of PO:0006018
relationship: part_of PO:0006019

[Term]
id: PO:0000349
name: epidermal initial
namespace: plant_structure
def: "A relatively unspecialized cell that will give rise to specialized cell types of the epidermis." [TAIR:lr]
is_a: PO:0004011

[Term]
id: PO:0000351
name: guard mother cell
namespace: plant_structure
def: "Epidermal cell that divides to produce the guard cells." [ISBN:0471245208]
is_a: PO:0004013
relationship: develops_from PO:0000070
relationship: develops_from PO:0000349

[Term]
id: PO:0000352
name: myrosin cell
namespace: plant_structure
def: "Cell containing glucosinolates (\"mustard oil glucosides\") and myrosinases\, enzymes hydrolyzing the glucosinolates." [ISBN:0471245208]
is_a: PO:0009002

[Term]
id: PO:0000353
name: passage cell
namespace: plant_structure
def: "Cell in exodermis or endodermis that remains thin walled when the associated cells develop thick secondary walls." [ISBN:0471245208]
is_a: PO:0009002

[Term]
id: PO:0000355
name: fiber tracheid
namespace: plant_structure
def: "A fiber-like tracheid in the secondary xylem; commonly thick walled\, with pointed ends and bordered pits that have lenticular to slit-like apertures." [ISBN:0471245208]
is_a: PO:0000274

[Term]
id: PO:0000372
name: metaxylem
namespace: plant_structure
def: "Part of the primary xylem that differentiates after the protoxylem and before the secondary xylem\, if any of the latter is formed." [ISBN:047125208]
relationship: part_of PO:0005849

[Term]
id: PO:0000373
name: mucilage cell
namespace: plant_structure
def: "OBSOLETE. Cell containing mucilages or gums or similar carbohydrate material characterized by the property of swelling in water." [ISBN:0471245208]
comment: Functional term
is_obsolete: true

[Term]
id: PO:0000400
name: phloem initial
namespace: plant_structure
def: "A cambial cell that is the source of one or more cells that differentiate into phloem elements." [ISBN:0471245208]
comment: Phloem islands can be formed in the middle of the xylem.
synonym: "phloem mother cell" []
is_a: PO:0000295
relationship: part_of PO:0005043

[Term]
id: PO:0000423
name: zygote
namespace: plant_structure
def: "Diploid cell produced by the fusion of sperm cell nucleus and egg cell." [TAIR:ki]
is_a: PO:0009002

[Term]
id: PO:0000431
name: megasporocyte
namespace: plant_structure
def: "A diploid (2n) cell that undergoes meiosis and produces four haploid (1n) megaspores." [ISBN:0471245208]
synonym: "archesporial cell" []
synonym: "megaspore mother cell" []
is_a: PO:0006204
relationship: part_of PO:0020020

[Term]
id: PO:0002000
name: stomatal complex
namespace: plant_structure
def: "An opening in the epidermis of leaves and stems bordered by two guard cells and serving in gas exchange." [ISBN:0471245208]
relationship: part_of PO:0006018
relationship: part_of PO:0006019

[Term]
id: PO:0002001
name: papillae
namespace: plant_structure
def: "A soft protuberance on an epidermal cell of the stigma." [ISBN:0471245208]
relationship: part_of PO:0006061

[Term]
id: PO:0002002
name: basal cell
namespace: plant_structure
def: "The lowermost cell formed after the first division of the zygote." [ISBN:0471245208]
is_a: PO:0009002
relationship: develops_from PO:0000423
relationship: part_of PO:0009009

[Term]
id: PO:0002003
name: vessel member
namespace: plant_structure
def: "One of the cellular components of a vessel\, a dead cell with the wall between adjacent members being variously perforated and the walls that persist variously thickened. " [ISBN:0471245208]
synonym: "vessel element" []
synonym: "vessel segment" []
is_a: PO:0000290

[Term]
id: PO:0003000
name: transition zone
namespace: plant_structure
def: "A region of the root between the meristem and the region of rapid elongation in which isodiametric growth (cell expansion) occurs." [Agricola:IND23249552, http://search.epnet.com/direct.asp?an=IND23249552&db=agr]
relationship: part_of PO:0009005

[Term]
id: PO:0003003
name: primary root elongation zone
namespace: plant_structure
def: "A zone of small\, densely cytoplasmic cells that are dividing and expanding in size located behind the zone of cell division in the primary root." [TAIR:ki]
is_a: PO:0020125
relationship: part_of PO:0020127

[Term]
id: PO:0003004
name: haustorial root
namespace: plant_structure
def: "OBSOLETE. The root of particular parasitic plants that becomes cemented to the host axis and intrudes into the tissues of the host." [http://www.botgard.ucla.edu/html/botanytextbooks/generalbotany/typesofroots/]
comment: Term is specific for parasitic plants only.
is_obsolete: true

[Term]
id: PO:0003005
name: nodal root
alt_id: PO:0003008
alt_id: PO:0003009
namespace: plant_structure
def: "An adventitious root that forms at a node. " [http://www.botgard.ucla.edu/html/botanytextbooks/generalbotany/typesofroots/]
synonym: "crown root" []
synonym: "seminal root" []
is_a: PO:0020129

[Term]
id: PO:0003011
name: root vascular system
namespace: plant_structure
def: "Total of the vascular tissues in their specific arrangements in the root." [TAIR:ki, ISBN:0471245208]
comment: This term was brought back from OBSOLETE node (original reason for OBSOLETE\: synonym of term stele). Since stele encompasses both\, vascular system and the pith\, in roots with pith\, vascular system and stele are not synonymous.
is_a: PO:0000034
relationship: part_of PO:0020124

[Term]
id: PO:0003014
name: lateral root elongation zone
namespace: plant_structure
def: "The portion of the lateral root located behind the zone of cell division that includes small\, densely cytoplasmic cells that are dividing and expanding in size." [TAIR:ki]
is_a: PO:0020125
relationship: part_of PO:0020121

[Term]
id: PO:0003015
name: primary root differentiation zone
namespace: plant_structure
def: "A zone of cells that are differentiating into their final form and function located behind the elongation zone of the portion of the primary root." [TAIR:ki]
is_a: PO:0020135
relationship: part_of PO:0020127

[Term]
id: PO:0003016
name: lateral root differentiation zone
namespace: plant_structure
def: "The portion of the lateral root located behind the elongation zone containing cells that are differentiating into their final form and function." [TAIR:ki]
is_a: PO:0020135
relationship: part_of PO:0020121

[Term]
id: PO:0003017
name: root cap of the primary root
namespace: plant_structure
def: "A group of cells that covers the apical meristem of the primary root." [TAIR:ki]
is_a: PO:0020123
relationship: part_of PO:0000026

[Term]
id: PO:0003018
name: root cap of the lateral root
namespace: plant_structure
def: "A group of cells that covers the apical meristem of the lateral root." [TAIR:ki]
is_a: PO:0020123
relationship: part_of PO:0000027

[Term]
id: PO:0003019
name: central root cap of the lateral root
namespace: plant_structure
def: "The central part of a root cap of a lateral root in which the cells are arranged in longitudinal files." [TAIR:ki]
is_a: PO:0020130
relationship: part_of PO:0003018

[Term]
id: PO:0003020
name: lateral root cap of the lateral root
namespace: plant_structure
def: "In the lateral root\, the part of the root cap that is parallel to the sides of the axis." [TAIR:ki]
is_a: PO:0020131
relationship: part_of PO:0003018

[Term]
id: PO:0003021
name: central root cap of the primary root
namespace: plant_structure
def: "The central part of a root cap of the primary root in which the cells are arranged in longitudinal files." [TAIR:ki]
is_a: PO:0020130
relationship: part_of PO:0003017

[Term]
id: PO:0003022
name: lateral root cap of the primary root
namespace: plant_structure
def: "In the primary root\, the part of the root cap that is parallel to the sides of the axis." [TAIR:ki]
is_a: PO:0020131
relationship: part_of PO:0003017

[Term]
id: PO:0003023
name: nodule
namespace: plant_structure
def: "Enlargement or swelling on the roots of plants\, particularly in the Fabaceae\, inhabited by nitrogen-fixing bacteria." [ISBN:0471245208 ""]
relationship: part_of PO:0009005

[Term]
id: PO:0003024
name: stolon
namespace: plant_structure
def: "A slender\, prostrate or trailing above-ground stem\nwhich produces roots and sometimes erect shoots at its nodes." [APWeb:Glossary]
synonym: "runner" []
is_a: PO:0009006

[Term]
id: PO:0004000
name: apical cell
namespace: plant_structure
def: "The uppermost cell formed after the first division of the zygote." [ISBN:0471245208]
is_a: PO:0009002
relationship: develops_from PO:0000423
relationship: part_of PO:0009009

[Term]
id: PO:0004001
name: bulliform cell
namespace: plant_structure
def: "An enlarged more or less thin-walled epidermal cell present\, with other similar cells\, in longitudinal rows in leaves of monocots." [ISBN:0471245208]
comment: Also called motor cell because of its presumed participation in the mechanism of rolling and unrolling of leaves.
synonym: "motor cell" []
is_a: PO:0004013
relationship: part_of PO:0006016

[Term]
id: PO:0004002
name: contact cell
namespace: plant_structure
def: "OBSOLETE. An axial parenchyma or a ray cell physiologically associated with a tracheary element. Also a cell next to a stoma." [ISBN:0471245208]
comment: Not used in current plant literature.
is_obsolete: true

[Term]
id: PO:0004003
name: cork cell
alt_id: PO:0005049
namespace: plant_structure
def: "A phellem cell derived from cork cambium\, nonliving at maturity\, and having suberized walls. " [ISBN:0471245208]
comment: Protective in function because the walls are highly impervious to water.
synonym: "cork" []
synonym: "phellem" []
is_a: PO:0009002
relationship: develops_from PO:0005599

[Term]
id: PO:0004004
name: epithelium cell
namespace: plant_structure
def: "OBSOLETE. A compact layer of cells\, often secretory in function\, covering a free surface or lining a cavity." [ISBN:0471245208]
comment: Functional term
is_obsolete: true

[Term]
id: PO:0004005
name: laticiferous cell
namespace: plant_structure
def: "OBSOLETE. A specialized cells or ducts resembling vessels; they form branched networks of latex-secreting cells in the phloem and other parts of plants." [http://academic.kellogg.edu/herbrandsonc/bio111/glossary/glossary.htm]
comment: Obsoleted\: Too general definition of the term. Replaced by two terms\: non-articulated laticifer cell and articulated laticifer cell.
is_obsolete: true

[Term]
id: PO:0004006
name: mesophyll cell
namespace: plant_structure
def: "A Cell that constitutes leaf mesophyll." [TAIR:ki]
is_a: PO:0000076
relationship: part_of PO:0006070

[Term]
id: PO:0004007
name: phelloid cell
namespace: plant_structure
def: "OBSOLETE.  A cell within the phellem (cork) but distinct from the cork cell in having no suberin in its walls." [ISBN:0471245208]
comment: Not used in current plant literature. Confusing definition.
is_obsolete: true

[Term]
id: PO:0004008
name: photosynthetic cell
namespace: plant_structure
def: "OBSOLETE. A chloroplast-containing cell engaged in photosynthesis." [ISBN:0471245208]
comment: Functional characterization is not part of the criteria.
is_obsolete: true

[Term]
id: PO:0004009
name: sillica cell
namespace: plant_structure
def: "Cells with deposits of silica in them." [ISBN:0471245208]
comment: One of two types of short cells in the epidermis of grasses.
is_a: PO:0004013

[Term]
id: PO:0004010
name: meristematic cell
namespace: plant_structure
def: "A cell synthesizing protoplasm and producing new cells by division and with only a primary cell wall." [ISBN:0471245208]
is_a: PO:0009002
relationship: part_of PO:0009013

[Term]
id: PO:0004011
name: initial cell
namespace: plant_structure
def: "Cell in a meristem that by division gives rise to two cells one of which remains in the meristem\, the other is added to the plant body." [ISBN:0471245208]
is_a: PO:0004010

[Term]
id: PO:0004012
name: secretory cell
namespace: plant_structure
def: "OBSOLETE. Cell that produces secreted substances." [TAIR:ki]
comment: This is a functional term.
is_obsolete: true

[Term]
id: PO:0004013
name: epidermal cell
namespace: plant_structure
def: "Cell that constitutes dermal tissue." [TAIR:ki]
is_a: PO:0009002
relationship: part_of PO:0005679

[Term]
id: PO:0005039
name: primary thickening meristem
namespace: plant_structure
def: "A meristem derived directly from the shoot apical meristem and responsible for the primary increase in thickness of the shoot axis." [ISSN:0669014893]
comment: May appear as a distinct mantle like zone. Often found in monocotyledons
relationship: develops_from PO:0000225
relationship: part_of PO:0020148

[Term]
id: PO:0005040
name: root pith
namespace: plant_structure
def: "Non-vascular tissue in the center of root." [ISBN:0080280307]
is_a: PO:0006109
relationship: part_of PO:0020124

[Term]
id: PO:0005041
name: stem pith
namespace: plant_structure
def: "Non-vascular tissue in the center of stem." [ISBN:0080280307]
is_a: PO:0006109
relationship: part_of PO:0009047

[Term]
id: PO:0005043
name: secondary phloem
namespace: plant_structure
def: "The phloem tissue formed by the activity of the vascular cambium." [ISBN:0122151704]
comment: Part of the bark.
is_a: PO:0005417

[Term]
id: PO:0005046
name: periderm
namespace: plant_structure
def: "Secondary protective tissue that replaces the epidermis in stems and root\, rarely in other organs. " [ISBN:047124529, GR:pj]
is_a: PO:0009014

[Term]
id: PO:0005047
name: root periderm
namespace: plant_structure
def: "Secondary protective tissue that replaces the epidermis in root." [GR:pj]
is_a: PO:0005046
relationship: part_of PO:0009005

[Term]
id: PO:0005048
name: stem periderm
namespace: plant_structure
def: "Secondary protective tissue that replaces the epidermis in stem." [GR:pj]
is_a: PO:0005046
relationship: part_of PO:0009047

[Term]
id: PO:0005050
name: phelloderm
namespace: plant_structure
def: "A tissue often resembling cortical parenchyma produced centripetally by the cork cambium." [ISBN:0080374913]
relationship: develops_from PO:0005599
relationship: part_of PO:0005048

[Term]
id: PO:0005051
name: hypodermis
namespace: plant_structure
def: "A layer or layers of cells beneath the epidermis that is distinct in appearance from adjacent tissues. It is the outermost layer or layers of cells of the cortex." [ISBN:0080374913, GR:pj]
relationship: part_of PO:0005708

[Term]
id: PO:0005052
name: callus
namespace: plant_structure
def: "A tissue formed as a result of wounding\, or a tissue developing in a tissue culture." [GR:pj]
is_a: PO:0005421

[Term]
id: PO:0005053
name: laticifer
namespace: plant_structure
def: "A secretory structure that produces latex." [ISBN:0080374913]
is_a: PO:0005656
is_a: PO:0009002

[Term]
id: PO:0005057
name: stem hypodermis
namespace: plant_structure
def: "A layer or layers of cells beneath the stem epidermis distinct in appearance from adjacent tissues." [GR:pj, ISBN:0080374913]
is_a: PO:0005051
relationship: part_of PO:0000223
relationship: part_of PO:0009047

[Term]
id: PO:0005058
name: stem endodermis
namespace: plant_structure
def: "The innermost layer of cortex in the stem of seed plants." [GR:pj]
is_a: PO:0000252
relationship: part_of PO:0000223
relationship: part_of PO:0009047

[Term]
id: PO:0005059
name: root endodermis
namespace: plant_structure
def: "The innermost layer of the cortex in roots of  seed plants." [GR:pj]
is_a: PO:0000252
relationship: part_of PO:0000258

[Term]
id: PO:0005060
name: leaf endodermis
namespace: plant_structure
def: "The layer of tissue forming a sheath around the vascular region in a leaf." [GR:pj]
comment: Often found in the leaf of Gymnosperms and elsewhere.
is_a: PO:0000252
relationship: part_of PO:0009025

[Term]
id: PO:0005349
name: schizo-lysigenous aerenchyma
namespace: plant_structure
def: "OBSOLETE. Aerenchyma\, originating by a combination of two processes\, separation and degradation of cell walls." [ISBN:0080374913, GR:pj]
comment: The term was made obsolete because schizo-lysigenous form is an attribute of regular aerenchyma.
is_obsolete: true

[Term]
id: PO:0005352
name: xylem
namespace: plant_structure
def: "vascular tissue whose principal function is the upward translocation of water and solutes." [GR:pj]
comment: See also primary xylem and secondary xylem.
is_a: PO:0009015

[Term]
id: PO:0005360
name: aleurone layer
namespace: plant_structure
def: "The outermost endosperm tissue of the seeds\, its cells being characterized by presence of protein bodies containing seed storage proteins." [ISBN:0080374913, GR:pj]
relationship: part_of PO:0009089

[Term]
id: PO:0005415
name: endosperm parenchyma
namespace: plant_structure
def: "Relatively unspecialized ground tissue present in the seed endosperm\, often devoid of intercellular spaces." [ISBN:0080374913]
is_a: PO:0005421
relationship: part_of PO:0009089

[Term]
id: PO:0005417
name: phloem
namespace: plant_structure
def: "Vascular tissue whose principal function is conducting organic subtances." [GR:pj]
is_a: PO:0009015

[Term]
id: PO:0005421
name: parenchyma
namespace: plant_structure
def: "Relatively unspecialized tissue composed of polyhedral cells typically with thin\, non-lignified cellulose cell walls and nucleate living protoplasts." [GR:pj]
synonym: "parenchyma tissue" []
is_a: PO:0009007

[Term]
id: PO:0005423
name: collenchyma
namespace: plant_structure
def: "Living tissue composed of more or less elongated cells with thick nonlignified primary cell walls." [GR:pj]
synonym: "supporting tissue" []
is_a: PO:0009007

[Term]
id: PO:0005426
name: chlorenchyma
namespace: plant_structure
def: "Chloroplast-containing parenchyma tissue." [ISBN:0080374913]
synonym: "chlroenchyma tissue" []
is_a: PO:0005421

[Term]
id: PO:0005427
name: sclerenchyma
namespace: plant_structure
def: "A supporting tissue composed of fibers or sclereids." [ISBN:0080374913]
is_a: PO:0009007

[Term]
id: PO:0005597
name: cambium
namespace: plant_structure
def: "A lateral meristem\, the cells of which divide mostly periclinally. " [ISBN:0080374913]
is_a: PO:0020145

[Term]
id: PO:0005598
name: vascular cambium
namespace: plant_structure
def: "A lateral meristem\, the cells of which give rise to secondary xylem and phloem\, leading to an increase in stem girth." [GR:pj]
is_a: PO:0005597

[Term]
id: PO:0005599
name: cork cambium
namespace: plant_structure
def: "Lateral meristem which produces the phellem (cork) and the phelloderm." [ISBN:0080374913]
synonym: "phellogen" []
is_a: PO:0005597
relationship: part_of PO:0005048

[Term]
id: PO:0005621
name: angular collenchyma
namespace: plant_structure
def: "OBSOLETE. A form of collenchyma in which the primary wall thickening is most prominent in the angles where three or more cells are joined." [GR:pj, ISBN:0080374913]
comment: The term was made obsolete because angular form is a common attribute of ordinary collenchyma.
is_obsolete: true

[Term]
id: PO:0005632
name: lacunar collenchyma
namespace: plant_structure
def: "OBSOLETE. A collenchyma characterized by intercellular spaces and cell wall thickenings facing the intercellular spaces." [GR:pj, ISBN:0080374913]
comment: The term was made obsolete because the lacunar form is an attribute of regular collenchyma.
is_obsolete: true

[Term]
id: PO:0005633
name: lamellar collenchyma
namespace: plant_structure
def: "OBSOLETE. A collenchyma in which cell wall thickenings are deposited mainly on tangential walls." [ISBN:0080374913, GR:pj]
comment: The term was made obsolete because lamellar form is an attribute of regular collenchyma.
synonym: "plate collenchyma" []
synonym: "tangential collenchyma" []
is_obsolete: true

[Term]
id: PO:0005645
name: leaf mesophyll
namespace: plant_structure
def: "The chloroplast-containing\, photosynthetic parenchymatous tissue situated between the two epidermal layers of the foliage leaf." [GR:pj, ISBN:0080374913]
synonym: "foliage leaf mesophyll" []
synonym: "leaf parenchyma" []
is_a: PO:0006070
relationship: part_of PO:0009025

[Term]
id: PO:0005647
name: spongy parenchyma
namespace: plant_structure
def: "Leaf mesophyll parenchyma characterized by little elongated cells\, that are not closely packed and have conspicuous intercellular spaces." [GR:pj, ISBN:0080374913]
relationship: part_of PO:0005645

[Term]
id: PO:0005648
name: palisade parenchyma
namespace: plant_structure
def: "parenchyma containing closely packed elongated chlorenchymatous cells oriented perpendicular to the leaf surface and which are active in photosynthesis." [ISBN:0080374913, GR:pj]
relationship: part_of PO:0005645

[Term]
id: PO:0005656
name: secretory tissue
namespace: plant_structure
def: "Tissues that form specialized structures producing a secretion." [ISBN:047124529, GR:pj]
is_a: PO:0009007

[Term]
id: PO:0005660
name: hydathode
namespace: plant_structure
def: "A structural modification of vascular and non-vascular tissues\, usually in a leaf\, that permits the release of water through a pore in the epidermis." [ISBN:0080374913, GR:pj]
is_a: PO:0005656
is_a: PO:0009015

[Term]
id: PO:0005661
name: salt gland
namespace: plant_structure
def: "A specialized tissue where excess salt absorbed in water from the soil is concentrated\, being stores or excreted." [GR:pj]
comment: A crust of salt forms on leaves which tastes bad and the white surfaces act to reflect light. Example\, as is Mangrove vegetation
is_a: PO:0005656

[Term]
id: PO:0005665
name: resin canal
namespace: plant_structure
def: "A duct of schizogenous origin lined with resin-secreting cells and containing resin" [ISBN:0080374913, GR:pj]
synonym: "resin duct" []
is_a: PO:0005656

[Term]
id: PO:0005669
name: oil gland
namespace: plant_structure
def: "A gland or a cavity lined with cells that secrete oils." [GR:pj]
comment: Oil glands are schizogenous.
synonym: "oil cavity" []
is_a: PO:0005656

[Term]
id: PO:0005679
name: epidermis
namespace: plant_structure
def: "An outermost cell layer of primary tissues of the plant\, sometimes comprised of more than one layer. " [GR:pj, ISBN:0080374913]
synonym: "epidermal layer" []
synonym: "multiseriate epidermis" []
is_a: PO:0009014

[Term]
id: PO:0005702
name: aerenchyma
namespace: plant_structure
def: "Parenchyma tissue containing particularly large intercellular spaces of schizogenous or lysigenous origin." [ISBN:0080374913, GR:pj]
comment: As applied to an intercellular space\, originating by one or a combination of two processes\, separation and degradation of cell walls.
synonym: "aerenchyma tissue" []
is_a: PO:0005421

[Term]
id: PO:0005704
name: rhexigenous aerenchyma
namespace: plant_structure
def: "OBSOLETE. Aerenchyma originating by rupture of cells." [GR:pj, ISBN:0080374913]
comment: The term was made obsolete because rhexigenous form is an attribute of regular aerenchyma.
is_obsolete: true

[Term]
id: PO:0005706
name: lysigenous aerenchyma
namespace: plant_structure
def: "OBSOLETE. Aerenchyma originating by dissolution of cells." [GR:pj, ISBN:0080374913]
comment: The term was made obsolete because lysigenous form is an attribute of regular aerenchyma.
is_obsolete: true

[Term]
id: PO:0005708
name: cortex
namespace: plant_structure
def: "Tissue between the vascular system and the epidermis in stem and root. " [GR:pj]
is_a: PO:0009007

[Term]
id: PO:0005752
name: promeristem
namespace: plant_structure
def: "OBSOLETE. Meristematic tissue consisting of apical initials\, together with cells derived from them and which are still close to the initial." [GR:pj, ISBN:0080374913]
is_obsolete: true

[Term]
id: PO:0005772
name: exodermis
namespace: plant_structure
def: "The sub-epidermal layer or layers of cells of the root similar in structure and cytochemical characteristics of  the endodermis\, the outermost layer or layers of cells of the cortex." [GR:pj, ISBN:0080374913]
comment: The cell walls are thickened and contain suberin. Absent in pteridophytes\, fibrous in Phoenix and accompanied by sclerenchyma in Ananas.
synonym: "root hypodermis" []
is_a: PO:0005051
relationship: part_of PO:0000258

[Term]
id: PO:0005848
name: secondary xylem
namespace: plant_structure
def: "The xylem tissue formed by the activity of the vascular cambium." [GR:pj, ISBN:0471245194]
comment: It is absent in small dicot annuals and most monocots; the \"wood\" of broad leaf angiosperm tress.
is_a: PO:0005352

[Term]
id: PO:0005849
name: primary xylem
namespace: plant_structure
def: "The xylem of the primary plant body. " [ISBN:0471245194, GR:pj, ISBN:0122151704]
comment: In stem or root it is differentiated behind the apical meristem.
is_a: PO:0005352

[Term]
id: PO:0006001
name: phyllome
namespace: plant_structure
def: "A collective term for all the different types of leaves appearing on plants." [ISBN:0080374913]
relationship: part_of PO:0009006

[Term]
id: PO:0006002
name: lower glume
alt_id: PO:0006027
alt_id: PO:0006031
namespace: plant_structure
def: "The proximal/basal of the two glumes." [GR:pj]
synonym: "lower empty glume" []
synonym: "lower rudimentary glume" []
synonym: "outer empty glume" []
synonym: "outer glume" []
synonym: "outer rudimentary glume" []
is_a: PO:0009039

[Term]
id: PO:0006003
name: scale leaf
namespace: plant_structure
def: "A reduced and more or less non-photosynthetic leaf\, often associated with a vegetatively propagating organ such as a rhizome or perennating bud." [ISBN:0080374913]
comment: Sometimes referring specifically to such leaves on a seedling.
synonym: "cataphyll" []
is_a: PO:0006001

[Term]
id: PO:0006004
name: upper glume
alt_id: PO:0006028
alt_id: PO:0006030
namespace: plant_structure
def: "The apical/distal of the two glumes." [GR:pj]
synonym: "inner empty glume" []
synonym: "inner glume" []
synonym: "inner rudimentary glume" []
synonym: "upper empty glume" []
synonym: "upper rudimentary glume" []
is_a: PO:0009039

[Term]
id: PO:0006011
name: lateral vein
namespace: plant_structure
def: "Unbranched second order vein of the grass leaf blade." [GR:pj]
is_a: PO:0020140

[Term]
id: PO:0006012
name: leaf collar
namespace: plant_structure
def: "A thin band of intercalary meristematic tissue at the junction of the leaf blade (lamina) and the leaf sheath found in grasses." [GR:pj, ISBN:0080374913]
relationship: part_of PO:0009025

[Term]
id: PO:0006016
name: leaf epidermis
namespace: plant_structure
def: "Epidermal layer of a foliage leaf." [GR:pj]
synonym: "foliage leaf epidermis" []
is_a: PO:0006035
relationship: part_of PO:0009025

[Term]
id: PO:0006017
name: helobial endosperm
namespace: plant_structure
def: "Endosperm in which the first karyokinetic event is accompanied by the formation of a horizontal wall which divides the central cell into unequal regions. The larger one is the micropylar chamber in which cytokinesis does not occur and the smaller one is the chalazal chamber." [ISBN:0080374913]
is_a: PO:0009089

[Term]
id: PO:0006018
name: leaf adaxial epidermis
namespace: plant_structure
def: "The epidermal layer of adaxial/upper surface of the leaf." [ISBN:0080374913]
synonym: "upper epidermis" []
is_a: PO:0006016

[Term]
id: PO:0006019
name: leaf abaxial epidermis
namespace: plant_structure
def: "The epidermal layer of the abaxial/lower surface of the leaf." [ISBN:0080374913]
synonym: "lower epidermis" []
is_a: PO:0006016

[Term]
id: PO:0006020
name: apical meristem of lateral root
alt_id: PO:0003013
namespace: plant_structure
def: "Meristem found in the apex of the lateral root." [GR:pj]
comment: This is different from root lateral meristem.
synonym: "lateral root meristem" []
is_a: PO:0020147
relationship: part_of PO:0000027

[Term]
id: PO:0006021
name: adventitious root apical meristem
namespace: plant_structure
def: "Apical meristem of the adventitious root." [GR:pj]
synonym: "crown root meristem" []
synonym: "seminal root meristem" []
is_a: PO:0020147
relationship: part_of PO:0020129

[Term]
id: PO:0006022
name: bundle sheath extension
namespace: plant_structure
def: "A strip of ground tissue present along the leaf veins and extending from the bundle sheath to the epidermis. It may be present on one or both sides of the vein and may consist of parenchyma or sclerenchyma." [ISBN:0080374913]
is_a: PO:0009007

[Term]
id: PO:0006023
name: bundle sheath
namespace: plant_structure
def: "A layer or layers of cells surrounding the vascular bundles of leaves. It may consist of parenchyma or sclerenchyma." [ISBN:0080374913]
is_a: PO:0009007
relationship: part_of PO:0009025

[Term]
id: PO:0006024
name: parenchyma sheath
namespace: plant_structure
def: "A single layered\, parenchymatous bundle sheath characterized by presence of large quantity of starch." [ISBN:0080374913]
comment: Homologous to the endodermis.
synonym: "starch sheath" []
is_a: PO:0006023

[Term]
id: PO:0006025
name: mestome sheath
namespace: plant_structure
def: "The inner endodermal sheath of a two layered bundle sheath. The cells are smaller in diameter compared to those in outer wall (starch sheath). The cell  walls are thick and contain suberized lamellae. They are analogous to endodermis." [ISBN:0080374913]
is_a: PO:0006023

[Term]
id: PO:0006032
name: awn
namespace: plant_structure
def: "A long bristle-like appendage found on the tip or back of various parts of the grass spikelet." [APWeb:Glossary]
relationship: part_of PO:0009037

[Term]
id: PO:0006033
name: paleal apiculus
namespace: plant_structure
def: "A short\, abrupt\, flexible point present at the apex of the palea" [GR:pj]
synonym: "apiculus" []
relationship: part_of PO:0009038

[Term]
id: PO:0006034
name: leaflet margin
namespace: plant_structure
def: "The margin or edges of the leaflet." [GR:pj]
relationship: part_of PO:0020049

[Term]
id: PO:0006035
name: shoot epidermis
namespace: plant_structure
def: "Outer layer of the shoot organs." [GR:pj, ISBN:047124529]
comment: Often interrupted by stomata and other structures. The shoot epidermis is different from the root epidermis in its origin\, function and structure.
is_a: PO:0005679

[Term]
id: PO:0006036
name: root epidermis
alt_id: PO:0006037
namespace: plant_structure
def: "The outermost primary cell layer of the root." [ISBN:0080374913]
comment: The root epidermis is different from the shoot epidermis in its origin\, function and structure.
synonym: "epiblem" []
synonym: "rhizodermis" []
is_a: PO:0005679
relationship: part_of PO:0009005

[Term]
id: PO:0006039
name: adventitious root epidermis
alt_id: PO:0006038
namespace: plant_structure
def: "The outer most cell layer of the adventitious root." [GR:pj]
synonym: "crown root epidermis" []
relationship: part_of PO:0020129

[Term]
id: PO:0006040
name: sepal epidermis
namespace: plant_structure
def: "The outermost cell layer of the sepal." [GR:pj]
is_a: PO:0006035
relationship: part_of PO:0009031

[Term]
id: PO:0006041
name: petal epidermis
namespace: plant_structure
def: "The epidermal layer of the petal." [GR:pj]
is_a: PO:0006035
relationship: part_of PO:0009032

[Term]
id: PO:0006042
name: velamen
namespace: plant_structure
def: "A multiseriate epidermis found in aerial roots of some monocots. Most of its cells are dead and store water like a sponge." [ISBN:0080374913]
synonym: "velamen radicum" []
is_a: PO:0006036

[Term]
id: PO:0006043
name: integument epidermis
namespace: plant_structure
def: "The epidermis of an integument in an ovule." [GR:pj]
is_a: PO:0006035
relationship: part_of PO:0020021

[Term]
id: PO:0006044
name: inner integument epidermis
namespace: plant_structure
def: "The epidermis of the inner integument in an ovule." [GR:pj]
is_a: PO:0006043
relationship: part_of PO:0020022

[Term]
id: PO:0006045
name: outer integument epidermis
namespace: plant_structure
def: "The epidermis of the outer integument in an ovule." [GR:pj]
is_a: PO:0006043
relationship: part_of PO:0020023

[Term]
id: PO:0006048
name: seed coat epidermis
namespace: plant_structure
def: "The epidermal layer of the seed coat." [GR:pj]
is_a: PO:0005679
relationship: part_of PO:0009088

[Term]
id: PO:0006049
name: scutellum epidermis
namespace: plant_structure
def: "The epidermal layer of the scutellum." [GR:pj]
is_a: PO:0006035
relationship: part_of PO:0020110

[Term]
id: PO:0006050
name: exotesta
namespace: plant_structure
def: "That part of the seed coat that develops from the outer surface of the outer integument." [GR:pj]
synonym: "seed coat outer epidermis" []
is_a: PO:0006048
relationship: part_of PO:0020057

[Term]
id: PO:0006051
name: endotesta
namespace: plant_structure
def: "That part of the seed coat that develops from the inner epidermis of the outer integument." [GR:pj]
synonym: "seed coat inner epidermis" []
is_a: PO:0006048
relationship: part_of PO:0020057

[Term]
id: PO:0006052
name: petal abaxial epidermis
namespace: plant_structure
def: "The abaxial/lower epidermal cell layer of the petal." [GR:pj]
is_a: PO:0006041

[Term]
id: PO:0006053
name: petal adaxial epidermis
namespace: plant_structure
def: "The adaxial/upper epidermal cell layer of the petal." [GR:pj]
is_a: PO:0006041

[Term]
id: PO:0006054
name: sepal abaxial epidermis
namespace: plant_structure
def: "The abaxial/lower epidermal cell layer of the sepal." [GR:pj]
is_a: PO:0006040

[Term]
id: PO:0006055
name: sepal adaxial epidermis
namespace: plant_structure
def: "The adaxial/upper epidermal cell layer of the sepal." [GR:pj]
is_a: PO:0006040

[Term]
id: PO:0006056
name: cotyledon epidermis
namespace: plant_structure
def: "The epidermal cell layer of the cotyledon." [GR:pj]
is_a: PO:0006035
relationship: part_of PO:0020030

[Term]
id: PO:0006057
name: cotyledon abaxial epidermis
namespace: plant_structure
def: "The abaxial/lower epidermal cell layer of the cotyledon." [GR:pj]
is_a: PO:0006056

[Term]
id: PO:0006058
name: cotyledon adaxial epidermis
namespace: plant_structure
def: "The adaxial/upper epidermal cell layer of the cotyledon." [GR:pj]
is_a: PO:0006056

[Term]
id: PO:0006060
name: filament epidermis
namespace: plant_structure
def: "The epidermal cell layer of the stamen filament." [GR:pj]
is_a: PO:0006035
relationship: part_of PO:0009067

[Term]
id: PO:0006061
name: stigma epidermis
namespace: plant_structure
def: "The epidermal cell layer of the stigma." [GR:pj, PMID:11951033]
is_a: PO:0006035
relationship: part_of PO:0009073

[Term]
id: PO:0006062
name: style epidermis
namespace: plant_structure
def: "The epidermal cell layer of the style." [GR:pj]
synonym: "transmitting tract epidermis" []
is_a: PO:0006035
relationship: part_of PO:0009074

[Term]
id: PO:0006063
name: ovary epidermis
namespace: plant_structure
def: "The epidermal cell layer of the ovary." [GR:pj]
is_a: PO:0006035
relationship: part_of PO:0009072

[Term]
id: PO:0006065
name: hypocotyl endodermis
namespace: plant_structure
def: "It is the innermost layer of the cortex of hypocotyl." [GR:pj]
is_a: PO:0000252

[Term]
id: PO:0006066
name: petiole parenchyma
namespace: plant_structure
def: "Relatively unspecialized tissue present in the leaf petiole." [GR:pj]
is_a: PO:0005421

[Term]
id: PO:0006067
name: cambium-like transitional zone
namespace: plant_structure
def: "OBSOLETE. A cup-shaped region in the shoot apical meristem found between the central mother cell and the rib and peripheral zone. The cells of this zone are derived from the corpus intials\, but in some cases they arise also from tunica initials." [ISBN:0080374913]
comment: If found\, this zone is a temporary feature mostly in Gymnosperms.
synonym: "adaxial meristem" []
synonym: "leaf meristem" []
synonym: "ventral meristem" []
is_obsolete: true

[Term]
id: PO:0006068
name: sepal parenchyma
namespace: plant_structure
def: "Relatively unspecialized tissue present in the sepals." [GR:pj]
is_a: PO:0005421

[Term]
id: PO:0006069
name: petal parenchyma
namespace: plant_structure
def: "Relatively unspecialized tissue present in the petals." [GR:pj]
is_a: PO:0005421

[Term]
id: PO:0006070
name: mesophyll
namespace: plant_structure
def: "The chloroplast-containing\, photosynthetic parenchymatous tissue situated between the two epidermal layers of the leaf or leaf like organs." [GR:pj]
is_a: PO:0005426

[Term]
id: PO:0006071
name: petal mesophyll
namespace: plant_structure
def: "The chloroplast-containing\, photosynthetic parenchymatous tissue situated between the two epidermal layers of the petal." [GR:pj]
is_a: PO:0006070

[Term]
id: PO:0006072
name: sepal mesophyll
namespace: plant_structure
def: "The chloroplast-containing\, photosynthetic parenchymatous tissue situated between the two epidermal layers of the sepal." [GR:pj]
is_a: PO:0006070

[Term]
id: PO:0006073
name: intercalary meristem
namespace: plant_structure
def: "Meristematic tissue separated from the apical meristem in the primary body by more or less mature tissues." [ISBN:0080374913, ISBN:0122151704]
is_a: PO:0006079
is_a: PO:0009013

[Term]
id: PO:0006074
name: procambium
namespace: plant_structure
def: "A primary cambium which undergoes differentiation to form the primary vascular tissue." [ISBN:0080374913]
relationship: part_of PO:0020144

[Term]
id: PO:0006075
name: primary phloem
namespace: plant_structure
def: "The phloem of the primary plant body." [ISBN:0122151704]
comment: In stem or root it is differentiated behind the apical meristem.
is_a: PO:0005417

[Term]
id: PO:0006076
name: metaphloem
namespace: plant_structure
def: "Part of the primary phloem that differentiates after the protophloem and before the secondary phloem\, if any of the latter is formed." [ISBN:0471245194]
relationship: part_of PO:0006075

[Term]
id: PO:0006077
name: protophloem
namespace: plant_structure
def: "The first-formed elements of the primary phloem." [ISBN:0471245194]
relationship: part_of PO:0006075

[Term]
id: PO:0006078
name: primary vascular tissue
namespace: plant_structure
def: "OBSOLETE. The vascular tissue of the primary plant body at the embryonic stage. " [GR:pj]
comment: Redundant to sec ...
is_obsolete: true

[Term]
id: PO:0006079
name: shoot meristem
namespace: plant_structure
def: "Meristem found in a shoot." [GR:pj]
is_a: PO:0009013
relationship: part_of PO:0009006

[Term]
id: PO:0006080
name: secondary vascular tissue
namespace: plant_structure
def: "OBSOLETE. The vascular tissue derived from the vascular cambium because of the secondary growth." [GR:pj]
comment: Redundant sec phloem and xylem
is_obsolete: true

[Term]
id: PO:0006081
name: apical meristem of primary root
namespace: plant_structure
def: "Meristem found in the apex of the primary root." [GR:pj]
synonym: "embryonic root meristem" []
is_a: PO:0020147
relationship: part_of PO:0000026
relationship: part_of PO:0020031

[Term]
id: PO:0006082
name: abaxial protoderm
namespace: plant_structure
def: "The outermost layer of the shoot apical meristem which gives rise to the abaxial/lower leaf epidermis. " [ISBN:0080374913, GR:pj]
is_a: PO:0006210

[Term]
id: PO:0006083
name: adaxial protoderm
namespace: plant_structure
def: "The outermost layer of the shoot apical meristem which gives rise to the adaxial/upper leaf epidermis." [ISBN:0080374913, GR:pj]
is_a: PO:0006210

[Term]
id: PO:0006084
name: transfusion tissue
namespace: plant_structure
def: "Tissue consisting of tracheids and parenchyma cells\, associated with the vascular bundle." [ISBN:0080374913]
comment: Found generally in gymnosperm leaves.
is_a: PO:0009007

[Term]
id: PO:0006085
name: root meristem
alt_id: PO:0003001
namespace: plant_structure
def: "Meristem found in a root." [GR:pj]
synonym: "meristematic zone" []
is_a: PO:0009013
relationship: part_of PO:0009005

[Term]
id: PO:0006086
name: accessory transfusion tissue
namespace: plant_structure
def: "OBSOLETE. The accessory tissue extending laterally into the mesophyll rather than remaining associated with the vascular bundles." [ISBN:0080374913]
comment: Not in current literature.
is_obsolete: true

[Term]
id: PO:0006087
name: proliferation tissue
namespace: plant_structure
def: "OBSOLETE. Tissue that develops from phloem parenchyma in the outer portion of the inner bark accommodating the expansion in circumference." [ISBN:0080374913]
comment: check the definition.
is_obsolete: true

[Term]
id: PO:0006109
name: pith
namespace: plant_structure
def: "Non-vascular tissue in the center of stem or root" [ISBN:0080280307]
is_a: PO:0009007

[Term]
id: PO:0006200
name: fascicular cambium
namespace: plant_structure
def: "Vascular cambium  originating from procambium within vascular bundles or fascicles." [ISBN:047124529]
is_a: PO:0005598

[Term]
id: PO:0006201
name: interfascicular cambium
namespace: plant_structure
def: "Vascular cambium arising between vascular bundles or fascicles\, in the interfascicular parenchyma or pith." [ISBN:047124529]
is_a: PO:0005598

[Term]
id: PO:0006202
name: interfascicular region
namespace: plant_structure
def: "Region located between vascular bundles in the stem. " [ISBN:047124529]
comment: Check for the relationship. Inapplicable for nearly all monocots.
synonym: "medullary ray" []
synonym: "pith ray" []
is_a: PO:0006109
relationship: part_of PO:0009047

[Term]
id: PO:0006203
name: pericycle
namespace: plant_structure
def: "Part of the tissue of the stele located between the phloem and endodermis." [ISBN:047124529]
is_a: PO:0009007
relationship: part_of PO:0020124

[Term]
id: PO:0006204
name: sporocyte
namespace: plant_structure
def: "A diploid (2n) cell that undergoes meiosis and produces four haploid (1n) spores." [GR:pj]
is_a: PO:0009002

[Term]
id: PO:0006205
name: spongy mesophyll cell
namespace: plant_structure
def: "Irregularly-shaped\, chlorenchymatous cell\, separated by large air spaces. " [GR:pj]
comment: Usually found in the abaxial/lower part of the leaf mesophyll as in a dorsiventral leaf\, but between two palisade parenchyma layers in an isobilateral leaf.
is_a: PO:0004006
relationship: part_of PO:0005647

[Term]
id: PO:0006206
name: palisade mesophyll cell
namespace: plant_structure
def: "Elongated chlorenchymatous cell oriented perpendicular to the leaf surface and which is active in photosynthesis." [GR:pj]
comment: Usually found in the adaxil/upper part of the leaf mesophyll.
is_a: PO:0004006
relationship: part_of PO:0005648

[Term]
id: PO:0006207
name: exodermal passage cell
namespace: plant_structure
def: "A short cell in the dimorphic type of exodermis with cell wall that remains non-thickened." [TAIR:ki, PMID:11709575]
is_a: PO:0000353
relationship: part_of PO:0005772

[Term]
id: PO:0006208
name: endodermal passage cell
namespace: plant_structure
def: "Cell in the endodermal layer of the root with cell wall that remains non-thickened." [TAIR:ki]
is_a: PO:0000353
relationship: part_of PO:0000252

[Term]
id: PO:0006209
name: lateral root epidermis
namespace: plant_structure
def: "OBSOLETE. The outer most cell layer of the lateral roots." [GR:pj]
is_obsolete: true

[Term]
id: PO:0006210
name: protoderm
namespace: plant_structure
def: "The undifferentiated surface cell layer of the primary plant body\, which gives rise to epidermis." [ISBN:047124529, GR:pj]
comment: It may or may not arise from independent initials.  Some researchers also call it an epidermis in meristematic state.
relationship: part_of PO:0009013

[Term]
id: PO:0006211
name: separation layer
namespace: plant_structure
def: "Cells that develop an abnormal wall chemistry and swelling resulting in easily being pulled apart along the pectin-rich middle lamella; directly involved in the weakening process of abscission." [ISBN:0122151704]
relationship: part_of PO:0000146

[Term]
id: PO:0006212
name: protective layer
namespace: plant_structure
def: "The layer of cells in the abscission zone that have lignin and suberin depositions and are found on the axial side of the break or exposed surface of abscission." [ISBN:0122151704]
relationship: part_of PO:0000146

[Term]
id: PO:0006213
name: root aerenchyma
namespace: plant_structure
def: "Parenchyma tissue containing particularly large intercellular spaces in the tissue of roots." [GR:pj]
is_a: PO:0005702
relationship: part_of PO:0009005

[Term]
id: PO:0006214
name: stem aerenchyma
namespace: plant_structure
def: "Parenchyma tissue containing particularly large intercellular spaces." [GR:pj]
is_a: PO:0005702
relationship: part_of PO:0009047

[Term]
id: PO:0006215
name: leaf aerenchyma
namespace: plant_structure
def: "Spongy parenchyma tissue containing particularly large intercellular spaces in the leaf mesophyll. " [GR:pj]
is_a: PO:0005702
relationship: part_of PO:0009025

[Term]
id: PO:0006216
name: internal phloem
namespace: plant_structure
def: "Primary phloem tissue positioned internal to the primary xylem" [ISBN:0122151704]
synonym: "intraxylary phloem" []
is_a: PO:0006075

[Term]
id: PO:0006218
name: exotegmen
namespace: plant_structure
def: "That part of the seed coat that develops from the outer surface of the inner integument." [GR:pj]
is_a: PO:0006048
relationship: part_of PO:0020056

[Term]
id: PO:0006219
name: endotegmen
namespace: plant_structure
def: "That part of the seed coat that develops from the inner epidermis of the inner integument." [GR:pj]
is_a: PO:0006048
relationship: part_of PO:0020056

[Term]
id: PO:0006220
name: central endosperm
namespace: plant_structure
def: "The central region of the endosperm composed of cells that are significantly larger than those at the periphery\, especially the aleurone and sub-aleurone layers." [TAIR:ki]
comment: Also called starchy endosperm region (characteristic of some grasses).
is_a: PO:0009089

[Term]
id: PO:0006221
name: articulated laticifer cell
namespace: plant_structure
def: "A cell that is part of a compound laticifer in which the cell walls between contiguous cells partly or completely disappear." [ISBN:0471245208, TAIR:ki]
synonym: "laticiferous vessel" []
relationship: part_of PO:0005053

[Term]
id: PO:0006222
name: non-articulated laticifer cell
namespace: plant_structure
def: "Latex-containing cell that elongates indefinitely and grows intrusively between the walls of meristematic cells." [PMID:11732189]
synonym: "simple laticifer" []
relationship: part_of PO:0005053

[Term]
id: PO:0006300
name: obsolete plant structure
namespace: plant_structure
def: "The instances of this parent term are those anatomical terms which have become obsolete." [GR:pj]
is_obsolete: true

[Term]
id: PO:0006301
name: corpus
namespace: plant_structure
def: "OBSOLETE. Group of cells located beneath anticlinally dividing peripheral layers (tunica) and dividing in many planes. In apical shoot meristem. Such division cause the increase in the volume of shoot." [ISBN:0080374913, GR:pj]
comment: The term has been made obsolete because this concept is used in a very loose sense.
is_obsolete: true

[Term]
id: PO:0006302
name: tunica
namespace: plant_structure
def: "OBSOLETE. The outermost layer or layers in the shoot apical meristem of the Angiosperms in which the plane of division is almost anticlinal. This layer contributes to surface growth." [ISBN:047124529, GR:pj]
comment: The term has been made obsolete because this concept is used in a very loose sense.
is_obsolete: true

[Term]
id: PO:0006303
name: L1
namespace: plant_structure
def: "OBSOLETE. The outer layer of the tunica." [GR:pj]
comment: A similar term L1 meristem (PO\:0009020) occurs.
is_obsolete: true

[Term]
id: PO:0006304
name: L2
namespace: plant_structure
def: "OBSOLETE. The second layer of the tunica." [GR:pj]
comment: A similar term L2 meristem (PO\:0009021) occurs.
is_obsolete: true

[Term]
id: PO:0006305
name: L3
namespace: plant_structure
def: "OBSOLETE. The innermost layer of the tunica." [GR:pj]
comment: A similar term L3 meristem (PO\:0009022) occurs.
is_obsolete: true

[Term]
id: PO:0006306
name: shoot procambium
namespace: plant_structure
def: "A derivative of the apical mersitem which undergoes differentiation to form the primary vascular tissue of a shoot." [GR:pj]
is_a: PO:0006074
relationship: part_of PO:0020148

[Term]
id: PO:0006307
name: root procambium
namespace: plant_structure
def: "A derivative of the apical meristem which undergoes differentiation to form the primary vascular tissue of a root." [GR:pj]
is_a: PO:0006074
relationship: part_of PO:0006085

[Term]
id: PO:0006308
name: root lateral meristem
namespace: plant_structure
def: "Meristem of the root located parallel to the sides of the axis." [ISBN:047124529]
comment: Generally causes root thickening. Not to be confused with lateral root meristem\, which is the meristem of the lateral root.
is_a: PO:0006085
is_a: PO:0020145
relationship: part_of PO:0020121

[Term]
id: PO:0006309
name: tassel spikelet
namespace: plant_structure
def: "Ultimate inflorescence branch of the maize tassel." [GR:pj]
is_a: PO:0009051
relationship: part_of PO:0020126

[Term]
id: PO:0006310
name: tassel floret
namespace: plant_structure
def: "Flowers of the spikelets of maize tassel." [GR:pj]
is_a: PO:0006318
relationship: part_of PO:0006309

[Term]
id: PO:0006311
name: tassel sessile spikelet
namespace: plant_structure
def: "Ultimate inflorescence branch of the maize tassel without a pedicel\, developing from the spikelet pair meristem." [GR:pj]
is_a: PO:0006309

[Term]
id: PO:0006312
name: tassel pedicellate spikelet
namespace: plant_structure
def: "Ultimate inflorescence branch of the maize tassel with a pedicel\, developing from the spikelet pair meristem." [GR:pj]
is_a: PO:0006309

[Term]
id: PO:0006313
name: lower floret of pedicellate spikelet of tassel
namespace: plant_structure
def: "The lower of the two florets of the pedicellate spikelet of a maize tassel." [GR:pj]
is_a: PO:0006310
relationship: part_of PO:0006312

[Term]
id: PO:0006314
name: upper floret of pedicellate spikelet of tassel
namespace: plant_structure
def: "One of the two florets placed above the lower floret on the pedicellate spikelet rachilla of a maize tassel " [GR:pj]
is_a: PO:0006310
relationship: part_of PO:0006312

[Term]
id: PO:0006315
name: lower floret of sessile spikelet of tassel
namespace: plant_structure
def: "The lower of the two florets of the sessile spikelet of a maize tassel." [GR:pj]
is_a: PO:0006310
relationship: part_of PO:0006311

[Term]
id: PO:0006316
name: upper floret of sessile spikelet of tassel
namespace: plant_structure
def: "One of the two florets placed above the lower floret on the sessile spikelet rachilla of a maize tassel." [GR:pj]
is_a: PO:0006310
relationship: part_of PO:0006311

[Term]
id: PO:0006317
name: gynoecium of tassel floret
namespace: plant_structure
def: "Collectively the carpels of a maize tassel floret. " [GR:pj]
comment: The development of the gynoecium in the tassel floret of a normal maize plant is aborted and is present in a rudimentary state.
is_a: PO:0006357
relationship: part_of PO:0006310

[Term]
id: PO:0006318
name: floret (sensu Poaceae)
namespace: plant_structure
def: "Small flowers of the spikelets of Poaceae." [Poc:curators]
is_a: PO:0009082
relationship: part_of PO:0009051

[Term]
id: PO:0006319
name: spikelet pedicel
namespace: plant_structure
def: "Inflorescence branch that terminates in a spikelet." [Poc:curators]
comment: This is not a pedicel in the strict sense\, but is the ultimate naked part of the inflorescence axis.
is_a: PO:0009052
relationship: part_of PO:0009051

[Term]
id: PO:0006320
name: ear spikelet
namespace: plant_structure
def: "Ultimate inflorescence branch of the maize ear." [GR:pj]
is_a: PO:0009051
relationship: part_of PO:0020136

[Term]
id: PO:0006321
name: second order inflorescence branch
namespace: plant_structure
def: "Any branch forming from the primary or first order inflorescence branch." [GR:pj]
synonym: "primary branch" []
is_a: PO:0009081

[Term]
id: PO:0006322
name: third order inflorescence branch
namespace: plant_structure
def: "Any branch forming from the second order inflorescence branch." [GR:pj]
synonym: "secondary inflorescence branch" []
is_a: PO:0009081

[Term]
id: PO:0006323
name: tassel branch
namespace: plant_structure
def: "Any branch forming from the primary or higher order tassel axes." [GR:pj]
is_a: PO:0006321
relationship: part_of PO:0020126

[Term]
id: PO:0006324
name: central spike of tassel
namespace: plant_structure
def: "The inflorescence axis of the tassel." [GR:pj]
synonym: "tassel rachis" []
is_a: PO:0020122
relationship: part_of PO:0020126

[Term]
id: PO:0006325
name: inflorescence node
namespace: plant_structure
def: "The region of the inflorescence axis where the spikelet\, flower\, floret or the branch is attached." [GR:pj]
relationship: part_of PO:0020122

[Term]
id: PO:0006326
name: inflorescence internode
namespace: plant_structure
def: "The region of rachis present between the two nodes." [GR:pj]
relationship: part_of PO:0020122

[Term]
id: PO:0006327
name: spikelet meristem
namespace: plant_structure
def: "Apical meristem that gives rise to the two or more florets of a grass inflorescence." [GR:pj]
is_a: PO:0000230
relationship: part_of PO:0009051

[Term]
id: PO:0006328
name: spikelet pair meristem
namespace: plant_structure
def: "The meristem that produces two spikelet meristems\, each of which produces two floral meristems." [GR:pj]
comment: Found in some grass inflorescences.
is_a: PO:0000230
relationship: part_of PO:0009049

[Term]
id: PO:0006329
name: floret meristem (sensu Poaceae)
namespace: plant_structure
def: "Meristem that gives rise to the organs of a floret of a grass plant." [GR:pj]
is_a: PO:0000229
relationship: part_of PO:0009051

[Term]
id: PO:0006330
name: gynophore
namespace: plant_structure
def: "The stalk at the base of the ovary." [Poc:curators]
comment: Typically receptacular in origin.
relationship: part_of PO:0009062

[Term]
id: PO:0006331
name: seed raphe
namespace: plant_structure
def: "The ridge along the body of the seed formed from the part of funiculus that was adnate to the ovule." [ISBN:047124529]
relationship: part_of PO:0009010

[Term]
id: PO:0006332
name: seed funicle
namespace: plant_structure
def: "Remnants of the funicle from ovary where it attaches the ovule to the placenta." [GR:pj]
relationship: part_of PO:0009010

[Term]
id: PO:0006333
name: seed chalaza
namespace: plant_structure
def: "Remnant of the ovular chalaza which is a region in the ovule where the integuments and the nucellus merge with the funiculus. " [GR:pj]
relationship: part_of PO:0009010

[Term]
id: PO:0006334
name: seed micropyle
namespace: plant_structure
def: "A pore on the seed coat which is a remnant of the ovular micropyle." [GR:pj]
relationship: part_of PO:0009010

[Term]
id: PO:0006336
name: seed obturator
namespace: plant_structure
def: "An outgrowth of the seed funicle\, that forms a bridge between the seed micropyle and other tissues. It is also a remnant form of the obturator found in the ovular funicle." [GR:pj]
relationship: part_of PO:0006332

[Term]
id: PO:0006337
name: inflorescence bract of ear
namespace: plant_structure
def: "The leaf subtending an ear of corn and acting as outer envelope of the ear." [GR:pj]
synonym: "corn husk" []
synonym: "husk leaf" []
is_a: PO:0009054
relationship: part_of PO:0020136

[Term]
id: PO:0006338
name: embryonic leaf
namespace: plant_structure
def: "The first few leaves developing from the embryonic shoot apical meristem." [GR:pj]
is_a: PO:0009025
relationship: part_of PO:0009009

[Term]
id: PO:0006339
name: juvenile leaf
namespace: plant_structure
def: "Distinct from adult leaves\, being characterized by particular anatomical traits namely\, wax and trichome distribution\, presence or absence of epidermal cell types\, cell wall shape and biochemistry." [MaizeGDB:lv, GR:pj]
comment: The first juvenile leaves are e.g. the embryonic leaves found in the grass kernel (caryopsis).
is_a: PO:0009025

[Term]
id: PO:0006340
name: adult leaf
namespace: plant_structure
def: "Adult leaves are characterized by particular anatomical traits namely\, wax and trichome distribution\, presence or absence of epidermal cell types\, cell wall shape and biochemistry." [GR:pj, MaizeGDB:lv]
comment: The adult leaves are placed above the juvenile (oldest) leaves. However in some plants the juvenile leaves may go on to establish as adult leaves.
is_a: PO:0009025

[Term]
id: PO:0006341
name: primary shoot
namespace: plant_structure
def: "The shoot developing from the embryonic shoot apical meristem." [UMSL:fz]
synonym: "main stalk" []
is_a: PO:0009006

[Term]
id: PO:0006342
name: infructescence
namespace: plant_structure
def: "The grouping or arrangement in which fruits are borne on a plant." [GR:pj]
relationship: part_of PO:0009003

[Term]
id: PO:0006343
name: axillary shoot
namespace: plant_structure
def: "The shoot developing from the axillary bud meristem." [GR:pj]
synonym: "tiller" []
is_a: PO:0009006

[Term]
id: PO:0006344
name: shoot lateral meristem
namespace: plant_structure
def: "Meristem of the shoot located parallel to the sides of the axis." [Poc:curators]
is_a: PO:0006079
is_a: PO:0020145

[Term]
id: PO:0006345
name: pollen tube
namespace: plant_structure
def: "A tubular cell extension formed by the germinating pollen grain; carries the male gametes into the ovule." [ISBN:0471245208]
relationship: part_of PO:0020091

[Term]
id: PO:0006346
name: leaf intercalary meristem
namespace: plant_structure
def: "The meristematic tissue in the primary body of the leaf separated from the apical meristem by non-meristematic tissues." [GR:pj]
is_a: PO:0006073
relationship: part_of PO:0009025

[Term]
id: PO:0006347
name: stem intercalary meristem
namespace: plant_structure
def: "Meristematic tissue in the primary body of stem separated from the apical meristem by more or less mature tissues." [GR:pj]
is_a: PO:0006073
relationship: part_of PO:0009047

[Term]
id: PO:0006348
name: ear pedicellate spikelet
namespace: plant_structure
def: "Ultimate pedicellate inflorescence branch of the maize ear that develops from the spikelet pair meristem." [GR:pj]
is_a: PO:0006320

[Term]
id: PO:0006349
name: ear sessile spikelet
namespace: plant_structure
def: "Ultimate sessile inflorescence branch of the maize ear that develops from the spikelet pair meristem." [GR:pj]
is_a: PO:0006320

[Term]
id: PO:0006350
name: upper floret of pedicellate spikelet of ear
namespace: plant_structure
def: "The uppermost of the two florets of the pedicellate spikelet rachilla of a maize ear. The upper floret on the ear usually develops into a functional one." [GR:pj]
is_a: PO:0006354
relationship: part_of PO:0006348

[Term]
id: PO:0006351
name: lower floret of sessile spikelet of ear
namespace: plant_structure
def: "The lower of the two florets on the sessile spikelet of a maize ear." [GR:pj]
comment: This floret does not usually develop into a functional one.
is_a: PO:0006354
relationship: part_of PO:0006349

[Term]
id: PO:0006352
name: upper floret of sessile spikelet of ear
namespace: plant_structure
def: "One of the two florets placed above the lower floret on the sessile spikelet rachilla of a maize ear. This floret usually develops into a functional one." [GR:pj]
is_a: PO:0006354
relationship: part_of PO:0006349

[Term]
id: PO:0006353
name: lower floret of pedicellate spikelet of ear
namespace: plant_structure
def: "The lower of the two florets of the pedicellate spikelet rachilla of a maize ear." [GR:pj]
comment: The lower floret on the ear does not usually develop into a functional one.
is_a: PO:0006354
relationship: part_of PO:0006348

[Term]
id: PO:0006354
name: ear floret
namespace: plant_structure
def: "Small flowers of the spikelets of maize ear." [GR:pj]
is_a: PO:0006318
relationship: part_of PO:0006320

[Term]
id: PO:0006355
name: androecium of ear floret
namespace: plant_structure
def: "Collectively the stamens of maize ear floret. " [GR:pj]
comment: The development of the androecium in the ear floret of a normal maize plant is aborted and is present in a rudimentary state.
is_a: PO:0006471
relationship: part_of PO:0006354

[Term]
id: PO:0006356
name: lemma of tassel floret
namespace: plant_structure
def: "The lower of the two bracts enclosing a flower in a maize tassel floret." [GR:pj]
is_a: PO:0009037
relationship: part_of PO:0006310

[Term]
id: PO:0006357
name: gynoecium (sensu Zea)
namespace: plant_structure
def: "Collectively the carpels of a maize floret." [GR:pj]
is_a: PO:0006384

[Term]
id: PO:0006358
name: tassel spikelet pair meristem
namespace: plant_structure
def: "The meristem that produces two spikelet meristems\, each of which produces two floral meristems in a maize tassel." [GR:pj]
is_a: PO:0006328

[Term]
id: PO:0006359
name: palea of tassel floret
namespace: plant_structure
def: "In a maize tassel floret\, the upper of the two bracts enclosing a flower." [GR:pj]
is_a: PO:0009038
relationship: part_of PO:0006310

[Term]
id: PO:0006360
name: ear spikelet pair meristem
namespace: plant_structure
def: "Apical meristem that produces two spikelet meristems\, each of which produces two floral meristems in a maize ear." [GR:pj]
is_a: PO:0006328

[Term]
id: PO:0006361
name: palea of ear floret
namespace: plant_structure
def: "In a maize ear floret\, the upper of the two bracts enclosing a flower." [GR:pj]
is_a: PO:0009038
relationship: part_of PO:0006354

[Term]
id: PO:0006362
name: embryonic shoot apical meristem
namespace: plant_structure
def: "Meristem at the apex of the embryonic axis." [GR:pj]
is_a: PO:0020148
relationship: part_of PO:0019018

[Term]
id: PO:0006363
name: lemma of ear floret
namespace: plant_structure
def: "The lower of the two bracts enclosing a flower in a maize ear floret." [GR:pj]
is_a: PO:0009037
relationship: part_of PO:0006354

[Term]
id: PO:0006365
name: gynoecium of ear floret
namespace: plant_structure
def: "Collectively the carpels of a maize ear floret." [GR:pj]
is_a: PO:0006357
relationship: part_of PO:0006354

[Term]
id: PO:0006366
name: androecium of tassel floret
namespace: plant_structure
def: "Collectively the stamens of one floret of a tassel inflorescence of maize." [GR:pj]
is_a: PO:0006471
relationship: part_of PO:0006310

[Term]
id: PO:0006367
name: glume of ear spikelet
namespace: plant_structure
def: "A bract in the ear inflorescence of a maize plant\, subtending two florets." [GR:pj]
is_a: PO:0009039
relationship: part_of PO:0006320

[Term]
id: PO:0006368
name: glume of tassel spikelet
namespace: plant_structure
def: "A bract in the tassel inflorescence of a maize plant\, subtending two florets." [GR:pj]
is_a: PO:0009039
relationship: part_of PO:0006309

[Term]
id: PO:0006369
name: lower glume of ear spikelet
namespace: plant_structure
def: "The proximal/basal of the two glumes in the ear spikelet." [GR:pj]
is_a: PO:0006002
is_a: PO:0006367

[Term]
id: PO:0006370
name: upper glume of tassel spikelet
namespace: plant_structure
def: "The apical/distal of the two glumes in the tassel spikelet." [GR:pj]
is_a: PO:0006004
is_a: PO:0006368

[Term]
id: PO:0006371
name: upper glume of ear spikelet
namespace: plant_structure
def: "TThe apical/distal of the two glumes in the ear spikelet." [GR:pj]
is_a: PO:0006004
is_a: PO:0006367

[Term]
id: PO:0006372
name: lower glume of tassel spikelet
namespace: plant_structure
def: "The proximal/basal of the two glumes in the tassel spikelet." [GR:pj]
is_a: PO:0006002
is_a: PO:0006368

[Term]
id: PO:0006373
name: ear floret meristem
namespace: plant_structure
def: "Apical shoot meristem that gives rise to the organs of a maize ear floret." [GR:pj]
is_a: PO:0006329
relationship: part_of PO:0006320

[Term]
id: PO:0006374
name: tassel floret meristem
namespace: plant_structure
def: "Apical meristem that gives rise to the organs of a maize tassel floret." [GR:pj]
is_a: PO:0006329
relationship: part_of PO:0006309

[Term]
id: PO:0006375
name: ear meristem
namespace: plant_structure
def: "Apical shoot meristem that gives rise to the maize ear." [GR:pj]
is_a: PO:0000230
relationship: part_of PO:0020136

[Term]
id: PO:0006376
name: tassel meristem
namespace: plant_structure
def: "Apical meristem that gives rise to the tassel inflorescence." [GR:pj]
is_a: PO:0000230
relationship: part_of PO:0020126

[Term]
id: PO:0006377
name: tassel spikelet meristem
namespace: plant_structure
def: "Apical meristem that gives rise to the upper and lower florets of the maize tassel spikelets. " [GR:pj]
is_a: PO:0006327
relationship: part_of PO:0020126

[Term]
id: PO:0006378
name: ear spikelet meristem
namespace: plant_structure
def: "Apical meristem that gives rise to the upper and lower florets of the maize ear spikelets." [GR:pj]
is_a: PO:0006327
relationship: part_of PO:0020136

[Term]
id: PO:0006379
name: tassel spikelet rachilla
namespace: plant_structure
def: "The axis of the tassel spikelet\, above the glumes." [GR:pj]
is_a: PO:0009080
relationship: part_of PO:0006309

[Term]
id: PO:0006380
name: ear spikelet rachilla
namespace: plant_structure
def: "The axis of the ear spikelet\, above the glumes. " [GR:pj]
is_a: PO:0009080
relationship: part_of PO:0006320

[Term]
id: PO:0006381
name: lodicule of tassel floret
namespace: plant_structure
def: "In a tassel floret\, one of two or three tiny scales or flaps of tissue outside the stamens\, possibly representing reduced perianth segments." [APWeb:Glossary, GR:pj]
is_a: PO:0009036
relationship: part_of PO:0006310

[Term]
id: PO:0006382
name: lodicule of ear floret
namespace: plant_structure
def: "In a Maize ear floret\, one of two or three tiny scales or flaps of tissue outside the stamens\, possibly representing reduced perianth segments." [APWeb:Glossary, GR:pj]
is_a: PO:0009036
relationship: part_of PO:0006354

[Term]
id: PO:0006383
name: androecium (sensu Poaceae)
namespace: plant_structure
def: "Collectively the stamens of one grass floret." [GR:pj]
is_a: PO:0009061
relationship: part_of PO:0006318

[Term]
id: PO:0006384
name: gynoecium (sensu Poaceae)
namespace: plant_structure
def: "Collectively the carpels of a grass floret." [GR:pj]
is_a: PO:0009062
relationship: part_of PO:0006318

[Term]
id: PO:0006385
name: lower glume of pedicellate spikelet of tassel
namespace: plant_structure
def: "The proximal/basal of the two glumes in the tassel pedicellate spikelet." [GR:pj]
is_a: PO:0006372
relationship: part_of PO:0006312

[Term]
id: PO:0006386
name: lower glume of sessile spikelet of tassel
namespace: plant_structure
def: "The proximal/basal of the two glumes in the tassel sessile spikelet." [GR:pj]
is_a: PO:0006372
relationship: part_of PO:0006311

[Term]
id: PO:0006387
name: upper glume of sessile spikelet of tassel
namespace: plant_structure
def: "The apical/distal of the two glumes in a tassel sessile spikelet." [GR:pj]
is_a: PO:0006370
relationship: part_of PO:0006311

[Term]
id: PO:0006388
name: upper glume of pedicellate spikelet of tassel
namespace: plant_structure
def: "The apical/distal of the two glumes in a tassel pedicellate spikelet." [GR:pj]
is_a: PO:0006370
relationship: part_of PO:0006312

[Term]
id: PO:0006389
name: rachilla of sessile spikelet of tassel
namespace: plant_structure
def: "The axis of the tassel sessile spikelet\, above the glumes." [GR:pj]
is_a: PO:0006379
relationship: part_of PO:0006311
relationship: part_of PO:0006349

[Term]
id: PO:0006390
name: rachilla of pedicellate spikelet of tassel
namespace: plant_structure
def: "The axis of the tassel pedicellate spikelet\, above the glumes." [GR:pj]
is_a: PO:0006379
relationship: part_of PO:0006312

[Term]
id: PO:0006391
name: gynoecium of lower floret of sessile spikelet of tassel
namespace: plant_structure
def: "Collectively the carpels of a lower floret of sessile spikelet of maize tassel." [GR:pj]
comment: A non-functional or rudimentary gynoecium.
is_a: PO:0006317
relationship: part_of PO:0006315

[Term]
id: PO:0006392
name: androecium of upper floret of sessile spikelet of tassel
namespace: plant_structure
def: "Collectively the stamens of upper floret of a sessile spikelet of tassel inflorescence of maize." [GR:pj]
is_a: PO:0006366
relationship: part_of PO:0006316

[Term]
id: PO:0006393
name: androecium of lower floret of sessile spikelet of tassel
namespace: plant_structure
def: "Collectively the stamens of lower floret of a sessile spikelet of tassel inflorescence of maize." [GR:pj]
is_a: PO:0006366
relationship: part_of PO:0006315

[Term]
id: PO:0006394
name: gynoecium of upper floret of sessile spikelet of tassel
namespace: plant_structure
def: "Collectively the carpels of a upper floret of sessile spikelet of maize tassel." [GR:pj]
comment: A non-functional or rudimentary gynoecium.
is_a: PO:0006317
relationship: part_of PO:0006316

[Term]
id: PO:0006395
name: lemma of upper floret of sessile spikelet of tassel
namespace: plant_structure
def: "The lower of the two bracts enclosing a flower in a maize tassel sessile spikelet upper floret." [GR:pj]
is_a: PO:0006356
relationship: part_of PO:0006316

[Term]
id: PO:0006397
name: lemma of lower floret of sessile spikelet of tassel
namespace: plant_structure
def: "The lower of the two bracts enclosing a flower in a maize tassel sessile spikelet lower floret." [GR:pj]
is_a: PO:0006356
relationship: part_of PO:0006315

[Term]
id: PO:0006399
name: palea of lower floret of sessile spikelet of tassel
namespace: plant_structure
def: "The upper of the two bracts enclosing a flower in a maize tassel sessile spikelet lower floret." [GR:pj]
is_a: PO:0006359
relationship: part_of PO:0006315

[Term]
id: PO:0006401
name: palea of upper floret of sessile spikelet of tassel
namespace: plant_structure
def: "The upper of the two bracts enclosing a flower in a maize tassel sessile spikelet upper floret." [GR:pj]
is_a: PO:0006359
relationship: part_of PO:0006316

[Term]
id: PO:0006403
name: gynoecium of lower floret of pedicellate spikelet of tassel
namespace: plant_structure
def: "Collectively the carpels of a lower floret of pedicellate spikelet of maize tassel." [GR:pj]
comment: A non-functional or rudimentary gynoecium.
is_a: PO:0006317
relationship: part_of PO:0006313

[Term]
id: PO:0006404
name: gynoecium of upper floret of pedicellate spikelet of tassel
namespace: plant_structure
def: "Collectively the carpels of a upper floret of pedicellate spikelet of maize tassel." [GR:pj]
comment: A non-functional or rudimentary gynoecium.
is_a: PO:0006317
relationship: part_of PO:0006314

[Term]
id: PO:0006405
name: androecium of upper floret of pedicellate spikelet of tassel
namespace: plant_structure
def: "Collectively the stamens of upper floret of a pedicellate spikelet of tassel inflorescence of maize. " [GR:pj]
comment: This consitutes a functional androecium.
is_a: PO:0006366
relationship: part_of PO:0006314

[Term]
id: PO:0006406
name: androecium of lower floret of pedicellate spikelet of tassel
namespace: plant_structure
def: "Collectively the stamens of lower floret of a pedicellate spikelet of tassel inflorescence of maize." [GR:pj]
comment: This consitutes a functional androecium.
is_a: PO:0006366
relationship: part_of PO:0006313

[Term]
id: PO:0006407
name: lemma of lower floret of pedicellate spikelet of tassel
namespace: plant_structure
def: "The lower of the two bracts enclosing a flower in a maize tassel pedicellate spikelet lower floret." [GR:pj]
is_a: PO:0006356
relationship: part_of PO:0006313

[Term]
id: PO:0006409
name: lemma of upper floret of pedicellate spikelet of tassel
namespace: plant_structure
def: "The lower of the two bracts enclosing a flower in a maize tassel pedicellate spikelet upper floret." [GR:pj]
is_a: PO:0006356
relationship: part_of PO:0006314

[Term]
id: PO:0006411
name: palea of lower floret of pedicellate spikelet of tassel
namespace: plant_structure
def: "The upper of the two bracts enclosing a flower in a maize tassel pedicellate spikelet lower floret." [GR:pj]
is_a: PO:0006359
relationship: part_of PO:0006313

[Term]
id: PO:0006413
name: palea of upper floret of pedicellate spikelet of tassel
namespace: plant_structure
def: "The upper of the two bracts enclosing a flower in a maize tassel pedicellate spikelet upper floret." [GR:pj]
is_a: PO:0006359
relationship: part_of PO:0006314

[Term]
id: PO:0006415
name: pedicel of ear spikelet
namespace: plant_structure
def: "This is the ultimate branch of the pedicellate ear spikelet." [GR:pj]
is_a: PO:0006319
relationship: part_of PO:0006348

[Term]
id: PO:0006416
name: pedicel of tassel spikelet
namespace: plant_structure
def: "This is the ultimate branch of the pedicellate tassel spikelet." [GR:pj]
is_a: PO:0006319
relationship: part_of PO:0006312

[Term]
id: PO:0006417
name: tassel peduncle
namespace: plant_structure
def: "The axis of a maize tassel below the lowest tassel node." [GR:pj]
is_a: PO:0009053
relationship: part_of PO:0020126

[Term]
id: PO:0006418
name: ear peduncle
namespace: plant_structure
def: "The stalk of a maize ear below the lowest ear node." [GR:pj]
synonym: "lateral branch (sensu Zea)" []
synonym: "shank" []
is_a: PO:0009053
relationship: part_of PO:0020136

[Term]
id: PO:0006419
name: androecium of lower floret of pedicellate spikelet of ear
namespace: plant_structure
def: "Collectively the stamens of lower floret of a pedicellate spikelet of maize ear inflorescence." [GR:pj]
comment: The development of the androecium in the ear floret of a normal maize plant is aborted and is present in a rudimentary state.
is_a: PO:0006355
relationship: part_of PO:0006353

[Term]
id: PO:0006420
name: androecium of lower floret of sessile spikelet of ear
namespace: plant_structure
def: "Collectively the stamens of lower floret of a sessile spikelet of maize ear inflorescence. " [GR:pj]
comment: The development of the androecium in the ear floret of a normal maize plant is aborted and is present in a rudimentary state.
is_a: PO:0006355
relationship: part_of PO:0006351

[Term]
id: PO:0006421
name: androecium of upper floret of sessile spikelet of ear
namespace: plant_structure
def: "Collectively the stamens of upper floret of a sessile spikelet of maize ear inflorescence. " [GR:pj]
comment: The development of the androecium in the ear floret of a normal maize plant is aborted and is present in a rudimentary state.
is_a: PO:0006355
relationship: part_of PO:0006352

[Term]
id: PO:0006422
name: androecium of upper floret of pedicellate spikelet of ear
namespace: plant_structure
def: "Collectively the stamens of upper floret of a pedicellate spikelet of maize ear inflorescence. " [GR:pj]
comment: The development of the androecium in the ear floret of a normal maize plant is aborted and is present in a rudimentary state.
is_a: PO:0006355
relationship: part_of PO:0006350

[Term]
id: PO:0006423
name: gynoecium of lower floret of sessile spikelet of ear
namespace: plant_structure
def: "Collectively the carpels of a lower floret of sessile spikelet of maize ear." [GR:pj]
comment: A non-functional or rudimentary gynoecium.
is_a: PO:0006365
relationship: part_of PO:0006351

[Term]
id: PO:0006424
name: gynoecium of lower floret of pedicellate spikelet of ear
namespace: plant_structure
def: "Collectively the carpels of a lower floret of pedicellate spikelet of a maize ear. " [GR:pj]
comment: A non-functional or rudimentary gynoecium.
is_a: PO:0006365
relationship: part_of PO:0006353

[Term]
id: PO:0006425
name: gynoecium of upper floret of sessile spikelet of ear
namespace: plant_structure
def: "Collectively the carpels of a upper floret of sessile spikelet of maize ear." [GR:pj]
comment: A functional gynoecium.
is_a: PO:0006365
relationship: part_of PO:0006352

[Term]
id: PO:0006426
name: gynoecium of upper floret of pedicellate spikelet of ear
namespace: plant_structure
def: "Collectively the carpels of a upper floret of pedicellate spikelet of maize ear." [GR:pj]
comment: A functional gynoecium.
is_a: PO:0006365
relationship: part_of PO:0006350

[Term]
id: PO:0006427
name: palea of upper floret of sessile spikelet of ear
namespace: plant_structure
def: "The upper of the two bracts enclosing a flower in a maize ear sessile spikelet upper floret." [GR:pj]
is_a: PO:0006361
relationship: part_of PO:0006352

[Term]
id: PO:0006428
name: palea of lower floret of sessile spikelet of ear
namespace: plant_structure
def: "The upper of the two bracts enclosing a flower in a maize ear sessile spikelet lower floret." [GR:pj]
is_a: PO:0006361
relationship: part_of PO:0006351

[Term]
id: PO:0006429
name: palea of upper floret of pedicellate spikelet of ear
namespace: plant_structure
def: "The upper of the two bracts enclosing a flower in a maize ear pedicellate spikelet upper floret." [GR:pj]
is_a: PO:0006361
relationship: part_of PO:0006350

[Term]
id: PO:0006430
name: palea of lower floret of pedicellate spikelet of ear
namespace: plant_structure
def: "The upper of the two bracts enclosing a flower in a maize ear pedicellate spikelet lower floret." [GR:pj]
is_a: PO:0006361
relationship: part_of PO:0006353

[Term]
id: PO:0006431
name: lemma of lower floret of pedicellate spikelet of ear
namespace: plant_structure
def: "The lower of the two bracts enclosing a flower in a maize ear pedicellate spikelet lower floret." [GR:pj]
is_a: PO:0006363
relationship: part_of PO:0006353

[Term]
id: PO:0006432
name: lemma of upper floret of pedicellate spikelet of ear
namespace: plant_structure
def: "The lower of the two bracts enclosing a flower in a maize ear pedicellate spikelet upper floret." [GR:pj]
is_a: PO:0006363
relationship: part_of PO:0006350

[Term]
id: PO:0006433
name: lemma of lower floret of sessile spikelet of ear
namespace: plant_structure
def: "The lower of the two bracts enclosing a flower in a maize ear sessile spikelet lower floret." [GR:pj]
is_a: PO:0006363
relationship: part_of PO:0006351

[Term]
id: PO:0006434
name: lemma of upper floret of sessile spikelet of ear
namespace: plant_structure
def: "The lower of the two bracts enclosing a flower in a maize ear sessile spikelet upper floret." [GR:pj]
is_a: PO:0006363
relationship: part_of PO:0006352

[Term]
id: PO:0006435
name: rachilla of pedicellate spikelet of ear
namespace: plant_structure
def: "The axis of the ear pedicellate spikelet\, above the glumes." [GR:pj]
is_a: PO:0006380
relationship: part_of PO:0006348

[Term]
id: PO:0006436
name: rachilla of sessile spikelet of ear
namespace: plant_structure
def: "The axis of the ear sessile spikelet\, above the glumes." [GR:pj]
is_a: PO:0006380

[Term]
id: PO:0006437
name: lower glume of pedicellate spikelet of ear
namespace: plant_structure
def: "The proximal/basal of the two glumes in the ear pedicellate spikelet." [GR:pj]
is_a: PO:0006369
relationship: part_of PO:0006348

[Term]
id: PO:0006438
name: lower glume of sessile spikelet of ear
namespace: plant_structure
def: "The proximal/basal of the two glumes in the ear sessile spikelet." [GR:pj]
is_a: PO:0006369
relationship: part_of PO:0006349

[Term]
id: PO:0006439
name: upper glume of pedicellate spikelet of ear
namespace: plant_structure
def: "The apical/distal of the two glumes in the pedicellate spikelet." [GR:pj]
is_a: PO:0006371
relationship: part_of PO:0006348

[Term]
id: PO:0006440
name: upper glume of sessile spikelet of ear
namespace: plant_structure
def: "The apical/distal of the two glumes in the sessile spikelet." [GR:pj]
is_a: PO:0006371
relationship: part_of PO:0006349

[Term]
id: PO:0006441
name: stamen (sensu Poaceae)
namespace: plant_structure
def: "A microsporophyll\, bearing four microsporangia in a grass floret." [GR:pj]
is_a: PO:0009029
relationship: part_of PO:0006383

[Term]
id: PO:0006442
name: anther (sensu Poaceae)
namespace: plant_structure
def: "The pollen-bearing part of a stamen of a grass floret." [GR:pj]
is_a: PO:0009066
relationship: part_of PO:0006441

[Term]
id: PO:0006443
name: connective (sensu Poaceae)
namespace: plant_structure
def: "The part of the stamen of a grass floret\, that connects the microsporangia/pollen sacs." [GR:pj]
is_a: PO:0009068
relationship: part_of PO:0006442

[Term]
id: PO:0006444
name: microsporangium (sensu Poaceae)
namespace: plant_structure
def: "Sporangium in the anther of a grass stamen producing microspores\, usually many in number." [GR:pj]
is_a: PO:0009070
relationship: part_of PO:0006442

[Term]
id: PO:0006445
name: anther wall (sensu Poaceae)
namespace: plant_structure
def: "A multicellular layer with outer epidermis and an inner endothecium of an anther of a grass stamen." [GR:pj]
is_a: PO:0000002
relationship: part_of PO:0006444

[Term]
id: PO:0006446
name: endothecium (sensu Poaceae)
namespace: plant_structure
def: "The hypodermis of an anther sac of a grass stamen with distinctively thickened walls and involved in its dehiscence." [GR:pj]
is_a: PO:0020002
relationship: part_of PO:0006445

[Term]
id: PO:0006447
name: exothecium (sensu Poaceae)
namespace: plant_structure
def: "The epidermis of an anther sac of a grass stamen." [GR:pj]
is_a: PO:0020004
relationship: part_of PO:0006445

[Term]
id: PO:0006448
name: placentoid (sensu Poaceae)
namespace: plant_structure
def: "An inpushing of the anther wall of a grass stamen." [GR:pj]
is_a: PO:0020005
relationship: part_of PO:0006445

[Term]
id: PO:0006449
name: stomium (sensu Poaceae)
namespace: plant_structure
def: "A fissure in the anther lobe through which the pollen is released in grasses." [GR:pj]
is_a: PO:0020101
relationship: part_of PO:0006445

[Term]
id: PO:0006450
name: tapetum (sensu Poaceae)
namespace: plant_structure
def: "Innermost part of the anther wall\, involved in the nutrition of the pollen in grasses." [GR:pj]
is_a: PO:0009071
relationship: part_of PO:0006445

[Term]
id: PO:0006451
name: microsporocyte (sensu Poaceae)
namespace: plant_structure
def: "A diploid (2n) cell that undergoes meiosis and produces four haploid (1n) microspores in a grass plant." [GR:pj]
is_a: PO:0020047
relationship: part_of PO:0006444

[Term]
id: PO:0006452
name: microspore (sensu Poaceae)
namespace: plant_structure
def: "The smaller\, in general\, of the two kinds of spores produced in the life cycle of a grass plant. It gives rise to the male gametophyte." [GR:pj]
is_a: PO:0020048
relationship: develops_from PO:0006451

[Term]
id: PO:0006453
name: theca (sensu Poaceae)
namespace: plant_structure
def: "A part of the anther of a grass stamen consisting of paired sporangia that dehisce down a common slit." [GR:pj]
is_a: PO:0006444
is_a: PO:0009069

[Term]
id: PO:0006454
name: filament (sensu Poaceae)
namespace: plant_structure
def: "The stalk of the stamen of a grass floret." [GR:pj]
is_a: PO:0009067
relationship: part_of PO:0006441

[Term]
id: PO:0006455
name: carpel (sensu Poaceae)
namespace: plant_structure
def: "A megasporophyll at the center of a grass floret enclosing the ovule." [GR:pj]
is_a: PO:0009030
relationship: part_of PO:0006384

[Term]
id: PO:0006456
name: ovary (sensu Poaceae)
namespace: plant_structure
def: "The basal portion of a carpel that encloses the ovule(s) in a grass floret." [GR:pj]
is_a: PO:0009072
relationship: part_of PO:0006455

[Term]
id: PO:0006457
name: ovule (sensu Poaceae)
namespace: plant_structure
def: "A stalked or sessile structure in a grass carpel within which one or more megaspores are formed and later the female gametophyte or embryo sac develops." [GR:pj]
is_a: PO:0020003
relationship: part_of PO:0006456

[Term]
id: PO:0006458
name: chalaza (sensu Poaceae)
namespace: plant_structure
def: "Region in the grass ovule where the integuments and the nucellus merge with the funiculus." [GR:pj]
is_a: PO:0020026
relationship: part_of PO:0006457

[Term]
id: PO:0006459
name: outer integumet (sensu Poaceae)
namespace: plant_structure
def: "One of the two layers of tissue that usually covers the ovule of a grass\, contiguous to the inner integument and usually involved in forming the micropyle at the apex." [GR:pj]
is_a: PO:0020023
relationship: part_of PO:0006465

[Term]
id: PO:0006460
name: inner integument (sensu Poaceae)
namespace: plant_structure
def: "The innermost of the two layers of tissue that cover the ovule of a grass\, contiguous to the nucellus and usually involved in forming the micropyle at the apex." [GR:pj]
is_a: PO:0020022
relationship: part_of PO:0006465

[Term]
id: PO:0006461
name: micropyle (sensu Poaceae)
namespace: plant_structure
def: "A small canal through the inner integument(s) at the apex of a grass ovule." [GR:pj]
is_a: PO:0020025
relationship: part_of PO:0006457

[Term]
id: PO:0006462
name: nucellus (sensu Poaceae)
namespace: plant_structure
def: "Subepidermal tissue in the ovule of a grass plant surrounding the megasporocyte." [GR:pj]
is_a: PO:0020020
relationship: part_of PO:0006457

[Term]
id: PO:0006463
name: megasporocyte (sensu Poaceae)
namespace: plant_structure
def: "A diploid (2n) cell that undergoes meiosis and produces four haploid (1n) megaspores in a grass plant." [GR:pj]
is_a: PO:0000431
relationship: part_of PO:0006462

[Term]
id: PO:0006464
name: megaspore (sensu Poaceae)
namespace: plant_structure
def: "The larger\, in general\, of the two kinds of spores produced after meiosis in the life cycle of a grass plant\, and on germination giving rise to the female gametophyte (embryo sac)." [GR:pj]
is_a: PO:0020019
relationship: develops_from PO:0006463

[Term]
id: PO:0006465
name: integument (sensu Poaceae)
namespace: plant_structure
def: "One of the layers of tissue that covers the ovule of a grass carpel\, enveloping the nucellus and forming the micropyle at the apex." [GR:pj]
is_a: PO:0020021
relationship: part_of PO:0006457

[Term]
id: PO:0006466
name: funicle (sensu Poaceae)
namespace: plant_structure
def: "The stalk which attaches the ovule to the placenta in a grass carpel." [GR:pj]
is_a: PO:0020006
relationship: part_of PO:0006456

[Term]
id: PO:0006467
name: placenta (sensu Poaceae)
namespace: plant_structure
def: "The region within an ovary to which ovules are attached in a grass carpel." [GR:pj]
is_a: PO:0020001
relationship: part_of PO:0006456

[Term]
id: PO:0006468
name: stigma (sensu Poaceae)
namespace: plant_structure
def: "The apical part of a carpel of a grass floret on which the pollen germinates." [GR:pj]
is_a: PO:0009073
relationship: part_of PO:0006455

[Term]
id: PO:0006469
name: style (sensu Poaceae)
namespace: plant_structure
def: "An elongated part of a carpel between the ovary and the stigma of a grass floret\, through which the pollen tube grows." [GR:pj]
is_a: PO:0009074
relationship: part_of PO:0006455

[Term]
id: PO:0006470
name: carpel (sensu Zea)
namespace: plant_structure
def: "A megasporophyll at the center of a maize floret enclosing the ovule." [GR:pj]
is_a: PO:0006455
relationship: part_of PO:0006365

[Term]
id: PO:0006471
name: androecium (sensu Zea)
namespace: plant_structure
def: "Collectively the stamens of one floret of a maize plant." [GR:pj]
is_a: PO:0006383

[Term]
id: PO:0006472
name: stamen (sensu Zea)
namespace: plant_structure
def: "A microsporophyll bearing four microsporangia in a maize floret." [GR:pj]
is_a: PO:0006441
relationship: part_of PO:0006366

[Term]
id: PO:0006473
name: anther (sensu Zea)
namespace: plant_structure
def: "The pollen-bearing part of a stamen of a maize floret." [GR:pj]
is_a: PO:0006442
relationship: part_of PO:0006472

[Term]
id: PO:0006474
name: filament (sensu Zea)
namespace: plant_structure
def: "The stalk of the stamen of a maize floret." [GR:pj]
is_a: PO:0006454
relationship: part_of PO:0006472

[Term]
id: PO:0006475
name: connective (sensu Zea)
namespace: plant_structure
def: "The part of the stamen of a maize floret\, that connects the microsporangia or pollen sacs " [GR:pj]
is_a: PO:0006443
relationship: part_of PO:0006473

[Term]
id: PO:0006476
name: microsporangium (sensu Zea)
namespace: plant_structure
def: "Sporangium in the anther of a maize stamen producing microspores\, usually many in number ." [GR:pj]
is_a: PO:0006444
relationship: part_of PO:0006473

[Term]
id: PO:0006477
name: anther wall (sensu Zea)
namespace: plant_structure
def: "A multicellular layer with outer epidermis and an inner endothecium of an anther of a maize stamen." [GR:pj]
is_a: PO:0006445
relationship: part_of PO:0006476

[Term]
id: PO:0006478
name: theca (sensu Zea)
namespace: plant_structure
def: "A part of the anther of a maize stamen consisting of paired sporangia that dehisce down a common slit." [GR:pj]
is_a: PO:0006453
is_a: PO:0006476

[Term]
id: PO:0006479
name: microsporocyte (sensu Zea)
namespace: plant_structure
def: "A diploid (2n) cell that undergoes meiosis and produces four haploid (1n) microspores in a maize plant." [GR:pj]
is_a: PO:0006451
relationship: part_of PO:0006476

[Term]
id: PO:0006480
name: microspore (sensu Zea)
namespace: plant_structure
def: "The smaller\, in general\, of the two kinds of spores produced in the life cycle of a maize plant. It gives rise to the male gametophyte." [GR:pj]
is_a: PO:0006452
relationship: develops_from PO:0006479

[Term]
id: PO:0006481
name: endothecium (sensu Zea)
namespace: plant_structure
def: "The hypodermis of an anther sac of a maize stamen with distinctively thickened walls and involved in its dehiscence." [GR:pj]
is_a: PO:0006446
relationship: part_of PO:0006477

[Term]
id: PO:0006482
name: exothecium (sensu Zea)
namespace: plant_structure
def: "The epidermis of an anther sac of a maize stamen." [GR:pj]
is_a: PO:0006447
relationship: part_of PO:0006477

[Term]
id: PO:0006483
name: placentoid (sensu Zea)
namespace: plant_structure
def: "An inpushing of the anther wall of a maize stamen." [GR:pj]
is_a: PO:0006448
relationship: part_of PO:0006477

[Term]
id: PO:0006484
name: tapetum (sensu Zea)
namespace: plant_structure
def: "Innermost part of the anther wall\, involved in the nutrition of the pollen in maize." [GR:pj]
is_a: PO:0006450
relationship: part_of PO:0006477

[Term]
id: PO:0006485
name: stomium (sensu Zea)
namespace: plant_structure
def: "A fissure in the anther lobe through which the pollen is released in maize." [GR:pj]
is_a: PO:0006449
relationship: part_of PO:0006477

[Term]
id: PO:0006486
name: ovary (sensu Zea)
namespace: plant_structure
def: "The basal portion of a carpel that encloses the ovule(s) in a maize floret." [GR:pj]
is_a: PO:0006456
relationship: part_of PO:0006470

[Term]
id: PO:0006487
name: stigma (sensu Zea)
namespace: plant_structure
def: "The apical part of a carpel of a maize floret on which the pollen germinates." [GR:pj]
is_a: PO:0006468
relationship: part_of PO:0006470

[Term]
id: PO:0006488
name: silk
namespace: plant_structure
def: "The style of a maize floret." [GR:pj]
synonym: "style (sensu Zea)" []
is_a: PO:0006469
relationship: part_of PO:0006470

[Term]
id: PO:0006489
name: funicle (sensu Zea)
namespace: plant_structure
def: "The stalk which attaches the ovule to the placenta in a maize carpel." [GR:pj]
is_a: PO:0006466
relationship: part_of PO:0006486

[Term]
id: PO:0006490
name: placenta (sensu Zea)
namespace: plant_structure
def: "The region within an ovary to which ovules are attached in a maize carpel." [GR:pj]
is_a: PO:0006467
relationship: part_of PO:0006486

[Term]
id: PO:0006491
name: ovule (sensu Zea)
namespace: plant_structure
def: "A stalked or sessile structure in a maize carpel within which one or more megaspores are formed and later the female gametophyte or embryo sac develops." [GR:pj]
is_a: PO:0006457
relationship: part_of PO:0006486

[Term]
id: PO:0006492
name: nucellus (sensu Zea)
namespace: plant_structure
def: "Subepidermal tissue in the ovule of a maize plant surrounding the megasporocyte." [GR:pj]
is_a: PO:0006462
relationship: part_of PO:0006491

[Term]
id: PO:0006493
name: megasporocyte (sensu Zea)
namespace: plant_structure
def: "A diploid (2n) cell that undergoes meiosis and produces four haploid (1n) megaspores in a maize plant." [GR:pj]
is_a: PO:0006463
relationship: part_of PO:0006492

[Term]
id: PO:0006494
name: megaspore (sensu Zea)
namespace: plant_structure
def: "The larger\, in general\, of the two kinds of spores produced after meiosis in the life cycle of a maize plant\, and on germination giving rise to the female gametophyte (embryo sac)." [GR:pj]
is_a: PO:0006464
relationship: develops_from PO:0006493

[Term]
id: PO:0006495
name: degenerate megaspore (sensu Poaceae)
namespace: plant_structure
def: "The megaspores in a grass plant that would not participate in megagametogenesis." [GR:pj]
is_a: PO:0000245
is_a: PO:0006464

[Term]
id: PO:0006496
name: functional megaspore (sensu Poaceae)
namespace: plant_structure
def: "The megaspore that forms the embryo sac in grasses." [GR:pj]
is_a: PO:0000244
is_a: PO:0006464

[Term]
id: PO:0006497
name: stigma epidermis (sensu Poaceae)
namespace: plant_structure
def: "The epidermal cell layer of the grass stigma." [GR:pj]
is_a: PO:0006061
relationship: part_of PO:0006468

[Term]
id: PO:0006498
name: style epidermis (sensu Poaceae)
namespace: plant_structure
def: "The epidermal cell layer of the style of a grass carpel." [GR:pj]
is_a: PO:0006062
relationship: part_of PO:0006469

[Term]
id: PO:0006499
name: transmitting tissue (sensu Poaceae)
namespace: plant_structure
def: "Tissue in the style of a grass carpel\, through which the pollen tube grows; it connects the stigma and the inside of ovary." [GR:pj]
is_a: PO:0020102
relationship: part_of PO:0006469

[Term]
id: PO:0006500
name: ovary epidermis (sensu Poaceae)
namespace: plant_structure
def: "The epidermal cell layer of the ovary of a grass carpel." [GR:pj]
is_a: PO:0006063
relationship: part_of PO:0006456

[Term]
id: PO:0006501
name: leaf abscission zone
namespace: plant_structure
def: "Zone at base of the leaf that contains an abscission (or separation) layer and a protective layer\, both involved in the abscission of the leaf." [GR:pj]
is_a: PO:0000146
relationship: part_of PO:0009025

[Term]
id: PO:0006502
name: flower abscission zone
namespace: plant_structure
def: "Zone at base of the flower that contains an abscission (or separation) layer and a protective layer\, both involved in the abscission of the flower and its parts." [GR:pj]
is_a: PO:0000146
relationship: part_of PO:0009046

[Term]
id: PO:0006503
name: fruit abscission zone
namespace: plant_structure
def: "Zone at base of the fruit that contains an abscission (or separation) layer and a protective layer\, both involved in the abscission of the fruit." [GR:pj]
is_a: PO:0000146
relationship: part_of PO:0009001

[Term]
id: PO:0006504
name: leaf trichome
namespace: plant_structure
def: "Trichome on/from the epidermis of a leaf." [GR:pj]
is_a: PO:0000282
relationship: part_of PO:0006018
relationship: part_of PO:0006019

[Term]
id: PO:0006505
name: central spike of ear
namespace: plant_structure
def: "The inflorescence axis of the ear." [GR:pj]
synonym: "cob (sensu zea)" []
synonym: "ear rachis" []
is_a: PO:0020122
relationship: part_of PO:0020136

[Term]
id: PO:0006506
name: chalaza (sensu Zea)
namespace: plant_structure
def: "Region in the maize ovule where the integuments and the nucellus merge with the funiculus." [GR:pj]
is_a: PO:0006458
relationship: part_of PO:0006491

[Term]
id: PO:0006507
name: integument (sensu Zea)
namespace: plant_structure
def: "One of the layers of tissue that covers the ovule of a maize carpel\, enveloping the nucellus and forming the micropyle at the apex." [GR:pj]
is_a: PO:0006465
relationship: part_of PO:0006491

[Term]
id: PO:0006508
name: integument epidermis (sensu Poaceae)
namespace: plant_structure
def: "The epidermis of an integument in a grass ovule." [GR:pj]
is_a: PO:0006043
relationship: part_of PO:0006465

[Term]
id: PO:0009001
name: fruit
alt_id: PO:0020067
alt_id: PO:0020068
alt_id: PO:0020069
alt_id: PO:0020070
alt_id: PO:0020071
alt_id: PO:0020072
alt_id: PO:0020073
alt_id: PO:0020074
alt_id: PO:0020076
alt_id: PO:0020077
alt_id: PO:0020078
alt_id: PO:0020079
alt_id: PO:0020080
alt_id: PO:0020082
alt_id: PO:0020083
alt_id: PO:0020087
alt_id: PO:0020107
namespace: plant_structure
def: "The seed-bearing structure in angiosperms\, formed from the ovary after flowering." [Poc:curators, APWeb:Glossary]
synonym: "achene" []
synonym: "berry" []
synonym: "capsule" []
synonym: "caryopsis" []
synonym: "circumcissile capsule" []
synonym: "cypsela" []
synonym: "drupe" []
synonym: "follicle" []
synonym: "grain" []
synonym: "kernel" []
synonym: "legume" []
synonym: "loculicidal capsule" []
synonym: "lomentum" []
synonym: "nut" []
synonym: "pod" []
synonym: "poricidal capsule" []
synonym: "schizocarp" []
synonym: "septicidal capsule" []
synonym: "septifragal capsule" []
synonym: "silicula" []
synonym: "siliqua" []
synonym: "silique" []
relationship: part_of PO:0006342

[Term]
id: PO:0009002
name: cell
namespace: plant_structure
def: "Structural and physiological unit of a living organism; it (i.e.\, plant cell) consists of protoplast and cell wall; in nonliving state\, of cell wall only\, or cell wall and some nonliving inclusions." [ISBN:0471245208]
is_a: PO:0009011

[Term]
id: PO:0009003
name: sporophyte
namespace: plant_structure
def: "A diploid plant\, or phase of a life cycle\, that bears spores formed by meiosis." [APWeb:Glossary]
is_a: PO:0009011

[Term]
id: PO:0009004
name: gametophyte
namespace: plant_structure
def: "A haploid plant\, or phase of a plant's life cycle\, that bears gametes after mitotic events." [APWeb:Glossary]
is_a: PO:0009011

[Term]
id: PO:0009005
name: root
alt_id: PO:0003006
namespace: plant_structure
def: "An axial system which is usually underground and more or less positively geotropic\, does not bear leaves and only rarely shoots\, is endogenous in origin\, indeterminate in growth and often with secondary thickening." [APWeb:Glossary]
comment: Commonly thought of as one of the three basic parts of the seed plant body.
synonym: "aerial root" []
relationship: part_of PO:0009003

[Term]
id: PO:0009006
name: shoot
namespace: plant_structure
def: "All the parts developed that can trace their origin to the apical cell of the two celled embryo." [Poc:curators]
relationship: part_of PO:0009003

[Term]
id: PO:0009007
name: tissue
namespace: plant_structure
def: "Group of cells organized into a structural and functional unit; the component cells may be alike (simple tissue) or varied (complex tissue)." [TAIR:lr]
is_a: PO:0009011

[Term]
id: PO:0009008
name: organ
namespace: plant_structure
def: "OBSOLETE. A natural part or structure in a plant\, capable of performing some special action (termed its function)\, which is essential to the life or well-being of the whole." [MaizeGDB:lv]
comment: All organs are represented under sporophyte.
is_obsolete: true

[Term]
id: PO:0009009
name: embryo
namespace: plant_structure
def: "A young sporophyte contained within a seed." [APWeb:Glossary, GR:pj]
relationship: part_of PO:0009010

[Term]
id: PO:0009010
name: seed
namespace: plant_structure
def: "A propagating organ formed in the reproductive cycle of gymnosperms and angiosperms\, derived from the ovule and enclosing an embryo." [APWeb:Glossary, GR:pj]
comment: The seed is representative of a next generation of sporophyte.
is_a: PO:0009003
relationship: part_of PO:0009001

[Term]
id: PO:0009011
name: plant structure
namespace: plant_structure
def: "Any morphological or anatomical feature of a plant." [Poc:curators]

[Term]
id: PO:0009013
name: meristem
namespace: plant_structure
def: "Regions of a plant in which cells that have retained their embryonic characteristics\, or have reverted to them secondarily\, and that divide to produce new cells that can undergo differentiation to form mature tissues\, i.e. they have a capacity for morphogenesis and growth." [APWeb:Glossary, GR:pj]
is_a: PO:0009007

[Term]
id: PO:0009014
name: dermal tissue
namespace: plant_structure
def: "Tissue derived from the protoderm that covers the surface of the plant body." [GR:pj, ISBN:0122151704]
is_a: PO:0009007

[Term]
id: PO:0009015
name: vascular tissue
namespace: plant_structure
def: "Conducting tissues made up of xylem and phloem." [APWeb:Glossary]
comment: In the stem it is often found as a stele\, surrounded by the cortex and surrounding the pith.
relationship: part_of PO:0000034

[Term]
id: PO:0009016
name: ground tissue
namespace: plant_structure
def: "OBSOLETE. Tissues other than the vascular tissues\, epidermis and the periderm." [GR:pj]
comment: Uninformative definition. Check it again.
is_obsolete: true

[Term]
id: PO:0009020
name: meristem L1
namespace: plant_structure
def: "The outermost layer of the shoot apical meristem which gives rise to the shoot epidermis." [PMID:12221985, GR:pj]
relationship: part_of PO:0020148

[Term]
id: PO:0009021
name: meristem L2
namespace: plant_structure
def: "The cell layer beneath the L1 layer in the shoot meristem which gives rise to subepidermal tissue." [PMID:12221985, GR:pj]
relationship: part_of PO:0020148

[Term]
id: PO:0009022
name: meristem L3
namespace: plant_structure
def: "The multicellular layer beneath the L2 layer in the shoot meristem which gives rise to internal tissues of leaf and stem." [PMID:12221985, GR:pj]
relationship: part_of PO:0020148

[Term]
id: PO:0009025
name: leaf
namespace: plant_structure
def: "Commonly thought of as one of the three basic parts of the seed plant body\, a structure usually of determinate growth\, without secondary thickening\, and of superficial origin\, often flattened and photosynthetic in part\, and in the axil of which is found a bud." [APWeb:Glossary]
synonym: "foliage leaf" []
is_a: PO:0006001

[Term]
id: PO:0009026
name: sporophyll
namespace: plant_structure
def: "A leaf-like organ on which one or more sporangia are borne." [APWeb:Glossary]
is_a: PO:0006001

[Term]
id: PO:0009027
name: megasporophyll
namespace: plant_structure
def: "A structure upon which (or in the axil of which) one or more megasporangia are borne; in flowering plants\, a carpel." [APWeb:Glossary]
is_a: PO:0009026

[Term]
id: PO:0009028
name: microsporophyll
namespace: plant_structure
def: "A structure on which one or more microsporangia are borne; in flowering plants\, the stamen." [APWeb:Glossary]
is_a: PO:0009026

[Term]
id: PO:0009029
name: stamen
namespace: plant_structure
def: "A microsporophyll bearing one or more microsporangia." [APWeb:Glossary]
is_a: PO:0009028
relationship: part_of PO:0009061

[Term]
id: PO:0009030
name: carpel
namespace: plant_structure
def: "A megasporophyll\, almost always at the center of a flower\, its margins more or less fused together or with other carpels to enclose the ovule(s).\n" [APWeb:Glossary]
comment: If carpels are fused\, the gynoecium is a syncarpous gynoecium\, as in Poaceae\, Brassicaceae and Solanaceae.  If carpels are free\, the gynoecium is an apocarpous gynoecium\, as in Fabaceae.
is_a: PO:0009027
relationship: part_of PO:0009062

[Term]
id: PO:0009031
name: sepal
namespace: plant_structure
def: "A member of the (usually green) outer whorl of non-fertile parts surrounding the fertile organs of a flower." [APWeb:Glossary]
relationship: part_of PO:0009060

[Term]
id: PO:0009032
name: petal
namespace: plant_structure
def: "A member of the corolla\, the inner whorl of non-fertile parts surrounding the fertile organs of a flower\, usually soft and colored conspicuously." [APWeb:Glossary]
relationship: part_of PO:0009059

[Term]
id: PO:0009033
name: tepal
namespace: plant_structure
def: "A perianth segment in a flower in which there are two whorls of such segments\, but all are similar in appearance." [APWeb:Glossary]
relationship: part_of PO:0009058

[Term]
id: PO:0009034
name: floral bract
namespace: plant_structure
def: "Leaf like structure subtending a flower." [Poc:curators]
synonym: "chaff" []
is_a: PO:0009055
relationship: part_of PO:0009049

[Term]
id: PO:0009035
name: nectary
namespace: plant_structure
def: "A multicellular glandular structure secreting a liquid containing organic substances especially sugars." [GR:pj]
relationship: part_of PO:0009006

[Term]
id: PO:0009036
name: lodicule
namespace: plant_structure
def: "In a grass floret\, one of two or three tiny scales or flaps of tissue outside the stamens\, possibly representing reduced perianth segments." [APWeb:Glossary]
relationship: part_of PO:0006318

[Term]
id: PO:0009037
name: lemma
namespace: plant_structure
def: "In a grass floret\, the lower of two bracts enclosing a flower." [APWeb:Glossary, GR:pj]
is_a: PO:0009034
relationship: part_of PO:0006318

[Term]
id: PO:0009038
name: palea
namespace: plant_structure
def: "In a grass floret\, the upper of the two bracts enclosing a flower." [APWeb:Glossary, GR:pj]
comment: Possibly a prophyll/bracteole.
is_a: PO:0009034
relationship: part_of PO:0006318

[Term]
id: PO:0009039
name: glume
alt_id: PO:0006026
namespace: plant_structure
def: "A \"bract\" in the inflorescence of a grass\, sedge or similar plant." [APWeb:Glossary, GR:pj]
synonym: "rudimentary glume" []
is_a: PO:0009054
relationship: part_of PO:0009051

[Term]
id: PO:0009040
name: sterile lemma
alt_id: PO:0006029
namespace: plant_structure
def: "A bract in the position of a lemma\, but not enclosing floral organs" [UMSL:tk]
comment: An undeveloped androecium or gynoecium may or may not be detectable.
synonym: "empty glume" []
is_a: PO:0009037

[Term]
id: PO:0009041
name: fertile lemma
namespace: plant_structure
def: "A lemma that encloses a functional flower\, with androecium\, gynoecium or both." [UMSL:tk]
is_a: PO:0009037

[Term]
id: PO:0009042
name: prophyll
namespace: plant_structure
def: "The first leaf or two leaves formed at the base of an axillary shoot\, often smaller and/or in a distinctively different position from those formed subsequently." [APWeb:Glossary]
is_a: PO:0006001

[Term]
id: PO:0009043
name: bracteole
namespace: plant_structure
def: "A small leaf or leaves borne singly or in pairs on the pedicel\, the prophyll(s) of the flower-shoot (pedicel plus flower)." [APWeb:Glossary]
is_a: PO:0009042
relationship: part_of PO:0009052

[Term]
id: PO:0009044
name: perigynium
namespace: plant_structure
def: "Sac-like bract subtending the pistillate flower\, as in Carex." [GR:pj]
is_a: PO:0009042

[Term]
id: PO:0009045
name: phyllary
namespace: plant_structure
def: "Equals inflorescence bract of an involucre\, as in Asteraceae." [APWeb:Glossary]
is_a: PO:0009054

[Term]
id: PO:0009046
name: flower
namespace: plant_structure
def: "A heterosporangiate strobilus\, typically consisting of androecium\, gynoecium\, usually surrounded by a perianth and borne on an axis or receptacle." [APWeb:Glossary, GR:pj]
comment: The characteristic reproductive structure of angiosperms.
relationship: part_of PO:0009049

[Term]
id: PO:0009047
name: stem
namespace: plant_structure
def: "The axial system of plants that bears leaves and buds.\n" [APWeb:Glossary]
comment: It is usually above ground and more or less negatively geotropic\, is exogenous in origin\, often indeterminate in growth and with secondary thickening.
synonym: "cane" []
synonym: "culm" []
synonym: "stalk" []
relationship: part_of PO:0009006

[Term]
id: PO:0009049
name: inflorescence
alt_id: PO:0009048
alt_id: PO:0009050
alt_id: PO:0020088
alt_id: PO:0020111
alt_id: PO:0020112
alt_id: PO:0020113
alt_id: PO:0020114
alt_id: PO:0020115
alt_id: PO:0020116
alt_id: PO:0020117
alt_id: PO:0020118
alt_id: PO:0020119
alt_id: PO:0020120
namespace: plant_structure
def: "That part of the axial system of plants above the uppermost foliage leaf/pair of foliage leaves that bears flowers." [APWeb:Glossary]
comment: Some plants have only solitary flowers\, e.g. Magnolia.
synonym: "cob (sensu sorghum)" []
synonym: "corymb" []
synonym: "cyme" []
synonym: "dichasium" []
synonym: "drepanium" []
synonym: "helicoid cyme" []
synonym: "monochasium" []
synonym: "panicle" []
synonym: "raceme" []
synonym: "rhipidium" []
synonym: "scorpioid cyme" []
synonym: "spike (sensu Triticeae)" []
synonym: "umbel" []
synonym: "verticillaster" []
relationship: part_of PO:0009006

[Term]
id: PO:0009051
name: spikelet
namespace: plant_structure
def: "Ultimate and congested inflorescence branch of the grasses." [APWeb:Glossary]
comment: It consists of one to many closely-packed flowers and associated glumes etc.
relationship: part_of PO:0009049

[Term]
id: PO:0009052
name: pedicel
namespace: plant_structure
def: "Basal part of the ultimate branch of the inflorescence." [APWeb:Glossary]
comment: The bracteoles are borne on the pedicel\, which terminates in a flower.
relationship: part_of PO:0009049

[Term]
id: PO:0009053
name: peduncle
namespace: plant_structure
def: "The stalk of an inflorescence; that part of the inflorescence below the first flower or inflorescence branch and above the last foliage leaf/pair of foliage leaves." [APWeb:Glossary]
relationship: part_of PO:0009049

[Term]
id: PO:0009054
name: inflorescence bract
namespace: plant_structure
def: "A leaf\, modified or not\, subtending a branch of the inflorescence or borne on the inflorescence axis below any branches or flowers." [APWeb:Glossary]
is_a: PO:0009055
relationship: part_of PO:0009049

[Term]
id: PO:0009055
name: bract
namespace: plant_structure
def: "A leaf\, usually different in form from the foliage leaves\, subtending a flower or inflorescence." [APWeb:Glossary]
comment: Often used to refer to what is called here floral bract.
synonym: "hypsophyll" []
is_a: PO:0006001

[Term]
id: PO:0009056
name: floral nectary
namespace: plant_structure
def: "A multicellular glandular structure found in the flower secreting a liquid containing organic substances especially sugars." [ISBN:047124529]
is_a: PO:0009035
relationship: part_of PO:0009046

[Term]
id: PO:0009057
name: extrafloral nectary
namespace: plant_structure
def: "A multicellular glandular structure found in places other than flower secreting a liquid containing organic substances especially sugar." [ISBN:047124529]
is_a: PO:0009035

[Term]
id: PO:0009058
name: perianth
namespace: plant_structure
def: "Non-fertile parts of a flower surrounding the fertile organs\, collectively the calyx and corolla of a flower\, or only a singe whorl." [APWeb:Glossary]
relationship: part_of PO:0009046

[Term]
id: PO:0009059
name: corolla
namespace: plant_structure
def: "The petals of a flower collectively." [APWeb:Glossary]
relationship: part_of PO:0009058

[Term]
id: PO:0009060
name: calyx
namespace: plant_structure
def: "The sepals of one flower collectively." [APWeb:Glossary]
relationship: part_of PO:0009058

[Term]
id: PO:0009061
name: androecium
namespace: plant_structure
def: "Collectively the stamens of one flower." [APWeb:Glossary, GR:pj]
relationship: part_of PO:0009046

[Term]
id: PO:0009062
name: gynoecium
namespace: plant_structure
def: "Collectively the carpels of a flower." [APWeb:Glossary, GR:pj, TAIR:lr, MaizeGDB:lv]
synonym: "pistil" []
relationship: part_of PO:0009046

[Term]
id: PO:0009063
name: epicalyx
namespace: plant_structure
def: "A whorl of structures immediately outside the calyx whorl." [APWeb:Glossary]
relationship: part_of PO:0009046

[Term]
id: PO:0009064
name: receptacle
namespace: plant_structure
def: "The region at end of pedicel or axis to which parts of flower are attached." [Poc:curators, APWeb:Glossary]
relationship: part_of PO:0009046

[Term]
id: PO:0009065
name: hypanthium
namespace: plant_structure
def: "A cup- or tube-like structure bearing perianth and stamens on its rim\, so these arise above the base\, and often above the top\, of the ovary of a flower." [Poc:curators, APWeb:Glossary]
relationship: part_of PO:0009046

[Term]
id: PO:0009066
name: anther
namespace: plant_structure
def: "The pollen-bearing part of a stamen." [APWeb:Glossary]
relationship: part_of PO:0009029

[Term]
id: PO:0009067
name: filament
namespace: plant_structure
def: "The stalk of a stamen." [GR:pj, MaizeGDB:lv]
relationship: part_of PO:0009029

[Term]
id: PO:0009068
name: connective
namespace: plant_structure
def: "The part of the stamen that connects the microsporangia/pollen sacs." [APWeb:Glossary]
relationship: part_of PO:0009066

[Term]
id: PO:0009069
name: theca
namespace: plant_structure
def: "A part of the anther consisting of paired sporangia that dehisce down a common slit." [APWeb:Glossary]
is_a: PO:0009070

[Term]
id: PO:0009070
name: microsporangium
namespace: plant_structure
def: "Sporangium producing microspores\, usually many in number." [APWeb:Glossary]
synonym: "anther lobe" []
synonym: "pollen sac" []
relationship: part_of PO:0009066

[Term]
id: PO:0009071
name: tapetum
namespace: plant_structure
def: "Innermost part of the anther wall\, involved in the nutrition of the pollen." [APWeb:Glossary, TAIR:lr]
relationship: part_of PO:0000002

[Term]
id: PO:0009072
name: ovary
namespace: plant_structure
def: "The basal portion of a carpel or group of fused carpels\, that encloses the ovule(s)." [APWeb:Glossary, TAIR:lr]
relationship: part_of PO:0009030

[Term]
id: PO:0009073
name: stigma
namespace: plant_structure
def: "Part of a carpel or group of fused carpels on which the pollen germinates\, usually apical." [APWeb:Glossary, TAIR:lr]
relationship: part_of PO:0009030

[Term]
id: PO:0009074
name: style
namespace: plant_structure
def: "An elongated part of a carpel or group of fused carpels between the ovary and the stigma\, and through which the pollen tube grows." [APWeb:Glossary, TAIR:lr]
synonym: "silk" []
relationship: part_of PO:0009030

[Term]
id: PO:0009075
name: plant ontology
namespace: plant_structure
def: "OBSOLETE. A controlled vocabulary to describe the various plant parts and the growth and developmental stages." [Poc:curators]
comment: This term was made obsolete because its child term \"plant structure\" (PO\:0009011) has become a new top level term. This takes effect with transition of ontology file formats from GO to the OBO format.
is_obsolete: true

[Term]
id: PO:0009077
name: staminode
namespace: plant_structure
def: "Sterile stamen." [APWeb:Glossary, GR:pj]
is_a: PO:0009028
relationship: part_of PO:0009061

[Term]
id: PO:0009078
name: pistillode
namespace: plant_structure
def: "A sterile pistil\, often rudimentary." [APWeb:Glossary]
is_a: PO:0009062

[Term]
id: PO:0009080
name: spikelet rachilla
namespace: plant_structure
def: "The axis of the spikelet\, above the glumes." [Poc:curators]
is_a: PO:0009081
relationship: part_of PO:0009051

[Term]
id: PO:0009081
name: inflorescence branch
namespace: plant_structure
def: "Any branch forming from the primary or the higher order inflorescence axis." [Poc:curators]
synonym: "coflorescence" []
relationship: part_of PO:0009049

[Term]
id: PO:0009082
name: floret
namespace: plant_structure
def: "Small flowers\, esp. of the spikelets of Poaceae and Cyperaceae and the capitula of Asteraceae." [APWeb:Glossary]
is_a: PO:0009046

[Term]
id: PO:0009083
name: reproductive structures
namespace: plant_structure
def: "OBSOLETE. Aggregation of gamete producing structures." [Poc:curators]
is_obsolete: true

[Term]
id: PO:0009084
name: pericarp
namespace: plant_structure
def: "The wall of a fruit\, developed from the ovary or carpel wall." [APWeb:Glossary, GR:pj, TAIR:lr]
relationship: part_of PO:0009001

[Term]
id: PO:0009085
name: epicarp
alt_id: PO:0006046
alt_id: PO:0006217
namespace: plant_structure
def: "The outer layer of the fruit wall or pericarp." [GR:pj]
synonym: "ectocarp" []
synonym: "epicarp" []
synonym: "exocarp" []
synonym: "outer epidermis of pericarp" []
synonym: "pericarp epidermis" []
relationship: part_of PO:0009084

[Term]
id: PO:0009086
name: endocarp
alt_id: PO:0006047
namespace: plant_structure
def: "The innermost differentiated layer of the fruit wall or pericarp." [GR:pj]
synonym: "endocarp" []
synonym: "inner epidermis of pericarp" []
relationship: part_of PO:0009084

[Term]
id: PO:0009087
name: mesocarp
namespace: plant_structure
def: "Middle layer of the fruit wall or pericarp." [GR:pj]
relationship: part_of PO:0009084

[Term]
id: PO:0009088
name: seed coat
namespace: plant_structure
def: "Covering of seed derived from ovular - mainly integumentary - tissue." [APWeb:Glossary, TAIR:lr, GR:pj]
comment: Used only when not specified more precisely; see testa\, tegmen.
relationship: part_of PO:0009010

[Term]
id: PO:0009089
name: endosperm
namespace: plant_structure
def: "Nutritive tissue in a seed\, in angiosperms usually triploid and formed after fertilization by the fusion of one gamete with the polar nucleus\, sometimes diploid or polyploid. " [GR:pj, APWeb:Glossary]
is_a: PO:0009007
relationship: part_of PO:0009010

[Term]
id: PO:0009090
name: aril
namespace: plant_structure
def: "A structure associated with and often partly or wholly covering a seed and developed from the funicle or raphe." [APWeb:Glossary]
comment: Also used more generally to refer to a similar structure derived from any part of the ovule - there has been much and sometimes acrimonious debate over the correct definition of the term\, so when used the origin of the aril should generally be given for clarity.
relationship: develops_from PO:0020006
relationship: part_of PO:0009010

[Term]
id: PO:0009091
name: mature dispersal unit
namespace: plant_structure
def: "OBSOLETE. provisional term" [Poc:curators]
is_obsolete: true

[Term]
id: PO:0019018
name: embryo axis
namespace: plant_structure
def: "Axial part of the young sporophyte comprising the hypocotyl\, and the root meristem\, or the radicle if one is present." [ISBN:0471245208]
synonym: "hypocotyl-root axis" []
relationship: part_of PO:0009009

[Term]
id: PO:0019022
name: arilloid
namespace: plant_structure
def: "An outgrowth from parts of the seed other than from the funiculus or raphe." [ISBN:0080280293]
relationship: part_of PO:0009010

[Term]
id: PO:0019023
name: strophiole
namespace: plant_structure
def: "An outgrowth occurring on the raphe." [ISBN:0080280293]
is_a: PO:0019022
relationship: part_of PO:0020027

[Term]
id: PO:0019024
name: seed operculum
namespace: plant_structure
def: "A plug-like structure formed in the micropylar region of the seed coat." [ISBN:0080280293]
relationship: part_of PO:0009010

[Term]
id: PO:0019026
name: tracheid bar
namespace: plant_structure
def: "A distinct ring-like structure\, composed of tracheid cells\, which surrounds the hilum of some taxa e.g.\, Phaseolus\, and forms a groove in the surface of the pericarp (immediately adjacent to the hilum)." [ISBN:0080280293]
relationship: part_of PO:0009010

[Term]
id: PO:0020001
name: placenta
namespace: plant_structure
def: "A more or less localized region within an ovary to which ovules are attached." [APWeb:Glossary]
relationship: part_of PO:0009072

[Term]
id: PO:0020002
name: endothecium
namespace: plant_structure
def: "The hypodermis of an anther sac with distinctively thickened walls and involved in its dehiscence\, especially when this is by slits." [APWeb:Glossary]
synonym: "anther sac hypodermis" []
is_a: PO:0005051
relationship: part_of PO:0000002

[Term]
id: PO:0020003
name: ovule
namespace: plant_structure
def: "A stalked or sessile structure in a seed plant within which one or more megaspores are formed and later the female gametophyte or embryo sac develops." [APWeb:Glossary]
relationship: part_of PO:0009072

[Term]
id: PO:0020004
name: exothecium
alt_id: PO:0006059
namespace: plant_structure
def: "The epidermis of an anther sac\, sometimes with distinctively thickened walls and involved in its dehiscence\, usually only when this is poricidal." [APWeb:Glossary]
synonym: "anther epidermis" []
synonym: "anther sac epidermis" []
is_a: PO:0006035
relationship: part_of PO:0000002

[Term]
id: PO:0020005
name: placentoid
namespace: plant_structure
def: "An inpushing of the anther wall." [APWeb:Glossary]
relationship: part_of PO:0000002

[Term]
id: PO:0020006
name: funicle
namespace: plant_structure
def: "The stalk which attaches the ovule to the placenta." [APWeb:Glossary, GR:pj]
synonym: "funiculus" []
relationship: part_of PO:0009072

[Term]
id: PO:0020008
name: exine
namespace: plant_structure
def: "The outer layer of the pollen grain wall\, highly resistant to strong acids and bases\, and composed primarily of sporopollenin." [APWeb:Glossary]
relationship: part_of PO:0020059

[Term]
id: PO:0020009
name: ectexine
namespace: plant_structure
def: "The outer part of the exine\, which stains positively with basic fuchsin in optical microscopy and has higher electron density in conventionally prepared TEM sections." [APWeb:Glossary]
comment: Although the term endexine as originally defined (see APWeb) was more or less synonymous with nexine it no longer is because endexine is now invariably used in the sense of F?gri (see APWeb). Nexine and sexine are distinguished on purely morphological criteria\, whereas ectexine and endexine differ in their staining properties.
relationship: part_of PO:0020008

[Term]
id: PO:0020010
name: endexine
namespace: plant_structure
def: "The inner part of the exine\, which stains." [APWeb:Glossary]
comment: Although the term endexine as originally defined (see APWeb) was more or less synonymous with nexine it no longer is because endexine is now invariably used in the sense of F?gri (see APWeb). Nexine and sexine are distinguished on purely morphological criteria\, whereas ectexine and endexine differ in their staining properties.
relationship: part_of PO:0020008

[Term]
id: PO:0020011
name: nexine
namespace: plant_structure
def: "The inner\, non-sculptured part of the exine which lies below the sexine." [APWeb:Glossary]
comment: Although the term endexine as originally defined (see APWeb) was more or less synonymous with nexine it no longer is because endexine is now invariably used in the sense of F?gri (see APWeb). Nexine and sexine are distinguished on purely morphological criteria\, whereas ectexine and endexine differ in their staining properties.
relationship: part_of PO:0020008

[Term]
id: PO:0020012
name: sexine
namespace: plant_structure
def: "The outer\, sculptured layer of the exine\, which lies above the nexine." [APWeb:Glossary]
comment: Although the term ectexine as originally defined (see APWeb) was more or less synonymous with sexine\, it no longer is because ectexine is now invariably used in the redefined sense (see APWeb). Unlike ectexine\, sexine does not include the foot layer. Sexine and nexine are distinguished on purely morphological criteria\, whereas ectexine and endexine differ in their staining properties. The two sets of terms are therefore suited for slightly different applications.  A system of sexine stratification in which sexine 1 is the innermost and sexine 5 is the outermost layer of the sexine. Comment\: Usually the sexine consists of 3 layers (sexine 1 = columellae; sexine 2 = tectum; sexine 3 = sculpture elements).
relationship: part_of PO:0020008

[Term]
id: PO:0020013
name: tectum
namespace: plant_structure
def: "The layer of sexine\, which forms a roof over the columellae\, granules or other infratectal elements." [APWeb:Glossary]
synonym: "sexine 2" []
relationship: part_of PO:0020012

[Term]
id: PO:0020014
name: columella
namespace: plant_structure
def: "A rod-like element of the sexine/ectexine\, either supporting the tectum or a caput." [APWeb:Glossary]
synonym: "sexine 1" []
relationship: part_of PO:0020012

[Term]
id: PO:0020015
name: sculpture elements
namespace: plant_structure
def: "Third layer of sexine." [APWeb:Glossary]
synonym: "sexine 3" []
relationship: part_of PO:0020012

[Term]
id: PO:0020016
name: foot layer
namespace: plant_structure
def: "The inner layer of the ectexine." [APWeb:Glossary]
synonym: "nexine 1" []
relationship: part_of PO:0020009

[Term]
id: PO:0020017
name: intine
namespace: plant_structure
def: "The innermost of the major layers of the pollen grain wall\, underlies the exine and borders the cytoplasm\, not acetolysis resistant and is therefore absent in conventionally prepared palynological material." [APWeb:Glossary]
relationship: part_of PO:0020059

[Term]
id: PO:0020018
name: germination pore
namespace: plant_structure
def: "Area through which the pollen imports the nutrition during its development\, at the time of pollen germination\, the pollen tube emerges through it." [GR:pj]
synonym: "pollen pore" []
relationship: part_of PO:0020059

[Term]
id: PO:0020019
name: megaspore
namespace: plant_structure
def: "The larger\, in general\, of the two kinds of spores produced after meiosis in the life cycle of a heterosporous plant\, and on germination giving rise to the female gametophyte (embryo sac)." [APWeb:Glossary]
is_a: PO:0009002
relationship: develops_from PO:0000431

[Term]
id: PO:0020020
name: nucellus
namespace: plant_structure
def: "Subepidermal tissue in the ovule surrounding the megasporocyte." [APWeb:Glossary]
synonym: "megasporangium" []
relationship: part_of PO:0020003

[Term]
id: PO:0020021
name: integument
namespace: plant_structure
def: "One of the layers of tissue that usually covers the ovule\, enveloping the nucellus and forming the micropyle at the apex." [APWeb:Glossary]
relationship: part_of PO:0020003

[Term]
id: PO:0020022
name: inner integument
namespace: plant_structure
def: "The innermost of the two layers of tissue that usually cover the ovule\, contiguous to the nucellus and usually contributing to the formation of the micropyle at the apex." [APWeb:Glossary]
is_a: PO:0020021

[Term]
id: PO:0020023
name: outer integument
namespace: plant_structure
def: "One of the two layers of tissue that usually cover the ovule\, contiguous to the inner integument and usually involved in forming the micropyle at the apex." [APWeb:Glossary]
is_a: PO:0020021

[Term]
id: PO:0020024
name: endothelium
namespace: plant_structure
def: "Cells of the inner epidermis of the inner (or only) integument of the ovule that are radially elongated and metabolically very active." [APWeb:Glossary]
relationship: part_of PO:0020022

[Term]
id: PO:0020025
name: micropyle
namespace: plant_structure
def: "A small canal or opening through the integument(s) at the apex of an ovule." [APWeb:Glossary]
comment: In a mature seed the micropyle may remain visible as an occluded pore or may be obliterated. The micropyle originates as an opening in the integuments of an ovule through which the pollen tube usually enters the embryo sac.
relationship: part_of PO:0020003

[Term]
id: PO:0020026
name: chalaza
namespace: plant_structure
def: "Region in the ovule where the integuments and the nucellus join with the funiculus. " [ISBN:047124529]
comment: The chalaza is recognized as the region which initiates the two integuments at its flank.
relationship: part_of PO:0020003

[Term]
id: PO:0020027
name: raphe
namespace: plant_structure
def: "That part of the funiculus that is adnate to the ovule." [APWeb:Glossary, ISBN:047124529]
comment: see antiraphe.
relationship: part_of PO:0020003
relationship: part_of PO:0020006

[Term]
id: PO:0020028
name: antiraphe
namespace: plant_structure
def: "The region on the other side of the ovule from the raphe." [APWeb:Glossary]
comment: see raphe.
relationship: part_of PO:0020003

[Term]
id: PO:0020029
name: obturator
namespace: plant_structure
def: "An outgrowth of the funicle\, that forms a bridge between the micropyle and other tissues." [APWeb:Glossary]
comment: Most commonly arising from the funicle\, also developing from placenta\, integument\, etc.
relationship: develops_from PO:0020006

[Term]
id: PO:0020030
name: cotyledon
namespace: plant_structure
def: "A leaf or leaves formed at the first node of a sporophyte." [APWeb:Glossary, GR:pj]
is_a: PO:0006001
relationship: part_of PO:0009009

[Term]
id: PO:0020031
name: radicle
namespace: plant_structure
def: "The radicle is the basal continuation of the hypocotyl in an embryo and gives rise to the root system of the adult plant; sometimes more or less abortive." [APWeb:Glossary]
is_a: PO:0020127
relationship: part_of PO:0019018

[Term]
id: PO:0020032
name: plumule
namespace: plant_structure
def: "The somewhat differentiated terminal bud in several embryo types above the cotyledonary node\, in which one or more internodes and leaves or scales can be discerned in a primordial stage." [APWeb:Glossary]
synonym: "embryonic shoot" []
relationship: part_of PO:0009009

[Term]
id: PO:0020033
name: coleoptile
namespace: plant_structure
def: "A tubular structure developed at the junction of the cotyledonary sheath with the seedling axis\, and surrounding the plumule of a monocot embryo or seedling." [APWeb:Glossary]
is_a: PO:0009025
relationship: part_of PO:0009009

[Term]
id: PO:0020034
name: coleorhiza
namespace: plant_structure
def: "Tissue surrounding the radicle in the embryo or seedling of some monocots." [APWeb:Glossary]
relationship: part_of PO:0009009

[Term]
id: PO:0020035
name: epicotyl
namespace: plant_structure
def: "The first internode of the stem above the hypocotyl. In literature also used for the entire embryonic axis\, consisting of several internodes\, above the cotyledonary node. " [APWeb:Glossary]
relationship: part_of PO:0009009

[Term]
id: PO:0020036
name: epiblast
namespace: plant_structure
def: "A flap of tissue in an embryo or seedling arising opposite to the insertion of the cotyledon/scutellum." [APWeb:Glossary]
relationship: part_of PO:0009009

[Term]
id: PO:0020037
name: mesocotyl
namespace: plant_structure
def: "The internode between the cotyledon or cotyledons and the leaf or leaves at the next node of a young sporophyte." [APWeb:Glossary]
relationship: part_of PO:0009009

[Term]
id: PO:0020038
name: petiole
namespace: plant_structure
def: "The stalk of a leaf." [APWeb:Glossary, GR:pj]
relationship: part_of PO:0009025

[Term]
id: PO:0020039
name: leaf lamina
namespace: plant_structure
def: "The blade of a leaf\, usually dorsiventrally flattened\, and expanded." [APWeb:Glossary]
synonym: "leaf blade" []
relationship: part_of PO:0009025

[Term]
id: PO:0020040
name: leaf base
namespace: plant_structure
def: "The bottom part of a leaf where it attaches to the stem." [APWeb:Glossary]
synonym: "leaf sheath base" []
relationship: part_of PO:0009025

[Term]
id: PO:0020041
name: stipule
namespace: plant_structure
def: "One of (usually) a pair of appendages at the bases of leaves in many broad-leaved angiosperms." [APWeb:Glossary]
comment: The term not used for monocot leaves.
relationship: part_of PO:0009025

[Term]
id: PO:0020042
name: simple leaf
namespace: plant_structure
def: "A leaf in which the lamina is undivided." [Poc:curators]
is_a: PO:0009025

[Term]
id: PO:0020043
name: compound leaf
namespace: plant_structure
def: "A leaf having two or more distinct leaflets that are evident as such from early in development." [APWeb:Glossary]
is_a: PO:0009025

[Term]
id: PO:0020044
name: hyperphyll
namespace: plant_structure
def: "The unifacial terete apical portion of a monocot cotyledon\, sometimes also visible on other leaves." [APWeb:Glossary]
relationship: part_of PO:0020030

[Term]
id: PO:0020045
name: pinnate leaf
namespace: plant_structure
def: "A once-compound leaf with leaflets borne along a rachis." [APWeb:Glossary]
comment: The total number of leaflets may be even or odd\, in which case the leaf is called even-pinnate or odd-pinnate respectively.
is_a: PO:0020043

[Term]
id: PO:0020046
name: palmate leaf
namespace: plant_structure
def: "A once-compound leaf divided into several leaflets which arise at the same point\, there being no rachis." [APWeb:Glossary]
is_a: PO:0020043

[Term]
id: PO:0020047
name: microsporocyte
namespace: plant_structure
def: "A diploid (2n) cell that undergoes meiosis and produces four haploid (1n) microspores." [ISBN:0878934030]
synonym: "microspore mother cell" []
synonym: "pollen mother cell" []
is_a: PO:0006204
relationship: part_of PO:0009070

[Term]
id: PO:0020048
name: microspore
namespace: plant_structure
def: "The smaller\, in general\, of the two kinds of spores produced after meiosis in the life cycle of a heterosporous plant\, and on germination giving rise to the male gametophyte." [APWeb:Glossary]
is_a: PO:0009002
relationship: develops_from PO:0000032

[Term]
id: PO:0020049
name: leaflet
namespace: plant_structure
def: "One of the ultimate segments of a compound leaf." [APWeb:Glossary]
relationship: part_of PO:0020043

[Term]
id: PO:0020050
name: petiolule
namespace: plant_structure
def: "The stalk of a leaflet." [APWeb:Glossary]
relationship: part_of PO:0020049

[Term]
id: PO:0020051
name: stipel
namespace: plant_structure
def: "Stipule-like appendage(s) at the base of a leaflet (in unifoliolate or simple leaves\, found at the top of the petiole)." [APWeb:Glossary]
relationship: part_of PO:0020049

[Term]
id: PO:0020052
name: megaphyll
namespace: plant_structure
def: "OBSOLETE. Literally a large leaf\, a leaf of any size whose vascular supply leaves one or more gaps as it departs from the stem vascular tissue." [APWeb:Glossary]
is_obsolete: true

[Term]
id: PO:0020053
name: microphyll
namespace: plant_structure
def: "OBSOLETE. Literally a small leaf\, a leaf of any size in which any vascular trace supplying it does not interrupt the central vascular cylinder when it departs\, i.e. there are no leaf gaps." [APWeb:Glossary]
is_obsolete: true

[Term]
id: PO:0020054
name: bud scale
namespace: plant_structure
def: "A reduced leaf surrounding a dormant bud." [UMSL:tk]
is_a: PO:0006003

[Term]
id: PO:0020055
name: leaf rachis
namespace: plant_structure
def: "That part of the main axis of a pinnate or more highly compound leaf\, that bears leaflets or divisions of the axis." [APWeb:Glossary]
relationship: part_of PO:0020043

[Term]
id: PO:0020056
name: tegmen
namespace: plant_structure
def: "That part of the seed coat that develops from the inner integument." [APWeb:Glossary, ISBN:0080374913]
relationship: part_of PO:0009088

[Term]
id: PO:0020057
name: testa
namespace: plant_structure
def: "That part of the seed coat that develops from the outer integument\, or from the single integument when there is only one." [APWeb:Glossary, ISBN:0080374913]
relationship: part_of PO:0009088

[Term]
id: PO:0020058
name: perisperm
alt_id: PO:0006335
namespace: plant_structure
def: "Diploid nutritive tissue in an angiospermous seed derived from nucellar tissue." [APWeb:Glossary]
synonym: "seed nucellus" []
is_a: PO:0009007
relationship: part_of PO:0009010

[Term]
id: PO:0020059
name: pollen wall
namespace: plant_structure
def: "Complex wall surrounding the micrsopore." [UMSL:fz]
relationship: part_of PO:0020091

[Term]
id: PO:0020060
name: caruncle
namespace: plant_structure
def: "An outgrowth from the surface of a seed\, usually near the hilum or micropyle." [APWeb:Glossary]
is_a: PO:0019022

[Term]
id: PO:0020061
name: coma
namespace: plant_structure
def: "A tuft of hairs at one end of a seed." [APWeb:Glossary]
relationship: part_of PO:0009010

[Term]
id: PO:0020062
name: elaiosome
namespace: plant_structure
def: "An appendage of a seed\, usually rich in oil\, attractive to animals\, especially ants." [APWeb:Glossary]
is_a: PO:0019022

[Term]
id: PO:0020063
name: hilum
namespace: plant_structure
def: "The scar on a seed at the place where it was attached to its funicle." [APWeb:Glossary]
relationship: part_of PO:0009010

[Term]
id: PO:0020064
name: dehiscent fruit
namespace: plant_structure
def: "OBSOLETE. Fruit that breaks open at maturity to release the contents." [APWeb:Glossary]
is_obsolete: true

[Term]
id: PO:0020065
name: indehiscent fruit
namespace: plant_structure
def: "OBSOLETE. Fruit that does not open at maturity." [APWeb:Glossary]
is_obsolete: true

[Term]
id: PO:0020066
name: fleshy fruit
namespace: plant_structure
def: "OBSOLETE. The fruit may be derived from monocarpellate or multicarpellate gynoecia. Their walls may consist of the pericarp or of pericarp fused with extracarpellary tissue. The outer part of the fruit wall or the entire fruit wall may become fleshy by differentiating into soft\, succulent parenchyma. Parts other than the wall such as placentae and partitions in multilocular ovaries may become fleshy." [ISBN:047124529]
is_obsolete: true

[Term]
id: PO:0020075
name: mericarp
namespace: plant_structure
def: "OBSOLETE. One segment of a fruit of a schizocarp consisting of pericarp plus seed(s)." [APWeb:Glossary]
is_obsolete: true

[Term]
id: PO:0020081
name: seed as dispersal unit
namespace: plant_structure
def: "OBSOLETE." [Poc:curators]
is_obsolete: true

[Term]
id: PO:0020084
name: pyrene
namespace: plant_structure
def: "OBSOLETE. The 'stone' or 'pit' (endocarp plus seed) of a succulent fruit." [APWeb:Glossary]
is_obsolete: true

[Term]
id: PO:0020085
name: seed and fruit wall as dispersal unit
namespace: plant_structure
def: "OBSOLETE." [Poc:curators]
is_obsolete: true

[Term]
id: PO:0020086
name: multiple fruit
namespace: plant_structure
def: "OBSOLETE. Fruit on a common axis derived from the ovaries of several flowers." [APWeb:Glossary]
is_obsolete: true

[Term]
id: PO:0020089
name: tap root
namespace: plant_structure
def: "The main\, descending root of a plant that has a single\, dominant root axis derived from the radicle of the seedling." [APWeb:Glossary]
comment: see radicle\, primary root.
is_a: PO:0020127

[Term]
id: PO:0020090
name: central cell
namespace: plant_structure
def: "The largest cell of the mature embryo sac. Contains two polar nuclei\, which (after double fertilization) will develop into the endosperm." [TAIR:ki]
is_a: PO:0009002
relationship: develops_from PO:0020095
relationship: part_of PO:0020092

[Term]
id: PO:0020091
name: male gametophyte
alt_id: PO:0020007
namespace: plant_structure
def: "A plant body or cell lineage formed by vegetative growth of the microspore\, producing male gametes." [APWeb:Glossary]
synonym: "microgametophyte" []
synonym: "pollen" []
synonym: "pollen grain" []
is_a: PO:0009004

[Term]
id: PO:0020092
name: female gametophyte
namespace: plant_structure
def: "Embryo sac in flowering plants." [APWeb:Glossary]
synonym: "embryo sac" []
synonym: "megagametophyte" []
is_a: PO:0009004

[Term]
id: PO:0020093
name: antipodal cell
namespace: plant_structure
def: "Cell\, commonly three in number as in the eight-nucleate embryo sac\, located at the other end of the embryo sac from the female gamete. " [APWeb:Glossary]
comment: More or less persistent\, multiplicative or not.
is_a: PO:0009002
relationship: part_of PO:0020092

[Term]
id: PO:0020094
name: egg cell
namespace: plant_structure
def: "A non motile cell at the apex of the embryo sac immediately adjacent to the micropyle and associated with the synergid cells." [APWeb:Glossary]
is_a: PO:0009002
relationship: part_of PO:0020096

[Term]
id: PO:0020095
name: polar nucleus
namespace: plant_structure
def: "Usually two nuclei in the center of the eight-nucleate embryo sac that fuse\, and subsequently fuse with one of the male gametes to produce the endosperm." [APWeb:Glossary]
comment: see endosperm.
relationship: part_of PO:0020092

[Term]
id: PO:0020096
name: egg apparatus
namespace: plant_structure
def: "The egg cell and two synergids located at the micropylar end of the female gametophyte\, or the embryo sac\, in angiosperms." [TAIR:lr]
relationship: part_of PO:0020092

[Term]
id: PO:0020097
name: generative cell
namespace: plant_structure
def: "A cell of the male gametophyte of angiosperms that divides to produce two male gametes or sperm cells." [APWeb:Glossary]
is_a: PO:0009002
relationship: part_of PO:0020091

[Term]
id: PO:0020099
name: vegetative cell
namespace: plant_structure
def: "The larger cell of the male gametophyte of angiosperms that does not divide further." [APWeb:Glossary]
is_a: PO:0009002
relationship: part_of PO:0020091

[Term]
id: PO:0020100
name: hypocotyl
namespace: plant_structure
def: "The part of the stem below the cotyledonary node and transitional to a root\, found in a young sporophyte." [APWeb:Glossary]
relationship: part_of PO:0019018

[Term]
id: PO:0020101
name: stomium
namespace: plant_structure
def: "A fissure or pore in the anther lobe through which the pollen is released." [GR:pj]
relationship: part_of PO:0000002

[Term]
id: PO:0020102
name: transmitting tissue
namespace: plant_structure
def: "Tissue in the style of a carpel through which the pollen tube grows; it connects the stigma and the inside of ovary." [GR:pj, ISBN:0080374913]
synonym: "transmitting tract" []
is_a: PO:0009007
relationship: part_of PO:0009074

[Term]
id: PO:0020103
name: flag leaf
namespace: plant_structure
def: "The last mature leaf before the inflorescence in a cereal crop plant." [GR:pj]
is_a: PO:0006340

[Term]
id: PO:0020104
name: leaf sheath
namespace: plant_structure
def: "Any tubular portion of the leaf surrounding the stem\, as in the Poaceae." [GR:pj]
relationship: part_of PO:0009025

[Term]
id: PO:0020105
name: ligule
namespace: plant_structure
def: "A membranous or hairy appendage on the adaxial/upper surface of a leaf\, at the junction between sheath and blade\, especially in grasses" [APWeb:Glossary]
relationship: part_of PO:0009025

[Term]
id: PO:0020106
name: auricle
namespace: plant_structure
def: "Outgrowth at the base of a leaf blade that may wrap around the stem." [GR:pj]
relationship: part_of PO:0009025

[Term]
id: PO:0020108
name: suspensor
namespace: plant_structure
def: "A nearly always single file of cells at the base of the embryo derived from the basal cell." [GR:pj]
comment: It anchors the embryo in the embryo sac and pushes it into the endosperm.
relationship: part_of PO:0009009

[Term]
id: PO:0020109
name: hypophysis
namespace: plant_structure
def: "The uppermost cell of the suspensor from which part of the root and root cap in the embryo of angiosperms are derived." [ISBN:047124529]
is_a: PO:0009002
relationship: part_of PO:0020108

[Term]
id: PO:0020110
name: scutellum
namespace: plant_structure
def: "A more or less shield-shaped and absorptive portion of an embryo of grasses\, probably a modified cotyledon." [APWeb:Glossary]
synonym: "haustorial cotyledon" []
relationship: part_of PO:0009009

[Term]
id: PO:0020121
name: lateral root
namespace: plant_structure
def: "Root developing from the pericycle layer of the primary root." [ISBN:0122151704]
is_a: PO:0009005

[Term]
id: PO:0020122
name: inflorescence axis
namespace: plant_structure
def: "The central supporting structure around which flowers are borne." [UMSL:fz]
comment: cob (sensu Zea) is different from the cob inflorescence found in Sorghum.
synonym: "first order inflorescence branch" []
synonym: "inflorescence rachis" []
relationship: part_of PO:0009049

[Term]
id: PO:0020123
name: root cap
namespace: plant_structure
def: "A group of cells that covers the apical meristem of the root." [APWeb:Glossary]
relationship: part_of PO:0009005

[Term]
id: PO:0020124
name: root stele
alt_id: PO:0003012
namespace: plant_structure
def: "The central column of primary vascular tissue in the root and any tissue that it surrounds." [APWeb:Glossary]
comment: Includes the pericycle as the outermost layer of the stele
synonym: "root vascular cylinder" []
relationship: part_of PO:0009005

[Term]
id: PO:0020125
name: elongation zone
namespace: plant_structure
def: "The portion of the root that includes small\, densely cytoplasmic cells that are dividing and expanding in size." [GR:pj]
synonym: "region of cell elongation" []
synonym: "region of radial enlargement" []
relationship: part_of PO:0009005

[Term]
id: PO:0020126
name: tassel
namespace: plant_structure
def: "The functionally-staminate flowering structure that terminates the stem of a Zea mays plant." [MaizeGDB:lv]
comment: Branched inflorescence with a central axis and about 10-50 lateral branches.
is_a: PO:0009049

[Term]
id: PO:0020127
name: primary root
namespace: plant_structure
def: "The root which develops directly from the embryonic radicle." [ISBN:0122151704]
is_a: PO:0009005

[Term]
id: PO:0020128
name: leaf margin
namespace: plant_structure
def: "The margin or edge of the lamina." [UMSL:fz]
synonym: "leaf lamina margin" []
relationship: part_of PO:0020039

[Term]
id: PO:0020129
name: adventitious root
alt_id: PO:0003007
namespace: plant_structure
def: "Root developing from any plant part other than near the root apex." [ISBN:0878934030]
comment: see radicle\, lateral root\, primary root.
synonym: "stilt root" []
is_a: PO:0009005

[Term]
id: PO:0020130
name: central root cap
namespace: plant_structure
def: "The central part of a root cap in which the cells are arranged in longitudinal files." [GR:pj]
synonym: "columella cells" []
relationship: part_of PO:0020123

[Term]
id: PO:0020131
name: lateral root cap
namespace: plant_structure
def: "The part of the root cap that is parallel to the sides of the axis." [ISBN:0122151704]
synonym: "peripheral cells" []
relationship: part_of PO:0020123

[Term]
id: PO:0020132
name: columella root cap cell
namespace: plant_structure
def: "Cell that constitutes the central part of the root cap\, arranged in longitudinal files." [TAIR:ki, PMID:9384380]
is_a: PO:0009002
relationship: develops_from PO:0020133

[Term]
id: PO:0020133
name: columella root cap initial
namespace: plant_structure
def: "Cell that produces columella cells in the root cap. In direct contact with quiescent center." [TAIR:ki, ISBN:0471245208]
is_a: PO:0004011

[Term]
id: PO:0020134
name: statolith
namespace: plant_structure
def: "OBSOLETE. Solid cell inclusion of starch containing plastids occurring in root cap cells." [GR:pj]
comment: This is sub-cellular term
is_obsolete: true

[Term]
id: PO:0020135
name: differentiation zone
alt_id: PO:0003002
namespace: plant_structure
def: "The portion of the root located behind the elongation zone containing cells that are differentiating into their final form and function." [GR:pj]
synonym: "maturation zone" []
synonym: "specialization zone" []
relationship: part_of PO:0009005

[Term]
id: PO:0020136
name: ear (sensu Zea)
namespace: plant_structure
def: "The distal part of a lateral (axillary) branch in Zea that bears the functionally-carpellate florets in a highly contracted inflorescence." [MaizeGDB:lv]
is_a: PO:0009049

[Term]
id: PO:0020137
name: leaf apex
namespace: plant_structure
def: "The top part of the leaf\, usually the apex of the leaf blade." [UMSL:fz]
synonym: "leaf tip" []
relationship: part_of PO:0020039

[Term]
id: PO:0020138
name: leaf vein
namespace: plant_structure
def: "A strand of vascular tissue in the leaf blade." [APWeb:Glossary]
relationship: part_of PO:0020039

[Term]
id: PO:0020139
name: midvein
namespace: plant_structure
def: "The central\, and usually the most prominent\, vein of a leaf or leaf-like organ." [APWeb:Glossary]
synonym: "mid rib" []
is_a: PO:0020138

[Term]
id: PO:0020140
name: secondary vein
namespace: plant_structure
def: "Second order veins in the leaf blade." [GR:pj]
synonym: "veinlet" []
is_a: PO:0020138

[Term]
id: PO:0020141
name: node
namespace: plant_structure
def: "The level (transverse plane) of a stem at which one or more leaves and associated axillary bud(s) arise." [APWeb:Glossary]
relationship: part_of PO:0009047

[Term]
id: PO:0020142
name: internode
namespace: plant_structure
def: "The portion of a stem between the level of insertion of two successive leaves\, leaf pairs or leaf whorls\, or branches of an inflorescence\, i.e. between two nodes." [APWeb:Glossary]
comment: see node.
relationship: part_of PO:0009047

[Term]
id: PO:0020144
name: apical meristem
namespace: plant_structure
def: "The meristems located at the apices of the main and lateral shoots and roots." [GR:pj]
synonym: "primary meristem" []
is_a: PO:0009013

[Term]
id: PO:0020145
name: lateral meristem
namespace: plant_structure
def: "Cells along the stem or root that first differentiate and function as members of a mature tissue system but then again take up meristematic activity." [APWeb:Glossary]
synonym: "secondary meristem" []
is_a: PO:0009013

[Term]
id: PO:0020147
name: root apical meristem
namespace: plant_structure
def: "Meristem at the root apex." [UMSL:fz, GR:pj]
comment: In most cases it is involved in root elongation.
synonym: "promeristem" []
is_a: PO:0006085
is_a: PO:0020144

[Term]
id: PO:0020148
name: shoot apical meristem
namespace: plant_structure
def: "Meristem formed in the apex of the shoot\, including meristems originating as axillary shoot meristems." [UMSL:fz]
synonym: "apical meristem" []
synonym: "primary shoot meristem" []
is_a: PO:0006079
is_a: PO:0020144
relationship: part_of PO:0000037

[Term]
id: PO:0020149
name: quiescent center
namespace: plant_structure
def: "Hemispherically shaped aggregation of mitotically and metabolically inactive cells positioned behind the root cap." [ISBN:0122151704]
relationship: part_of PO:0006085

[Term]
id: PO:0007001
name: FR.01 early stage of fruit ripening
namespace: plant_growth_and_development_stage
def: "The early stage in fruit ripening." [GR:ap, ISBN:3826331524]
synonym: "09-dough development" [GRO:0007110]
synonym: "7 linear grain-filling in maize" [MaizeGDB:64632]
synonym: "7.03-early dough in maize" [GRO:0007034]
synonym: "7.3 early dough stage/embryo 3 in maize" [MaizeGDB:67374]
synonym: "8.03 Early ripening in soybean" [SOY:0000086]
synonym: "8.1-early dough stage in rice" [GRO:0007152]
synonym: "9.01-early dough" [GRO:0007111]
synonym: "9.01-early dough in barley" [GRO:0007111]
synonym: "9.01-early dough in oat" [GRO:0007111]
synonym: "9.01-early dough in wheat" [GRO:0007111]
synonym: "BBCH principal growth stage 83" [ISBN:3826331524]
synonym: "R4 in maize" [MaizeGDB:67374]
synonym: "dough stage in maize" [MaizeGDB:67374]
synonym: "early dough stage in maize" [MaizeGDB:67374]
synonym: "early dough\, kernel content soft\, about 45% dry matter" [ISBN:3826331524]
synonym: "embryo stage 3 in maize" [MaizeGDB:67374]
synonym: "rice growth stage-8.1" [GRO:0007152]
is_a: PO:0007010 ! 6 ripening

[Term]
id: PO:0007002
name: IE.03 3/4 of inflorescence emerged from flag leaf sheath
namespace: plant_growth_and_development_stage
def: "The stage at which 3/4 of inflorescence has emerged from flag leaf sheath." [GR:ap]
synonym: "6.04-3/4 of inflorescence emerged in barley" [GRO:0007099]
synonym: "6.04-3/4 of inflorescence emerged in oat" [GRO:0007099]
synonym: "6.04-3/4 of inflorescence emerged in wheat" [GRO:0007099]
synonym: "70% of panicle emerged in rice" []
is_a: PO:0007041 ! inflorescence emergence from flag leaf sheath

[Term]
id: PO:0007003
name: IL.03 full inflorescence length reached
namespace: plant_growth_and_development_stage
def: "The stage when the inflorescence reaches full length." [GR:ap]
synonym: "4.04 full inflorescence length reached in soybean" [SOY:0000070]
is_a: PO:0007047 ! 3 inflorescence visible

[Term]
id: PO:0007004
name: 3 rapid growth stage
namespace: plant_growth_and_development_stage
def: "The stage at which the plant grows rapidly by either or both stem elongation and expansion of the rosette/foliage. " [GR:ap ""]
comment: Many stages like leaf production PO\:0007112\, axillary shoot formation PO\:0007073\, inflorescence PO\:0007047 often overlap with this stage
is_obsolete: true

[Term]
id: PO:0007005
name: IL.02 1/2 inflorescence length reached
namespace: plant_growth_and_development_stage
def: "The stage when 1/2 Inflorescence is visible. " [GR:ap]
synonym: "4.03 1/2 of inflorescence length reached in soybean" [SOY:0000069]
is_a: PO:0007047 ! 3 inflorescence visible

[Term]
id: PO:0007006
name: IL.00 inflorescence just visible
namespace: plant_growth_and_development_stage
def: "Inflorescence just visible to the naked eye." [Poc:curators]
synonym: "4.01 Inflorescence just visible in soybean" [SOY:0000067]
synonym: "visible flower buds in Arabidopsis" [TAIR:0000420]
is_a: PO:0007047 ! 3 inflorescence visible

[Term]
id: PO:0007007
name: FF.03 fruit size 70%
namespace: plant_growth_and_development_stage
def: "The stage when the size of the fruit is about 70% of final fruit size." [GR:ap, ISBN:3826331524]
synonym: "7.07 Pod 70% of final length in soybean" [SOY:0000082]
synonym: "8.02-early milk in barley" [GRO:0007107]
synonym: "8.02-early milk in oat" [GRO:0007107]
synonym: "8.02-early milk in wheat" [GRO:0007107]
synonym: "Zadok scale-73\, Haun scale-13" [GRO:0007107]
synonym: "early milk stage" [GRO:0007107]
synonym: "early milk stage in maize" [ISBN:3826331524]
synonym: "late milk" [GRO:0007109]
is_a: PO:0007042 ! 5 fruit formation

[Term]
id: PO:0007008
name: IE.02 1/2 of inflorescence emerged from flag leaf sheath
namespace: plant_growth_and_development_stage
def: "The stage at which 1/2 of inflorescence has emerged from flag leaf sheath." [GR:ap]
synonym: "08-heading" [GRO:0007131]
synonym: "6.03-1/2 of inflorescence emerged in barley" [GRO:0007098]
synonym: "6.03-1/2 of inflorescence emerged in oat" [GRO:0007098]
synonym: "6.03-1/2 of inflorescence emerged in wheat" [GRO:0007098]
synonym: "first individual flowers visible" []
synonym: "half bloom" [GRO:0007131]
synonym: "middle of heading" []
synonym: "middle of panicle emergence in rice" []
synonym: "sorghum growth stage-7" [GRO:0007131]
is_a: PO:0007041 ! inflorescence emergence from flag leaf sheath

[Term]
id: PO:0007009
name: FF.01 fruit size 30%
namespace: plant_growth_and_development_stage
def: "The stage when the size of the fruit is about 30% of final fruit size." [GR:ap, ISBN:3826331524]
synonym: "7.02 Pod 30% of final length in soybean" [SOY:0000080]
is_a: PO:0007042 ! 5 fruit formation

[Term]
id: PO:0007010
name: 6 ripening
namespace: plant_growth_and_development_stage
def: "Maturation of the fruit." [Poc:curators]
comment: Although the use of stages like dough or particular ripening stages properly refer to the development of an individual fruit\, they are commonly used as here to extrapolate to a growth of a whole plant or a group of plants.
synonym: "08-dough stage in rice" [GRO:0007042]
synonym: "09-dough development in barley" [GRO:0007110]
synonym: "09-dough development in oat" [GRO:0007110]
synonym: "09-dough development in wheat" [GRO:0007110]
synonym: "10-dough stage in sorghum" [GRO:0007132]
synonym: "8 Bean Development in soybean" [SOY:0000078]
synonym: "BBCH principal growth stage 8" []
synonym: "dough stage" [GRO:0007132]
synonym: "dough stage in maize" [MaizeGDB:67379]
synonym: "dough stage kernels yellowish\, about 55% dry matter" [ISBN:3826331524]
synonym: "fruit maturity" []
synonym: "fruit ripening" []
synonym: "kernel ripening" []
synonym: "maturity of fruit and seed" []
synonym: "rice growth stage-8" []
synonym: "silique ripening in Arabidopsis" [TAIR:0000034]
is_a: PO:0007130 ! B reproductive growth

[Term]
id: PO:0007011
name: root development stage
namespace: plant_growth_and_development_stage
def: "OBSOLETE" [GR:ap]
is_obsolete: true

[Term]
id: PO:0007012
name: inflorescence visible (sensu Poaceae)
namespace: plant_growth_and_development_stage
def: "The stage at which grass plant is producing inflorescence(s)." [Poc:curators]
comment: There is no one-to-one correspondence between growth stages of inflorescences formation in members of Poaceae with that of other families.
synonym: "BBCH principal growth stage 4" [ISBN:3826331524]
is_a: PO:0007047 ! 3 inflorescence visible

[Term]
id: PO:0007013
name: BO.03 late boot stage
namespace: plant_growth_and_development_stage
def: "The flag leaf sheath swollen." [GR:ap, ISBN:3826331524]
comment: In rice the flag leaf sheath is more than 10cm out of the penultimate leaf sheath.
synonym: "5.2-late booting stage in rice" [GRO:0007150]
synonym: "flag leaf sheath swollen" []
synonym: "rice growth stage-5.2" [GRO:0007150]
is_a: PO:0007014 ! booting

[Term]
id: PO:0007014
name: booting
namespace: plant_growth_and_development_stage
def: "Stage characterized by a swelling of the flag leaf sheath\, caused by an increase in the size of the inflorescence as it grows up the leaf sheath." [GR:pj ""]
synonym: "05-booting in barley" [GRO:0007090]
synonym: "05-booting in oat" [GRO:0007090]
synonym: "05-booting in wheat" [GRO:0007090]
synonym: "05-booting stage" [GRO:0007148]
synonym: "07-boot stage in sorghum" [GRO:0007130]
synonym: "BBCH growth stage 40" [ISBN:3826331524]
synonym: "development of vegetatively propogated organs" []
synonym: "rice growth stage-5" [GRO:0007148]
synonym: "sorghum growth stage-6" [GRO:0007130]
is_a: PO:0007012 ! inflorescence visible (sensu Poaceae)

[Term]
id: PO:0007015
name: radicle emergence
namespace: plant_growth_and_development_stage
def: "Radicle or root emerged from seed." [ISBN:3826331524, GR:ap]
synonym: "0.02-radicle emergence from seed in maize" [GRO:0007005]
synonym: "0.2 radicle emergence from seed in maize" [MaizeGDB:67351]
synonym: "05 radicle emergence from seed coat in soybean" [SOY:0000011]
synonym: "1.04-radicle emerged from seed in Triticeae" [GRO:0007055]
synonym: "1.04-radicle emerged from seed in barley" [GRO:0007055]
synonym: "1.04-radicle emerged from seed in oat" [GRO:0007055]
synonym: "1.04-radicle emerged from seed in wheat" [GRO:0007055]
synonym: "BBCH growth stage 05" [ISBN:3826331524]
synonym: "Zadok scale-5" [GRO:0007055]
synonym: "maize growth stage-0.2" [GRO:0007005]
synonym: "radicle emergence in Arabidopsis" [TAIR:T0000395]
relationship: part_of PO:0007131 ! 0.2 seedling growth

[Term]
id: PO:0007016
name: 4 flowering
namespace: plant_growth_and_development_stage
def: "The stage at which any flower(s) on the plant are open." [Poc:curators]
comment: This stage refers to the whole plant.
synonym: "07-anthesis in barley" [GRO:0007101]
synonym: "07-anthesis in oat" [GRO:0007101]
synonym: "07-anthesis in wheat" [GRO:0007101]
synonym: "09-flowering in sorghum" [GRO:0007153]
synonym: "5 flowering in maize" [MaizeGDB:13811]
synonym: "5.01-anthesis in maize " [GRO:0007021]
synonym: "5.02-silking in maize" [GRO:0007022]
synonym: "5.1 anthesis in maize" [MaizeGDB:67361]
synonym: "5.2 silking in maize" [MaizeGDB:67362]
synonym: "6 Flowering in soybean" [SOY:0000006]
synonym: "6.1-flowering stage in rice" [GRO:0007151]
synonym: "BBCH principal growth stage 6" [ISBN:3826331524]
synonym: "R1 in maize" [MaizeGDB:67362]
synonym: "VT in maize" [MaizeGDB:67361]
synonym: "anthesis in maize" [MaizeGDB:67361]
synonym: "anthesis stage" [GRO:0007151]
synonym: "flowering in maize" [MaizeGDB:13811]
synonym: "pollen shed in maize" [MaizeGDB:67361]
synonym: "rice growth stage-6.1" [GRO:0007151]
synonym: "silk emergence in maize" [MaizeGDB:67362]
synonym: "sorghum growth stage 8" [GRO:0007153]
is_a: PO:0007130 ! B reproductive growth

[Term]
id: PO:0007017
name: C senescence
namespace: plant_growth_and_development_stage
def: "The processes that occur near the end of a plant's active life that are associated with the dismantling of cell components and membranes\, loss of functional chloroplasts\, and an overall decline in metabolism. " [Poc:curators]
synonym: "10.03-kernel loosening in daytime in Triticeae" [GRO:0007117]
synonym: "10.03-kernel loosening in daytime in barley" [GRO:0007117]
synonym: "10.03-kernel loosening in daytime in oat" [GRO:0007117]
synonym: "10.03-kernel loosening in daytime in wheat" [GRO:0007117]
synonym: "10.04-overripe\, straw dead and collapsing in Triticeae" [GRO:0007118]
synonym: "10.04-overripe\, straw dead and collapsing in barley" [GRO:0007118]
synonym: "10.04-overripe\, straw dead and collapsing in oat" [GRO:0007118]
synonym: "10.04-overripe\, straw dead and collapsing in wheat" [GRO:0007118]
synonym: "9 Senescence in soybean" [SOY:0000008]
synonym: "BBCH principal growth stage 9" [ISBN:3826331524]
synonym: "senescence in Arabidopsis" [TAIR:0000035]
is_a: PO:0007033 ! whole plant growth stage

[Term]
id: PO:0007018
name: BO.01 early boot stage
namespace: plant_growth_and_development_stage
def: "The flag leaf sheath has started to extend." [GR:ap, ISBN:3826331524]
comment: In rice the flag leaf sheath is 5cm out of the penultimate leaf sheath. Upper part of the stem is slightly thickened.
synonym: "5.01-flag leaf sheath extending in barley" [GRO:0007091]
synonym: "5.01-flag leaf sheath extending in oat" [GRO:0007091]
synonym: "5.01-flag leaf sheath extending in wheat" [GRO:0007091]
synonym: "5.1-early booting stage in rice" [GRO:0007149]
synonym: "flag leaf sheath extending" [GRO:0007091]
synonym: "rice growth stage-5.1" [GRO:0007149]
is_a: PO:0007014 ! booting

[Term]
id: PO:0007019
name: BO.05 flag leaf sheath opened
namespace: plant_growth_and_development_stage
def: "The first awns are visible and the flag leaf sheath has opened. " [ISBN:3826331524, GR:ap]
comment: Awns will be visible only in those species and varieties where they are known to be present.
synonym: "5.04-flag leaf sheath extending in barley" [GRO:0007094]
synonym: "5.04-flag leaf sheath extending in oat" [GRO:0007094]
synonym: "5.04-flag leaf sheath extending in wheat" [GRO:0007094]
synonym: "first awns visible" [GRO:0007094]
is_a: PO:0007014 ! booting

[Term]
id: PO:0007020
name: embryo development stage
namespace: plant_growth_and_development_stage
def: "OBSOLETE" [GR:ap]
is_obsolete: true

[Term]
id: PO:0007021
name: plant part development stage
namespace: plant_growth_and_development_stage
def: "The succession of changes during the development of plant parts." [POC:curators]
is_a: PO:0009012 ! plant growth and development stage

[Term]
id: PO:0007022
name: 0.1 imbibition
namespace: plant_growth_and_development_stage
def: "Absorption of water by the seed." [ISBN:0306416875, GR:ap]
synonym: "0.1 imbibition in maize" [MaizeGDB:64054]
synonym: "01 Beginning of seed imbibition in soybean" [SOY:0000090]
synonym: "03 Seed imbibition complete in soybean" [SOY:0000091]
synonym: "1.02-start of imbibition in Triticeae" [GRO:0007053]
synonym: "1.02-start of imbibition in barley" [GRO:0007053]
synonym: "1.02-start of imbibition in oat" [GRO:0007053]
synonym: "1.02-start of imbibition in wheat" [GRO:0007053]
synonym: "1.03-imbibition complete in Tricticeae" [GRO:0007054]
synonym: "1.03-imbibition complete in barley" [GRO:0007054]
synonym: "1.03-imbibition complete in oat" [GRO:0007054]
synonym: "1.03-imbibition complete in wheat" [GRO:0007054]
synonym: "BBCH growth stage 01" [ISBN:3826331524]
synonym: "imbibition in Arabidopsis" [TAIR:0000394]
relationship: part_of PO:0007057 ! 0 germination

[Term]
id: PO:0007023
name: IE.04 inflorescence fully emerged from flag leaf sheath
namespace: plant_growth_and_development_stage
def: "The stage at which the  inflorescence  has fully emerged from the flag leaf sheath." [GR:ap]
synonym: "6.05-emergence of inflorescence completed in barley" [GRO:0007100]
synonym: "6.05-emergence of inflorescence completed in oat" [GRO:0007100]
synonym: "6.05-emergence of inflorescence completed in wheat" [GRO:0007100]
synonym: "end of panicle emergence in rice" []
is_a: PO:0007041 ! inflorescence emergence from flag leaf sheath

[Term]
id: PO:0007024
name: FL.04 end of flowering
namespace: plant_growth_and_development_stage
def: "The stage at which flowering is complete." [GR:ap]
comment: This stage refers to the whole plant.
synonym: "6.09 End of flowering in soybean" [SOY:0000076]
synonym: "7.03-anthesis completed in barley" [GRO:0007104]
synonym: "7.03-anthesis completed in oat" [GRO:0007104]
synonym: "7.03-anthesis completed in wheat" [GRO:0007104]
synonym: "Zadok scale-69\, Haun scale-11.6" [GRO:0007104]
synonym: "anthesis completed" []
synonym: "flowering complete" []
synonym: "fruit set visible" []
synonym: "late reproductive" []
is_a: PO:0007016 ! 4 flowering

[Term]
id: PO:0007025
name: IE.00 inflorescence tip just visible above flag leaf sheath
namespace: plant_growth_and_development_stage
def: "The stage at which the inflorescence tip is just visible above flag leaf sheath" [GR:ap]
synonym: "6.01-first spikelet of inflorescence visible in barley" [GRO:0007096]
synonym: "6.01-first spikelet of inflorescence visible in oat" [GRO:0007096]
synonym: "6.01-first spikelet of inflorescence visible in wheat" [GRO:0007096]
synonym: "Zadok scale-50\, Feekes scale-10.1\, Haun scale-10.2" [GRO:0007096]
synonym: "beginning of heading" []
synonym: "beginning of panicle emergence in rice" []
synonym: "beginning of tassel emergence in maize" []
synonym: "first flower buds visible" []
synonym: "first spikelet visible" [GRO:0007096]
synonym: "visible flower buds" []
is_a: PO:0007041 ! inflorescence emergence from flag leaf sheath

[Term]
id: PO:0007026
name: FL.00 first flower(s) open
namespace: plant_growth_and_development_stage
def: "The stage at which the first flower(s) open." [GR:pj]
comment: These first flowers are not necessarily the oldest flowers in the inflorescence. In some cereal plants the flowering starts in the middle of the inflorescence. This stage refers to the whole plant.
synonym: "6.00 1st flowers on main stem open in soybean" [SOY:0000072]
synonym: "7.01-anthesis beginning in Triticeae" [GRO:0007102]
synonym: "7.01-anthesis beginning in barley" [GRO:0007102]
synonym: "7.01-anthesis beginning in oat" [GRO:0007102]
synonym: "7.01-anthesis beginning in wheat" [GRO:0007102]
synonym: "Stage R1 Open flower at any node on the main stem" [SOY:0000072]
synonym: "first open flower in Arabidopsis" [TAIR:0000421]
is_a: PO:0007016 ! 4 flowering

[Term]
id: PO:0007027
name: FF.04 final fruit size
namespace: plant_growth_and_development_stage
def: "The stage when the size of the fruit has reached the final fruit size." [GR:ap, ISBN:3826331524]
synonym: "7.09 Pod full size in soybean" [SOY:0000084]
synonym: "8.03-medium milk in barley" [GRO:0007108]
synonym: "8.03-medium milk in oat" [GRO:0007108]
synonym: "8.03-medium milk in wheat" [GRO:0007108]
synonym: "8.04-late milk in barley" [GRO:0007109]
synonym: "8.04-late milk in oat" [GRO:0007109]
synonym: "BBCH principal growth stage 75" [ISBN:3826331524]
synonym: "BBCH principal growth stage 79" [ISBN:3826331524]
synonym: "Kernels in middle of cob yellowish-white" [ISBN:3826331524]
synonym: "Stage R4 Full pod in soybean" [SOY:0000084]
synonym: "kernel content milky\, 40% dry matter" [ISBN:3826331524]
synonym: "nearly all kernels have reached final size" [ISBN:3826331524]
is_a: PO:0007042 ! 5 fruit formation

[Term]
id: PO:0007028
name: BO.04 flag leaf sheath opening
namespace: plant_growth_and_development_stage
def: "The flag leaf sheath starts opening." [ISBN:3826331524]
synonym: "5.03-flag leaf sheath extending in barley" [GRO:0007093]
synonym: "5.03-flag leaf sheath extending in oat" [GRO:0007093]
synonym: "5.03-flag leaf sheath extending in wheat" [GRO:0007093]
synonym: "Zadok scale-47" [GRO:0007093]
is_a: PO:0007014 ! booting

[Term]
id: PO:0007029
name: FF.02 fruit size 50%
namespace: plant_growth_and_development_stage
def: "The stage when the size of the fruit is about 50% of final fruit size." [GR:ap, ISBN:3826331524]
synonym: "7.01-blister stage in maize" [GRO:0007030]
synonym: "7.03 Pod 50% of final length in soybean" [SOY:0000081]
synonym: "8.01-kernel watery ripe in barley" [GRO:0007106]
synonym: "8.01-kernel watery ripe in oat" [GRO:0007106]
synonym: "8.01-kernel watery ripe in wheat" [GRO:0007106]
synonym: "BBCH principal growth stage 71" [ISBN:3826331524]
synonym: "R2 in maize" [MaizeGDB:67372]
synonym: "Stage R4 Full pod in soybean" [SOY:0000081]
synonym: "Zadok scale-71\, Feekes scale-10.54\, Haun scale-12.1" [GRO:0007106]
synonym: "beginning of grain development\, kernels at blister stage\, 16% dry matter" [ISBN:3826331524]
synonym: "blister stage in maize" [MaizeGDB:67372]
synonym: "caryopsis watery ripe" [GRO:0007106]
synonym: "kernel watery ripe" [GRO:0007106]
synonym: "watery ripe" [GRO:0007106]
is_a: PO:0007042 ! 5 fruit formation

[Term]
id: PO:0007030
name: shoot emergence
namespace: plant_growth_and_development_stage
def: "Shoot or leaf breaks through soil surface." [GR:ap, ISBN:3826331524]
synonym: "07 shoot emergence in soybean" [SOY:0000012]
synonym: "BBCH growth stage 09" [ISBN:3826331524]
relationship: part_of PO:0007131 ! 0.2 seedling growth

[Term]
id: PO:0007031
name: FR.02 mid stage of fruit ripening
namespace: plant_growth_and_development_stage
def: "The stage when fruit ripening is midway." [GR:ap, ISBN:3826331524]
synonym: "10.01-soft dough in sorghum" [GRO:0007133]
synonym: "7.4 late dough stage/embryo 4 in maize" [MaizeGDB:67379]
synonym: "8.05 Mid ripening in soybean" [SOY:0000087]
synonym: "9.02-soft dough in barley" [GRO:0007112]
synonym: "9.02-soft dough in oat" [GRO:0007112]
synonym: "9.02-soft dough in wheat" [GRO:0007112]
synonym: "BBCH principal growth stage 85" [ISBN:3826331524]
synonym: "DNA degradation (endosperm) in maize" [MaizeGDB:67373]
synonym: "R3 in maize" [MaizeGDB:67373]
synonym: "Stage R6 Full seed in soybean" [SOY:0000087]
synonym: "Zadok scale-85\, Feekes scale-11.2" [GRO:0007112]
synonym: "dough stage in maize" [MaizeGDB:67379]
synonym: "embryo stage 4 in maize" [MaizeGDB:67379]
synonym: "soft dough" [GRO:0007112]
is_a: PO:0007010 ! 6 ripening

[Term]
id: PO:0007032
name: FF.00 fruit size 10%
namespace: plant_growth_and_development_stage
def: "The stage when the size of the fruit is about 10% of final fruit size." [GR:ap, ISBN:3826331524]
synonym: "7.01 Pod 10% of final length in soybean" [SOY:0000079]
synonym: "Stage R3 in soybean" [SOY:0000079]
is_a: PO:0007042 ! 5 fruit formation

[Term]
id: PO:0007033
name: whole plant growth stage
namespace: plant_growth_and_development_stage
def: "The succession of changes during the growth of the whole plant." [GR:pj ""]
synonym: "cereal plant ontology " [GRO:0080001]
synonym: "maize growth stage" [GRO:0007002]
synonym: "plant growth stage ontology" [GRO:0007199]
synonym: "plant growth stages in Arabidopsis" [TAIR:0000021]
synonym: "rice growth stage" [GRO:0007040]
synonym: "sorghum growth stage" [GRO:0007124]
synonym: "wheat\, barley and oat growth stage" [GRO:0007156]
is_a: PO:0009012 ! plant growth and development stage

[Term]
id: PO:0007034
name: FL.01 1/4 of flowers open
namespace: plant_growth_and_development_stage
def: "The stage at which 1/4 of flowers open" [GR:ap]
comment: This stage refers to the whole plant.
synonym: "6.02 1/4 of flowers on the main stem open in soybean" [SOY:0000073]
is_a: PO:0007016 ! 4 flowering

[Term]
id: PO:0007035
name: 7-8 fruit formation and maturation
namespace: plant_growth_and_development_stage
def: "OBSOLETE\: This stage refers to the developmental and physiological changes that occur in the whole plant after fertilization and during fruit development\, maturation\, and provisioning. " [Poc:curators]
comment: We have chosen to use fruit size as a marker of these physiological processes to represent the whole plant growth stage.
synonym: "06-post-flowering in maize" [GRO:0007025]
synonym: "5.3 pollination in maize" [MaizeGDB:67364]
synonym: "5.4 fertilization in maize" [MaizeGDB:67365]
synonym: "6 post-flowering/lag phase in maize" [MaizeGDB:67370]
synonym: "7 Pod Formation in soybean" [SOY:0000077]
synonym: "7 linear grain-filling in maize" [MaizeGDB:64632]
synonym: "7-8 Fruit Formation and Maturation in soybean" [SOY:0000007]
synonym: "7.01-blister stage in maize" [GRO:0007030]
synonym: "BBCH principal growth stage 7" [ISBN:3826331524]
synonym: "C-embryo stage in rice" [GRO:0007141]
synonym: "R1in maize" [MaizeGDB:67370]
synonym: "double fertilization in maize" [MaizeGDB:67365]
synonym: "effective filling period in maize" [MaizeGDB:64632]
synonym: "first silique shattered" []
synonym: "grain-filling in maize" [MaizeGDB:64632]
synonym: "kernel watery ripe" [GRO:0007106]
synonym: "lag phase in maize" [MaizeGDB:67370]
synonym: "post-flowering in maize" [MaizeGDB:67370]
synonym: "pro embryo in maize" [MaizeGDB:67370]
is_obsolete: true

[Term]
id: PO:0007036
name: FR.00 beginning of fruit ripening
namespace: plant_growth_and_development_stage
def: "The stage at which fruit maturation begins." [GR:ap, ISBN:3826331524]
synonym: "8.01 Beginning of bean ripening in soybean" [SOY:0000085]
synonym: "beginning of fruit coloration" []
synonym: "first silique shattered" []
is_a: PO:0007010 ! 6 ripening

[Term]
id: PO:0007038
name: FR.04 fruit ripening complete
namespace: plant_growth_and_development_stage
def: "The stage at which fruit ripening is complete." [GR:ap, ISBN:3826331524]
synonym: "10-ripening in Triticeae" [GRO:0007114]
synonym: "10-ripening in barley" [GRO:0007114]
synonym: "10-ripening in oat" [GRO:0007114]
synonym: "10-ripening in wheat" [GRO:0007114]
synonym: "10.01-kernel medium hard" [GRO:0007115]
synonym: "10.02-kernel hard" [GRO:0007116]
synonym: "8.09 Final ripening in soybean" [SOY:0000089]
synonym: "9.02 dry kernel in maize" [GRO:0007037]
synonym: "9.2 dry kernel in maize" [MaizeGDB:67381]
synonym: "BBCH principal growth stage 89" [ISBN:3826331524]
synonym: "dry kernel in maize" [MaizeGDB:67381]
synonym: "dry seed in maize" [MaizeGDB:67381]
synonym: "fully ripe" []
synonym: "fully ripe grain hard\, difficult to divide by thumbnail in rice" [ISBN:3826331524]
synonym: "fully ripe kernels hard and shiny about 65% dry matter in maize" [ISBN:3826331524]
is_a: PO:0007010 ! 6 ripening

[Term]
id: PO:0007040
name: leaf development stage
namespace: plant_growth_and_development_stage
def: "OBSOLETE" [GR:ap]
is_obsolete: true

[Term]
id: PO:0007041
name: inflorescence emergence from flag leaf sheath
namespace: plant_growth_and_development_stage
def: "The stage at which the inflorescence emerges from the flag leaf sheath." [GR:ap]
synonym: "06-heading stage in rice" [GRO:0007044]
synonym: "06-inflorescence emergence in barley" [GRO:0007095]
synonym: "06-inflorescence emergence in oat" [GRO:0007095]
synonym: "06-inflorescence emergence in wheat" [GRO:0007095]
synonym: "08-heading in sorghum" [GRO:0007131]
synonym: "half bloom in sorghum" [GRO:0007131]
synonym: "heading" [GRO:0007095]
synonym: "rice growth stage-6" [GRO:0007044]
synonym: "sorghum growth stage-7" [GRO:0007131]
synonym: "tasseling" []
is_a: PO:0007012 ! inflorescence visible (sensu Poaceae)

[Term]
id: PO:0007042
name: 5 fruit formation
namespace: plant_growth_and_development_stage
def: "Formation of the seed-bearing structure after flowering." [Poc:curators]
comment: Although the use of stages like milk or particular fruit sizes properly refer to the development of an individual fruit\, they are commonly used as here to extrapolate to a growth of a whole plant or a group of plants.
synonym: "07-milk stage in rice" [GRO:0007046]
synonym: "08-milk development in barley" [GRO:0007105]
synonym: "08-milk development in oat" [GRO:0007105]
synonym: "08-milk development in wheat" [GRO:0007105]
synonym: "6.01-dilatory in maize" [GRO:0007026]
synonym: "6.02-exponential in maize" [GRO:0007027]
synonym: "6.1 dilatory in maize" [MaizeGDB:67371]
synonym: "6.2 exponential in maize" [MaizeGDB:67369]
synonym: "Zadok scale-70" [GRO:0007105]
synonym: "dilatory in maize" [MaizeGDB:67371]
synonym: "exponential in maize" [MaizeGDB:67369]
synonym: "free nuclear in maize" [MaizeGDB:67371]
synonym: "milk grain" []
synonym: "milk stage in rice" [GRO:0007046]
synonym: "mitotic in maize" [MaizeGDB:67369]
synonym: "pro embryo in maize" [MaizeGDB:67371]
synonym: "rice growth stage-7" [GRO:0007046]
synonym: "transition stage in maize" [MaizeGDB:67369]
is_a: PO:0007130 ! B reproductive growth

[Term]
id: PO:0007043
name: hypocotyl emergence
namespace: plant_growth_and_development_stage
def: "Emergence of the hypocotyl above ground." [GR:ap, ISBN:0306416875]
comment: Occurs in plants with epigeal germination.
synonym: "0.07.01 Cotyledons and hypocotyl emerge in soybean" [SOY:0000013]
synonym: "0.07.02 Hypocotyl emerges above soil in soybean" [SOY:0000092]
synonym: "BBCH growth stage 08" [ISBN:3826331524]
synonym: "hypocotyl and cotyledon emergence in Arabidopsis" [TAIR:0000396]
is_a: PO:0007030 ! shoot emergence

[Term]
id: PO:0007044
name: BO.02 mid boot stage
namespace: plant_growth_and_development_stage
def: "The flag leaf sheath is just visibly swollen. " [ISBN:3826331524, GR:ap]
comment: In rice the flag leaf sheath is 5-10cm out of the penultimate leaf sheath.
synonym: "5.02-flag leaf sheath extending in barley" [GRO:0007092]
synonym: "5.02-flag leaf sheath extending in oat" [GRO:0007092]
synonym: "5.02-flag leaf sheath extending in wheat" [GRO:0007092]
synonym: "Zadok scale-45\, Feekes scale-10\, Haun scale-9.2" [GRO:0007092]
synonym: "flag leaf sheath just visibly swollen" []
is_a: PO:0007014 ! booting

[Term]
id: PO:0007045
name: coleoptile emergence
namespace: plant_growth_and_development_stage
def: "Emergence of coleoptile above ground." [GR:ap, ISBN:3826331524]
synonym: "0.3 coleoptile emergence from seed in maize" [MaizeGDB:67352]
synonym: "BBCH growth stage 09" [ISBN:3826331524]
is_a: PO:0007030 ! shoot emergence

[Term]
id: PO:0007046
name: IL.01 1/4 inflorescence length reached
namespace: plant_growth_and_development_stage
def: "The stage when 1/4 Inflorescence is visible. " [GR:ap]
synonym: "4.02 1/4 of inflorescence length reached in soybean" [SOY:0000068]
is_a: PO:0007047 ! 3 inflorescence visible

[Term]
id: PO:0007047
name: 3 inflorescence visible
namespace: plant_growth_and_development_stage
def: "The stage at which plant is producing inflorescence(s)." [Poc:curators]
synonym: "4 Inflorescence Formation in soybean" [SOY:0000005]
synonym: "BBCH principal growth stage 5" [ISBN:3826331524]
is_a: PO:0007130 ! B reproductive growth

[Term]
id: PO:0007048
name: IE.01 1/4 of inflorescence emerged from flag leaf sheath
namespace: plant_growth_and_development_stage
def: "The stage at which 1/4 of inflorescence has emerged from flag leaf sheath." [GR:ap]
synonym: "30% of panicle emerged in rice" []
synonym: "6.02-1/4 of inflorescence emerged in barley" [GRO:0007097]
synonym: "6.02-1/4 of inflorescence emerged in oat" [GRO:0007097]
synonym: "6.02-1/4 of inflorescence emerged in wheat" [GRO:0007097]
synonym: "Zadok scale-53\, Feekes scale-10.2" [GRO:0007097]
is_a: PO:0007041 ! inflorescence emergence from flag leaf sheath

[Term]
id: PO:0007049
name: cotyledon emergence
alt_id: PO:0007069
namespace: plant_growth_and_development_stage
def: "Emergence of cotyledons above ground." [GR:ap, ISBN:3826331524]
comment: This cannot be used in plants with hypogeal germination.
synonym: "01-seedling emergence in sorghum" [GRO:0007125]
synonym: "1.00 Cotyledon visible in soybean" [SOY:0000014]
synonym: "1.00 imperfect leaf unrolled" []
synonym: "1.01-seedling emergence in maize" [GRO:0007008]
synonym: "1.1 seedling emergence in maize" [MaizeGDB:64057]
synonym: "2.01-first leaf through coleoptile in Triticeae" [GRO:0007059]
synonym: "2.01-first leaf through coleoptile in barley" [GRO:0007059]
synonym: "2.01-first leaf through coleoptile in oat" [GRO:0007059]
synonym: "2.01-first leaf through coleoptile in wheat" [GRO:0007059]
synonym: "BBCH growth stage 09" [ISBN:3826331524]
synonym: "BBCH growth stage 10" [ISBN:3826331524]
synonym: "LP.00 cotyledon visible" []
synonym: "VE in maize" [MaizeGDB:64057]
synonym: "VE stage in soybean" [SOY:0000014]
synonym: "Zadok scale-10\, Feekes scale-1" [GRO:0007059]
synonym: "cotyledons fully open in Arabidopsis" [TAIR:0000397]
synonym: "first leaf through coleoptile (sensu Oryza)" []
synonym: "first leaf through coleoptile (sensu Triticeae)" [GRO:0007059]
synonym: "hypocotyl and cotyledon emergence in Arabidopsis" [TAIR:0000396]
synonym: "maize growth stage-1.1" [GRO:0007008]
synonym: "seedling emergence (sensu Sorghum)" [GRO:0007125]
synonym: "sorghum growth stage-0" [GRO:0007125]
is_a: PO:0007030 ! shoot emergence

[Term]
id: PO:0007050
name: FR.03 late stage of fruit ripening
namespace: plant_growth_and_development_stage
def: "The late stage of fruit ripening." [GR:ap, ISBN:3826331524]
synonym: "09-maturity in maize" [GRO:0007037]
synonym: "10.02-hard dough in sorghum" [GRO:0007134]
synonym: "8 leveling off of grain-filling/embryo 5 in maize" [MaizeGDB:67382]
synonym: "8.07 Late ripening in soybean" [SOY:0000088]
synonym: "8.2-hard dough stage in rice" [GRO:0007154]
synonym: "9 maturity in maize" [MaizeGDB:11088]
synonym: "9.03-hard dough in barley" [GRO:0007113]
synonym: "9.03-hard dough in oat" [GRO:0007113]
synonym: "9.03-hard dough in wheat" [GRO:0007113]
synonym: "9.1 physiological maturity/embryo 6 in maize" [MaizeGDB:67380]
synonym: "BBCH principal growth stage 87" [ISBN:3826331524]
synonym: "R5 in maize" [MaizeGDB:67382]
synonym: "R6 in maize" [MaizeGDB:67380]
synonym: "Stage R7 Beginning maturity in soybean" [SOY:0000088]
synonym: "Zadok scale-87\, Haun scale-15" [GRO:0007113]
synonym: "attenuative in maize" [MaizeGDB:67382]
synonym: "black layer in maize" [MaizeGDB:67380]
synonym: "dent stage in maize" [MaizeGDB:67382]
synonym: "embryo stage 5 in maize" [MaizeGDB:67382]
synonym: "embryo stage 6 in maize" [MaizeGDB:67380]
synonym: "hard dough" []
synonym: "late dough grain in rice" [GRO:0007154]
synonym: "late dough stage in rice" [GRO:0007154]
synonym: "leveling off of dry matter accumulation" [MaizeGDB:67382]
synonym: "physiological maturity\, black dot\, about 60% dry matter in maize" [ISBN:3826331524]
synonym: "rice growth stage-8.2" [GRO:0007154]
synonym: "sorghum growth stage-10" [GRO:0007134]
synonym: "storage maturity in maize" [MaizeGDB:67381]
is_a: PO:0007010 ! 6 ripening

[Term]
id: PO:0007051
name: BO.00 booting begins
namespace: plant_growth_and_development_stage
def: "Booting has just begun." [ISBN:3826331524, GR:ap]
is_a: PO:0007014 ! booting

[Term]
id: PO:0007052
name: FL.03 3/4 of flowers open
namespace: plant_growth_and_development_stage
def: "The stage at which 3/4 of flowers open." [GR:ap]
comment: This stage refers to the whole plant.
synonym: "6.02 3/4 of flowers on main stem open in soybean" [SOY:0000074]
synonym: "Stage R2 Open flower at one of the two uppermost nodes on the main stem with fully developed leaf in soybean" [SOY:0000074]
synonym: "flowering finishing" []
is_a: PO:0007016 ! 4 flowering

[Term]
id: PO:0007053
name: FL.02 1/2 of flowers open
namespace: plant_growth_and_development_stage
def: "The stage at which 1/2 of flowers open." [GR:ap]
comment: This stage refers to the whole plant.
synonym: "6.02 1/2 of flowers on main stem open in soybean" [SOY:0000094]
synonym: "7.02-anthesis half-way in barley" [GRO:0007103]
synonym: "7.02-anthesis half-way in oat" [GRO:0007103]
synonym: "7.02-anthesis half-way in wheat" [GRO:0007103]
synonym: "Haun scale-11.5" [GRO:0007103]
synonym: "full flowering" []
is_a: PO:0007016 ! 4 flowering

[Term]
id: PO:0007054
name: epicotyl emergence
namespace: plant_growth_and_development_stage
def: "Emergence of the epicotyl above ground." [ISBN:0306416875, GR:ap]
comment: Only the first true foliage leaf or pair of leaves are visible.  Occurs in plants with hypogeal germination.
is_a: PO:0007030 ! shoot emergence

[Term]
id: PO:0007055
name: 0.0 dry seed
namespace: plant_growth_and_development_stage
def: "Mature seed with low moisture content." [GR:ap, ISBN:0306416875]
synonym: "00 Dry Seed in soybean" [SOY:0000009]
synonym: "1.01-dry seed in Tricticeae" [GRO:0007052]
synonym: "BBCH growth stage 00" [ISBN:3826331524]
synonym: "dry seed in Arabidopsis" [TAIR:0000213]
relationship: part_of PO:0007057 ! 0 germination

[Term]
id: PO:0007057
name: 0 germination
namespace: plant_growth_and_development_stage
def: "The resumption of growth by the embryo in a seed." [ISBN:047124529, GR:ap]
synonym: "0 Germination in soybean" [SOY:0000001]
synonym: "0 germination in maize" [MaizeGDB:64055]
synonym: "00-germination in maize" [GRO:0007003]
synonym: "01-germination in Triticeae" [GRO:0007051]
synonym: "01-germination in barley" [GRO:0007051]
synonym: "01-germination in oat" [GRO:0007051]
synonym: "01-germination in rice" [GRO:0007043]
synonym: "01-germination in wheat" [GRO:0007051]
synonym: "BBCH principal growth stage 0" [ISBN:3826331524]
synonym: "axillary bud development" []
synonym: "bud development" []
synonym: "germination in Arabidopsis" [TAIR:0000393]
synonym: "maize growth stage-0" [GRO:0007003]
synonym: "rice growth stage-1" [GRO:0007043]
synonym: "sprouting" []
synonym: "terminal bud development" []
is_a: PO:0007134 ! A vegetative growth

[Term]
id: PO:0007060
name: obsolete growth and development terms
namespace: plant_growth_and_development_stage
is_obsolete: true

[Term]
id: PO:0007061
name: 2.00 main shoot only
namespace: plant_growth_and_development_stage
def: "OBSOLETE" [GR:ap]
synonym: "3.01-main shoot only in Triticeae" [GRO:0007087]
synonym: "3.01-main shoot only in barley" [GRO:0007087]
synonym: "3.01-main shoot only in oat" [GRO:0007087]
synonym: "3.01-main shoot only in wheat" [GRO:0007087]
synonym: "Zadok scale-20" [GRO:0007087]
is_obsolete: true

[Term]
id: PO:0007062
name: SE.06 six nodes or internodes visible
namespace: plant_growth_and_development_stage
def: "The stage at which six nodes or six internodes are visible." [GR:pj ""]
comment: A measure of vegetative growth\, but leaf production is to be preferred.
synonym: "3.06 6 nodes/internodes visible in soybean" [SOY:0000055]
synonym: "4.07-sixth node detectable in barley" [GRO:0007087]
synonym: "4.07-sixth node detectable in oat" [GRO:0007087]
synonym: "4.07-sixth node detectable in wheat" [GRO:0007087]
synonym: "BBCH growth stage 36" [ISBN:3826331524]
synonym: "Zadok scale-36" [GRO:0007087]
is_a: PO:0007089 ! stem elongation

[Term]
id: PO:0007063
name: LP.07 seven leaves visible
namespace: plant_growth_and_development_stage
def: "The stage at which leaves at seven nodes\, other than the cotyledonary node\, are visible above ground." [GR:ap]
comment: The leaves can be a single leaf\, two\, or whorls of leaves at each node.
synonym: "1.07 6th trifoliolate leaf unfolded in soybean" [SOY:0000021]
synonym: "2.08-seven leaves unfolded in Triticeae" [GRO:0007066]
synonym: "2.08-seven leaves unfolded in barley" [GRO:0007066]
synonym: "2.08-seven leaves unfolded in oat" [GRO:0007066]
synonym: "2.08-seven leaves unfolded in wheat" [GRO:0007066]
synonym: "3.01-ear initiation" [GRO:0007013]
synonym: "3.1 ear initiation/mid-whorl stage in maize" [MaizeGDB:67356]
synonym: "6-8 leaves in maize" [MaizeGDB:67356]
synonym: "7 leaves unfolded" []
synonym: "7 rosette leaf in Arabidopsis" [TAIR:0000410]
synonym: "7-leaf in maize" [MaizeGDB:67356]
synonym: "BBCH growth stage 17" [ISBN:3826331524]
synonym: "Stage V6 in soybean" [SOY:0000021]
synonym: "V7 in maize" [MaizeGDB:67356]
synonym: "Zadok scale-\, Haun scale-6.+" [GRO:0007066]
synonym: "ear initiation in maize" [MaizeGDB:67356]
synonym: "maize growth stage-3.1" [GRO:0007013]
synonym: "mid-whorl stage in maize" [MaizeGDB:67356]
synonym: "seven leaves unfolded (sensu Triticeae)" [GRO:0007066]
synonym: "seven rosette leaves" []
synonym: "seventh leaf unfolded" []
is_a: PO:0007133 ! leaf production

[Term]
id: PO:0007064
name: LP.12 twelve leaves visible
namespace: plant_growth_and_development_stage
def: "The stage at which leaves at twelve nodes\, other than the cotyledonary node\, are visible above ground." [GR:ap]
comment: The leaves can be a single leaf\, two\, or whorls of leaves at each node.
synonym: "1.12 11th trifoliolate leaf unfolded in soybean" [SOY:0000026]
synonym: "12 rosette leaf in Arabidopsis" [TAIR:0000415]
synonym: "3.03-mid-vegetative" [GRO:0007013]
synonym: "3.3 mid-vegetative" [MaizeGDB:67359]
synonym: "3.3 mid-vegetative stage of maize" [GRO:0007013]
synonym: "Stage V11 in soybean" [SOY:0000026]
synonym: "V12 in maize" [MaizeGDB:67359]
synonym: "maize growth stage-3.3" [GRO:0007013]
synonym: "mid-vegetative in maize" [MaizeGDB:67359]
synonym: "mid-vegetative stage of maize" [GRO:0007013]
synonym: "twelve leaves unfolded" []
synonym: "twelve rosette leaves" []
is_a: PO:0007133 ! leaf production

[Term]
id: PO:0007065
name: LP.05 five leaves visible
namespace: plant_growth_and_development_stage
def: "The stage at which leaves at five nodes\, other than the cotyledonary node\, are visible above ground." [GR:ap]
comment: The leaves can be a single leaf\, two\, or whorls of leaves at each node.
synonym: "02-tassel initiation in maize" [GRO:0007011]
synonym: "04-five leaf stage in sorghum" [GRO:0007127]
synonym: "1.05 4th trifoliolate leaf unfolded in soybean" [SOY:0000019]
synonym: "2 tassel initiation/early whorl stage in maize" [MaizeGDB:67306]
synonym: "2.06-five leaves unfolded in Triticeae" [GRO:0007064]
synonym: "2.06-five leaves unfolded in barley" [GRO:0007064]
synonym: "2.06-five leaves unfolded in oat" [GRO:0007064]
synonym: "2.06-five leaves unfolded in wheat" [GRO:0007064]
synonym: "4-6 leaves in maize" [MaizeGDB:67306]
synonym: "5 leaves unfolded" []
synonym: "5 rosette leaf in Arabidopsis" [TAIR:0000408]
synonym: "BBCH growth stage 15" [ISBN:3826331524]
synonym: "Stage V4 in soybean" [SOY:0000019]
synonym: "V5 in maize" [MaizeGDB:67306]
synonym: "Zadok scale-15\, Haun scale-4.+" [GRO:0007064]
synonym: "early whorl stage in maize" [MaizeGDB:67306]
synonym: "fifth leaf unfolded" []
synonym: "five leaf stage (sensu Sorghum)" [GRO:0007127]
synonym: "five leaves unfolded (sensu Triticeae)" [GRO:0007064]
synonym: "five rosette leaves" []
synonym: "maize growth stage-2" [GRO:0007011]
synonym: "rice growth stage-3" [GRO:0007049]
synonym: "sorghum growth stage-3" [GRO:0007127]
synonym: "tassel differentiation in maize" [MaizeGDB:67306]
synonym: "tassel initiation in maize" [MaizeGDB:67306]
is_a: PO:0007133 ! leaf production

[Term]
id: PO:0007066
name: SE.09 nine nodes or internodes visible
namespace: plant_growth_and_development_stage
def: "The stage at which nine nodes or nine internodes are visible." [GR:pj ""]
comment: A measure of vegetative growth\, but leaf production is to be preferred.
synonym: "3.09 9 nodes/internodes visible in soybean" [SOY:0000058]
synonym: "BBCH growth stage 39" [ISBN:3826331524]
is_a: PO:0007089 ! stem elongation

[Term]
id: PO:0007067
name: LP.17 seventeen leaves visible
namespace: plant_growth_and_development_stage
def: "The stage at which leaves at seventeen nodes\, other than the cotyledonary node\, are visible above ground." [GR:ap]
comment: The leaves can be a single leaf\, two\, or whorls of leaves at each node.
synonym: "1.17 16th trifoliate leaf unfolded in soybean" [SOY:0000031]
synonym: "3.04-late vegetative" [GRO:0007016]
synonym: "3.4 late vegetative in maize" [MaizeGDB:67360]
synonym: "3.4 late vegetative stage of maize" [GRO:0007016]
synonym: "Stage V16 in soybean" [SOY:0000031]
synonym: "V17 in maize" [MaizeGDB:67360]
synonym: "late vegetative in maize" [MaizeGDB:67360]
synonym: "late vegetative stage of maize" [GRO:0007016]
synonym: "maize V17 stage" [GRO:0007016]
synonym: "maize growth stage-3.4" [GRO:0007016]
is_a: PO:0007133 ! leaf production

[Term]
id: PO:0007068
name: mid rosette growth
namespace: plant_growth_and_development_stage
def: "Rosette has reached approximately 50% of its final diameter." [Poc:curators]
comment: A measure of vegetative growth\, but leaf production is to be preferred.
synonym: "mid rosette growth in Arabidopsis" [TAIR:0000044]
is_a: PO:0007113 ! rosette growth

[Term]
id: PO:0007070
name: SE.08 eight nodes or internodes visible
namespace: plant_growth_and_development_stage
def: "The stage at which eight nodes or eight internodes are visible." [GR:ap]
comment: A measure of vegetative growth\, but leaf production is to be preferred.
synonym: "3.08 8 nodes/internodes visible in soybean" [SOY:0000057]
synonym: "BBCH growth stage 38" [ISBN:3826331524]
is_a: PO:0007089 ! stem elongation

[Term]
id: PO:0007071
name: 2.02 main shoot and axillary shoots visible at two nodes
namespace: plant_growth_and_development_stage
def: "The stage at which main shoot and axillary shoots at two nodes are visible." [GR:ap]
comment: The axillary shoot can be a single shoot or a pair of axillary shoots at each node.
synonym: "2.02 Main shoot and axillary shoots visible at 2 nodes in soybean" [SOY:0000041]
synonym: "3.03-main shoot and two tillers" [GRO:0007072]
synonym: "BBCH growth stage 22" [ISBN:3826331524]
synonym: "Zadok scale-22" [GRO:0007072]
synonym: "main shoot and 2 tillers" [GRO:0007072]
synonym: "main shoot and second tiller visible" [GRO:0007072]
synonym: "main shoot and two tillers in barley" [GRO:0007072]
synonym: "main shoot and two tillers in oat" [GRO:0007072]
synonym: "main shoot and two tillers in wheat" [GRO:0007072]
synonym: "second axillary shoot detectable" []
synonym: "second tiller detectable" []
is_a: PO:0007073 ! 2 formation of axillary shoot

[Term]
id: PO:0007072
name: LP.18 eighteen leaves visible
namespace: plant_growth_and_development_stage
def: "The stage at which leaves at eighteen nodes\, other than the cotyledonary node\, are visible above ground." [GR:ap]
comment: The leaves can be a single leaf\, two\, or whorls of leaves at each node.
synonym: "1.18 17th trifoliolate leaf unfolded in soybean" [SOY:0000032]
synonym: "3.04-late vegetative" [GRO:0007016]
synonym: "3.4 late vegetative in maize" [MaizeGDB:67360]
synonym: "3.4 late vegetative stage of maize" [GRO:0007016]
synonym: "Stage V17 in soybean" [SOY:0000032]
synonym: "V18 in maize" [MaizeGDB:67360]
synonym: "late vegetative in maize" [MaizeGDB:67360]
synonym: "late vegetative stage of maize" [GRO:0007016]
synonym: "maize V18 stage" [GRO:0007016]
synonym: "maize growth stage-3.4" [GRO:0007016]
is_a: PO:0007133 ! leaf production

[Term]
id: PO:0007073
name: 2 formation of axillary shoot
namespace: plant_growth_and_development_stage
def: "The stage at which the axillary shoots are forming." [Poc:curators]
synonym: "03-tillering in barley" [GRO:0007069]
synonym: "03-tillering in oat" [GRO:0007069]
synonym: "03-tillering in wheat" [GRO:0007069]
synonym: "03-tillering stage in rice" [GRO:0007049]
synonym: "2 axillary Shoot Formation in soybean" [SOY:0000003]
synonym: "BBCH principal growth stage 2" [ISBN:3826331524]
synonym: "formation of side shoot" []
synonym: "rice growth stage-3" [GRO:0007049]
synonym: "tillering" []
is_a: PO:0007134 ! A vegetative growth

[Term]
id: PO:0007074
name: SE.15 fifteen nodes or internodes visible
namespace: plant_growth_and_development_stage
def: "The stage at which fifteen nodes or fifteen internodes are visible." [GR:pj ""]
comment: A measure of vegetative growth\, but leaf production is to be preferred.
synonym: "3.15 15 nodes/internodes visible in soybean" [SOY:0000064]
is_a: PO:0007089 ! stem elongation

[Term]
id: PO:0007075
name: 5.02 20% of inflorescence emerged.
namespace: plant_growth_and_development_stage
def: "OBSOLETE" [GR:ap]
is_obsolete: true

[Term]
id: PO:0007076
name: late rosette growth
namespace: plant_growth_and_development_stage
def: "Rosette has reached approximately 70% of its final diameter." [Poc:curators]
comment: A measure of vegetative growth\, but leaf production is to be preferred.
synonym: "late rosette growth in Arabidopsis" [TAIR:0000045]
is_a: PO:0007113 ! rosette growth

[Term]
id: PO:0007077
name: 2.08 main shoot and axillary shoots visible at eight nodes
namespace: plant_growth_and_development_stage
def: "The stage at which main shoot and axillary shoots at eight nodes are visible." [GR:ap]
comment: The axillary shoot can be a single shoot or a pair of axillary shoots at each node.
synonym: "2.08 Main shoot and axillary shoots visible at 8 nodes in soybean" [SOY:0000047]
synonym: "3.09-main shoot and eight tillers" [GRO:0007078]
synonym: "BBCH growth stage 28" [ISBN:3826331524]
synonym: "Zadok scale-28" [GRO:0007078]
synonym: "eighth axillary shoot detectable" []
synonym: "eighth tiller detectable" []
synonym: "main shoot and 8 tillers" []
synonym: "main shoot and eight tillers in barley" [GRO:0007078]
synonym: "main shoot and eight tillers in oat" [GRO:0007078]
synonym: "main shoot and eight tillers in wheat" [GRO:0007078]
synonym: "main shoot and eighth tiller visible" []
is_a: PO:0007073 ! 2 formation of axillary shoot

[Term]
id: PO:0007078
name: rosette growth complete
namespace: plant_growth_and_development_stage
def: "Stage at which rosette no longer increases in diameter\, its leaf growth and expansion having ceased." [Poc:curators]
comment: A measure of vegetative growth\, but leaf production is to be preferred.
synonym: "complete rosette in Arabidopsis" [TAIR:0000418]
is_a: PO:0007113 ! rosette growth

[Term]
id: PO:0007079
name: SE.00 stem elongation begins
namespace: plant_growth_and_development_stage
def: "The stage at which the internodes begin to elongate. " [GR:pj ""]
comment: A measure of vegetative growth\, but leaf production is to be preferred.
synonym: "3.00 stem elongation begins in soybean" [SOY:0000049]
synonym: "4.01-pseudo stem erection in barley" [GRO:0007081]
synonym: "4.01-pseudo stem erection in oat" [GRO:0007081]
synonym: "4.01-pseudo stem erection in wheat" [GRO:0007081]
synonym: "4.1-panicle initiation stage" [GRO:0007147]
synonym: "4.2-panicle differentiation stage" [GRO:0007041]
synonym: "BBCH growth stage 30" [ISBN:3826331524]
synonym: "pseudo stem and tillers erect" []
synonym: "pseudo stem erection" []
synonym: "rice green ring stage" []
synonym: "rice panicle initiation" []
is_a: PO:0007089 ! stem elongation

[Term]
id: PO:0007080
name: 2.03 main shoot and axillary shoots visible at three nodes
namespace: plant_growth_and_development_stage
def: "The stage at which main shoot and axillary shoots at three nodes are visible." [GR:ap]
comment: The axillary shoot can be a single shoot or a pair of axillary shoots at each node.
synonym: "2.03 Main shoot and axillary shoots visible at 3 nodes in soybean" [SOY:0000042]
synonym: "3.04-main shoot and three tillers" [GRO:0007073]
synonym: "BBCH growth stage 23" [ISBN:3826331524]
synonym: "Zadok scale-23" [GRO:0007073]
synonym: "main shoot and 3 tillers" []
synonym: "main shoot and third tiller visible" []
synonym: "main shoot and three tillers in barley" [GRO:0007073]
synonym: "main shoot and three tillers in oat" [GRO:0007073]
synonym: "main shoot and three tillers in wheat" [GRO:0007073]
synonym: "third axillary shoot detectable" []
synonym: "third tiller detectable" []
is_a: PO:0007073 ! 2 formation of axillary shoot

[Term]
id: PO:0007081
name: early rosette growth
namespace: plant_growth_and_development_stage
def: "Rosette has reached approximately 20% of its final diameter." [Poc:curators]
comment: A measure of vegetative growth\, but leaf production is to be preferred.
synonym: "early rosette growth in Arabidopsis" [TAIR:0000043]
is_a: PO:0007113 ! rosette growth

[Term]
id: PO:0007082
name: LP.20 twenty or more leaves whorls visible
namespace: plant_growth_and_development_stage
def: "The stage at which leaves at twenty or more nodes\, other than the cotyledonary node\, are visible above ground." [GR:ap]
comment: The leaves can be a single leaf\, two\, or whorls of leaves at each node.
synonym: "1.20 19th trifoliolate leaf unfolded in soybean" [SOY:0000034]
synonym: "1.21 20th trifoliolate leaf unfolded in soybean" [SOY:0000035]
synonym: "1.22 21st trifoliolate leaf unfolded in soybean" [SOY:0000036]
synonym: "1.23 22nd trifoliolate leaf unfolded in soybean" [SOY:0000037]
synonym: "1.24 23rd trifoliolate leaf unfolded in soybean" [SOY:0000038]
synonym: "1.25 25 or more trifoliolate leaves unfolded in soybean" [SOY:0000039]
synonym: "3.04-late vegetative" [GRO:0007016]
synonym: "3.4 late vegetative in maize" [MaizeGDB:67360]
synonym: "3.4 late vegetative stage of maize" [GRO:0007016]
synonym: "Stage V20 in soybean" [SOY:0000035]
synonym: "Stage V21 in soybean" [SOY:0000036]
synonym: "Stage V22 in soybean" [SOY:0000037]
synonym: "Stage V23 in soybean" [SOY:0000038]
synonym: "Stage V25 in soybean" [SOY:0000039]
synonym: "V20 in maize" [MaizeGDB:67360]
synonym: "late vegetative in maize" [MaizeGDB:67360]
synonym: "late vegetative stage of maize" [GRO:0007016]
synonym: "maize V20 stage" []
synonym: "maize growth stage-3.4" [GRO:0007016]
is_a: PO:0007133 ! leaf production

[Term]
id: PO:0007083
name: LP.13 thirteen leaves visible
namespace: plant_growth_and_development_stage
def: "The stage at which leaves at thirteen nodes\, other than the cotyledonary node\, are visible above ground." [GR:ap]
comment: The leaves can be a single leaf\, two\, or whorls of leaves at each node.
synonym: "1.13 12th trifoliolate leaf unfolded in soybean" [SOY:0000027]
synonym: "13 rosette leaf in Arabidopsis" [TAIR:0000416]
synonym: "3.03-mid-vegetative" [GRO:0007015]
synonym: "3.3 mid-vegetative" [MaizeGDB:67359]
synonym: "3.3 mid-vegetative stage of maize" [GRO:0007015]
synonym: "Stage V12 in soybean" [SOY:0000027]
synonym: "V13 in maize" [MaizeGDB:67359]
synonym: "maize growth stage-3.3" [GRO:0007015]
synonym: "mid-vegetative in maize" [MaizeGDB:67359]
synonym: "mid-vegetative stage of maize" [GRO:0007015]
synonym: "thirteen leaves unfolded" []
synonym: "thirteen rosette leaves" []
is_a: PO:0007133 ! leaf production

[Term]
id: PO:0007084
name: SE.10 ten nodes or internodes visible
namespace: plant_growth_and_development_stage
def: "The stage at which ten nodes or ten internodes are visible." [GR:pj ""]
comment: A measure of vegetative growth\, but leaf production is to be preferred.
synonym: "3.10 10 nodes/internodes visible in soybean" [SOY:0000059]
is_a: PO:0007089 ! stem elongation

[Term]
id: PO:0007085
name: LP.14 fourteen leaves visible
namespace: plant_growth_and_development_stage
def: "The stage at which leaves at fourteen nodes\, other than the cotyledonary node\, are visible above ground." [GR:ap]
comment: The leaves can be a single leaf\, two\, or whorls of leaves at each node.
synonym: "1.14 13th trifoliolate leaf unfolded in soybean" [SOY:0000028]
synonym: "14 rosette leaf in Arabidopsis" [TAIR:0000417]
synonym: "3.03-mid-vegetative" [GRO:0007015]
synonym: "3.3 mid-vegetative" [MaizeGDB:67359]
synonym: "3.3 mid-vegetative stage of maize" [GRO:0007015]
synonym: "Stage V13 in soybean" [SOY:0000028]
synonym: "V14 in maize" [MaizeGDB:67359]
synonym: "fourteen leaves unfolded" []
synonym: "fourteen rosette leaves" []
synonym: "maize growth stage-3.3" [GRO:0007015]
is_a: PO:0007133 ! leaf production

[Term]
id: PO:0007086
name: SE.05 five nodes or internodes visible
namespace: plant_growth_and_development_stage
def: "The stage at which five nodes or five internodes are visible." [GR:pj ""]
comment: A measure of vegetative growth\, but leaf production is to be preferred.
synonym: "3.05 5 nodes/internodes visible in soybean" [SOY:0000054]
synonym: "4.06-fifth node detectable in barley" [GRO:0007086]
synonym: "4.06-fifth node detectable in oat" [GRO:0007086]
synonym: "4.06-fifth node detectable in wheat" [GRO:0007086]
synonym: "BBCH growth stage 35" [ISBN:3826331524]
synonym: "Zadok scale-35" [GRO:0007086]
is_a: PO:0007089 ! stem elongation

[Term]
id: PO:0007087
name: 2.01 main shoot and axillary shoots visible at one node
namespace: plant_growth_and_development_stage
def: "The stage at which main shoot and axillary shoot(s) at one node is (are) visible." [Poc:curators]
synonym: "2.01 Main shoot and axillary shoot visible at one node in soybean" [SOY:0000040]
synonym: "3.02-main shoot and one tiller" [GRO:0007071]
synonym: "BBCH growth stage 21" [ISBN:3826331524]
synonym: "Zadok scale-21\, Feekes scale-2" [GRO:0007071]
synonym: "first axillary shoot detectable" []
synonym: "first tiller detectable" []
synonym: "main shoot and 1 tiller" []
synonym: "main shoot and first tiller visible" []
synonym: "main shoot and one tiller in barley" [GRO:0007071]
synonym: "main shoot and one tiller in oat" [GRO:0007071]
synonym: "main shoot and one tiller in wheat" [GRO:0007071]
is_a: PO:0007073 ! 2 formation of axillary shoot

[Term]
id: PO:0007088
name: 2.04 main shoot and axillary shoots visible at four nodes
namespace: plant_growth_and_development_stage
def: "The stage at which main shoot and axillary shoots at four nodes are visible." [GR:ap]
comment: The axillary shoot can be a single shoot or a pair of axillary shoots at each node.
synonym: "2.04 Main shoot and axillary shoots visible at 4 nodes in soybean" [SOY:0000043]
synonym: "3.05-main shoot and four tillers" [GRO:0007074]
synonym: "BBCH growth stage 24" [ISBN:3826331524]
synonym: "Zadok scale-24" [GRO:0007074]
synonym: "fourth axillary shoot detectable" []
synonym: "fourth tiller detectable" []
synonym: "main shoot and 4 tillers" []
synonym: "main shoot and four tillers in barley" [GRO:0007074]
synonym: "main shoot and four tillers in oat" [GRO:0007074]
synonym: "main shoot and four tillers in wheat" [GRO:0007074]
synonym: "main shoot and fourth tiller visible" []
is_a: PO:0007073 ! 2 formation of axillary shoot

[Term]
id: PO:0007089
name: stem elongation
namespace: plant_growth_and_development_stage
def: "The stage at which the internodes elongate. " [GR:pj ""]
comment: A measure of vegetative growth\, but leaf production is to be preferred.
synonym: "04-stem elongation in barley" [GRO:0007080]
synonym: "04-stem elongation in oat" [GRO:0007080]
synonym: "04-stem elongation in wheat" [GRO:0007080]
synonym: "04-stem elongation stage in Triticeae" [GRO:0007080]
synonym: "05-growing point differentiation" []
synonym: "3 Stem Elongation in soybean" [SOY:0000004]
synonym: "3 rapid stem elongation in maize" [MaizeGDB:67358]
synonym: "BBCH principal growth stage 3" [ISBN:3826331524]
synonym: "internode elongation" []
synonym: "jointing stage" [GRO:0007048]
synonym: "rapid stem elongation" []
synonym: "rice growth stage-4" [GRO:0007048]
synonym: "shoot development" []
synonym: "sorghum growth stage-4" [GRO:0007128]
is_a: PO:0007112 ! 1 main shoot growth

[Term]
id: PO:0007090
name: SE.13 thirteen nodes or internodes visible
namespace: plant_growth_and_development_stage
def: "The stage at which thirteen nodes or thirteen internodes are visible." [GR:pj ""]
comment: A measure of vegetative growth\, but leaf production is to be preferred.
synonym: "3.13 13 nodes/internodes visible in soybean" [SOY:0000062]
is_a: PO:0007089 ! stem elongation

[Term]
id: PO:0007091
name: SE.01 one node or internode visible
namespace: plant_growth_and_development_stage
def: "The stage at which one node or one internode is visible. " [GR:pj ""]
comment: A measure of vegetative growth\, but leaf production is to be preferred.
synonym: "3.01 one node visible in soybean" [SOY:0000050]
synonym: "4.02-first node detectable in barley" [GRO:0007082]
synonym: "4.02-first node detectable in oat" [GRO:0007082]
synonym: "4.02-first node detectable in wheat" [GRO:0007082]
synonym: "BBCH growth stage 31" [ISBN:3826331524]
synonym: "Zadok scale-31\, Feekes scale-6" [GRO:0007082]
is_a: PO:0007089 ! stem elongation

[Term]
id: PO:0007092
name: SE.04 four nodes or internodes visible
namespace: plant_growth_and_development_stage
def: "The stage at which four nodes or four internodes are visible." [GR:pj ""]
comment: A measure of vegetative growth\, but leaf production is to be preferred.
synonym: "3.04 4 nodes/internodes visible in soybean" [SOY:0000053]
synonym: "4.05-fourth node detectable in barley" [GRO:0007085]
synonym: "4.05-fourth node detectable in oat" [GRO:0007085]
synonym: "4.05-fourth node detectable in wheat" [GRO:0007085]
synonym: "BBCH growth stage 34" [ISBN:3826331524]
synonym: "Zadok scale-34" [GRO:0007085]
is_a: PO:0007089 ! stem elongation

[Term]
id: PO:0007093
name: 2.05 main shoot and axillary shoots visible at five nodes
namespace: plant_growth_and_development_stage
def: "The stage at which main shoot and axillary shoots at five nodes are visible." [GR:ap]
comment: The axillary shoot can be a single shoot or a pair of axillary shoots at each node.
synonym: "2.05 Main shoot and axillary shoots visible at 5 nodes in soybean" [SOY:0000044]
synonym: "3.06-main shoot and five tillers in Triticeae" [GRO:0007075]
synonym: "3.06-main shoot and five tillers in barley" [GRO:0007075]
synonym: "3.06-main shoot and five tillers in oat" [GRO:0007075]
synonym: "3.06-main shoot and five tillers in wheat" [GRO:0007075]
synonym: "BBCH growth stage 25" [ISBN:3826331524]
synonym: "Zadok scale-25" [GRO:0007075]
synonym: "fifth axillary shoot detectable" []
synonym: "fifth tiller detectable" []
synonym: "main shoot and 5 tillers" []
synonym: "main shoot and fifth tiller visible" []
synonym: "main shoot and five tillers in barley" [GRO:0007075]
synonym: "main shoot and five tillers in oat" [GRO:0007075]
synonym: "main shoot and five tillers in wheat" [GRO:0007075]
is_a: PO:0007073 ! 2 formation of axillary shoot

[Term]
id: PO:0007094
name: LP.01 one leaf visible
namespace: plant_growth_and_development_stage
def: "The stage at which leaves at one node\, other than the cotyledonary node\, are visible above ground." [Poc:curators, GR:ap]
comment: In the taxa with hypogeal type germination the first leaf on the epicotyl is leaf 1\, and in grasses\, the coleoptile is leaf 1.  The leaves can be a single leaf\, two\, or whorls of leaves at each node.
synonym: "1-4 leaf stage in rice" [GRO:0007142]
synonym: "1.01 Unifoliolate leaves unfolded in soybean" [SOY:0000015]
synonym: "1.02-one to two leaves in maize" [GRO:0007009]
synonym: "1.2 1-2 leaves in maize" [Maize:67353]
synonym: "2.02-first leaf unfolded in Triticeae" [GRO:0007060]
synonym: "2.02-first leaf unfolded in barley" [GRO:0007060]
synonym: "2.02-first leaf unfolded in oat" [GRO:0007060]
synonym: "2.02-first leaf unfolded in wheat" [GRO:0007060]
synonym: "BBCH growth stage 11" [ISBN:3826331524]
synonym: "V01 stage (sensu Zea)" []
synonym: "V1 in maize " [Maize:67353]
synonym: "VC stage in soybean" [SOY:0000015]
synonym: "Zadok scale-11\, Haun scale-1.+" [GRO:0007060]
synonym: "maize growth stage-1.2" [GRO:0007009]
synonym: "pre tillering" [GRO:0007142]
synonym: "rice growth stage-2.1" [GRO:0007142]
is_a: PO:0007133 ! leaf production

[Term]
id: PO:0007095
name: LP.08 eight leaves visible
namespace: plant_growth_and_development_stage
def: "The stage at which leaves at eight nodes\, other than the cotyledonary node\, are visible above ground." [GR:ap]
comment: The leaves can be a single leaf\, two\, or whorls of leaves at each node.
synonym: "1.08 7th trifoliolate leaf unfolded in soybean" [SOY:0000022]
synonym: "2.09-eight leaves unfolded in Triticeae" [GRO:0007067]
synonym: "2.09-eight leaves unfolded in barley" [GRO:0007067]
synonym: "2.09-eight leaves unfolded in oat" [GRO:0007067]
synonym: "2.09-eight leaves unfolded in wheat" [GRO:0007067]
synonym: "3.01-ear initiation in Maize" [GRO:0007013]
synonym: "3.1 ear initiation/mid-whorl stage in maize" [MaizeGDB:67356]
synonym: "8 leaves unfolded" []
synonym: "8 rosette leaves in Arabidopsis" [TAIR:0000411]
synonym: "8-leaf in maize" [MaizeGDB:67356]
synonym: "BBCH growth stage 18" [ISBN:3826331524]
synonym: "Stage V7 in soybean" [SOY:0000022]
synonym: "V8 in maize" [MaizeGDB:67356]
synonym: "Zadok scale-18\, Haun scale-7.+" [GRO:0007067]
synonym: "ear initiation in maize" [MaizeGDB:67356]
synonym: "eight leaf unfolded" []
synonym: "eight leaves unfolded (sensu Triticeae)" [GRO:0007067]
synonym: "eight rosette leaves" []
synonym: "maize growth stage-3.1" [GRO:0007013]
synonym: "mid-whorl stage in maize" [MaizeGDB:67356]
is_a: PO:0007133 ! leaf production

[Term]
id: PO:0007096
name: SE.03 three nodes or internodes visible
namespace: plant_growth_and_development_stage
def: "The stage at which three nodes or three internodes are visible." [GR:pj ""]
comment: A measure of vegetative growth\, but leaf production is to be preferred.
synonym: "3.03 3 nodes/internodes visible in soybean" [SOY:0000052]
synonym: "4.04-third node detectable in barley" [GRO:0007084]
synonym: "4.04-third node detectable in oat" [GRO:0007084]
synonym: "4.04-third node detectable in wheat" [GRO:0007084]
synonym: "BBCH growth stage 33" [ISBN:3826331524]
synonym: "Zadok scale-33" [GRO:0007084]
is_a: PO:0007089 ! stem elongation

[Term]
id: PO:0007097
name: SE.14 fourteen nodes or internodes visible
namespace: plant_growth_and_development_stage
def: "The stage at which fourteen nodes or fourteen internodes are visible." [GR:pj ""]
comment: A measure of vegetative growth\, but leaf production is to be preferred.
synonym: "3.14 14 nodes/internodes visible in soybean" [SOY:0000063]
is_a: PO:0007089 ! stem elongation

[Term]
id: PO:0007098
name: LP.02 two leaves visible
namespace: plant_growth_and_development_stage
def: "The stage at which leaves at two nodes\, other than the cotyledonary node\, are visible above ground." [Poc:curators]
comment: In grasses\, the plant has one leaf plus the coleoptile.  The leaves can be a single leaf\, two\, or whorls of leaves at each node.
synonym: "1-4 leaf stage in rice" [GRO:0007142]
synonym: "1.02 First trifoliolate leaf unfolded in soybean" [SOY:0000016]
synonym: "1.02-one to two leaves in maize" [GRO:0007009]
synonym: "1.2 1-2 leaves in maize" [MaizeGDB:67353]
synonym: "2 leaves unfolded" []
synonym: "2 rosette leaves in Arabidopsis" [TAIR:0000398]
synonym: "2.03-two leaves unfolded in Triticeae" [GRO:0007061]
synonym: "2.03-two leaves unfolded in barley" [GRO:0007061]
synonym: "2.03-two leaves unfolded in oat" [GRO:0007061]
synonym: "2.03-two leaves unfolded in wheat" [GRO:0007061]
synonym: "BBCH growth stage 12" [ISBN:3826331524]
synonym: "V1 stage in soybean" [SOY:0000016]
synonym: "V2 in maize" [MaizeGDB:67353]
synonym: "Zadok scale-12\, Haun scale-1.+" [GRO:0007061]
synonym: "maize growth stage-1.2" [GRO:0007009]
synonym: "pre tillering" [GRO:0007142]
synonym: "rice growth stage-2.1" [GRO:0007142]
synonym: "two leaves unfolded (sensu Triticeae)" [GRO:0007061]
synonym: "two rosette leaves" []
is_a: PO:0007133 ! leaf production

[Term]
id: PO:0007099
name: SE.97 flag leaf visible
namespace: plant_growth_and_development_stage
def: "The stage at which the flag leaf is visible." [GR:ap]
comment: A measure of vegetative growth\, but leaf production is to be preferred.
synonym: "06-flag leaf visible in sorghum" [GRO:0007129]
synonym: "4.08-flag leaf just visible in barley" [GRO:0007088]
synonym: "4.08-flag leaf just visible in oat" [GRO:0007088]
synonym: "4.08-flag leaf just visible in wheat" [GRO:0007088]
synonym: "Zadok scale-37\, Feekes scale-8" [GRO:0007088]
is_a: PO:0007089 ! stem elongation

[Term]
id: PO:0007100
name: SE.16 sixteen or more nodes or internodes visible
namespace: plant_growth_and_development_stage
def: "The stage at which sixteen nodes or more\, or sixteen internodes or more are visible." [GR:pj ""]
comment: A measure of vegetative growth\, but leaf production is to be preferred.
synonym: "3.16 16 or more nodes/internodes visible in soybean" [SOY:0000065]
is_a: PO:0007089 ! stem elongation

[Term]
id: PO:0007101
name: LP.09 nine leaves visible
namespace: plant_growth_and_development_stage
def: "The stage at which leaves at nine nodes\, other than the cotyledonary node\, are visible above ground." [GR:ap]
comment: The leaves can be a single leaf\, two\, or whorls of leaves at each node.
synonym: "1.09 8th trifoliolate leaf unfolded in soybean" [SOY:0000023]
synonym: "10-leaf in maize" [MaizeGDB:67357]
synonym: "2.10 nine or more leaves unfolded in Triticeae" [GRO:0007068]
synonym: "2.10 nine or more leaves unfolded in barley" [GRO:0007068]
synonym: "2.10 nine or more leaves unfolded in oat" [GRO:0007068]
synonym: "2.10 nine or more leaves unfolded in wheat" [GRO:0007068]
synonym: "3.02-late whorl stage" [GRO:0007014]
synonym: "3.2 late whorl stage in maize" [MaizeGDB:67357]
synonym: "9 or more leaves unfolded" []
synonym: "9 rosette leaf in Arabidopsis" [TAIR:0000412]
synonym: "9-11 leaves in maize" [MaizeGDB:67357]
synonym: "9-leaf in maize" [MaizeGDB:67357]
synonym: "BBCH growth stage 19" [ISBN:3826331524]
synonym: "Stage V8 in soybean" [SOY:0000023]
synonym: "V9 in maize" [MaizeGDB:67357]
synonym: "Zadok scale-19" [GRO:0007068]
synonym: "maize growth stage-3.2" [GRO:0007014]
synonym: "nine rosette leaves" []
synonym: "ninth leaf unfolded" []
is_a: PO:0007133 ! leaf production

[Term]
id: PO:0007102
name: 5.04 40% of inflorescence emerged
namespace: plant_growth_and_development_stage
def: "OBSOLETE" [GR:ap]
is_obsolete: true

[Term]
id: PO:0007103
name: LP.10 ten leaves visible
namespace: plant_growth_and_development_stage
def: "The stage at which leaves at ten nodes\, other than the cotyledonary node\, are visible above ground" [GR:ap]
comment: The leaves can be a single leaf\, two\, or whorls of leaves at each node.
synonym: "10 rosette leaf in Arabidopsis" [TAIR:0000413]
synonym: "10-leaf in maize" [MaizeGDB:67357]
synonym: "3.02-late whorl stage" [GRO:0007014]
synonym: "9-11 leaves in maize" [MaizeGDB:67357]
synonym: "Stage V9 in soybean" [SOY:0000024]
synonym: "V10 in maize" [MaizeGDB:67357]
synonym: "maize growth stage-3.2" [GRO:0007014]
synonym: "ten rosette leaves" []
is_a: PO:0007133 ! leaf production

[Term]
id: PO:0007104
name: LP.15 fifteen leaves visible
namespace: plant_growth_and_development_stage
def: "The stage at which leaves at fifteen nodes\, other than the cotyledonary node\, are visible above ground." [GR:ap]
comment: The leaves can be a single leaf\, two\, or whorls of leaves at each node.
synonym: "1.15 14th trifoliolate leaf unfolded in soybean" [SOY:0000029]
synonym: "3.4 late vegetative in maize" [MaizeGDB:67360]
synonym: "3.4 late vegetative stage of maize" [GRO:0007016]
synonym: "Stage V14 in soybean" [SOY:0000029]
synonym: "V15 in maize" [MaizeGDB:67360]
synonym: "late vegetative in maize" [MaizeGDB:67360]
synonym: "maize growth stage-3.4" [GRO:0007016]
is_a: PO:0007133 ! leaf production

[Term]
id: PO:0007105
name: 5.06 60% of inflorescence emerged
namespace: plant_growth_and_development_stage
def: "OBSOLETE" [GR:ap]
is_obsolete: true

[Term]
id: PO:0007106
name: LP.03 three leaves visible
namespace: plant_growth_and_development_stage
def: "The stage at which leaves at three nodes\, other than the cotyledonary node\, are visible above ground." [GR:ap]
comment: The leaves can be a single leaf\, two\, or whorls of leaves at each node.
synonym: "02-three leaf stage in sorghum" [GRO:0007126]
synonym: "1-4 leaf stage in rice" [GRO:0007142]
synonym: "1.03 2nd trifoliolate leaf unfolded in soybean" [SOY:0000017]
synonym: "1.03-three to four leaves in maize" [GRO:0007010]
synonym: "1.3 3-4 leaves in maize" [Maize:25331]
synonym: "2.04-three leaves unfolded" [GRO:0007062]
synonym: "3 rosette leaf in Arabidopsis" [TAIR:0000407]
synonym: "3-leaf stage in maize" [Maize:25331]
synonym: "BBCH growth stage 13" [ISBN:3826331524]
synonym: "V2 stage in soybean" [SOY:0000017]
synonym: "V3 in maize" [Maize:25331]
synonym: "Zadok scale-13\, Haun scale-2.+" [GRO:0007062]
synonym: "maize growth stage-1.3" [GRO:0007010]
synonym: "pre tillering" [GRO:0007142]
synonym: "rice growth stage-2.1" [GRO:0007142]
synonym: "sorghum growth stage-1" [GRO:0007126]
is_a: PO:0007133 ! leaf production

[Term]
id: PO:0007107
name: 5.08 80% of inflorescence emerged
namespace: plant_growth_and_development_stage
def: "OBSOLETE" [GR:ap]
is_obsolete: true

[Term]
id: PO:0007108
name: SE.07 seven nodes or internodes visible
namespace: plant_growth_and_development_stage
def: "The stage at which seven nodes or seven internodes are visible." [GR:pj ""]
comment: A measure of vegetative growth\, but leaf production is to be preferred.
synonym: "3.07 7 nodes/internodes visible in soybean" [SOY:0000056]
synonym: "BBCH growth stage 37" [ISBN:3826331524]
is_a: PO:0007089 ! stem elongation

[Term]
id: PO:0007109
name: SE.99 maximum stem length reached
namespace: plant_growth_and_development_stage
def: "The stage at which maximum stem length is reached." [GR:ap]
comment: A measure of vegetative growth\, but leaf production is to be preferred.
synonym: "3.99 Maximum stem length reached in soybean" [SOY:0000066]
synonym: "4.09-flag leaf ligule/collar just visible in barley" [GRO:0007089]
synonym: "4.09-flag leaf ligule/collar just visible in oat" [GRO:0007089]
synonym: "4.09-flag leaf ligule/collar just visible in wheat" [GRO:0007089]
synonym: "Zadok scale-39\, Feekes scale-9" [GRO:0007089]
synonym: "flag leaf fully unrolled" []
synonym: "flag leaf stage" []
synonym: "flag leaf stage in sorghum" [GRO:0007089]
synonym: "ligule just visible" []
synonym: "sorghum growth stage-5" [GRO:0007089]
is_a: PO:0007089 ! stem elongation

[Term]
id: PO:0007110
name: 2.09 main shoot and axillary shoots visible at  nine or more nodes
namespace: plant_growth_and_development_stage
def: "The stage at which main shoot and axillary shoots at nine nodes or more are visible." [GR:ap]
comment: The axillary shoot can be a single shoot or a pair of axillary shoots at each node.
synonym: "2.09 Main shoot and axillary shoots visible at 9 or more nodes in soybean" [SOY:0000048]
synonym: "3.1-maximum tillering" [GRO:0007144]
synonym: "3.10-main shoot and nine or more tillers in Triticeae" [GRO:0007079]
synonym: "BBCH growth stage 29" [ISBN:3826331524]
synonym: "Zadok scale-29" [GRO:0007079]
synonym: "main shoot and 9 or more tiller" [GRO:0007079]
synonym: "main shoot and nine or more tillers in barley" []
synonym: "main shoot and nine or more tillers in oat" []
synonym: "main shoot and nine or more tillers in wheat" []
synonym: "maximum number of tillers detectable in" []
synonym: "maximum number of tillers visible" []
synonym: "maximum number of tillers visible in rice" []
synonym: "nine or more axillary shoots detectable" []
is_a: PO:0007073 ! 2 formation of axillary shoot

[Term]
id: PO:0007111
name: SE.12 twelve nodes or internodes visible
namespace: plant_growth_and_development_stage
def: "The stage at which twelve nodes or twelve internodes are visible." [GR:pj ""]
comment: A measure of vegetative growth\, but leaf production is to be preferred.
synonym: "3.12 12 nodes/internodes visible in soybean" [SOY:0000061]
is_a: PO:0007089 ! stem elongation

[Term]
id: PO:0007112
name: 1 main shoot growth
namespace: plant_growth_and_development_stage
def: "The stage at which vegetative structures are being produced by SAM." [Poc:curators]
comment: In monocots each leaf stage is defined according to the uppermost leaf whose collar is visible (Handbook of plant and crop physiology)
synonym: "01-seedling stage of maize" [GRO:0007007]
synonym: "02-seedling growth of barley" [GRO:0007058]
synonym: "02-seedling growth of oat" [GRO:0007058]
synonym: "02-seedling growth of wheat" [GRO:0007058]
synonym: "02-seedling stage of rice" [GRO:0007047]
synonym: "1 seedling in maize" [MaizeGDB:1863]
synonym: "BBCH principal growth stage 1" [ISBN:3826331524]
synonym: "maize growth stage-1.1" [GRO:0007007]
synonym: "sorghum principal growth stage 1" [GRO:0007126]
is_a: PO:0007134 ! A vegetative growth

[Term]
id: PO:0007113
name: rosette growth
namespace: plant_growth_and_development_stage
def: "Stages of growth based on expansion of the rosette in Arabidopsis" [TAIR:ki]
comment: A measure of vegetative growth\, but leaf production is to be preferred.
synonym: "rosette growth in Arabidopsis" [TAIR:0000042]
is_a: PO:0007112 ! 1 main shoot growth

[Term]
id: PO:0007114
name: SE.11 eleven nodes or internodes visible
namespace: plant_growth_and_development_stage
def: "The stage at which eleven nodes or eleven internodes are visible." [GR:pj ""]
comment: A measure of vegetative growth\, but leaf production is to be preferred.
synonym: "3.11 11 nodes/internodes visible in soybean" [SOY:0000060]
is_a: PO:0007089 ! stem elongation

[Term]
id: PO:0007115
name: LP.04 four leaves visible
namespace: plant_growth_and_development_stage
def: "The stage at which leaves at four nodes\, other than the cotyledonary node\, are visible above ground." [GR:ap]
comment: The leaves can be a single leaf\, two\, or whorls of leaves at each node.
synonym: "02-tassel initiation in maize" [GRO:0007011]
synonym: "03-four leaf stage in sorghum" [GRO:0007143]
synonym: "1-4 leaf stage in rice" [GRO:0007142]
synonym: "1.03-three to four leaves in maize" [GRO:0007010]
synonym: "1.04 3rd trifoliolate leaf unfolded in soybean" [SOY:0000018]
synonym: "2 tassel initiation/early whorl stage in maize" [MaizeGDB:67306]
synonym: "2.05-four leaves unfolded in Triticeae" [GRO:0007063]
synonym: "4 leaves unfolded" []
synonym: "4 rosette leaf in Arabidopsis" [TAIR:0000399]
synonym: "4-6 leaves in maize" [MaizeGDB:67306]
synonym: "BBCH growth stage 14" [ISBN:3826331524]
synonym: "Stage V3 in soybean" [SOY:0000018]
synonym: "V4 in maize" [MaizeGDB:67306]
synonym: "Zadok scale-14\, Haun scale-3.+" [GRO:0007063]
synonym: "early whorl stage in maize" [MaizeGDB:67306]
synonym: "four rosette leaves" []
synonym: "fourth leaf unfolded" []
synonym: "maize growth stage-2" [GRO:0007011]
synonym: "pre tillering" [GRO:0007142]
synonym: "rice growth stage-2.1" [GRO:0007142]
synonym: "sorghum growth stage-2" [GRO:0007143]
synonym: "tassel differentiation in maize" [MaizeGDB:67306]
synonym: "tassel initiation in maize" [MaizeGDB:67306]
is_a: PO:0007133 ! leaf production

[Term]
id: PO:0007116
name: LP.11 eleven leaves visible
namespace: plant_growth_and_development_stage
def: "The stage at which leaves at eleven nodes\, other than the cotyledonary node\, are visible above ground." [GR:ap]
comment: The leaves can be a single leaf\, two\, or whorls of leaves at each node.
synonym: "1.11 10th trifoliolate leaf unfolded in soybean" [SOY:0000025]
synonym: "11 rosette leaves in Arabidopsis" [TAIR:0000414]
synonym: "3.02-late whorl stage in maize" [GRO:0007014]
synonym: "3.2 late whorl stage of maize" [GRO:0007014]
synonym: "9-11 leaves in maize" [MaizeGDB:67357]
synonym: "Stage V10 in soybean" [SOY:0000025]
synonym: "V11 in maize" [MaizeGDB:67357]
synonym: "eleven rosette leaves" []
synonym: "late whorl stage of maize" [GRO:0007014]
synonym: "maize growth stage-3.2" [GRO:0007014]
is_a: PO:0007133 ! leaf production

[Term]
id: PO:0007117
name: SE.02 two nodes or internodes visible
namespace: plant_growth_and_development_stage
def: "The stage at which two nodes or two internodes are visible." [GR:pj ""]
comment: A measure of vegetative growth\, but leaf production is to be preferred.
synonym: "3.02 2 nodes/internode visible in soybean" [SOY:0000051]
synonym: "4.03-second node detectable in barley" [GRO:0007083]
synonym: "4.03-second node detectable in oat" [GRO:0007083]
synonym: "4.03-second node detectable in wheat" [GRO:0007083]
synonym: "BBCH growth stage 32" [ISBN:3826331524]
synonym: "Zadok scale-32\, Feekes scale-7" [GRO:0007083]
synonym: "maize growth stage-3.1" [GRO:0007013]
is_a: PO:0007089 ! stem elongation

[Term]
id: PO:0007118
name: 2.06 main shoot and axillary shoots visible at six nodes
namespace: plant_growth_and_development_stage
def: "The stage at which main shoot and axillary shoots at six nodes are visible." [GR:ap]
comment: The axillary shoot can be a single shoot or a pair of axillary shoots at each node.
synonym: "2.06 Main shoot and axillary shoots visible at 6 nodes in soybean" [SOY:0000045]
synonym: "3.07-main shoot and six tillers" [GRO:0007076]
synonym: "BBCH growth stage 26" [ISBN:3826331524]
synonym: "Zadok scale-26\, Feekes scale-3" [GRO:0007076]
synonym: "main shoot and 6 tillers" []
synonym: "main shoot and six tillers in barley" [GRO:0007076]
synonym: "main shoot and six tillers in oat" [GRO:0007076]
synonym: "main shoot and six tillers in wheat" [GRO:0007076]
synonym: "sixth axillary shoot detectable" []
synonym: "sixth tiller detectable" []
is_a: PO:0007073 ! 2 formation of axillary shoot

[Term]
id: PO:0007119
name: LP.16 sixteen leaves visible
namespace: plant_growth_and_development_stage
def: "The stage at which leaves at sixteen nodes\, other than the cotyledonary node\, are visible above ground." [GR:ap]
comment: The leaves can be a single leaf\, two\, or whorls of leaves at each node.
synonym: "1.16 15th trifoliolate leaf unfolded in soybean" [SOY:0000030]
synonym: "16 rosette leaf in Arabidopsis" [TAIR:0000036]
synonym: "3.04-late vegetative" [GRO:0007016]
synonym: "3.4 late vegetative in maize" [MaizeGDB:67360]
synonym: "3.4 late vegetative stage of maize" [GRO:0007016]
synonym: "Stage V15 in soybean" [SOY:0000030]
synonym: "V16 in maize" [MaizeGDB:67360]
synonym: "late vegetative in maize" [MaizeGDB:67360]
synonym: "late vegetative stage of maize" [GRO:0007016]
synonym: "maize growth stage-3.4" [GRO:0007016]
is_a: PO:0007133 ! leaf production

[Term]
id: PO:0007120
name: LP.19 nineteen leaves visible
namespace: plant_growth_and_development_stage
def: "The stage at which leaves at nineteen nodes\, other than the cotyledonary node\, are visible above ground." [GR:ap]
comment: The leaves can be a single leaf\, two\, or whorls of leaves at each node.
synonym: "1.19 18th trifoliolate leaf unfolded in soybean" [SOY:0000033]
synonym: "3.04-late vegetative" [GRO:0007016]
synonym: "3.4 late vegetative in maize" [MaizeGDB:67360]
synonym: "3.4 late vegetative stage of maize" [GRO:0007016]
synonym: "Stage V18 in soybean" [SOY:0000033]
synonym: "V19 in maize" [MaizeGDB:67360]
synonym: "late vegetative in maize" [MaizeGDB:67360]
synonym: "late vegetative stage of maize" [GRO:0007016]
synonym: "maize growth stage-3.4" [GRO:0007016]
is_a: PO:0007133 ! leaf production

[Term]
id: PO:0007121
name: 6.01 10% of flowers open
namespace: plant_growth_and_development_stage
def: "OBSOLETE" [GR:ap]
is_obsolete: true

[Term]
id: PO:0007122
name: 2.07 main shoot and axillary shoots visible at seven nodes
namespace: plant_growth_and_development_stage
def: "The stage at which main shoot and axillary shoots at seven nodes are visible." [GR:ap]
comment: The axillary shoot can be a single shoot or a pair of axillary shoots at each node.
synonym: "2.07 Main shoot and axillary shoots visible at 7 nodes in soybean" [SOY:0000046]
synonym: "3.08-main shoot and seven tillers" [GRO:0007077]
synonym: "BBCH growth stage 27" [ISBN:3826331524]
synonym: "Zadok scale-27" [GRO:0007077]
synonym: "main shoot and 7 tillers" []
synonym: "main shoot and seven tillers in barley" [GRO:0007077]
synonym: "main shoot and seven tillers in oat" [GRO:0007077]
synonym: "main shoot and seven tillers in wheat" [GRO:0007077]
synonym: "main shoot and seventh tiller visible" []
synonym: "seventh axillary shoot detectable" []
synonym: "seventh tiller detectable" []
is_a: PO:0007073 ! 2 formation of axillary shoot

[Term]
id: PO:0007123
name: LP.06 six leaves visible
namespace: plant_growth_and_development_stage
def: "The stage at which leaves at six nodes\, other than the cotyledonary node\, are visible above ground." [GR:ap]
comment: The leaves can be a single leaf\, two\, or whorls of leaves at each node.
synonym: "03-tillering stage in rice" [GRO:0007049]
synonym: "1.06 5th trifoliolate leaf unfolded in soybean" [SOY:0000020]
synonym: "2 tassel initiation/early whorl stage in maize" [MaizeGDB:67306]
synonym: "2.07-six leaves unfolded in Triticeae" [GRO:0007065]
synonym: "3.01-ear initiation in maize" [GRO:0007013]
synonym: "3.1 ear initiation/mid-whorl stage in maize" [MaizeGDB:67356]
synonym: "6 leaves unfolded" []
synonym: "6 rosette leaf in Arabidopsis" [TAIR:0000409]
synonym: "6-8 leaves in maize" [MaizeGDB:67356]
synonym: "6-leaf in maize" [MaizeGDB:67356]
synonym: "BBCH growth stage 16" [ISBN:3826331524]
synonym: "Stage V5 in soybean" [SOY:0000020]
synonym: "V6 in maize" [MaizeGDB:67306]
synonym: "Zadok scale-16\, Haun scale-5.+" [GRO:0007065]
synonym: "ear initiation in maize" [MaizeGDB:67356]
synonym: "early whorl stage in maize" [MaizeGDB:67306]
synonym: "maize growth stage-3.1" [GRO:0007012]
synonym: "mid-whorl stage in maize" [MaizeGDB:67356]
synonym: "rice growth stage-3" [GRO:0007049]
synonym: "six leaves unfolded (sensu Triticeae)" [GRO:0007065]
synonym: "six rosette leaves" []
synonym: "sixth leaf unfolded" []
is_a: PO:0007133 ! leaf production

[Term]
id: PO:0007124
name: 6.03 30% of flowers open
namespace: plant_growth_and_development_stage
def: "OBSOLETE" [GR:ap]
is_obsolete: true

[Term]
id: PO:0007125
name: 6.04 40% of flowers open
namespace: plant_growth_and_development_stage
def: "OBSOLETE" [GR:ap]
is_obsolete: true

[Term]
id: PO:0007126
name: 7.02 fruit size 20%
namespace: plant_growth_and_development_stage
def: "OBSOLETE" [GR:ap]
is_obsolete: true

[Term]
id: PO:0007127
name: 7.04 fruit size 40%
namespace: plant_growth_and_development_stage
def: "OBSOLETE" [GR:ap]
synonym: "7.2 milk stage/embryo 2 in maize" [MaizeGDB:67373]
is_obsolete: true

[Term]
id: PO:0007128
name: 7.06 fruit size 60%
namespace: plant_growth_and_development_stage
def: "OBSOLETE" [GR:ap]
is_obsolete: true

[Term]
id: PO:0007129
name: 7.08 fruit size 80%
namespace: plant_growth_and_development_stage
def: "OBSOLETE" [GR:ap]
is_obsolete: true

[Term]
id: PO:0007130
name: B reproductive growth
namespace: plant_growth_and_development_stage
def: "Stage of growth when reproductive structures are being produced." [Poc:curators ""]
synonym: "B-reproductive stage in rice" [GRO:0007140]
synonym: "reproductive in Arabidopsis" [TAIR:0000306]
is_a: PO:0007033 ! whole plant growth stage

[Term]
id: PO:0007131
name: 0.2 seedling growth
namespace: plant_growth_and_development_stage
def: "Growth of embryo after imbibition up to the development of the first adult leaves." [Poc:curators ""]
synonym: "seedling in Arabidopsis" [TAIR:0000027]
relationship: part_of PO:0007057 ! 0 germination

[Term]
id: PO:0007132
name: D dormancy
namespace: plant_growth_and_development_stage
def: "A suspension of physiological activity that can be reactivated once it is broken." [Poc:curators ""]
synonym: "10.05-seed dormant in Triticeae" [GRO:0007119]
synonym: "10.05-seed dormant in barley" [GRO:0007119]
synonym: "10.05-seed dormant in oat" [GRO:0007119]
synonym: "10.05-seed dormant in wheat" [GRO:0007119]
synonym: "10.06-viable seed germination in Triticeae" [GRO:0007120]
synonym: "10.06-viable seed germination in barley" [GRO:0007120]
synonym: "10.06-viable seed germination in oat" [GRO:0007120]
synonym: "10.06-viable seed germination in wheat" [GRO:0007120]
synonym: "10.07-seed not dormant in Triticeae" [GRO:0007121]
synonym: "10.07-seed not dormant in barley" [GRO:0007121]
synonym: "10.07-seed not dormant in oat" [GRO:0007121]
synonym: "10.07-seed not dormant in wheat" [GRO:0007121]
synonym: "10.08-secondary dormancy induced in Triticeae" [GRO:0007122]
synonym: "10.08-secondary dormancy induced in barley" [GRO:0007122]
synonym: "10.08-secondary dormancy induced in oat" [GRO:0007122]
synonym: "10.08-secondary dormancy induced in wheat" [GRO:0007122]
synonym: "10.09-secondary dormancy lost in Triticeae" [GRO:0007123]
synonym: "10.09-secondary dormancy lost in barley" [GRO:0007123]
synonym: "10.09-secondary dormancy lost in oat" [GRO:0007123]
synonym: "10.09-secondary dormancy lost in wheat" [GRO:0007123]
is_a: PO:0007033 ! whole plant growth stage

[Term]
id: PO:0007133
name: leaf production
namespace: plant_growth_and_development_stage
def: "The stage at which the leaves produced by SAM are visible above the ground in a seedling or mature plant." [Poc:curators ""]
comment: This stage is recommended over rosette growth or stem elongation as it is most easily observed and least ambiguous.
is_a: PO:0007112 ! 1 main shoot growth

[Term]
id: PO:0007134
name: A vegetative growth
namespace: plant_growth_and_development_stage
def: "Stage of growth when vegetative structures are being produced." [Poc:curators ""]
synonym: "A-vegetative stage in rice" [GRO:0007139]
synonym: "vegetative in Arabidopsis" [TAIR:0000305]
is_a: PO:0007033 ! whole plant growth stage

[Term]
id: PO:0009012
name: plant growth and development stage
namespace: plant_growth_and_development_stage
def: "The succession of changes leading from the zygote to the mature plant. " [Poc:curators ""]
synonym: "Arabidopsis growth" [TAIR:0000205]

[Typedef]
id: develops_from
name: develops from

[Typedef]
id: part_of
name: part of

