format-version: 1.2
date: 21:04:2010 15:56
auto-generated-by: OBO-Edit 2.1-beta3
default-namespace: plant_ontology

[Term]
id: PO:0001000
name: meristem eloboration
namespace: plant_growth_and_development_stage
def: "OBSOLETE. the root meristem gets organized" [GR:ap]
comment: This  term has been obsoleted to keep the structure simple.
is_obsolete: true

[Term]
id: PO:0001002
name: fruit development stages
namespace: plant_growth_and_development_stage
def: "Stages of development of a fruit defined by characteristic morphological, structural, histological or other visible features. " [POC:curators]
synonym: "stage 17 flower in Arabidopsis" RELATED []
synonym: "stage 18 flower in Arabidopsis" RELATED []
is_a: PO:0007021 ! plant structure development stages

[Term]
id: PO:0001003
name: formation of the leaf founder cells
namespace: plant_growth_and_development_stage
def: "The initial stage of leaf development  where cells in the SAM are already determined to form a leaf primordium, but the primordium itself is not distinguishable morphologically." [TAIR:ki]
synonym: "P0 stage" RELATED []
is_a: PO:0001051 ! 1 leaf initiation stage

[Term]
id: PO:0001004
name: anther developmental stages
namespace: plant_growth_and_development_stage
def: "Stages of development of the anther defined by characteristic morphological, cytological, histological or other visible features." [POC:fz]
is_a: PO:0007605 ! androecium developmental stages

[Term]
id: PO:0001005
name: A archesporial cells visible
namespace: plant_growth_and_development_stage
def: "An initial stage during which archesporial cells arise in four corners of L2 layer. Change in shape of primordia to more oval." [TAIR:ki]
is_a: PO:0001004 ! anther developmental stages

[Term]
id: PO:0001006
name: B enlarged microsporocyte stage
namespace: plant_growth_and_development_stage
def: "Stage during which the microsporocytes become conspicuous." [TAIR:ki]
synonym: "pollen stage 2 in Arabidopsis" RELATED []
is_a: PO:0001007 ! pollen developmental stages

[Term]
id: PO:0001007
name: pollen developmental stages
namespace: plant_growth_and_development_stage
def: "Stages of development of the pollen defined by characteristic morphological, cytological, histological or other visible features." [POC:fz]
synonym: "pollen development in Arabidopsis" RELATED []
is_a: PO:0007605 ! androecium developmental stages

[Term]
id: PO:0001008
name: C callose wall formation in pollen mother cells
namespace: plant_growth_and_development_stage
def: "Stage during which diploid pollen mother cells become separated from each other and from tapetum by a callose wall." [TAIR:ki]
synonym: "pollen mother cell stage" RELATED []
synonym: "pollen stage 3 in Arabidopsis" RELATED []
is_a: PO:0001007 ! pollen developmental stages

[Term]
id: PO:0001009
name: D pollen mother cell meiosis stage
namespace: plant_growth_and_development_stage
def: "Stage during which pollen mother cells undergo meiosis to form tetrads of microspores." [TAIR:ki]
synonym: "pollen stage 4 in Arabidopsis" RELATED []
is_a: PO:0001007 ! pollen developmental stages

[Term]
id: PO:0001010
name: F microspore release stage
namespace: plant_growth_and_development_stage
def: "Stage of microgametophyte development during which the callose wall between the tetrads breaks down and haploid microspores are released and lie freely in locules. " [TAIR:ki]
synonym: "pollen stage 5 in Arabidopsis" RELATED []
is_a: PO:0001007 ! pollen developmental stages

[Term]
id: PO:0001011
name: A microsporogenous mass stage
namespace: plant_growth_and_development_stage
def: "An initial stage during which the archesporial cells divide to give rise to primary parietal and sporogenous cells." [TAIR:ki]
synonym: "pollen stage 1 in Arabidopsis" RELATED []
is_a: PO:0001007 ! pollen developmental stages

[Term]
id: PO:0001012
name: G early unicellular microspore stage
namespace: plant_growth_and_development_stage
def: "Stage of microgametophyte development during which the microspores round up and small vacuoles appear in their cytoplasm.  The microspore walls thicken due to the formation of the exine." [TAIR:ki]
synonym: "pollen stage 6 in Arabidopsis" RELATED []
is_a: PO:0001007 ! pollen developmental stages

[Term]
id: PO:0001013
name: H late unicellular microspore stage
namespace: plant_growth_and_development_stage
def: "Stage of microgametophyte development during which a large vacuole is formed in each microspore causing a rapid increase in size and a displacement of the nucleus to one side." [TAIR:ki]
synonym: "pollen stage 7 in Arabidopsis" RELATED []
is_a: PO:0001007 ! pollen developmental stages

[Term]
id: PO:0001014
name: I first mitotic division stage
namespace: plant_growth_and_development_stage
def: "Stage of microgametophyte development during which the asymmetric, first mitotic division of the microspores occurs producing a large vegetative cell and small generative cell, located near pollen wall." [TAIR:ki]
synonym: "pollen stage 8 in Arabidopsis" RELATED []
is_a: PO:0001007 ! pollen developmental stages

[Term]
id: PO:0001015
name: K second mitotic division stage
namespace: plant_growth_and_development_stage
def: "Stage of microgametophyte development during which the generative cell undergoes mitotic division to form two male gametes, the sperm cells." [TAIR:ki]
comment: In taxa with mature two-celled pollen, the second mitotic division takes place after pollen germination, in germinating pollen tube.
synonym: "pollen stage 9 in Arabidopsis" RELATED []
is_a: PO:0001007 ! pollen developmental stages

[Term]
id: PO:0001016
name: L mature pollen stage
namespace: plant_growth_and_development_stage
def: "Stage of microgametophyte development during which the pollen reaches mature stage and desiccates. " [TAIR:ki]
comment: Mature pollen stages is reached at three-celled pollen in some angiosperms (maize, rice and Arabidopsis), while in others, the maturepollen has  two haploid cells  (tobacco, snapdragon).
synonym: "pollen stage 10 in Arabidopsis" RELATED []
is_a: PO:0001007 ! pollen developmental stages

[Term]
id: PO:0001017
name: M germinated pollen stage
namespace: plant_growth_and_development_stage
def: "The final stage in the life cycle of the male gametophyte. Upon rehydration, mature pollen grain forms a tubular outgrowth, the pollen tube, which carries the male gametes." [TAIR:ki]
synonym: "germinated pollen grain in Arabidopsis" RELATED []
is_a: PO:0001007 ! pollen developmental stages

[Term]
id: PO:0001018
name: B formation of primary parietal and sporogenous cells
namespace: plant_growth_and_development_stage
def: "Stage during which the primary parietal and  primary sporogenous layers are derived from archesporial cells." [TAIR:ki]
is_a: PO:0001004 ! anther developmental stages

[Term]
id: PO:0001019
name: formation of leaf primordium
namespace: plant_growth_and_development_stage
def: "Stage of leaf development  when leaf primordium is formed as a small protrusion on the flank of SAM." [TAIR:ki]
synonym: "P1 stage" RELATED []
is_a: PO:0001052 ! 2 leaf expansion stage

[Term]
id: PO:0001020
name: hood-shaped primordium
namespace: plant_growth_and_development_stage
def: "Stage of leaf development  when a hood-shaped  primordium is formed, partially enclosing P1 and SAM, as in Poaceae." [TAIR:ki]
synonym: "P2 stage" RELATED []
is_a: PO:0001052 ! 2 leaf expansion stage

[Term]
id: PO:0001021
name: formation of ligule primordium
namespace: plant_growth_and_development_stage
def: "Stage of leaf development  when conical P3 leaf completely encloses SAM, and the ligule primordium is visible, as in Poaceae. " [TAIR:ki]
synonym: "P3 stage" RELATED []
is_a: PO:0001052 ! 2 leaf expansion stage

[Term]
id: PO:0001023
name: rapid elongation of leaf blade
namespace: plant_growth_and_development_stage
def: "Stage of leaf development  during which a rapid elongation of the leaf blade occurs; the elongation of the leaf sheath has not started, as in Poaceae." [TAIR:ki]
synonym: "P4 stage" RELATED []
is_a: PO:0001052 ! 2 leaf expansion stage

[Term]
id: PO:0001024
name: rapid elongation of leaf sheath
namespace: plant_growth_and_development_stage
def: "Stage of leaf development  during which a rapid elongation of the leaf sheath occurs, as in Poaceae." [TAIR:ki]
synonym: "P5 stage" RELATED []
is_a: PO:0001052 ! 2 leaf expansion stage

[Term]
id: PO:0001025
name: C four anther lobes formed
namespace: plant_growth_and_development_stage
def: "Stage during which the four-lobed anther pattern with two developing stomium regions (notch) are formed." [TAIR:ki]
is_a: PO:0001004 ! anther developmental stages

[Term]
id: PO:0001026
name: D locules established
namespace: plant_growth_and_development_stage
def: "Stage during which the four clearly defined locules are established. All anther cell types present and microspore mother cells appear." [TAIR:ki]
synonym: "stage 8 flower in Arabidopsis" RELATED []
is_a: PO:0001004 ! anther developmental stages

[Term]
id: PO:0001027
name: meristamtic zone formation
namespace: plant_growth_and_development_stage
def: "OBSOLETE. The meristematic zone is formed" [GR:ap]
is_obsolete: true

[Term]
id: PO:0001028
name: elongation zone formation
namespace: plant_growth_and_development_stage
def: "OBSOLETE. The cells of root primordium undergo elonagtion" [GR:ap]
is_obsolete: true

[Term]
id: PO:0001029
name: E tetrad stage
namespace: plant_growth_and_development_stage
def: "Stage immediately following meiosis, during which the tetrads of microspores are still hold together, enclosed by the callose wall. " [TAIR:ki]
is_a: PO:0001007 ! pollen developmental stages

[Term]
id: PO:0001030
name: specialization zone formation
namespace: plant_growth_and_development_stage
def: "OBSOLETE. The cells develop their characteristic morphology." [GR:ap]
is_obsolete: true

[Term]
id: PO:0001031
name: 4 root elongation
namespace: plant_growth_and_development_stage
def: "The stage at which root is elongating." [POC:cuartors]
comment: In some plant species this stage is subdivided into distal and proximal elongating zones.
synonym: "Benfey's stage 2 of root development" RELATED []
is_a: PO:0007520 ! root development stages

[Term]
id: PO:0001032
name: E tapetum degeneration initiated
namespace: plant_growth_and_development_stage
def: "Stage during which degeneration of the tapetum is initiated, as the deposition on the surface of the microspore primexine proceeds." [TAIR:ki]
comment: Microspores within single locule are at unicellular stage.
is_a: PO:0001004 ! anther developmental stages

[Term]
id: PO:0001034
name: F bilocular anther stage
namespace: plant_growth_and_development_stage
def: "Stage during which anther becomes bilocular, after degeneration and breakage of septum below stomium." [TAIR:ki]
is_a: PO:0001004 ! anther developmental stages

[Term]
id: PO:0001035
name: G anther dehiscence
namespace: plant_growth_and_development_stage
def: "Stage during which the dehiscence of anthers occurs. Anther breaks along stomium and pollen is released." [TAIR:ki]
is_a: PO:0001004 ! anther developmental stages

[Term]
id: PO:0001036
name: H anther senescence
namespace: plant_growth_and_development_stage
def: "Stage during which the senescence of anther and stamen occurs. Shrinkage of cells and anther structure takes place." [TAIR:ki]
is_a: PO:0001004 ! anther developmental stages

[Term]
id: PO:0001040
name: dry seed stage
namespace: plant_growth_and_development_stage
alt_id: PO:0007055
def: "Mature seed with low moisture content." [TAIR:ki]
synonym: "00 Dry Seed in soybean" RELATED [SOY:0000009]
synonym: "1.01-dry seed in Tricticeae" RELATED [GRO:0007052]
synonym: "BBCH growth stage 00" RELATED [ISBN:3826331524]
synonym: "dry seed in Arabidopsis" RELATED [TAIR:0000213]
is_a: PO:0001170 ! seed development stages
xref_unknown: GRO:0007052
xref_unknown: ISBN:3826331524
xref_unknown: SOY:0000009
xref_unknown: TAIR:0000213

[Term]
id: PO:0001041
name: chalazal and micropylar domain establishment
namespace: plant_growth_and_development_stage
def: "The initial stage of endosperm development during which the chalazal and micropilar domains are established." [TAIR:ki]
is_a: PO:0007633 ! endosperm development stages

[Term]
id: PO:0001042
name: functional specialization of the endosperm
namespace: plant_growth_and_development_stage
def: "Stage of endosperm development during which the functional specialization of the maturing endosperm occurs." [TAIR:ki]
is_a: PO:0007633 ! endosperm development stages

[Term]
id: PO:0001044
name: sepal differentiation and expansion stage
namespace: plant_growth_and_development_stage
def: "Stage of calyx development defined by differentiation and expansion of sepal." [POC:fz]
is_a: PO:0007603 ! calyx developmental stages

[Term]
id: PO:0001045
name: fully expanded sepal
namespace: plant_growth_and_development_stage
def: "Stage of calyx development when sepal is fully expanded." [POC:fz]
is_a: PO:0007603 ! calyx developmental stages

[Term]
id: PO:0001047
name: lemma developmental stages
namespace: plant_growth_and_development_stage
def: "Stages of development of the lemma defined by characteristic morphological, structural, histological or other visible features." [GR:ap, POC:fz]
is_a: PO:0007600 ! 3 floral organ development stages

[Term]
id: PO:0001048
name: palea developmental stages
namespace: plant_growth_and_development_stage
def: "Stages of development of the palea defined by characteristic morphological, structural, histological or other visible features." [GR:ap, POC:fz]
is_a: PO:0007600 ! 3 floral organ development stages

[Term]
id: PO:0001049
name: lodicule developmental stages
namespace: plant_growth_and_development_stage
def: "Stages of development of the lodicule defined by characteristic morphological, structural, histological or other visible features." [GR:ap, POC:fz]
is_a: PO:0007600 ! 3 floral organ development stages

[Term]
id: PO:0001050
name: leaf development stages
namespace: plant_growth_and_development_stage
alt_id: PO:0007040
def: "Stages of development of a leaf defined by characteristic morphological, structural, histological or other visible features. " [POC:curators, TAIR:tb]
synonym: "leaf development in Arabidopsis" RELATED []
synonym: "leaf development stage" RELATED []
is_a: PO:0007021 ! plant structure development stages

[Term]
id: PO:0001051
name: 1 leaf initiation stage
namespace: plant_growth_and_development_stage
alt_id: PO:0001003
def: "The earliest histological evidence of leaf initiation, i.e, a change in the orientation of cell division both in the epidermis and in internal layers of the shoot meristem occurs at this stage (Poethig S, 1997, Plant Cell 9:1077-1087)." [PMID:9254931]
comment: Cells in the primordium are not yet differentiated.
synonym: "leaf initiation in Arabidopsis" RELATED []
is_a: PO:0001050 ! leaf development stages

[Term]
id: PO:0001052
name: 2 leaf expansion stage
namespace: plant_growth_and_development_stage
def: "Stage of leaf development which begins when cell differentiation and cell expansion occurs and finishes when the leaf reaches its full size.\n" [TAIR:ki]
synonym: "leaf expansion stage in Arabidopsis" RELATED []
is_a: PO:0001050 ! leaf development stages

[Term]
id: PO:0001053
name: 3 leaf fully expanded
namespace: plant_growth_and_development_stage
def: "Stage of leaf development when leaf is fully expanded." [TAIR:ki]
synonym: "fully expanded leaf stage in Arabidopsis" RELATED []
is_a: PO:0001050 ! leaf development stages

[Term]
id: PO:0001054
name: 4 leaf senescence stage
namespace: plant_growth_and_development_stage
def: "The final stage of leaf development when the leaf ceases metabolic activity and senesces." [TAIR:tb]
synonym: "leaf senescence stage in Arabidopsis" RELATED []
is_a: PO:0001050 ! leaf development stages

[Term]
id: PO:0001055
name: lemma primordia visible
namespace: plant_growth_and_development_stage
def: "Stage of lemma development that begins when the lemma primordia arise." [POC:fz]
comment: The lemma primordium forms in 1/2 alternate phylotaxy in rice spikelet.
is_a: PO:0001047 ! lemma developmental stages

[Term]
id: PO:0001056
name: lemma differentiation and expansion stage
namespace: plant_growth_and_development_stage
def: "Stage of lemma development defined by differentiation and expansion of lemma." [POC:fz]
is_a: PO:0001047 ! lemma developmental stages

[Term]
id: PO:0001057
name: fully expanded lemma
namespace: plant_growth_and_development_stage
def: "Stage of lemma development when lemma is fully expanded." [POC:fz]
is_a: PO:0001047 ! lemma developmental stages

[Term]
id: PO:0001058
name: palea primordia visible
namespace: plant_growth_and_development_stage
def: "Stage of palea development that begins when the palea primordia arise." [POC:fz]
comment: The palea primordium forms in 1/2 alternate phylotaxy in rice spikelet.
is_a: PO:0001048 ! palea developmental stages

[Term]
id: PO:0001059
name: J bicellular pollen stage
namespace: plant_growth_and_development_stage
def: "Stage of microgametophyte development during which the small generative cell moves inward, becoming completely surrounded by the cytoplasm of the vegetative cell. " [TAIR:ki]
is_a: PO:0001007 ! pollen developmental stages

[Term]
id: PO:0001070
name: palea differentiation and expansion stage
namespace: plant_growth_and_development_stage
def: "Stage of palea development defined by differentiation and expansion of palea." [POC:fz]
is_a: PO:0001048 ! palea developmental stages

[Term]
id: PO:0001071
name: fully expanded palea
namespace: plant_growth_and_development_stage
def: "Stage of palea development when palea is fully expanded." [POC:fz]
is_a: PO:0001048 ! palea developmental stages

[Term]
id: PO:0001072
name: lodicule primordia visible
namespace: plant_growth_and_development_stage
def: "Stage of lodicule development that begins when the lodicule primordia arise." [POC:fz]
comment: Two lodicules form on the side of the lemma in rice spikelet.
is_a: PO:0001049 ! lodicule developmental stages

[Term]
id: PO:0001074
name: N second mitotic division stage in germinating pollen
namespace: plant_growth_and_development_stage
def: "Stage of microgametophyte development during which the generative cell undergoes a mitotic division to form two male gametes, the sperm cells." [TAIR:ki]
is_a: PO:0001017 ! M germinated pollen stage

[Term]
id: PO:0001077
name: lodicule differentiation and expansion stage
namespace: plant_growth_and_development_stage
def: "Stage of lodicule development defined by differentiation and expansion of lodicule." [POC:fz]
is_a: PO:0001049 ! lodicule developmental stages

[Term]
id: PO:0001078
name: E expanded cotyledon stage
namespace: plant_growth_and_development_stage
alt_id: PO:0001076
def: "The stage during which embryo axis and cotyledons rapidly elongate as a result of cell division and cell expansion." [TAIR:ki]
synonym: "curled cotyledon stage in Arabidopsis" RELATED []
synonym: "torpedo stage in Arabidopsis" RELATED []
is_a: PO:0007631 ! embryo development stages

[Term]
id: PO:0001079
name: fully expanded lodicule
namespace: plant_growth_and_development_stage
def: "Stage of lodicule development when lodicule is fully expanded." [POC:fz]
is_a: PO:0001049 ! lodicule developmental stages

[Term]
id: PO:0001081
name: F mature embryo stage
namespace: plant_growth_and_development_stage
def: "Stage at which the embryo is fully developed. " [APWeb:glossary, TAIR:ki]
comment: In some taxa, this occurs some time after the ripe fruit stage and after the dispersal of the seed.
synonym: "mature (stage) in Arabidopsis" RELATED []
is_a: PO:0007631 ! embryo development stages

[Term]
id: PO:0001083
name: inflorescence development stages
namespace: plant_growth_and_development_stage
def: "Stages of development of an inflorescence defined by characteristic morphological, structural, histological or other visible features. " [POC:curators]
is_a: PO:0007021 ! plant structure development stages

[Term]
id: PO:0001094
name: coleoptilar stage
namespace: plant_growth_and_development_stage
def: "The coleoptilar primordium, SAM and radicle are formed in the embryo of grasses." [TAIR:ki]
synonym: "SAM and radicle formation stage" RELATED []
is_a: PO:0007631 ! embryo development stages

[Term]
id: PO:0001095
name: true leaf formation
namespace: plant_growth_and_development_stage
def: "During this stage, the protrusion of the first leaf primordia takes place in succession." [TAIR:ki]
comment: Not all embryos form true leaves during the embryonic development; this occurs post-embryonically in some taxa.
is_a: PO:0007631 ! embryo development stages

[Term]
id: PO:0001096
name: primary endosperm cell stage
namespace: plant_growth_and_development_stage
def: "One cell stage that takes place following the fertilization, produced by the fusion of sperm cell nucleus and one or more polar nuclei." [TAIR:ki]
is_a: PO:0007633 ! endosperm development stages

[Term]
id: PO:0001097
name: A zygotic stage
namespace: plant_growth_and_development_stage
def: "One cell stage that results from fertilization." [PO:KI]
synonym: "one cell stage" RELATED []
synonym: "zygote in Arabidopsis" RELATED []
is_a: PO:0007631 ! embryo development stages

[Term]
id: PO:0001098
name: formation of starchy endosperm
namespace: plant_growth_and_development_stage
def: "OBSOLETE. Stage of endosperm development during wich the formation of starchy endosperm occurs." [TAIR:ki]
is_obsolete: true

[Term]
id: PO:0001099
name: formation of aleurone and starchy layers
namespace: plant_growth_and_development_stage
def: "Differentiation of aleurone layer, the outermost endosperm tissue, and the internal starchy tissue." [TAIR:ki]
is_a: PO:0001042 ! functional specialization of the endosperm

[Term]
id: PO:0001170
name: seed development stages
namespace: plant_growth_and_development_stage
def: "Stages of seed development, from fertilization to the dry or quiescent state." [TAIR:ki]
synonym: "seed development in Arabidopsis" RELATED []
is_a: PO:0007021 ! plant structure development stages

[Term]
id: PO:0001180
name: B proembryo stage
namespace: plant_growth_and_development_stage
def: "Early embryo development from two cell stage to a multicellular globular stage before three main tissue systems are differentiated." [APWeb:glossary, TAIR:ki]
synonym: "eight-celled stage in Arabidopsis" RELATED []
synonym: "two-celled stage in Arabidopsis" RELATED []
is_a: PO:0007631 ! embryo development stages

[Term]
id: PO:0001185
name: C globular stage
namespace: plant_growth_and_development_stage
def: "During this stage the embryo proper retains radial symmetry (increasing in diameter), and three main tissue systems are established." [TAIR:ki]
synonym: "dermatogen stage in Arabidopsis" RELATED []
synonym: "globular stage in Arabidopsis" RELATED []
synonym: "late globular stage in Arabidopsis" RELATED []
synonym: "mid-globular stage in Arabidopsis" RELATED []
is_a: PO:0007631 ! embryo development stages

[Term]
id: PO:0001378
name: sepals enclosing meristem
namespace: plant_growth_and_development_stage
def: "Stage of calyx development that begins when the developing sepals overlie the floral meristem." [ISBN:0387940898]
synonym: "stage 4 flower in Arabidopsis " RELATED []
is_a: PO:0001044 ! sepal differentiation and expansion stage

[Term]
id: PO:0001380
name: sepals enclosing floral bud
namespace: plant_growth_and_development_stage
def: "Stage of calyx development that begins when the sepals enclose the floral bud." [ISBN:0387940898]
synonym: "stage 6 flower in Arabidopsis " RELATED []
is_a: PO:0001044 ! sepal differentiation and expansion stage

[Term]
id: PO:0004500
name: formation of leaflet primordia
namespace: plant_growth_and_development_stage
def: "Stage at which leaflet primordia are initiated on the leaf primordium of a compound leaf." [TAIR:ki]
is_a: PO:0001052 ! 2 leaf expansion stage

[Term]
id: PO:0004501
name: gynoecium differentiation and expansion
namespace: plant_growth_and_development_stage
def: "Stage of gynoecium development defined by differentiation and expansion of carpels." [TAIR:ki]
is_a: PO:0007606 ! gynoecium developmental stages

[Term]
id: PO:0004502
name: closure of carpel(s)
namespace: plant_growth_and_development_stage
def: "Stage of gynoecium development defined by the closure of the carpel(s).\n" [TAIR:ki]
comment: Closure of the carpel can occur in various ways, by fusion or secretion.
is_a: PO:0007606 ! gynoecium developmental stages

[Term]
id: PO:0004503
name: stigma cell differentiation
namespace: plant_growth_and_development_stage
def: "Epidermal cells at the top of developing style differentiate stigma." [TAIR:ki]
is_a: PO:0007606 ! gynoecium developmental stages

[Term]
id: PO:0004504
name: ovule differentiation and expansion
namespace: plant_growth_and_development_stage
def: "Stage of ovule development defined by differentiation and expansion of ovules." [TAIR:ki]
is_a: PO:0007619 ! ovule developmental stages

[Term]
id: PO:0004505
name: fertilized ovule stage
namespace: plant_growth_and_development_stage
def: "The earliest stage of seed development immediately following double fertilization." [TAIR:ki]
is_a: PO:0001170 ! seed development stages

[Term]
id: PO:0004506
name: developing seed stage
namespace: plant_growth_and_development_stage
def: "Stage of seed development characterized by seed growth and differentiation." [TAIR:ki]
is_a: PO:0001170 ! seed development stages

[Term]
id: PO:0004507
name: D bilateral stage
namespace: plant_growth_and_development_stage
alt_id: PO:0001043
alt_id: PO:0001177
def: "Change from radial to bilateral symmetry takes place during this embryonic stage." [TAIR:ki]
synonym: "heart stage in Arabidopsis" RELATED []
synonym: "heart-shape stage" RELATED []
synonym: "transition stage in maize" RELATED []
synonym: "triangle stage in Arabidopsis" RELATED []
is_a: PO:0007631 ! embryo development stages

[Term]
id: PO:0007001
name: FR.01 early stage of fruit ripening
namespace: plant_growth_and_development_stage
def: "The early stage in fruit ripening." [GR:ap, ISBN:3826331524]
synonym: "09-dough development" RELATED [GRO:0007110]
synonym: "7 linear grain-filling in maize" RELATED [MaizeGDB:64632]
synonym: "7.03-early dough in maize" RELATED [GRO:0007034]
synonym: "7.3 early dough stage/embryo 3 in maize" RELATED [MaizeGDB:67374]
synonym: "8.03 Early ripening in soybean" RELATED [SOY:0000086]
synonym: "8.1-early dough stage in rice" RELATED [GRO:0007152]
synonym: "9.01-early dough" RELATED [GRO:0007111]
synonym: "9.01-early dough in barley" RELATED [GRO:0007111]
synonym: "9.01-early dough in oat" RELATED [GRO:0007111]
synonym: "9.01-early dough in wheat" RELATED [GRO:0007111]
synonym: "BBCH principal growth stage 83" RELATED [ISBN:3826331524]
synonym: "dough stage in maize" RELATED [MaizeGDB:67374]
synonym: "early dough stage in maize" RELATED [MaizeGDB:67374]
synonym: "early dough, kernel content soft, about 45% dry matter" RELATED [ISBN:3826331524]
synonym: "embryo stage 3 in maize" RELATED [MaizeGDB:67374]
synonym: "FR.01 early stage of fruit ripening in Solanaceae" RELATED [SGN:0000048]
synonym: "R4 in maize" RELATED [MaizeGDB:67374]
synonym: "rice growth stage-8.1" RELATED [GRO:0007152]
synonym: "tomato turning stage" RELATED [SGN:0000048]
is_a: PO:0007010 ! 6 ripening

[Term]
id: PO:0007002
name: IE.03 3/4 of inflorescence emerged from flag leaf sheath
namespace: plant_growth_and_development_stage
def: "The stage at which 3/4 of inflorescence has emerged from flag leaf sheath." [GR:ap]
synonym: "6.04-3/4 of inflorescence emerged in barley" RELATED [GRO:0007099]
synonym: "6.04-3/4 of inflorescence emerged in oat" RELATED [GRO:0007099]
synonym: "6.04-3/4 of inflorescence emerged in wheat" RELATED [GRO:0007099]
synonym: "70% of panicle emerged in rice" RELATED []
is_a: PO:0007041 ! inflorescence emergence from flag leaf sheath

[Term]
id: PO:0007003
name: IL.03 full inflorescence length reached
namespace: plant_growth_and_development_stage
def: "The stage when the inflorescence reaches full length." [GR:ap]
synonym: "4.04 full inflorescence length reached in soybean" RELATED [SOY:0000070]
is_a: PO:0007047 ! 3 inflorescence visible

[Term]
id: PO:0007004
name: 3 rapid growth stage
namespace: plant_growth_and_development_stage
def: "OBSOLETE.The stage at which the plant grows rapidly by either or both stem elongation and expansion of the rosette/foliage. " [GR:ap]
comment: Many stages like leaf production PO:0007112, axillary shoot formation PO:0007073, inflorescence PO:0007047 often overlap with this stage
is_obsolete: true

[Term]
id: PO:0007005
name: IL.02 1/2 inflorescence length reached
namespace: plant_growth_and_development_stage
def: "The stage when 1/2 Inflorescence is visible. " [GR:ap]
synonym: "4.03 1/2 of inflorescence length reached in soybean" RELATED [SOY:0000069]
is_a: PO:0007047 ! 3 inflorescence visible

[Term]
id: PO:0007006
name: IL.00 inflorescence just visible
namespace: plant_growth_and_development_stage
def: "Inflorescence just visible to the naked eye." [Poc:curators]
synonym: "4.01 Inflorescence just visible in soybean" RELATED [SOY:0000067]
synonym: "visible flower buds in Arabidopsis" RELATED [TAIR:0000420]
is_a: PO:0007047 ! 3 inflorescence visible

[Term]
id: PO:0007007
name: FF.03 fruit size 70%
namespace: plant_growth_and_development_stage
def: "The stage when the size of the fruit is about 70% of final fruit size." [GR:ap, ISBN:3826331524]
synonym: "7.07 Pod 70% of final length in soybean" RELATED [SOY:0000082]
synonym: "8.02-early milk in barley" RELATED [GRO:0007107]
synonym: "8.02-early milk in oat" RELATED [GRO:0007107]
synonym: "8.02-early milk in wheat" RELATED [GRO:0007107]
synonym: "early milk stage" RELATED [GRO:0007107]
synonym: "early milk stage in maize" RELATED [ISBN:3826331524]
synonym: "FF.03 fruit size 70% in Solanaceae" RELATED [SGN:0000044]
synonym: "late milk" RELATED [GRO:0007109]
synonym: "tomato immature green" RELATED [SGN:0000044]
synonym: "Zadok scale-73, Haun scale-13" RELATED [GRO:0007107]
is_a: PO:0007042 ! 5 fruit formation

[Term]
id: PO:0007008
name: IE.02 1/2 of inflorescence emerged from flag leaf sheath
namespace: plant_growth_and_development_stage
def: "The stage at which 1/2 of inflorescence has emerged from flag leaf sheath." [GR:ap]
synonym: "08-heading" RELATED [GRO:0007131]
synonym: "6.03-1/2 of inflorescence emerged in barley" RELATED [GRO:0007098]
synonym: "6.03-1/2 of inflorescence emerged in oat" RELATED [GRO:0007098]
synonym: "6.03-1/2 of inflorescence emerged in wheat" RELATED [GRO:0007098]
synonym: "first individual flowers visible" RELATED []
synonym: "half bloom" RELATED [GRO:0007131]
synonym: "middle of heading" RELATED []
synonym: "middle of panicle emergence in rice" RELATED []
synonym: "sorghum growth stage-7" RELATED [GRO:0007131]
is_a: PO:0007041 ! inflorescence emergence from flag leaf sheath

[Term]
id: PO:0007009
name: FF.01 fruit size 30%
namespace: plant_growth_and_development_stage
def: "The stage when the size of the fruit is about 30% of final fruit size." [GR:ap, ISBN:3826331524]
synonym: "7.02 Pod 30% of final length in soybean" RELATED [SOY:0000080]
synonym: "FF.01 fruit size 30% in Solanaceae" RELATED [SGN:0000042]
synonym: "tomato immature green" RELATED [SGN:0000042]
is_a: PO:0007042 ! 5 fruit formation

[Term]
id: PO:0007010
name: 6 ripening
namespace: plant_growth_and_development_stage
def: "Maturation of the fruit." [Poc:curators]
comment: Although the use of stages like dough or particular ripening stages properly refer to the development of an individual fruit, they are commonly used as here to extrapolate to a growth of a whole plant or a group of plants.
synonym: "08-dough stage in rice" RELATED [GRO:0007042]
synonym: "09-dough development in barley" RELATED [GRO:0007110]
synonym: "09-dough development in oat" RELATED [GRO:0007110]
synonym: "09-dough development in wheat" RELATED [GRO:0007110]
synonym: "10-dough stage in sorghum" RELATED [GRO:0007132]
synonym: "6 ripening in Solanaceae" RELATED [SGN:0000046]
synonym: "8 Bean Development in soybean" RELATED [SOY:0000078]
synonym: "BBCH principal growth stage 8" RELATED []
synonym: "dough stage" RELATED [GRO:0007132]
synonym: "dough stage in maize" RELATED [MaizeGDB:67379]
synonym: "dough stage kernels yellowish, about 55% dry matter" RELATED [ISBN:3826331524]
synonym: "fruit maturity" RELATED []
synonym: "fruit ripening" RELATED []
synonym: "kernel ripening" RELATED []
synonym: "maturity of fruit and seed" RELATED []
synonym: "rice growth stage-8" RELATED []
synonym: "silique ripening in Arabidopsis" RELATED [TAIR:0000034]
is_a: PO:0007130 ! B reproductive growth

[Term]
id: PO:0007012
name: inflorescence visible (sensu Poaceae)
namespace: plant_growth_and_development_stage
def: "The stage at which grass plant is producing inflorescence(s)." [Poc:curators]
comment: There is no one-to-one correspondence between growth stages of inflorescences formation in members of Poaceae with that of other families.
synonym: "BBCH principal growth stage 4" RELATED [ISBN:3826331524]
is_a: PO:0007047 ! 3 inflorescence visible

[Term]
id: PO:0007013
name: BO.03 late boot stage
namespace: plant_growth_and_development_stage
def: "The flag leaf sheath swollen." [GR:ap, ISBN:3826331524]
comment: In rice the flag leaf sheath is more than 10cm out of the penultimate leaf sheath.
synonym: "5.2-late booting stage in rice" RELATED [GRO:0007150]
synonym: "flag leaf sheath swollen" RELATED []
synonym: "rice growth stage-5.2" RELATED [GRO:0007150]
is_a: PO:0007014 ! booting

[Term]
id: PO:0007014
name: booting
namespace: plant_growth_and_development_stage
def: "Stage characterized by a swelling of the flag leaf sheath, caused by an increase in the size of the inflorescence as it grows up the leaf sheath." [GR:pj]
synonym: "05-booting in barley" RELATED [GRO:0007090]
synonym: "05-booting in oat" RELATED [GRO:0007090]
synonym: "05-booting in wheat" RELATED [GRO:0007090]
synonym: "05-booting stage" RELATED [GRO:0007148]
synonym: "07-boot stage in sorghum" RELATED [GRO:0007130]
synonym: "BBCH growth stage 40" RELATED [ISBN:3826331524]
synonym: "development of vegetatively propogated organs" RELATED []
synonym: "rice growth stage-5" RELATED [GRO:0007148]
synonym: "sorghum growth stage-6" RELATED [GRO:0007130]
is_a: PO:0007012 ! inflorescence visible (sensu Poaceae)

[Term]
id: PO:0007015
name: radicle emergence
namespace: plant_growth_and_development_stage
alt_id: PO:0007507
def: "The stage at which the radicle or root emerges from seed." [GR:ap, ISBN:3826331524]
synonym: "0.02-radicle emergence from seed in maize" RELATED [GRO:0007005]
synonym: "0.2 radicle emergence from seed in maize" RELATED [MaizeGDB:67351]
synonym: "05 radicle emergence from seed coat in soybean" RELATED [SOY:0000011]
synonym: "1.04-radicle emerged from seed in barley" RELATED [GRO:0007055]
synonym: "1.04-radicle emerged from seed in oat" RELATED [GRO:0007055]
synonym: "1.04-radicle emerged from seed in Triticeae" RELATED [GRO:0007055]
synonym: "1.04-radicle emerged from seed in wheat" RELATED [GRO:0007055]
synonym: "BBCH growth stage 05" RELATED [ISBN:3826331524]
synonym: "maize growth stage-0.2" RELATED [GRO:0007005]
synonym: "radicle emergence" RELATED []
synonym: "radicle emergence in Arabidopsis" RELATED [TAIR:T0000395]
synonym: "radicle emergence in Solanaceae" RELATED [SGN:0000006]
synonym: "Zadok scale-5" RELATED [GRO:0007055]
is_a: PO:0007510 ! root emergence
relationship: part_of PO:0007131 ! seedling growth

[Term]
id: PO:0007016
name: 4 flowering
namespace: plant_growth_and_development_stage
def: "The stage at which any flower(s) on the plant are open." [Poc:curators]
comment: This stage refers to the whole plant.
synonym: "07-anthesis in barley" RELATED [GRO:0007101]
synonym: "07-anthesis in oat" RELATED [GRO:0007101]
synonym: "07-anthesis in wheat" RELATED [GRO:0007101]
synonym: "09-flowering in sorghum" RELATED [GRO:0007153]
synonym: "4 flowering in Solanaceae" RELATED [SGN:0000034]
synonym: "5 flowering in maize" RELATED [MaizeGDB:13811]
synonym: "5.01-anthesis in maize " RELATED [GRO:0007021]
synonym: "5.02-silking in maize" RELATED [GRO:0007022]
synonym: "5.1 anthesis in maize" RELATED [MaizeGDB:67361]
synonym: "5.2 silking in maize" RELATED [MaizeGDB:67362]
synonym: "6 Flowering in soybean" RELATED [SOY:0000006]
synonym: "6.1-flowering stage in rice" RELATED [GRO:0007151]
synonym: "anthesis in maize" RELATED [MaizeGDB:67361]
synonym: "anthesis stage" RELATED [GRO:0007151]
synonym: "BBCH principal growth stage 6" RELATED [ISBN:3826331524]
synonym: "flowering in maize" RELATED [MaizeGDB:13811]
synonym: "pollen shed in maize" RELATED [MaizeGDB:67361]
synonym: "R1 in maize" RELATED [MaizeGDB:67362]
synonym: "rice growth stage-6.1" RELATED [GRO:0007151]
synonym: "silk emergence in maize" RELATED [MaizeGDB:67362]
synonym: "sorghum growth stage 8" RELATED [GRO:0007153]
synonym: "VT in maize" RELATED [MaizeGDB:67361]
is_a: PO:0007130 ! B reproductive growth

[Term]
id: PO:0007017
name: C senescence
namespace: plant_growth_and_development_stage
def: "The processes that occur near the end of a plant's active life that are associated with the dismantling of cell components and membranes, loss of functional chloroplasts, and an overall decline in metabolism. " [Poc:curators]
synonym: "10.03-kernel loosening in daytime in barley" RELATED [GRO:0007117]
synonym: "10.03-kernel loosening in daytime in oat" RELATED [GRO:0007117]
synonym: "10.03-kernel loosening in daytime in Triticeae" RELATED [GRO:0007117]
synonym: "10.03-kernel loosening in daytime in wheat" RELATED [GRO:0007117]
synonym: "10.04-overripe, straw dead and collapsing in barley" RELATED [GRO:0007118]
synonym: "10.04-overripe, straw dead and collapsing in oat" RELATED [GRO:0007118]
synonym: "10.04-overripe, straw dead and collapsing in Triticeae" RELATED [GRO:0007118]
synonym: "10.04-overripe, straw dead and collapsing in wheat" RELATED [GRO:0007118]
synonym: "9 Senescence in soybean" RELATED [SOY:0000008]
synonym: "BBCH principal growth stage 9" RELATED [ISBN:3826331524]
synonym: "C senescence in Solanaceae" RELATED [SGN:0000052]
synonym: "senescence in Arabidopsis" RELATED [TAIR:0000035]
is_a: PO:0007033 ! whole plant growth stages

[Term]
id: PO:0007018
name: BO.01 early boot stage
namespace: plant_growth_and_development_stage
def: "The flag leaf sheath has started to extend." [GR:ap, ISBN:3826331524]
comment: In rice the flag leaf sheath is 5cm out of the penultimate leaf sheath. Upper part of the stem is slightly thickened.
synonym: "5.01-flag leaf sheath extending in barley" RELATED [GRO:0007091]
synonym: "5.01-flag leaf sheath extending in oat" RELATED [GRO:0007091]
synonym: "5.01-flag leaf sheath extending in wheat" RELATED [GRO:0007091]
synonym: "5.1-early booting stage in rice" RELATED [GRO:0007149]
synonym: "flag leaf sheath extending" RELATED [GRO:0007091]
synonym: "rice growth stage-5.1" RELATED [GRO:0007149]
is_a: PO:0007014 ! booting

[Term]
id: PO:0007019
name: BO.05 flag leaf sheath opened
namespace: plant_growth_and_development_stage
def: "The first awns are visible and the flag leaf sheath has opened. " [GR:ap, ISBN:3826331524]
comment: Awns will be visible only in those species and varieties where they are known to be present.
synonym: "5.04-flag leaf sheath extending in barley" RELATED [GRO:0007094]
synonym: "5.04-flag leaf sheath extending in oat" RELATED [GRO:0007094]
synonym: "5.04-flag leaf sheath extending in wheat" RELATED [GRO:0007094]
synonym: "first awns visible" RELATED [GRO:0007094]
is_a: PO:0007014 ! booting

[Term]
id: PO:0007021
name: plant structure development stages
namespace: plant_growth_and_development_stage
def: "The succession of changes during the development of plant parts." [POC:curators]
is_a: PO:0009012 ! plant growth and development stages

[Term]
id: PO:0007022
name: imbibition
namespace: plant_growth_and_development_stage
def: "Absorption of water by the seed." [GR:ap, ISBN:0306416875]
synonym: "0.1 imbibition in maize" RELATED [MaizeGDB:64054]
synonym: "01 Beginning of seed imbibition in soybean" RELATED [SOY:0000090]
synonym: "03 Seed imbibition complete in soybean" RELATED [SOY:0000091]
synonym: "1.02-start of imbibition in barley" RELATED [GRO:0007053]
synonym: "1.02-start of imbibition in oat" RELATED [GRO:0007053]
synonym: "1.02-start of imbibition in Triticeae" RELATED [GRO:0007053]
synonym: "1.02-start of imbibition in wheat" RELATED [GRO:0007053]
synonym: "1.03-imbibition complete in barley" RELATED [GRO:0007054]
synonym: "1.03-imbibition complete in oat" RELATED [GRO:0007054]
synonym: "1.03-imbibition complete in Tricticeae" RELATED [GRO:0007054]
synonym: "1.03-imbibition complete in wheat" RELATED [GRO:0007054]
synonym: "BBCH growth stage 01" RELATED [ISBN:3826331524]
synonym: "imbibition in Arabidopsis" RELATED [TAIR:0000394]
synonym: "imbibition in Solanaceae" RELATED [SGN:0000004]
relationship: part_of PO:0007057 ! 0 germination

[Term]
id: PO:0007023
name: IE.04 inflorescence fully emerged from flag leaf sheath
namespace: plant_growth_and_development_stage
def: "The stage at which the  inflorescence  has fully emerged from the flag leaf sheath." [GR:ap]
synonym: "6.05-emergence of inflorescence completed in barley" RELATED [GRO:0007100]
synonym: "6.05-emergence of inflorescence completed in oat" RELATED [GRO:0007100]
synonym: "6.05-emergence of inflorescence completed in wheat" RELATED [GRO:0007100]
synonym: "end of panicle emergence in rice" RELATED []
is_a: PO:0007041 ! inflorescence emergence from flag leaf sheath

[Term]
id: PO:0007024
name: FL.04 end of flowering
namespace: plant_growth_and_development_stage
def: "The stage at which flowering is complete." [GR:ap]
comment: This stage refers to the whole plant.
synonym: "6.09 End of flowering in soybean" RELATED [SOY:0000076]
synonym: "7.03-anthesis completed in barley" RELATED [GRO:0007104]
synonym: "7.03-anthesis completed in oat" RELATED [GRO:0007104]
synonym: "7.03-anthesis completed in wheat" RELATED [GRO:0007104]
synonym: "anthesis completed" RELATED []
synonym: "FL.04 end of flowering in Solanaceae" RELATED [SGN:0000039]
synonym: "flowering complete" RELATED []
synonym: "fruit set visible" RELATED []
synonym: "late reproductive" RELATED []
synonym: "Zadok scale-69, Haun scale-11.6" RELATED [GRO:0007104]
is_a: PO:0007016 ! 4 flowering

[Term]
id: PO:0007025
name: IE.00 inflorescence tip just visible above flag leaf sheath
namespace: plant_growth_and_development_stage
def: "The stage at which the inflorescence tip is just visible above flag leaf sheath" [GR:ap]
synonym: "6.01-first spikelet of inflorescence visible in barley" RELATED [GRO:0007096]
synonym: "6.01-first spikelet of inflorescence visible in oat" RELATED [GRO:0007096]
synonym: "6.01-first spikelet of inflorescence visible in wheat" RELATED [GRO:0007096]
synonym: "beginning of heading" RELATED []
synonym: "beginning of panicle emergence in rice" RELATED []
synonym: "beginning of tassel emergence in maize" RELATED []
synonym: "first flower buds visible" RELATED []
synonym: "first spikelet visible" RELATED [GRO:0007096]
synonym: "visible flower buds" RELATED []
synonym: "Zadok scale-50, Feekes scale-10.1, Haun scale-10.2" RELATED [GRO:0007096]
is_a: PO:0007041 ! inflorescence emergence from flag leaf sheath

[Term]
id: PO:0007026
name: FL.00 first flower(s) open
namespace: plant_growth_and_development_stage
def: "The stage at which the first flower(s) open." [GR:pj]
comment: These first flowers are not necessarily the oldest flowers in the inflorescence. In some cereal plants the flowering starts in the middle of the inflorescence. This stage refers to the whole plant.
synonym: "6.00 1st flowers on main stem open in soybean" RELATED [SOY:0000072]
synonym: "7.01-anthesis beginning in barley" RELATED [GRO:0007102]
synonym: "7.01-anthesis beginning in oat" RELATED [GRO:0007102]
synonym: "7.01-anthesis beginning in Triticeae" RELATED [GRO:0007102]
synonym: "7.01-anthesis beginning in wheat" RELATED [GRO:0007102]
synonym: "first open flower in Arabidopsis" RELATED [TAIR:0000421]
synonym: "FL.00 first flower(s) open in Solanaceae" RELATED [SGN:0000035]
synonym: "Stage R1 Open flower at any node on the main stem" RELATED [SOY:0000072]
is_a: PO:0007016 ! 4 flowering

[Term]
id: PO:0007027
name: FF.04 final fruit size
namespace: plant_growth_and_development_stage
def: "The stage when the size of the fruit has reached the final fruit size." [GR:ap, ISBN:3826331524]
synonym: "7.09 Pod full size in soybean" RELATED [SOY:0000084]
synonym: "8.03-medium milk in barley" RELATED [GRO:0007108]
synonym: "8.03-medium milk in oat" RELATED [GRO:0007108]
synonym: "8.03-medium milk in wheat" RELATED [GRO:0007108]
synonym: "8.04-late milk in barley" RELATED [GRO:0007109]
synonym: "8.04-late milk in oat" RELATED [GRO:0007109]
synonym: "BBCH principal growth stage 75" RELATED [ISBN:3826331524]
synonym: "BBCH principal growth stage 79" RELATED [ISBN:3826331524]
synonym: "FF.04 final fruit size in Solanaceae" RELATED [SGN:0000045]
synonym: "kernel content milky, 40% dry matter" RELATED [ISBN:3826331524]
synonym: "Kernels in middle of cob yellowish-white" RELATED [ISBN:3826331524]
synonym: "nearly all kernels have reached final size" RELATED [ISBN:3826331524]
synonym: "Stage R4 Full pod in soybean" RELATED [SOY:0000084]
synonym: "tomato mature green" RELATED [SGN:0000045]
is_a: PO:0007042 ! 5 fruit formation

[Term]
id: PO:0007028
name: BO.04 flag leaf sheath opening
namespace: plant_growth_and_development_stage
def: "The flag leaf sheath starts opening." [ISBN:3826331524]
synonym: "5.03-flag leaf sheath extending in barley" RELATED [GRO:0007093]
synonym: "5.03-flag leaf sheath extending in oat" RELATED [GRO:0007093]
synonym: "5.03-flag leaf sheath extending in wheat" RELATED [GRO:0007093]
synonym: "Zadok scale-47" RELATED [GRO:0007093]
is_a: PO:0007014 ! booting

[Term]
id: PO:0007029
name: FF.02 fruit size 50%
namespace: plant_growth_and_development_stage
def: "The stage when the size of the fruit is about 50% of final fruit size." [GR:ap, ISBN:3826331524]
synonym: "7.01-blister stage in maize" RELATED [GRO:0007030]
synonym: "7.03 Pod 50% of final length in soybean" RELATED [SOY:0000081]
synonym: "8.01-kernel watery ripe in barley" RELATED [GRO:0007106]
synonym: "8.01-kernel watery ripe in oat" RELATED [GRO:0007106]
synonym: "8.01-kernel watery ripe in wheat" RELATED [GRO:0007106]
synonym: "BBCH principal growth stage 71" RELATED [ISBN:3826331524]
synonym: "beginning of grain development, kernels at blister stage, 16% dry matter" RELATED [ISBN:3826331524]
synonym: "blister stage in maize" RELATED [MaizeGDB:67372]
synonym: "caryopsis watery ripe" RELATED [GRO:0007106]
synonym: "FF.02 fruit size 50% in Solanaceae" RELATED [SGN:0000043]
synonym: "kernel watery ripe" RELATED [GRO:0007106]
synonym: "R2 in maize" RELATED [MaizeGDB:67372]
synonym: "Stage R4 Full pod in soybean" RELATED [SOY:0000081]
synonym: "tomato immature green" RELATED [SGN:0000043]
synonym: "watery ripe" RELATED [GRO:0007106]
synonym: "Zadok scale-71, Feekes scale-10.54, Haun scale-12.1" RELATED [GRO:0007106]
is_a: PO:0007042 ! 5 fruit formation

[Term]
id: PO:0007030
name: shoot emergence
namespace: plant_growth_and_development_stage
def: "Shoot or leaf breaks through soil surface." [GR:ap, ISBN:3826331524]
synonym: "07 shoot emergence in soybean" RELATED [SOY:0000012]
synonym: "BBCH growth stage 09" RELATED [ISBN:3826331524]
synonym: "shoot emergence in Solanaceae" RELATED [SGN:0000007]
relationship: part_of PO:0007131 ! seedling growth

[Term]
id: PO:0007031
name: FR.02 mid stage of fruit ripening
namespace: plant_growth_and_development_stage
def: "The stage when fruit ripening is midway." [GR:ap, ISBN:3826331524]
synonym: "10.01-soft dough in sorghum" RELATED [GRO:0007133]
synonym: "7.4 late dough stage/embryo 4 in maize" RELATED [MaizeGDB:67379]
synonym: "8.05 Mid ripening in soybean" RELATED [SOY:0000087]
synonym: "9.02-soft dough in barley" RELATED [GRO:0007112]
synonym: "9.02-soft dough in oat" RELATED [GRO:0007112]
synonym: "9.02-soft dough in wheat" RELATED [GRO:0007112]
synonym: "BBCH principal growth stage 85" RELATED [ISBN:3826331524]
synonym: "DNA degradation (endosperm) in maize" RELATED [MaizeGDB:67373]
synonym: "dough stage in maize" RELATED [MaizeGDB:67379]
synonym: "embryo stage 4 in maize" RELATED [MaizeGDB:67379]
synonym: "FR.02 mid stage of fruit ripening in Solanaceae" RELATED [SGN:0000049]
synonym: "R3 in maize" RELATED [MaizeGDB:67373]
synonym: "soft dough" RELATED [GRO:0007112]
synonym: "Stage R6 Full seed in soybean" RELATED [SOY:0000087]
synonym: "tomato orange fruit" RELATED [SGN:0000049]
synonym: "Zadok scale-85, Feekes scale-11.2" RELATED [GRO:0007112]
is_a: PO:0007010 ! 6 ripening

[Term]
id: PO:0007032
name: FF.00 fruit size 10%
namespace: plant_growth_and_development_stage
def: "The stage when the size of the fruit is about 10% of final fruit size." [GR:ap, ISBN:3826331524]
synonym: "7.01 Pod 10% of final length in soybean" RELATED [SOY:0000079]
synonym: "FF.00 fruit size 10% in Solanaceae" RELATED [SGN:0000041]
synonym: "stage R3 in soybean" RELATED [SOY:0000079]
synonym: "tomato immature green" RELATED [SGN:0000041]
is_a: PO:0007042 ! 5 fruit formation

[Term]
id: PO:0007033
name: whole plant growth stages
namespace: plant_growth_and_development_stage
def: "The succession of changes during the growth of the whole plant." [GR:pj]
synonym: "cereal plant ontology " RELATED [GRO:0080001]
synonym: "maize growth stage" RELATED [GRO:0007002]
synonym: "plant growth stage ontology" RELATED [GRO:0007199]
synonym: "plant growth stages in Arabidopsis" RELATED [TAIR:0000021]
synonym: "rice growth stage" RELATED [GRO:0007040]
synonym: "Solanaceae whole plant growth stages" RELATED [SGN:0000001]
synonym: "sorghum growth stage" RELATED [GRO:0007124]
synonym: "wheat, barley and oat growth stage" RELATED [GRO:0007156]
is_a: PO:0009012 ! plant growth and development stages

[Term]
id: PO:0007034
name: FL.01 1/4 of flowers open
namespace: plant_growth_and_development_stage
def: "The stage at which 1/4 of flowers open" [GR:ap]
comment: This stage refers to the whole plant.
synonym: "6.02 1/4 of flowers on the main stem open in soybean" RELATED [SOY:0000073]
synonym: "FL.01 1/4 of flowers open in Solanaceae" RELATED [SGN:0000036]
is_a: PO:0007016 ! 4 flowering

[Term]
id: PO:0007035
name: 7-8 fruit formation and maturation
namespace: plant_growth_and_development_stage
def: "OBSOLETE: This stage refers to the developmental and physiological changes that occur in the whole plant after fertilization and during fruit development, maturation, and provisioning. " [Poc:curators]
comment: We have chosen to use fruit size as a marker of these physiological processes to represent the whole plant growth stage.
synonym: "06-post-flowering in maize" RELATED [GRO:0007025]
synonym: "5.3 pollination in maize" RELATED [MaizeGDB:67364]
synonym: "5.4 fertilization in maize" RELATED [MaizeGDB:67365]
synonym: "6 post-flowering/lag phase in maize" RELATED [MaizeGDB:67370]
synonym: "7 linear grain-filling in maize" RELATED [MaizeGDB:64632]
synonym: "7 Pod Formation in soybean" RELATED [SOY:0000077]
synonym: "7-8 Fruit Formation and Maturation in soybean" RELATED [SOY:0000007]
synonym: "7.01-blister stage in maize" RELATED [GRO:0007030]
synonym: "BBCH principal growth stage 7" RELATED [ISBN:3826331524]
synonym: "C-embryo stage in rice" RELATED [GRO:0007141]
synonym: "double fertilization in maize" RELATED [MaizeGDB:67365]
synonym: "effective filling period in maize" RELATED [MaizeGDB:64632]
synonym: "first silique shattered" RELATED []
synonym: "grain-filling in maize" RELATED [MaizeGDB:64632]
synonym: "kernel watery ripe" RELATED [GRO:0007106]
synonym: "lag phase in maize" RELATED [MaizeGDB:67370]
synonym: "post-flowering in maize" RELATED [MaizeGDB:67370]
synonym: "proembryo in maize" RELATED [MaizeGDB:67370]
synonym: "R1in maize" RELATED [MaizeGDB:67370]
is_obsolete: true

[Term]
id: PO:0007036
name: FR.00 beginning of fruit ripening
namespace: plant_growth_and_development_stage
def: "The stage at which fruit maturation begins." [GR:ap, ISBN:3826331524]
synonym: "8.01 Beginning of bean ripening in soybean" RELATED [SOY:0000085]
synonym: "beginning of fruit coloration" RELATED []
synonym: "first silique shattered" RELATED []
synonym: "FR.00 beginning of fruit ripening in Solanaceae" RELATED [SGN:0000047]
is_a: PO:0007010 ! 6 ripening

[Term]
id: PO:0007037
name: inflorescence bifurcation stage
namespace: plant_growth_and_development_stage
def: "Stage of inflorescence development marked by the formation of two, oftern equal-sized, inflorescence meristems from one inflorescence meristem." [POC:curators]
is_a: PO:0001083 ! inflorescence development stages

[Term]
id: PO:0007038
name: FR.04 fruit ripening complete
namespace: plant_growth_and_development_stage
def: "The stage at which fruit ripening is complete." [GR:ap, ISBN:3826331524]
synonym: "10-ripening in barley" RELATED [GRO:0007114]
synonym: "10-ripening in oat" RELATED [GRO:0007114]
synonym: "10-ripening in Triticeae" RELATED [GRO:0007114]
synonym: "10-ripening in wheat" RELATED [GRO:0007114]
synonym: "10.01-kernel medium hard" RELATED [GRO:0007115]
synonym: "10.02-kernel hard" RELATED [GRO:0007116]
synonym: "8.09 Final ripening in soybean" RELATED [SOY:0000089]
synonym: "9.02 dry kernel in maize" RELATED [GRO:0007037]
synonym: "9.2 dry kernel in maize" RELATED [MaizeGDB:67381]
synonym: "BBCH principal growth stage 89" RELATED [ISBN:3826331524]
synonym: "dry kernel in maize" RELATED [MaizeGDB:67381]
synonym: "dry seed in maize" RELATED [MaizeGDB:67381]
synonym: "FR.04 fruit ripening complete in Solanaceae" RELATED [SGN:0000051]
synonym: "fully ripe" RELATED []
synonym: "fully ripe grain hard, difficult to divide by thumbnail in rice" RELATED [ISBN:3826331524]
synonym: "fully ripe kernels hard and shiny about 65% dry matter in maize" RELATED [ISBN:3826331524]
synonym: "tomato fully red ripe fruit" RELATED [SGN:0000051]
is_a: PO:0007010 ! 6 ripening

[Term]
id: PO:0007039
name: leaf trichome development stage
namespace: plant_growth_and_development_stage
def: "Stages of development of a trichome defined by characteristic morphological, structural, histological or other visible features" [GR:cwt]
is_a: PO:0001050 ! leaf development stages

[Term]
id: PO:0007041
name: inflorescence emergence from flag leaf sheath
namespace: plant_growth_and_development_stage
def: "The stage at which the inflorescence emerges from the flag leaf sheath." [GR:ap]
synonym: "06-heading stage in rice" RELATED [GRO:0007044]
synonym: "06-inflorescence emergence in barley" RELATED [GRO:0007095]
synonym: "06-inflorescence emergence in oat" RELATED [GRO:0007095]
synonym: "06-inflorescence emergence in wheat" RELATED [GRO:0007095]
synonym: "08-heading in sorghum" RELATED [GRO:0007131]
synonym: "half bloom in sorghum" RELATED [GRO:0007131]
synonym: "heading" RELATED [GRO:0007095]
synonym: "rice growth stage-6" RELATED [GRO:0007044]
synonym: "sorghum growth stage-7" RELATED [GRO:0007131]
synonym: "tasseling" RELATED []
is_a: PO:0007012 ! inflorescence visible (sensu Poaceae)

[Term]
id: PO:0007042
name: 5 fruit formation
namespace: plant_growth_and_development_stage
def: "Formation of the seed-bearing structure after flowering." [Poc:curators]
comment: Although the use of stages like milk or particular fruit sizes properly refer to the development of an individual fruit, they are commonly used as here to extrapolate to a growth of a whole plant or a group of plants.
synonym: "07-milk stage in rice" RELATED [GRO:0007046]
synonym: "08-milk development in barley" RELATED [GRO:0007105]
synonym: "08-milk development in oat" RELATED [GRO:0007105]
synonym: "08-milk development in wheat" RELATED [GRO:0007105]
synonym: "5 fruit formation in Solanaceae" RELATED [SGN:0000040]
synonym: "6.01-dilatory in maize" RELATED [GRO:0007026]
synonym: "6.02-exponential in maize" RELATED [GRO:0007027]
synonym: "6.1 dilatory in maize" RELATED [MaizeGDB:67371]
synonym: "6.2 exponential in maize" RELATED [MaizeGDB:67369]
synonym: "dilatory in maize" RELATED [MaizeGDB:67371]
synonym: "exponential in maize" RELATED [MaizeGDB:67369]
synonym: "free nuclear in maize" RELATED [MaizeGDB:67371]
synonym: "milk grain" RELATED []
synonym: "milk stage in rice" RELATED [GRO:0007046]
synonym: "mitotic in maize" RELATED [MaizeGDB:67369]
synonym: "proembryo in maize" RELATED [MaizeGDB:67371]
synonym: "rice growth stage-7" RELATED [GRO:0007046]
synonym: "transition stage in maize" RELATED [MaizeGDB:67369]
synonym: "Zadok scale-70" RELATED [GRO:0007105]
is_a: PO:0007130 ! B reproductive growth

[Term]
id: PO:0007043
name: hypocotyl emergence
namespace: plant_growth_and_development_stage
def: "Emergence of the hypocotyl above ground." [GR:ap, ISBN:0306416875]
comment: Occurs in plants with epigeal germination.
synonym: "0.07.01 Cotyledons and hypocotyl emerge in soybean" RELATED [SOY:0000013]
synonym: "0.07.02 Hypocotyl emerges above soil in soybean" RELATED [SOY:0000092]
synonym: "BBCH growth stage 08" RELATED [ISBN:3826331524]
synonym: "hypocotyl and cotyledon emergence in Arabidopsis" RELATED [TAIR:0000396]
synonym: "hypocotyl emergence in Solanaceae" RELATED [SGN:0000010]
is_a: PO:0007030 ! shoot emergence

[Term]
id: PO:0007044
name: BO.02 mid boot stage
namespace: plant_growth_and_development_stage
def: "The flag leaf sheath is just visibly swollen. " [GR:ap, ISBN:3826331524]
comment: In rice the flag leaf sheath is 5-10cm out of the penultimate leaf sheath.
synonym: "5.02-flag leaf sheath extending in barley" RELATED [GRO:0007092]
synonym: "5.02-flag leaf sheath extending in oat" RELATED [GRO:0007092]
synonym: "5.02-flag leaf sheath extending in wheat" RELATED [GRO:0007092]
synonym: "flag leaf sheath just visibly swollen" RELATED []
synonym: "Zadok scale-45, Feekes scale-10, Haun scale-9.2" RELATED [GRO:0007092]
is_a: PO:0007014 ! booting

[Term]
id: PO:0007045
name: coleoptile emergence
namespace: plant_growth_and_development_stage
def: "Emergence of coleoptile above ground." [GR:ap, ISBN:3826331524]
synonym: "0.3 coleoptile emergence from seed in maize" RELATED [MaizeGDB:67352]
synonym: "BBCH growth stage 09" RELATED [ISBN:3826331524]
is_a: PO:0007030 ! shoot emergence

[Term]
id: PO:0007046
name: IL.01 1/4 inflorescence length reached
namespace: plant_growth_and_development_stage
def: "The stage when 1/4 Inflorescence is visible. " [GR:ap]
synonym: "4.02 1/4 of inflorescence length reached in soybean" RELATED [SOY:0000068]
is_a: PO:0007047 ! 3 inflorescence visible

[Term]
id: PO:0007047
name: 3 inflorescence visible
namespace: plant_growth_and_development_stage
def: "The stage at which plant is producing inflorescence(s)." [Poc:curators]
synonym: "3 inflorescence visible in Solanaceae" RELATED [SGN:0000033]
synonym: "4 Inflorescence Formation in soybean" RELATED [SOY:0000005]
synonym: "BBCH principal growth stage 5" RELATED [ISBN:3826331524]
is_a: PO:0007130 ! B reproductive growth

[Term]
id: PO:0007048
name: IE.01 1/4 of inflorescence emerged from flag leaf sheath
namespace: plant_growth_and_development_stage
def: "The stage at which 1/4 of inflorescence has emerged from flag leaf sheath." [GR:ap]
synonym: "30% of panicle emerged in rice" RELATED []
synonym: "6.02-1/4 of inflorescence emerged in barley" RELATED [GRO:0007097]
synonym: "6.02-1/4 of inflorescence emerged in oat" RELATED [GRO:0007097]
synonym: "6.02-1/4 of inflorescence emerged in wheat" RELATED [GRO:0007097]
synonym: "Zadok scale-53, Feekes scale-10.2" RELATED [GRO:0007097]
is_a: PO:0007041 ! inflorescence emergence from flag leaf sheath

[Term]
id: PO:0007049
name: cotyledon emergence
namespace: plant_growth_and_development_stage
alt_id: PO:0007069
def: "Emergence of cotyledons above ground." [GR:ap, ISBN:3826331524]
comment: This cannot be used in plants with hypogeal germination.
synonym: "01-seedling emergence in sorghum" RELATED [GRO:0007125]
synonym: "1.00 Cotyledon visible in soybean" RELATED [SOY:0000014]
synonym: "1.00 imperfect leaf unrolled" RELATED []
synonym: "1.01-seedling emergence in maize" RELATED [GRO:0007008]
synonym: "1.1 seedling emergence in maize" RELATED [MaizeGDB:64057]
synonym: "2.01-first leaf through coleoptile in barley" RELATED [GRO:0007059]
synonym: "2.01-first leaf through coleoptile in oat" RELATED [GRO:0007059]
synonym: "2.01-first leaf through coleoptile in Triticeae" RELATED [GRO:0007059]
synonym: "2.01-first leaf through coleoptile in wheat" RELATED [GRO:0007059]
synonym: "BBCH growth stage 09" RELATED [ISBN:3826331524]
synonym: "BBCH growth stage 10" RELATED [ISBN:3826331524]
synonym: "cotyledon emergence in Solanaceae" RELATED [SGN:0000008]
synonym: "cotyledons fully open in Arabidopsis" RELATED [TAIR:0000397]
synonym: "first leaf through coleoptile (sensu Oryza)" RELATED []
synonym: "first leaf through coleoptile (sensu Triticeae)" RELATED [GRO:0007059]
synonym: "hypocotyl and cotyledon emergence in Arabidopsis" RELATED [TAIR:0000396]
synonym: "LP.00 cotyledon visible" RELATED []
synonym: "maize growth stage-1.1" RELATED [GRO:0007008]
synonym: "seedling emergence (sensu Sorghum)" RELATED [GRO:0007125]
synonym: "sorghum growth stage-0" RELATED [GRO:0007125]
synonym: "VE in maize" RELATED [MaizeGDB:64057]
synonym: "VE stage in soybean" RELATED [SOY:0000014]
synonym: "Zadok scale-10, Feekes scale-1" RELATED [GRO:0007059]
is_a: PO:0007030 ! shoot emergence

[Term]
id: PO:0007050
name: FR.03 late stage of fruit ripening
namespace: plant_growth_and_development_stage
def: "The late stage of fruit ripening." [GR:ap, ISBN:3826331524]
synonym: "09-maturity in maize" RELATED [GRO:0007037]
synonym: "10.02-hard dough in sorghum" RELATED [GRO:0007134]
synonym: "8 leveling off of grain-filling/embryo 5 in maize" RELATED [MaizeGDB:67382]
synonym: "8.07 Late ripening in soybean" RELATED [SOY:0000088]
synonym: "8.2-hard dough stage in rice" RELATED [GRO:0007154]
synonym: "9 maturity in maize" RELATED [MaizeGDB:11088]
synonym: "9.03-hard dough in barley" RELATED [GRO:0007113]
synonym: "9.03-hard dough in oat" RELATED [GRO:0007113]
synonym: "9.03-hard dough in wheat" RELATED [GRO:0007113]
synonym: "9.1 physiological maturity/embryo 6 in maize" RELATED [MaizeGDB:67380]
synonym: "attenuative in maize" RELATED [MaizeGDB:67382]
synonym: "BBCH principal growth stage 87" RELATED [ISBN:3826331524]
synonym: "black layer in maize" RELATED [MaizeGDB:67380]
synonym: "dent stage in maize" RELATED [MaizeGDB:67382]
synonym: "embryo stage 5 in maize" RELATED [MaizeGDB:67382]
synonym: "embryo stage 6 in maize" RELATED [MaizeGDB:67380]
synonym: "FR.03 late stage of fruit ripening in Solanaceae" RELATED [SGN:0000050]
synonym: "hard dough" RELATED []
synonym: "late dough grain in rice" RELATED [GRO:0007154]
synonym: "late dough stage in rice" RELATED [GRO:0007154]
synonym: "leveling off of dry matter accumulation" RELATED [MaizeGDB:67382]
synonym: "physiological maturity, black dot, about 60% dry matter in maize" RELATED [ISBN:3826331524]
synonym: "R5 in maize" RELATED [MaizeGDB:67382]
synonym: "R6 in maize" RELATED [MaizeGDB:67380]
synonym: "rice growth stage-8.2" RELATED [GRO:0007154]
synonym: "sorghum growth stage-10" RELATED [GRO:0007134]
synonym: "Stage R7 Beginning maturity in soybean" RELATED [SOY:0000088]
synonym: "storage maturity in maize" RELATED [MaizeGDB:67381]
synonym: "tomato red firm fruit" RELATED [SGN:0000050]
synonym: "Zadok scale-87, Haun scale-15" RELATED [GRO:0007113]
is_a: PO:0007010 ! 6 ripening

[Term]
id: PO:0007051
name: BO.00 booting begins
namespace: plant_growth_and_development_stage
def: "Booting has just begun." [GR:ap, ISBN:3826331524]
is_a: PO:0007014 ! booting

[Term]
id: PO:0007052
name: FL.03 3/4 of flowers open
namespace: plant_growth_and_development_stage
def: "The stage at which 3/4 of flowers open." [GR:ap]
comment: This stage refers to the whole plant.
synonym: "6.02 3/4 of flowers on main stem open in soybean" RELATED [SOY:0000074]
synonym: "FL.03 3/4 of flowers open in Solanaceae" RELATED [SGN:0000038]
synonym: "flowering finishing" RELATED []
synonym: "Stage R2 Open flower at one of the two uppermost nodes on the main stem with fully developed leaf in soybean" RELATED [SOY:0000074]
is_a: PO:0007016 ! 4 flowering

[Term]
id: PO:0007053
name: FL.02 1/2 of flowers open
namespace: plant_growth_and_development_stage
def: "The stage at which 1/2 of flowers open." [GR:ap]
comment: This stage refers to the whole plant.
synonym: "6.02 1/2 of flowers on main stem open in soybean" RELATED [SOY:0000094]
synonym: "7.02-anthesis half-way in barley" RELATED [GRO:0007103]
synonym: "7.02-anthesis half-way in oat" RELATED [GRO:0007103]
synonym: "7.02-anthesis half-way in wheat" RELATED [GRO:0007103]
synonym: "FL.02 1/2 of flowers open in Solanaceae" RELATED [SGN:0000037]
synonym: "full flowering" RELATED []
synonym: "Haun scale-11.5" RELATED [GRO:0007103]
is_a: PO:0007016 ! 4 flowering

[Term]
id: PO:0007054
name: epicotyl emergence
namespace: plant_growth_and_development_stage
def: "Emergence of the epicotyl above ground." [GR:ap, ISBN:0306416875]
comment: Only the first true foliage leaf or pair of leaves are visible.  Occurs in plants with hypogeal germination.
is_a: PO:0007030 ! shoot emergence

[Term]
id: PO:0007056
name: 1 pattern formation
namespace: plant_growth_and_development_stage
def: "trichome initiation stage that determine numbers of trichome are formed" [GR:cwt]
relationship: part_of PO:0007039 ! leaf trichome development stage

[Term]
id: PO:0007057
name: 0 germination
namespace: plant_growth_and_development_stage
def: "The resumption of growth by the embryo in a seed." [GR:ap, ISBN:047124529]
synonym: "0 germination in maize" RELATED [MaizeGDB:64055]
synonym: "0 germination in Solanaceae" RELATED [SGN:0000003]
synonym: "0 Germination in soybean" RELATED [SOY:0000001]
synonym: "00-germination in maize" RELATED [GRO:0007003]
synonym: "01-germination in barley" RELATED [GRO:0007051]
synonym: "01-germination in oat" RELATED [GRO:0007051]
synonym: "01-germination in rice" RELATED [GRO:0007043]
synonym: "01-germination in Triticeae" RELATED [GRO:0007051]
synonym: "01-germination in wheat" RELATED [GRO:0007051]
synonym: "BBCH principal growth stage 0" RELATED [ISBN:3826331524]
synonym: "germination in Arabidopsis" RELATED [TAIR:0000393]
synonym: "maize growth stage-0" RELATED [GRO:0007003]
synonym: "rice growth stage-1" RELATED [GRO:0007043]
is_a: PO:0007134 ! A vegetative growth

[Term]
id: PO:0007058
name: 2 endoreduplication
namespace: plant_growth_and_development_stage
def: "the stage trichome nuclei continue to replicate their DNA after mitosis and cytokinesis have ceased, and as a consequence have a DNA content much greater than 2C" [GR:cwt]
relationship: part_of PO:0007039 ! leaf trichome development stage

[Term]
id: PO:0007059
name: 3 branch formation
namespace: plant_growth_and_development_stage
def: "ths stage trichome develops branches " [GR:cwt]
relationship: part_of PO:0007039 ! leaf trichome development stage

[Term]
id: PO:0007060
name: obsolete growth and development terms
namespace: plant_growth_and_development_stage
is_obsolete: true

[Term]
id: PO:0007061
name: 2.00 main shoot only
namespace: plant_growth_and_development_stage
def: "OBSOLETE" [GR:ap]
synonym: "3.01-main shoot only in barley" RELATED [GRO:0007087]
synonym: "3.01-main shoot only in oat" RELATED [GRO:0007087]
synonym: "3.01-main shoot only in Triticeae" RELATED [GRO:0007087]
synonym: "3.01-main shoot only in wheat" RELATED [GRO:0007087]
synonym: "Zadok scale-20" RELATED [GRO:0007087]
is_obsolete: true

[Term]
id: PO:0007062
name: SE.06 six nodes or internodes visible
namespace: plant_growth_and_development_stage
def: "The stage at which six nodes or six internodes are visible." [GR:pj]
comment: A measure of vegetative growth, but leaf production is to be preferred.
synonym: "3.06 6 nodes/internodes visible in soybean" RELATED [SOY:0000055]
synonym: "4.07-sixth node detectable in barley" RELATED [GRO:0007087]
synonym: "4.07-sixth node detectable in oat" RELATED [GRO:0007087]
synonym: "4.07-sixth node detectable in wheat" RELATED [GRO:0007087]
synonym: "BBCH growth stage 36" RELATED [ISBN:3826331524]
synonym: "Zadok scale-36" RELATED [GRO:0007087]
is_a: PO:0007089 ! stem elongation

[Term]
id: PO:0007063
name: LP.07 seven leaves visible
namespace: plant_growth_and_development_stage
def: "The stage at which leaves at seven nodes, other than the cotyledonary node, are visible above ground." [GR:ap]
comment: The leaves can be a single leaf, two, or whorls of leaves at each node.
synonym: "1.07 6th trifoliolate leaf unfolded in soybean" RELATED [SOY:0000021]
synonym: "2.08-seven leaves unfolded in barley" RELATED [GRO:0007066]
synonym: "2.08-seven leaves unfolded in oat" RELATED [GRO:0007066]
synonym: "2.08-seven leaves unfolded in Triticeae" RELATED [GRO:0007066]
synonym: "2.08-seven leaves unfolded in wheat" RELATED [GRO:0007066]
synonym: "3.01-ear initiation" RELATED [GRO:0007013]
synonym: "3.1 ear initiation/mid-whorl stage in maize" RELATED [MaizeGDB:67356]
synonym: "6-8 leaves in maize" RELATED [MaizeGDB:67356]
synonym: "7 leaves unfolded" RELATED []
synonym: "7 rosette leaf in Arabidopsis" RELATED [TAIR:0000410]
synonym: "7-leaf in maize" RELATED [MaizeGDB:67356]
synonym: "BBCH growth stage 17" RELATED [ISBN:3826331524]
synonym: "ear initiation in maize" RELATED [MaizeGDB:67356]
synonym: "LP.07 seven leaves visible in Solanaceae" RELATED [SGN:0000019]
synonym: "maize growth stage-3.1" RELATED [GRO:0007013]
synonym: "mid-whorl stage in maize" RELATED [MaizeGDB:67356]
synonym: "seven leaves unfolded (sensu Triticeae)" RELATED [GRO:0007066]
synonym: "seven rosette leaves" RELATED []
synonym: "seventh leaf unfolded" RELATED []
synonym: "Stage V6 in soybean" RELATED [SOY:0000021]
synonym: "V7 in maize" RELATED [MaizeGDB:67356]
synonym: "Zadok scale-, Haun scale-6.+" RELATED [GRO:0007066]
is_a: PO:0007133 ! leaf production

[Term]
id: PO:0007064
name: LP.12 twelve leaves visible
namespace: plant_growth_and_development_stage
def: "The stage at which leaves at twelve nodes, other than the cotyledonary node, are visible above ground." [GR:ap]
comment: The leaves can be a single leaf, two, or whorls of leaves at each node.
synonym: "1.12 11th trifoliolate leaf unfolded in soybean" RELATED [SOY:0000026]
synonym: "12 rosette leaf in Arabidopsis" RELATED [TAIR:0000415]
synonym: "3.03-mid-vegetative" RELATED [GRO:0007013]
synonym: "3.3 mid-vegetative" RELATED [MaizeGDB:67359]
synonym: "3.3 mid-vegetative stage of maize" RELATED [GRO:0007013]
synonym: "maize growth stage-3.3" RELATED [GRO:0007013]
synonym: "mid-vegetative in maize" RELATED [MaizeGDB:67359]
synonym: "mid-vegetative stage of maize" RELATED [GRO:0007013]
synonym: "Stage V11 in soybean" RELATED [SOY:0000026]
synonym: "twelve leaves unfolded" RELATED []
synonym: "twelve rosette leaves" RELATED []
synonym: "V12 in maize" RELATED [MaizeGDB:67359]
is_a: PO:0007133 ! leaf production

[Term]
id: PO:0007065
name: LP.05 five leaves visible
namespace: plant_growth_and_development_stage
def: "The stage at which leaves at five nodes, other than the cotyledonary node, are visible above ground." [GR:ap]
comment: The leaves can be a single leaf, two, or whorls of leaves at each node.
synonym: "02-tassel initiation in maize" RELATED [GRO:0007011]
synonym: "04-five leaf stage in sorghum" RELATED [GRO:0007127]
synonym: "1.05 4th trifoliolate leaf unfolded in soybean" RELATED [SOY:0000019]
synonym: "2 tassel initiation/early whorl stage in maize" RELATED [MaizeGDB:67306]
synonym: "2.06-five leaves unfolded in barley" RELATED [GRO:0007064]
synonym: "2.06-five leaves unfolded in oat" RELATED [GRO:0007064]
synonym: "2.06-five leaves unfolded in Triticeae" RELATED [GRO:0007064]
synonym: "2.06-five leaves unfolded in wheat" RELATED [GRO:0007064]
synonym: "4-6 leaves in maize" RELATED [MaizeGDB:67306]
synonym: "5 leaves unfolded" RELATED []
synonym: "5 rosette leaf in Arabidopsis" RELATED [TAIR:0000408]
synonym: "BBCH growth stage 15" RELATED [ISBN:3826331524]
synonym: "early whorl stage in maize" RELATED [MaizeGDB:67306]
synonym: "fifth leaf unfolded" RELATED []
synonym: "five leaf stage (sensu Sorghum)" RELATED [GRO:0007127]
synonym: "five leaves unfolded (sensu Triticeae)" RELATED [GRO:0007064]
synonym: "five rosette leaves" RELATED []
synonym: "LP.05 five leaves visible in Solanaceae" RELATED [SGN:0000017]
synonym: "maize growth stage-2" RELATED [GRO:0007011]
synonym: "rice growth stage-3" RELATED [GRO:0007049]
synonym: "sorghum growth stage-3" RELATED [GRO:0007127]
synonym: "Stage V4 in soybean" RELATED [SOY:0000019]
synonym: "tassel differentiation in maize" RELATED [MaizeGDB:67306]
synonym: "tassel initiation in maize" RELATED [MaizeGDB:67306]
synonym: "V5 in maize" RELATED [MaizeGDB:67306]
synonym: "Zadok scale-15, Haun scale-4.+" RELATED [GRO:0007064]
is_a: PO:0007133 ! leaf production

[Term]
id: PO:0007066
name: SE.09 nine nodes or internodes visible
namespace: plant_growth_and_development_stage
def: "The stage at which nine nodes or nine internodes are visible." [GR:pj]
comment: A measure of vegetative growth, but leaf production is to be preferred.
synonym: "3.09 9 nodes/internodes visible in soybean" RELATED [SOY:0000058]
synonym: "BBCH growth stage 39" RELATED [ISBN:3826331524]
is_a: PO:0007089 ! stem elongation

[Term]
id: PO:0007067
name: LP.17 seventeen leaves visible
namespace: plant_growth_and_development_stage
def: "The stage at which leaves at seventeen nodes, other than the cotyledonary node, are visible above ground." [GR:ap]
comment: The leaves can be a single leaf, two, or whorls of leaves at each node.
synonym: "1.17 16th trifoliate leaf unfolded in soybean" RELATED [SOY:0000031]
synonym: "3.04-late vegetative" RELATED [GRO:0007016]
synonym: "3.4 late vegetative in maize" RELATED [MaizeGDB:67360]
synonym: "3.4 late vegetative stage of maize" RELATED [GRO:0007016]
synonym: "late vegetative in maize" RELATED [MaizeGDB:67360]
synonym: "late vegetative stage of maize" RELATED [GRO:0007016]
synonym: "maize growth stage-3.4" RELATED [GRO:0007016]
synonym: "maize V17 stage" RELATED [GRO:0007016]
synonym: "Stage V16 in soybean" RELATED [SOY:0000031]
synonym: "V17 in maize" RELATED [MaizeGDB:67360]
is_a: PO:0007133 ! leaf production

[Term]
id: PO:0007068
name: mid rosette growth
namespace: plant_growth_and_development_stage
def: "Rosette has reached approximately 50% of its final diameter." [Poc:curators]
comment: A measure of vegetative growth, but leaf production is to be preferred.
synonym: "mid rosette growth in Arabidopsis" RELATED [TAIR:0000044]
is_a: PO:0007113 ! rosette growth

[Term]
id: PO:0007070
name: SE.08 eight nodes or internodes visible
namespace: plant_growth_and_development_stage
def: "The stage at which eight nodes or eight internodes are visible." [GR:ap]
comment: A measure of vegetative growth, but leaf production is to be preferred.
synonym: "3.08 8 nodes/internodes visible in soybean" RELATED [SOY:0000057]
synonym: "BBCH growth stage 38" RELATED [ISBN:3826331524]
is_a: PO:0007089 ! stem elongation

[Term]
id: PO:0007071
name: 2.02 main shoot and axillary shoots visible at two nodes
namespace: plant_growth_and_development_stage
def: "The stage at which main shoot and axillary shoots at two nodes are visible." [GR:ap]
comment: The axillary shoot can be a single shoot or a pair of axillary shoots at each node.
synonym: "2.02 Main shoot and axillary shoots visible at 2 nodes in soybean" RELATED [SOY:0000041]
synonym: "2.02 main shoot and axillary shoots visible at two nodes in Solanaceae" RELATED [SGN:0000024]
synonym: "3.03-main shoot and two tillers" RELATED [GRO:0007072]
synonym: "BBCH growth stage 22" RELATED [ISBN:3826331524]
synonym: "main shoot and 2 tillers" RELATED [GRO:0007072]
synonym: "main shoot and second tiller visible" RELATED [GRO:0007072]
synonym: "main shoot and two tillers in barley" RELATED [GRO:0007072]
synonym: "main shoot and two tillers in oat" RELATED [GRO:0007072]
synonym: "main shoot and two tillers in wheat" RELATED [GRO:0007072]
synonym: "second axillary shoot detectable" RELATED []
synonym: "second tiller detectable" RELATED []
synonym: "Zadok scale-22" RELATED [GRO:0007072]
is_a: PO:0007073 ! 2 formation of axillary shoot

[Term]
id: PO:0007072
name: LP.18 eighteen leaves visible
namespace: plant_growth_and_development_stage
def: "The stage at which leaves at eighteen nodes, other than the cotyledonary node, are visible above ground." [GR:ap]
comment: The leaves can be a single leaf, two, or whorls of leaves at each node.
synonym: "1.18 17th trifoliolate leaf unfolded in soybean" RELATED [SOY:0000032]
synonym: "3.04-late vegetative" RELATED [GRO:0007016]
synonym: "3.4 late vegetative in maize" RELATED [MaizeGDB:67360]
synonym: "3.4 late vegetative stage of maize" RELATED [GRO:0007016]
synonym: "late vegetative in maize" RELATED [MaizeGDB:67360]
synonym: "late vegetative stage of maize" RELATED [GRO:0007016]
synonym: "maize growth stage-3.4" RELATED [GRO:0007016]
synonym: "maize V18 stage" RELATED [GRO:0007016]
synonym: "Stage V17 in soybean" RELATED [SOY:0000032]
synonym: "V18 in maize" RELATED [MaizeGDB:67360]
is_a: PO:0007133 ! leaf production

[Term]
id: PO:0007073
name: 2 formation of axillary shoot
namespace: plant_growth_and_development_stage
def: "The stage at which the axillary shoots are forming." [Poc:curators]
synonym: "03-tillering in barley" RELATED [GRO:0007069]
synonym: "03-tillering in oat" RELATED [GRO:0007069]
synonym: "03-tillering in wheat" RELATED [GRO:0007069]
synonym: "03-tillering stage in rice" RELATED [GRO:0007049]
synonym: "2 axillary Shoot Formation in soybean" RELATED [SOY:0000003]
synonym: "2 formation of axillary shoot in Solanaceae" RELATED [SGN:0000022]
synonym: "BBCH principal growth stage 2" RELATED [ISBN:3826331524]
synonym: "formation of side shoot" RELATED []
synonym: "rice growth stage-3" RELATED [GRO:0007049]
synonym: "tillering" RELATED []
is_a: PO:0007134 ! A vegetative growth

[Term]
id: PO:0007074
name: SE.15 fifteen nodes or internodes visible
namespace: plant_growth_and_development_stage
def: "The stage at which fifteen nodes or fifteen internodes are visible." [GR:pj]
comment: A measure of vegetative growth, but leaf production is to be preferred.
synonym: "3.15 15 nodes/internodes visible in soybean" RELATED [SOY:0000064]
is_a: PO:0007089 ! stem elongation

[Term]
id: PO:0007075
name: 5.02 20% of inflorescence emerged.
namespace: plant_growth_and_development_stage
def: "OBSOLETE" [GR:ap]
is_obsolete: true

[Term]
id: PO:0007076
name: late rosette growth
namespace: plant_growth_and_development_stage
def: "Rosette has reached approximately 70% of its final diameter." [Poc:curators]
comment: A measure of vegetative growth, but leaf production is to be preferred.
synonym: "late rosette growth in Arabidopsis" RELATED [TAIR:0000045]
is_a: PO:0007113 ! rosette growth

[Term]
id: PO:0007077
name: 2.08 main shoot and axillary shoots visible at eight nodes
namespace: plant_growth_and_development_stage
def: "The stage at which main shoot and axillary shoots at eight nodes are visible." [GR:ap]
comment: The axillary shoot can be a single shoot or a pair of axillary shoots at each node.
synonym: "2.08 Main shoot and axillary shoots visible at 8 nodes in soybean" RELATED [SOY:0000047]
synonym: "2.08 main shoot and axillary shoots visible at eight nodes in Solanaceae" RELATED [SGN:0000030]
synonym: "3.09-main shoot and eight tillers" RELATED [GRO:0007078]
synonym: "BBCH growth stage 28" RELATED [ISBN:3826331524]
synonym: "eighth axillary shoot detectable" RELATED []
synonym: "eighth tiller detectable" RELATED []
synonym: "main shoot and 8 tillers" RELATED []
synonym: "main shoot and eight tillers in barley" RELATED [GRO:0007078]
synonym: "main shoot and eight tillers in oat" RELATED [GRO:0007078]
synonym: "main shoot and eight tillers in wheat" RELATED [GRO:0007078]
synonym: "main shoot and eighth tiller visible" RELATED []
synonym: "Zadok scale-28" RELATED [GRO:0007078]
is_a: PO:0007073 ! 2 formation of axillary shoot

[Term]
id: PO:0007078
name: rosette growth complete
namespace: plant_growth_and_development_stage
def: "Stage at which rosette no longer increases in diameter, its leaf growth and expansion having ceased." [Poc:curators]
comment: A measure of vegetative growth, but leaf production is to be preferred.
synonym: "complete rosette in Arabidopsis" RELATED [TAIR:0000418]
is_a: PO:0007113 ! rosette growth

[Term]
id: PO:0007079
name: SE.00 stem elongation begins
namespace: plant_growth_and_development_stage
def: "The stage at which the internodes begin to elongate. " [GR:pj]
comment: A measure of vegetative growth, but leaf production is to be preferred.
synonym: "3.00 stem elongation begins in soybean" RELATED [SOY:0000049]
synonym: "4.01-pseudo stem erection in barley" RELATED [GRO:0007081]
synonym: "4.01-pseudo stem erection in oat" RELATED [GRO:0007081]
synonym: "4.01-pseudo stem erection in wheat" RELATED [GRO:0007081]
synonym: "4.1-panicle initiation stage" RELATED [GRO:0007147]
synonym: "4.2-panicle differentiation stage" RELATED [GRO:0007041]
synonym: "BBCH growth stage 30" RELATED [ISBN:3826331524]
synonym: "pseudo stem and tillers erect" RELATED []
synonym: "pseudo stem erection" RELATED []
synonym: "rice green ring stage" RELATED []
synonym: "rice panicle initiation" RELATED []
is_a: PO:0007089 ! stem elongation

[Term]
id: PO:0007080
name: 2.03 main shoot and axillary shoots visible at three nodes
namespace: plant_growth_and_development_stage
def: "The stage at which main shoot and axillary shoots at three nodes are visible." [GR:ap]
comment: The axillary shoot can be a single shoot or a pair of axillary shoots at each node.
synonym: "2.03 Main shoot and axillary shoots visible at 3 nodes in soybean" RELATED [SOY:0000042]
synonym: "2.03 main shoot and axillary shoots visible at three nodes in Solanaceae" RELATED [SGN:0000025]
synonym: "3.04-main shoot and three tillers" RELATED [GRO:0007073]
synonym: "BBCH growth stage 23" RELATED [ISBN:3826331524]
synonym: "main shoot and 3 tillers" RELATED []
synonym: "main shoot and third tiller visible" RELATED []
synonym: "main shoot and three tillers in barley" RELATED [GRO:0007073]
synonym: "main shoot and three tillers in oat" RELATED [GRO:0007073]
synonym: "main shoot and three tillers in wheat" RELATED [GRO:0007073]
synonym: "third axillary shoot detectable" RELATED []
synonym: "third tiller detectable" RELATED []
synonym: "Zadok scale-23" RELATED [GRO:0007073]
is_a: PO:0007073 ! 2 formation of axillary shoot

[Term]
id: PO:0007081
name: early rosette growth
namespace: plant_growth_and_development_stage
def: "Rosette has reached approximately 20% of its final diameter." [Poc:curators]
comment: A measure of vegetative growth, but leaf production is to be preferred.
synonym: "early rosette growth in Arabidopsis" RELATED [TAIR:0000043]
is_a: PO:0007113 ! rosette growth

[Term]
id: PO:0007082
name: LP.20 twenty or more leaves whorls visible
namespace: plant_growth_and_development_stage
def: "The stage at which leaves at twenty or more nodes, other than the cotyledonary node, are visible above ground." [GR:ap]
comment: The leaves can be a single leaf, two, or whorls of leaves at each node.
synonym: "1.20 19th trifoliolate leaf unfolded in soybean" RELATED [SOY:0000034]
synonym: "1.21 20th trifoliolate leaf unfolded in soybean" RELATED [SOY:0000035]
synonym: "1.22 21st trifoliolate leaf unfolded in soybean" RELATED [SOY:0000036]
synonym: "1.23 22nd trifoliolate leaf unfolded in soybean" RELATED [SOY:0000037]
synonym: "1.24 23rd trifoliolate leaf unfolded in soybean" RELATED [SOY:0000038]
synonym: "1.25 25 or more trifoliolate leaves unfolded in soybean" RELATED [SOY:0000039]
synonym: "3.04-late vegetative" RELATED [GRO:0007016]
synonym: "3.4 late vegetative in maize" RELATED [MaizeGDB:67360]
synonym: "3.4 late vegetative stage of maize" RELATED [GRO:0007016]
synonym: "late vegetative in maize" RELATED [MaizeGDB:67360]
synonym: "late vegetative stage of maize" RELATED [GRO:0007016]
synonym: "maize growth stage-3.4" RELATED [GRO:0007016]
synonym: "maize V20 stage" RELATED []
synonym: "Stage V20 in soybean" RELATED [SOY:0000035]
synonym: "Stage V21 in soybean" RELATED [SOY:0000036]
synonym: "Stage V22 in soybean" RELATED [SOY:0000037]
synonym: "Stage V23 in soybean" RELATED [SOY:0000038]
synonym: "Stage V25 in soybean" RELATED [SOY:0000039]
synonym: "V20 in maize" RELATED [MaizeGDB:67360]
is_a: PO:0007133 ! leaf production

[Term]
id: PO:0007083
name: LP.13 thirteen leaves visible
namespace: plant_growth_and_development_stage
def: "The stage at which leaves at thirteen nodes, other than the cotyledonary node, are visible above ground." [GR:ap]
comment: The leaves can be a single leaf, two, or whorls of leaves at each node.
synonym: "1.13 12th trifoliolate leaf unfolded in soybean" RELATED [SOY:0000027]
synonym: "13 rosette leaf in Arabidopsis" RELATED [TAIR:0000416]
synonym: "3.03-mid-vegetative" RELATED [GRO:0007015]
synonym: "3.3 mid-vegetative" RELATED [MaizeGDB:67359]
synonym: "3.3 mid-vegetative stage of maize" RELATED [GRO:0007015]
synonym: "maize growth stage-3.3" RELATED [GRO:0007015]
synonym: "mid-vegetative in maize" RELATED [MaizeGDB:67359]
synonym: "mid-vegetative stage of maize" RELATED [GRO:0007015]
synonym: "Stage V12 in soybean" RELATED [SOY:0000027]
synonym: "thirteen leaves unfolded" RELATED []
synonym: "thirteen rosette leaves" RELATED []
synonym: "V13 in maize" RELATED [MaizeGDB:67359]
is_a: PO:0007133 ! leaf production

[Term]
id: PO:0007084
name: SE.10 ten nodes or internodes visible
namespace: plant_growth_and_development_stage
def: "The stage at which ten nodes or ten internodes are visible." [GR:pj]
comment: A measure of vegetative growth, but leaf production is to be preferred.
synonym: "3.10 10 nodes/internodes visible in soybean" RELATED [SOY:0000059]
is_a: PO:0007089 ! stem elongation

[Term]
id: PO:0007085
name: LP.14 fourteen leaves visible
namespace: plant_growth_and_development_stage
def: "The stage at which leaves at fourteen nodes, other than the cotyledonary node, are visible above ground." [GR:ap]
comment: The leaves can be a single leaf, two, or whorls of leaves at each node.
synonym: "1.14 13th trifoliolate leaf unfolded in soybean" RELATED [SOY:0000028]
synonym: "14 rosette leaf in Arabidopsis" RELATED [TAIR:0000417]
synonym: "3.03-mid-vegetative" RELATED [GRO:0007015]
synonym: "3.3 mid-vegetative" RELATED [MaizeGDB:67359]
synonym: "3.3 mid-vegetative stage of maize" RELATED [GRO:0007015]
synonym: "fourteen leaves unfolded" RELATED []
synonym: "fourteen rosette leaves" RELATED []
synonym: "maize growth stage-3.3" RELATED [GRO:0007015]
synonym: "Stage V13 in soybean" RELATED [SOY:0000028]
synonym: "V14 in maize" RELATED [MaizeGDB:67359]
is_a: PO:0007133 ! leaf production

[Term]
id: PO:0007086
name: SE.05 five nodes or internodes visible
namespace: plant_growth_and_development_stage
def: "The stage at which five nodes or five internodes are visible." [GR:pj]
comment: A measure of vegetative growth, but leaf production is to be preferred.
synonym: "3.05 5 nodes/internodes visible in soybean" RELATED [SOY:0000054]
synonym: "4.06-fifth node detectable in barley" RELATED [GRO:0007086]
synonym: "4.06-fifth node detectable in oat" RELATED [GRO:0007086]
synonym: "4.06-fifth node detectable in wheat" RELATED [GRO:0007086]
synonym: "BBCH growth stage 35" RELATED [ISBN:3826331524]
synonym: "Zadok scale-35" RELATED [GRO:0007086]
is_a: PO:0007089 ! stem elongation

[Term]
id: PO:0007087
name: 2.01 main shoot and axillary shoots visible at one node
namespace: plant_growth_and_development_stage
def: "The stage at which main shoot and axillary shoot(s) at one node is (are) visible." [Poc:curators]
synonym: "2.01 Main shoot and axillary shoot visible at one node in soybean" RELATED [SOY:0000040]
synonym: "2.01 main shoot and axillary shoots visible at one node in Solanaceae" RELATED [SGN:0000023]
synonym: "3.02-main shoot and one tiller" RELATED [GRO:0007071]
synonym: "BBCH growth stage 21" RELATED [ISBN:3826331524]
synonym: "first axillary shoot detectable" RELATED []
synonym: "first tiller detectable" RELATED []
synonym: "main shoot and 1 tiller" RELATED []
synonym: "main shoot and first tiller visible" RELATED []
synonym: "main shoot and one tiller in barley" RELATED [GRO:0007071]
synonym: "main shoot and one tiller in oat" RELATED [GRO:0007071]
synonym: "main shoot and one tiller in wheat" RELATED [GRO:0007071]
synonym: "Zadok scale-21, Feekes scale-2" RELATED [GRO:0007071]
is_a: PO:0007073 ! 2 formation of axillary shoot

[Term]
id: PO:0007088
name: 2.04 main shoot and axillary shoots visible at four nodes
namespace: plant_growth_and_development_stage
def: "The stage at which main shoot and axillary shoots at four nodes are visible." [GR:ap]
comment: The axillary shoot can be a single shoot or a pair of axillary shoots at each node.
synonym: "2.04 Main shoot and axillary shoots visible at 4 nodes in soybean" RELATED [SOY:0000043]
synonym: "2.04 main shoot and axillary shoots visible at four nodes in Solanaceae" RELATED [SGN:0000026]
synonym: "3.05-main shoot and four tillers" RELATED [GRO:0007074]
synonym: "BBCH growth stage 24" RELATED [ISBN:3826331524]
synonym: "fourth axillary shoot detectable" RELATED []
synonym: "fourth tiller detectable" RELATED []
synonym: "main shoot and 4 tillers" RELATED []
synonym: "main shoot and four tillers in barley" RELATED [GRO:0007074]
synonym: "main shoot and four tillers in oat" RELATED [GRO:0007074]
synonym: "main shoot and four tillers in wheat" RELATED [GRO:0007074]
synonym: "main shoot and fourth tiller visible" RELATED []
synonym: "Zadok scale-24" RELATED [GRO:0007074]
is_a: PO:0007073 ! 2 formation of axillary shoot

[Term]
id: PO:0007089
name: stem elongation
namespace: plant_growth_and_development_stage
def: "The stage at which the internodes elongate. " [GR:pj]
comment: A measure of vegetative growth, but leaf production is to be preferred.
synonym: "04-stem elongation in barley" RELATED [GRO:0007080]
synonym: "04-stem elongation in oat" RELATED [GRO:0007080]
synonym: "04-stem elongation in wheat" RELATED [GRO:0007080]
synonym: "04-stem elongation stage in Triticeae" RELATED [GRO:0007080]
synonym: "05-growing point differentiation" RELATED []
synonym: "3 rapid stem elongation in maize" RELATED [MaizeGDB:67358]
synonym: "3 Stem Elongation in soybean" RELATED [SOY:0000004]
synonym: "BBCH principal growth stage 3" RELATED [ISBN:3826331524]
synonym: "crop cover in potato" RELATED [SGN:0000054]
synonym: "internode elongation" RELATED []
synonym: "jointing stage" RELATED [GRO:0007048]
synonym: "rapid stem elongation" RELATED []
synonym: "rice growth stage-4" RELATED [GRO:0007048]
synonym: "shoot development" RELATED []
synonym: "sorghum growth stage-4" RELATED [GRO:0007128]
synonym: "stem elongation in Solanaceae" RELATED [SGN:0000054]
is_a: PO:0007112 ! 1 main shoot growth

[Term]
id: PO:0007090
name: SE.13 thirteen nodes or internodes visible
namespace: plant_growth_and_development_stage
def: "The stage at which thirteen nodes or thirteen internodes are visible." [GR:pj]
comment: A measure of vegetative growth, but leaf production is to be preferred.
synonym: "3.13 13 nodes/internodes visible in soybean" RELATED [SOY:0000062]
is_a: PO:0007089 ! stem elongation

[Term]
id: PO:0007091
name: SE.01 one node or internode visible
namespace: plant_growth_and_development_stage
def: "The stage at which one node or one internode is visible. " [GR:pj]
comment: A measure of vegetative growth, but leaf production is to be preferred.
synonym: "3.01 one node visible in soybean" RELATED [SOY:0000050]
synonym: "4.02-first node detectable in barley" RELATED [GRO:0007082]
synonym: "4.02-first node detectable in oat" RELATED [GRO:0007082]
synonym: "4.02-first node detectable in wheat" RELATED [GRO:0007082]
synonym: "BBCH growth stage 31" RELATED [ISBN:3826331524]
synonym: "Zadok scale-31, Feekes scale-6" RELATED [GRO:0007082]
is_a: PO:0007089 ! stem elongation

[Term]
id: PO:0007092
name: SE.04 four nodes or internodes visible
namespace: plant_growth_and_development_stage
def: "The stage at which four nodes or four internodes are visible." [GR:pj]
comment: A measure of vegetative growth, but leaf production is to be preferred.
synonym: "3.04 4 nodes/internodes visible in soybean" RELATED [SOY:0000053]
synonym: "4.05-fourth node detectable in barley" RELATED [GRO:0007085]
synonym: "4.05-fourth node detectable in oat" RELATED [GRO:0007085]
synonym: "4.05-fourth node detectable in wheat" RELATED [GRO:0007085]
synonym: "BBCH growth stage 34" RELATED [ISBN:3826331524]
synonym: "Zadok scale-34" RELATED [GRO:0007085]
is_a: PO:0007089 ! stem elongation

[Term]
id: PO:0007093
name: 2.05 main shoot and axillary shoots visible at five nodes
namespace: plant_growth_and_development_stage
def: "The stage at which main shoot and axillary shoots at five nodes are visible." [GR:ap]
comment: The axillary shoot can be a single shoot or a pair of axillary shoots at each node.
synonym: "2.05 Main shoot and axillary shoots visible at 5 nodes in soybean" RELATED [SOY:0000044]
synonym: "2.05 main shoot and axillary shoots visible at five nodes in Solanaceae" RELATED [SGN:0000027]
synonym: "3.06-main shoot and five tillers in barley" RELATED [GRO:0007075]
synonym: "3.06-main shoot and five tillers in oat" RELATED [GRO:0007075]
synonym: "3.06-main shoot and five tillers in Triticeae" RELATED [GRO:0007075]
synonym: "3.06-main shoot and five tillers in wheat" RELATED [GRO:0007075]
synonym: "BBCH growth stage 25" RELATED [ISBN:3826331524]
synonym: "fifth axillary shoot detectable" RELATED []
synonym: "fifth tiller detectable" RELATED []
synonym: "main shoot and 5 tillers" RELATED []
synonym: "main shoot and fifth tiller visible" RELATED []
synonym: "main shoot and five tillers in barley" RELATED [GRO:0007075]
synonym: "main shoot and five tillers in oat" RELATED [GRO:0007075]
synonym: "main shoot and five tillers in wheat" RELATED [GRO:0007075]
synonym: "Zadok scale-25" RELATED [GRO:0007075]
is_a: PO:0007073 ! 2 formation of axillary shoot

[Term]
id: PO:0007094
name: LP.01 one leaf visible
namespace: plant_growth_and_development_stage
def: "The stage at which leaves at one node, other than the cotyledonary node, are visible above ground." [GR:ap, Poc:curators]
comment: In the taxa with hypogeal type germination the first leaf on the epicotyl is leaf 1, and in grasses, the coleoptile is leaf 1.  The leaves can be a single leaf, two, or whorls of leaves at each node.
synonym: "1-4 leaf stage in rice" RELATED [GRO:0007142]
synonym: "1.01 Unifoliolate leaves unfolded in soybean" RELATED [SOY:0000015]
synonym: "1.02-one to two leaves in maize" RELATED [GRO:0007009]
synonym: "1.2 1-2 leaves in maize" RELATED [Maize:67353]
synonym: "2.02-first leaf unfolded in barley" RELATED [GRO:0007060]
synonym: "2.02-first leaf unfolded in oat" RELATED [GRO:0007060]
synonym: "2.02-first leaf unfolded in Triticeae" RELATED [GRO:0007060]
synonym: "2.02-first leaf unfolded in wheat" RELATED [GRO:0007060]
synonym: "BBCH growth stage 11" RELATED [ISBN:3826331524]
synonym: "LP.01 one leaf visible in Solanaceae" RELATED [SGN:0000013]
synonym: "maize growth stage-1.2" RELATED [GRO:0007009]
synonym: "pre tillering" RELATED [GRO:0007142]
synonym: "rice growth stage-2.1" RELATED [GRO:0007142]
synonym: "V01 stage (sensu Zea)" RELATED []
synonym: "V1 in maize " RELATED [Maize:67353]
synonym: "VC stage in soybean" RELATED [SOY:0000015]
synonym: "Zadok scale-11, Haun scale-1.+" RELATED [GRO:0007060]
is_a: PO:0007133 ! leaf production

[Term]
id: PO:0007095
name: LP.08 eight leaves visible
namespace: plant_growth_and_development_stage
def: "The stage at which leaves at eight nodes, other than the cotyledonary node, are visible above ground." [GR:ap]
comment: The leaves can be a single leaf, two, or whorls of leaves at each node.
synonym: "1.08 7th trifoliolate leaf unfolded in soybean" RELATED [SOY:0000022]
synonym: "2.09-eight leaves unfolded in barley" RELATED [GRO:0007067]
synonym: "2.09-eight leaves unfolded in oat" RELATED [GRO:0007067]
synonym: "2.09-eight leaves unfolded in Triticeae" RELATED [GRO:0007067]
synonym: "2.09-eight leaves unfolded in wheat" RELATED [GRO:0007067]
synonym: "3.01-ear initiation in Maize" RELATED [GRO:0007013]
synonym: "3.1 ear initiation/mid-whorl stage in maize" RELATED [MaizeGDB:67356]
synonym: "8 leaves unfolded" RELATED []
synonym: "8 rosette leaves in Arabidopsis" RELATED [TAIR:0000411]
synonym: "8-leaf in maize" RELATED [MaizeGDB:67356]
synonym: "BBCH growth stage 18" RELATED [ISBN:3826331524]
synonym: "ear initiation in maize" RELATED [MaizeGDB:67356]
synonym: "eight leaf unfolded" RELATED []
synonym: "eight leaves unfolded (sensu Triticeae)" RELATED [GRO:0007067]
synonym: "eight rosette leaves" RELATED []
synonym: "LP.08 eight leaves visible in Solanaceae" RELATED [SGN:0000020]
synonym: "maize growth stage-3.1" RELATED [GRO:0007013]
synonym: "mid-whorl stage in maize" RELATED [MaizeGDB:67356]
synonym: "Stage V7 in soybean" RELATED [SOY:0000022]
synonym: "V8 in maize" RELATED [MaizeGDB:67356]
synonym: "Zadok scale-18, Haun scale-7.+" RELATED [GRO:0007067]
is_a: PO:0007133 ! leaf production

[Term]
id: PO:0007096
name: SE.03 three nodes or internodes visible
namespace: plant_growth_and_development_stage
def: "The stage at which three nodes or three internodes are visible." [GR:pj]
comment: A measure of vegetative growth, but leaf production is to be preferred.
synonym: "3.03 3 nodes/internodes visible in soybean" RELATED [SOY:0000052]
synonym: "4.04-third node detectable in barley" RELATED [GRO:0007084]
synonym: "4.04-third node detectable in oat" RELATED [GRO:0007084]
synonym: "4.04-third node detectable in wheat" RELATED [GRO:0007084]
synonym: "BBCH growth stage 33" RELATED [ISBN:3826331524]
synonym: "Zadok scale-33" RELATED [GRO:0007084]
is_a: PO:0007089 ! stem elongation

[Term]
id: PO:0007097
name: SE.14 fourteen nodes or internodes visible
namespace: plant_growth_and_development_stage
def: "The stage at which fourteen nodes or fourteen internodes are visible." [GR:pj]
comment: A measure of vegetative growth, but leaf production is to be preferred.
synonym: "3.14 14 nodes/internodes visible in soybean" RELATED [SOY:0000063]
is_a: PO:0007089 ! stem elongation

[Term]
id: PO:0007098
name: LP.02 two leaves visible
namespace: plant_growth_and_development_stage
def: "The stage at which leaves at two nodes, other than the cotyledonary node, are visible above ground." [Poc:curators]
comment: In grasses, the plant has one leaf plus the coleoptile.  The leaves can be a single leaf, two, or whorls of leaves at each node.
synonym: "1-4 leaf stage in rice" RELATED [GRO:0007142]
synonym: "1.02 First trifoliolate leaf unfolded in soybean" RELATED [SOY:0000016]
synonym: "1.02-one to two leaves in maize" RELATED [GRO:0007009]
synonym: "1.2 1-2 leaves in maize" RELATED [MaizeGDB:67353]
synonym: "2 leaves unfolded" RELATED []
synonym: "2 rosette leaves in Arabidopsis" RELATED [TAIR:0000398]
synonym: "2.03-two leaves unfolded in barley" RELATED [GRO:0007061]
synonym: "2.03-two leaves unfolded in oat" RELATED [GRO:0007061]
synonym: "2.03-two leaves unfolded in Triticeae" RELATED [GRO:0007061]
synonym: "2.03-two leaves unfolded in wheat" RELATED [GRO:0007061]
synonym: "BBCH growth stage 12" RELATED [ISBN:3826331524]
synonym: "LP.02 two leaves visible in Solanaceae" RELATED [SGN:0000014]
synonym: "maize growth stage-1.2" RELATED [GRO:0007009]
synonym: "pre tillering" RELATED [GRO:0007142]
synonym: "rice growth stage-2.1" RELATED [GRO:0007142]
synonym: "two leaves unfolded (sensu Triticeae)" RELATED [GRO:0007061]
synonym: "two rosette leaves" RELATED []
synonym: "V1 stage in soybean" RELATED [SOY:0000016]
synonym: "V2 in maize" RELATED [MaizeGDB:67353]
synonym: "Zadok scale-12, Haun scale-1.+" RELATED [GRO:0007061]
is_a: PO:0007133 ! leaf production

[Term]
id: PO:0007099
name: SE.97 flag leaf visible
namespace: plant_growth_and_development_stage
def: "The stage at which the flag leaf is visible." [GR:ap]
comment: A measure of vegetative growth, but leaf production is to be preferred.
synonym: "06-flag leaf visible in sorghum" RELATED [GRO:0007129]
synonym: "4.08-flag leaf just visible in barley" RELATED [GRO:0007088]
synonym: "4.08-flag leaf just visible in oat" RELATED [GRO:0007088]
synonym: "4.08-flag leaf just visible in wheat" RELATED [GRO:0007088]
synonym: "Zadok scale-37, Feekes scale-8" RELATED [GRO:0007088]
is_a: PO:0007089 ! stem elongation

[Term]
id: PO:0007100
name: SE.16 sixteen or more nodes or internodes visible
namespace: plant_growth_and_development_stage
def: "The stage at which sixteen nodes or more, or sixteen internodes or more are visible." [GR:pj]
comment: A measure of vegetative growth, but leaf production is to be preferred.
synonym: "3.16 16 or more nodes/internodes visible in soybean" RELATED [SOY:0000065]
is_a: PO:0007089 ! stem elongation

[Term]
id: PO:0007101
name: LP.09 nine leaves visible
namespace: plant_growth_and_development_stage
def: "The stage at which leaves at nine nodes, other than the cotyledonary node, are visible above ground." [GR:ap]
comment: The leaves can be a single leaf, two, or whorls of leaves at each node.
synonym: "1.09 8th trifoliolate leaf unfolded in soybean" RELATED [SOY:0000023]
synonym: "10-leaf in maize" RELATED [MaizeGDB:67357]
synonym: "2.10 nine or more leaves unfolded in barley" RELATED [GRO:0007068]
synonym: "2.10 nine or more leaves unfolded in oat" RELATED [GRO:0007068]
synonym: "2.10 nine or more leaves unfolded in Triticeae" RELATED [GRO:0007068]
synonym: "2.10 nine or more leaves unfolded in wheat" RELATED [GRO:0007068]
synonym: "3.02-late whorl stage" RELATED [GRO:0007014]
synonym: "3.2 late whorl stage in maize" RELATED [MaizeGDB:67357]
synonym: "9 or more leaves unfolded" RELATED []
synonym: "9 rosette leaf in Arabidopsis" RELATED [TAIR:0000412]
synonym: "9-11 leaves in maize" RELATED [MaizeGDB:67357]
synonym: "9-leaf in maize" RELATED [MaizeGDB:67357]
synonym: "BBCH growth stage 19" RELATED [ISBN:3826331524]
synonym: "LP.09 nine or more leaves whorls visible" RELATED [SGN:0000021]
synonym: "maize growth stage-3.2" RELATED [GRO:0007014]
synonym: "nine rosette leaves" RELATED []
synonym: "ninth leaf unfolded" RELATED []
synonym: "Stage V8 in soybean" RELATED [SOY:0000023]
synonym: "V9 in maize" RELATED [MaizeGDB:67357]
synonym: "Zadok scale-19" RELATED [GRO:0007068]
is_a: PO:0007133 ! leaf production

[Term]
id: PO:0007102
name: 5.04 40% of inflorescence emerged
namespace: plant_growth_and_development_stage
def: "OBSOLETE" [GR:ap]
is_obsolete: true

[Term]
id: PO:0007103
name: LP.10 ten leaves visible
namespace: plant_growth_and_development_stage
def: "The stage at which leaves at ten nodes, other than the cotyledonary node, are visible above ground" [GR:ap]
comment: The leaves can be a single leaf, two, or whorls of leaves at each node.
synonym: "10 rosette leaf in Arabidopsis" RELATED [TAIR:0000413]
synonym: "10-leaf in maize" RELATED [MaizeGDB:67357]
synonym: "3.02-late whorl stage" RELATED [GRO:0007014]
synonym: "9-11 leaves in maize" RELATED [MaizeGDB:67357]
synonym: "maize growth stage-3.2" RELATED [GRO:0007014]
synonym: "Stage V9 in soybean" RELATED [SOY:0000024]
synonym: "ten rosette leaves" RELATED []
synonym: "V10 in maize" RELATED [MaizeGDB:67357]
is_a: PO:0007133 ! leaf production

[Term]
id: PO:0007104
name: LP.15 fifteen leaves visible
namespace: plant_growth_and_development_stage
def: "The stage at which leaves at fifteen nodes, other than the cotyledonary node, are visible above ground." [GR:ap]
comment: The leaves can be a single leaf, two, or whorls of leaves at each node.
synonym: "1.15 14th trifoliolate leaf unfolded in soybean" RELATED [SOY:0000029]
synonym: "3.4 late vegetative in maize" RELATED [MaizeGDB:67360]
synonym: "3.4 late vegetative stage of maize" RELATED [GRO:0007016]
synonym: "late vegetative in maize" RELATED [MaizeGDB:67360]
synonym: "maize growth stage-3.4" RELATED [GRO:0007016]
synonym: "Stage V14 in soybean" RELATED [SOY:0000029]
synonym: "V15 in maize" RELATED [MaizeGDB:67360]
is_a: PO:0007133 ! leaf production

[Term]
id: PO:0007105
name: 5.06 60% of inflorescence emerged
namespace: plant_growth_and_development_stage
def: "OBSOLETE" [GR:ap]
is_obsolete: true

[Term]
id: PO:0007106
name: LP.03 three leaves visible
namespace: plant_growth_and_development_stage
def: "The stage at which leaves at three nodes, other than the cotyledonary node, are visible above ground." [GR:ap]
comment: The leaves can be a single leaf, two, or whorls of leaves at each node.
synonym: "02-three leaf stage in sorghum" RELATED [GRO:0007126]
synonym: "1-4 leaf stage in rice" RELATED [GRO:0007142]
synonym: "1.03 2nd trifoliolate leaf unfolded in soybean" RELATED [SOY:0000017]
synonym: "1.03-three to four leaves in maize" RELATED [GRO:0007010]
synonym: "1.3 3-4 leaves in maize" RELATED [Maize:25331]
synonym: "2.04-three leaves unfolded" RELATED [GRO:0007062]
synonym: "3 rosette leaf in Arabidopsis" RELATED [TAIR:0000407]
synonym: "3-leaf stage in maize" RELATED [Maize:25331]
synonym: "BBCH growth stage 13" RELATED [ISBN:3826331524]
synonym: "LP.03 three leaves visible in Solanaceae" RELATED [SGN:0000015]
synonym: "maize growth stage-1.3" RELATED [GRO:0007010]
synonym: "pre tillering" RELATED [GRO:0007142]
synonym: "rice growth stage-2.1" RELATED [GRO:0007142]
synonym: "sorghum growth stage-1" RELATED [GRO:0007126]
synonym: "V2 stage in soybean" RELATED [SOY:0000017]
synonym: "V3 in maize" RELATED [Maize:25331]
synonym: "Zadok scale-13, Haun scale-2.+" RELATED [GRO:0007062]
is_a: PO:0007133 ! leaf production

[Term]
id: PO:0007107
name: 5.08 80% of inflorescence emerged
namespace: plant_growth_and_development_stage
def: "OBSOLETE" [GR:ap]
is_obsolete: true

[Term]
id: PO:0007108
name: SE.07 seven nodes or internodes visible
namespace: plant_growth_and_development_stage
def: "The stage at which seven nodes or seven internodes are visible." [GR:pj]
comment: A measure of vegetative growth, but leaf production is to be preferred.
synonym: "3.07 7 nodes/internodes visible in soybean" RELATED [SOY:0000056]
synonym: "BBCH growth stage 37" RELATED [ISBN:3826331524]
is_a: PO:0007089 ! stem elongation

[Term]
id: PO:0007109
name: SE.99 maximum stem length reached
namespace: plant_growth_and_development_stage
def: "The stage at which maximum stem length is reached." [GR:ap]
comment: A measure of vegetative growth, but leaf production is to be preferred.
synonym: "3.99 Maximum stem length reached in soybean" RELATED [SOY:0000066]
synonym: "4.09-flag leaf ligule/collar just visible in barley" RELATED [GRO:0007089]
synonym: "4.09-flag leaf ligule/collar just visible in oat" RELATED [GRO:0007089]
synonym: "4.09-flag leaf ligule/collar just visible in wheat" RELATED [GRO:0007089]
synonym: "flag leaf fully unrolled" RELATED []
synonym: "flag leaf stage" RELATED []
synonym: "flag leaf stage in sorghum" RELATED [GRO:0007089]
synonym: "ligule just visible" RELATED []
synonym: "sorghum growth stage-5" RELATED [GRO:0007089]
synonym: "Zadok scale-39, Feekes scale-9" RELATED [GRO:0007089]
is_a: PO:0007089 ! stem elongation

[Term]
id: PO:0007110
name: 2.09 main shoot and axillary shoots visible at  nine or more nodes
namespace: plant_growth_and_development_stage
def: "The stage at which main shoot and axillary shoots at nine nodes or more are visible." [GR:ap]
comment: The axillary shoot can be a single shoot or a pair of axillary shoots at each node.
synonym: "2.09 main shoot and axillary shoots visible at  nine or more nodes in Solanaceae" RELATED [SGN:0000031]
synonym: "2.09 Main shoot and axillary shoots visible at 9 or more nodes in soybean" RELATED [SOY:0000048]
synonym: "3.1-maximum tillering" RELATED [GRO:0007144]
synonym: "3.10-main shoot and nine or more tillers in Triticeae" RELATED [GRO:0007079]
synonym: "BBCH growth stage 29" RELATED [ISBN:3826331524]
synonym: "main shoot and 9 or more tiller" RELATED [GRO:0007079]
synonym: "main shoot and nine or more tillers in barley" RELATED []
synonym: "main shoot and nine or more tillers in oat" RELATED []
synonym: "main shoot and nine or more tillers in wheat" RELATED []
synonym: "maximum number of tillers detectable in" RELATED []
synonym: "maximum number of tillers visible" RELATED []
synonym: "maximum number of tillers visible in rice" RELATED []
synonym: "nine or more axillary shoots detectable" RELATED []
synonym: "Zadok scale-29" RELATED [GRO:0007079]
is_a: PO:0007073 ! 2 formation of axillary shoot

[Term]
id: PO:0007111
name: SE.12 twelve nodes or internodes visible
namespace: plant_growth_and_development_stage
def: "The stage at which twelve nodes or twelve internodes are visible." [GR:pj]
comment: A measure of vegetative growth, but leaf production is to be preferred.
synonym: "3.12 12 nodes/internodes visible in soybean" RELATED [SOY:0000061]
is_a: PO:0007089 ! stem elongation

[Term]
id: PO:0007112
name: 1 main shoot growth
namespace: plant_growth_and_development_stage
def: "The stage at which vegetative structures are being produced by SAM." [Poc:curators]
comment: In monocots each leaf stage is defined according to the uppermost leaf whose collar is visible (Handbook of plant and crop physiology)
synonym: "01-seedling stage of maize" RELATED [GRO:0007007]
synonym: "02-seedling growth of barley" RELATED [GRO:0007058]
synonym: "02-seedling growth of oat" RELATED [GRO:0007058]
synonym: "02-seedling growth of wheat" RELATED [GRO:0007058]
synonym: "02-seedling stage of rice" RELATED [GRO:0007047]
synonym: "1 main shoot growth in Solanaceae" RELATED [SGN:0000011]
synonym: "1 seedling in maize" RELATED [MaizeGDB:1863]
synonym: "BBCH principal growth stage 1" RELATED [ISBN:3826331524]
synonym: "maize growth stage-1.1" RELATED [GRO:0007007]
synonym: "sorghum principal growth stage 1" RELATED [GRO:0007126]
is_a: PO:0007134 ! A vegetative growth

[Term]
id: PO:0007113
name: rosette growth
namespace: plant_growth_and_development_stage
def: "Stages of growth based on expansion of the rosette in Arabidopsis" [TAIR:ki]
comment: A measure of vegetative growth, but leaf production is to be preferred.
synonym: "rosette growth in Arabidopsis" RELATED [TAIR:0000042]
is_a: PO:0007112 ! 1 main shoot growth

[Term]
id: PO:0007114
name: SE.11 eleven nodes or internodes visible
namespace: plant_growth_and_development_stage
def: "The stage at which eleven nodes or eleven internodes are visible." [GR:pj]
comment: A measure of vegetative growth, but leaf production is to be preferred.
synonym: "3.11 11 nodes/internodes visible in soybean" RELATED [SOY:0000060]
is_a: PO:0007089 ! stem elongation

[Term]
id: PO:0007115
name: LP.04 four leaves visible
namespace: plant_growth_and_development_stage
def: "The stage at which leaves at four nodes, other than the cotyledonary node, are visible above ground." [GR:ap]
comment: The leaves can be a single leaf, two, or whorls of leaves at each node.
synonym: "02-tassel initiation in maize" RELATED [GRO:0007011]
synonym: "03-four leaf stage in sorghum" RELATED [GRO:0007143]
synonym: "1-4 leaf stage in rice" RELATED [GRO:0007142]
synonym: "1.03-three to four leaves in maize" RELATED [GRO:0007010]
synonym: "1.04 3rd trifoliolate leaf unfolded in soybean" RELATED [SOY:0000018]
synonym: "2 tassel initiation/early whorl stage in maize" RELATED [MaizeGDB:67306]
synonym: "2.05-four leaves unfolded in Triticeae" RELATED [GRO:0007063]
synonym: "4 leaves unfolded" RELATED []
synonym: "4 rosette leaf in Arabidopsis" RELATED [TAIR:0000399]
synonym: "4-6 leaves in maize" RELATED [MaizeGDB:67306]
synonym: "BBCH growth stage 14" RELATED [ISBN:3826331524]
synonym: "early whorl stage in maize" RELATED [MaizeGDB:67306]
synonym: "four rosette leaves" RELATED []
synonym: "fourth leaf unfolded" RELATED []
synonym: "LP.04 four leaves visible in Solanaceae" RELATED [SGN:0000016]
synonym: "maize growth stage-2" RELATED [GRO:0007011]
synonym: "pre tillering" RELATED [GRO:0007142]
synonym: "rice growth stage-2.1" RELATED [GRO:0007142]
synonym: "sorghum growth stage-2" RELATED [GRO:0007143]
synonym: "Stage V3 in soybean" RELATED [SOY:0000018]
synonym: "tassel differentiation in maize" RELATED [MaizeGDB:67306]
synonym: "tassel initiation in maize" RELATED [MaizeGDB:67306]
synonym: "V4 in maize" RELATED [MaizeGDB:67306]
synonym: "Zadok scale-14, Haun scale-3.+" RELATED [GRO:0007063]
is_a: PO:0007133 ! leaf production

[Term]
id: PO:0007116
name: LP.11 eleven leaves visible
namespace: plant_growth_and_development_stage
def: "The stage at which leaves at eleven nodes, other than the cotyledonary node, are visible above ground." [GR:ap]
comment: The leaves can be a single leaf, two, or whorls of leaves at each node.
synonym: "1.11 10th trifoliolate leaf unfolded in soybean" RELATED [SOY:0000025]
synonym: "11 rosette leaves in Arabidopsis" RELATED [TAIR:0000414]
synonym: "3.02-late whorl stage in maize" RELATED [GRO:0007014]
synonym: "3.2 late whorl stage of maize" RELATED [GRO:0007014]
synonym: "9-11 leaves in maize" RELATED [MaizeGDB:67357]
synonym: "eleven rosette leaves" RELATED []
synonym: "late whorl stage of maize" RELATED [GRO:0007014]
synonym: "maize growth stage-3.2" RELATED [GRO:0007014]
synonym: "Stage V10 in soybean" RELATED [SOY:0000025]
synonym: "V11 in maize" RELATED [MaizeGDB:67357]
is_a: PO:0007133 ! leaf production

[Term]
id: PO:0007117
name: SE.02 two nodes or internodes visible
namespace: plant_growth_and_development_stage
def: "The stage at which two nodes or two internodes are visible." [GR:pj]
comment: A measure of vegetative growth, but leaf production is to be preferred.
synonym: "3.02 2 nodes/internode visible in soybean" RELATED [SOY:0000051]
synonym: "4.03-second node detectable in barley" RELATED [GRO:0007083]
synonym: "4.03-second node detectable in oat" RELATED [GRO:0007083]
synonym: "4.03-second node detectable in wheat" RELATED [GRO:0007083]
synonym: "BBCH growth stage 32" RELATED [ISBN:3826331524]
synonym: "maize growth stage-3.1" RELATED [GRO:0007013]
synonym: "Zadok scale-32, Feekes scale-7" RELATED [GRO:0007083]
is_a: PO:0007089 ! stem elongation

[Term]
id: PO:0007118
name: 2.06 main shoot and axillary shoots visible at six nodes
namespace: plant_growth_and_development_stage
def: "The stage at which main shoot and axillary shoots at six nodes are visible." [GR:ap]
comment: The axillary shoot can be a single shoot or a pair of axillary shoots at each node.
synonym: "2.06 Main shoot and axillary shoots visible at 6 nodes in soybean" RELATED [SOY:0000045]
synonym: "2.06 main shoot and axillary shoots visible at six nodes in Solanaceae" RELATED [SGN:0000028]
synonym: "3.07-main shoot and six tillers" RELATED [GRO:0007076]
synonym: "BBCH growth stage 26" RELATED [ISBN:3826331524]
synonym: "main shoot and 6 tillers" RELATED []
synonym: "main shoot and six tillers in barley" RELATED [GRO:0007076]
synonym: "main shoot and six tillers in oat" RELATED [GRO:0007076]
synonym: "main shoot and six tillers in wheat" RELATED [GRO:0007076]
synonym: "sixth axillary shoot detectable" RELATED []
synonym: "sixth tiller detectable" RELATED []
synonym: "Zadok scale-26, Feekes scale-3" RELATED [GRO:0007076]
is_a: PO:0007073 ! 2 formation of axillary shoot

[Term]
id: PO:0007119
name: LP.16 sixteen leaves visible
namespace: plant_growth_and_development_stage
def: "The stage at which leaves at sixteen nodes, other than the cotyledonary node, are visible above ground." [GR:ap]
comment: The leaves can be a single leaf, two, or whorls of leaves at each node.
synonym: "1.16 15th trifoliolate leaf unfolded in soybean" RELATED [SOY:0000030]
synonym: "16 rosette leaf in Arabidopsis" RELATED [TAIR:0000036]
synonym: "3.04-late vegetative" RELATED [GRO:0007016]
synonym: "3.4 late vegetative in maize" RELATED [MaizeGDB:67360]
synonym: "3.4 late vegetative stage of maize" RELATED [GRO:0007016]
synonym: "late vegetative in maize" RELATED [MaizeGDB:67360]
synonym: "late vegetative stage of maize" RELATED [GRO:0007016]
synonym: "maize growth stage-3.4" RELATED [GRO:0007016]
synonym: "Stage V15 in soybean" RELATED [SOY:0000030]
synonym: "V16 in maize" RELATED [MaizeGDB:67360]
is_a: PO:0007133 ! leaf production

[Term]
id: PO:0007120
name: LP.19 nineteen leaves visible
namespace: plant_growth_and_development_stage
def: "The stage at which leaves at nineteen nodes, other than the cotyledonary node, are visible above ground." [GR:ap]
comment: The leaves can be a single leaf, two, or whorls of leaves at each node.
synonym: "1.19 18th trifoliolate leaf unfolded in soybean" RELATED [SOY:0000033]
synonym: "3.04-late vegetative" RELATED [GRO:0007016]
synonym: "3.4 late vegetative in maize" RELATED [MaizeGDB:67360]
synonym: "3.4 late vegetative stage of maize" RELATED [GRO:0007016]
synonym: "late vegetative in maize" RELATED [MaizeGDB:67360]
synonym: "late vegetative stage of maize" RELATED [GRO:0007016]
synonym: "maize growth stage-3.4" RELATED [GRO:0007016]
synonym: "Stage V18 in soybean" RELATED [SOY:0000033]
synonym: "V19 in maize" RELATED [MaizeGDB:67360]
is_a: PO:0007133 ! leaf production

[Term]
id: PO:0007121
name: 6.01 10% of flowers open
namespace: plant_growth_and_development_stage
def: "OBSOLETE" [GR:ap]
is_obsolete: true

[Term]
id: PO:0007122
name: 2.07 main shoot and axillary shoots visible at seven nodes
namespace: plant_growth_and_development_stage
def: "The stage at which main shoot and axillary shoots at seven nodes are visible." [GR:ap]
comment: The axillary shoot can be a single shoot or a pair of axillary shoots at each node.
synonym: "2.07 Main shoot and axillary shoots visible at 7 nodes in soybean" RELATED [SOY:0000046]
synonym: "2.07 main shoot and axillary shoots visible at seven nodes in Solanaceae" RELATED [SGN:0000029]
synonym: "3.08-main shoot and seven tillers" RELATED [GRO:0007077]
synonym: "BBCH growth stage 27" RELATED [ISBN:3826331524]
synonym: "main shoot and 7 tillers" RELATED []
synonym: "main shoot and seven tillers in barley" RELATED [GRO:0007077]
synonym: "main shoot and seven tillers in oat" RELATED [GRO:0007077]
synonym: "main shoot and seven tillers in wheat" RELATED [GRO:0007077]
synonym: "main shoot and seventh tiller visible" RELATED []
synonym: "seventh axillary shoot detectable" RELATED []
synonym: "seventh tiller detectable" RELATED []
synonym: "Zadok scale-27" RELATED [GRO:0007077]
is_a: PO:0007073 ! 2 formation of axillary shoot

[Term]
id: PO:0007123
name: LP.06 six leaves visible
namespace: plant_growth_and_development_stage
def: "The stage at which leaves at six nodes, other than the cotyledonary node, are visible above ground." [GR:ap]
comment: The leaves can be a single leaf, two, or whorls of leaves at each node.
synonym: "03-tillering stage in rice" RELATED [GRO:0007049]
synonym: "1.06 5th trifoliolate leaf unfolded in soybean" RELATED [SOY:0000020]
synonym: "2 tassel initiation/early whorl stage in maize" RELATED [MaizeGDB:67306]
synonym: "2.07-six leaves unfolded in Triticeae" RELATED [GRO:0007065]
synonym: "3.01-ear initiation in maize" RELATED [GRO:0007013]
synonym: "3.1 ear initiation/mid-whorl stage in maize" RELATED [MaizeGDB:67356]
synonym: "6 leaves unfolded" RELATED []
synonym: "6 rosette leaf in Arabidopsis" RELATED [TAIR:0000409]
synonym: "6-8 leaves in maize" RELATED [MaizeGDB:67356]
synonym: "6-leaf in maize" RELATED [MaizeGDB:67356]
synonym: "BBCH growth stage 16" RELATED [ISBN:3826331524]
synonym: "ear initiation in maize" RELATED [MaizeGDB:67356]
synonym: "early whorl stage in maize" RELATED [MaizeGDB:67306]
synonym: "LP.06 six leaves visible in Solanaceae" RELATED [SGN:0000018]
synonym: "maize growth stage-3.1" RELATED [GRO:0007012]
synonym: "mid-whorl stage in maize" RELATED [MaizeGDB:67356]
synonym: "rice growth stage-3" RELATED [GRO:0007049]
synonym: "six leaves unfolded (sensu Triticeae)" RELATED [GRO:0007065]
synonym: "six rosette leaves" RELATED []
synonym: "sixth leaf unfolded" RELATED []
synonym: "Stage V5 in soybean" RELATED [SOY:0000020]
synonym: "V6 in maize" RELATED [MaizeGDB:67306]
synonym: "Zadok scale-16, Haun scale-5.+" RELATED [GRO:0007065]
is_a: PO:0007133 ! leaf production

[Term]
id: PO:0007124
name: 6.03 30% of flowers open
namespace: plant_growth_and_development_stage
def: "OBSOLETE" [GR:ap]
is_obsolete: true

[Term]
id: PO:0007125
name: 6.04 40% of flowers open
namespace: plant_growth_and_development_stage
def: "OBSOLETE" [GR:ap]
is_obsolete: true

[Term]
id: PO:0007126
name: 7.02 fruit size 20%
namespace: plant_growth_and_development_stage
def: "OBSOLETE" [GR:ap]
is_obsolete: true

[Term]
id: PO:0007127
name: 7.04 fruit size 40%
namespace: plant_growth_and_development_stage
def: "OBSOLETE" [GR:ap]
synonym: "7.2 milk stage/embryo 2 in maize" RELATED [MaizeGDB:67373]
is_obsolete: true

[Term]
id: PO:0007128
name: 7.06 fruit size 60%
namespace: plant_growth_and_development_stage
def: "OBSOLETE" [GR:ap]
is_obsolete: true

[Term]
id: PO:0007129
name: 7.08 fruit size 80%
namespace: plant_growth_and_development_stage
def: "OBSOLETE" [GR:ap]
is_obsolete: true

[Term]
id: PO:0007130
name: B reproductive growth
namespace: plant_growth_and_development_stage
def: "Stage of growth when reproductive structures are being produced." [Poc:curators]
synonym: "B reproductive growth in Solanaceae" RELATED [SGN:0000032]
synonym: "B-reproductive stage in rice" RELATED [GRO:0007140]
synonym: "reproductive in Arabidopsis" RELATED [TAIR:0000306]
is_a: PO:0007033 ! whole plant growth stages

[Term]
id: PO:0007131
name: seedling growth
namespace: plant_growth_and_development_stage
def: "Growth of embryo after imbibition up to the development of the first adult leaves." [Poc:curators]
synonym: "seedling growth in Solanaceae" RELATED [SGN:0000005]
synonym: "seedling in Arabidopsis" RELATED [TAIR:0000027]
relationship: part_of PO:0007057 ! 0 germination

[Term]
id: PO:0007132
name: D dormancy
namespace: plant_growth_and_development_stage
def: "A suspension of physiological activity that can be reactivated once it is broken." [Poc:curators]
synonym: "10.05-seed dormant in barley" RELATED [GRO:0007119]
synonym: "10.05-seed dormant in oat" RELATED [GRO:0007119]
synonym: "10.05-seed dormant in Triticeae" RELATED [GRO:0007119]
synonym: "10.05-seed dormant in wheat" RELATED [GRO:0007119]
synonym: "10.06-viable seed germination in barley" RELATED [GRO:0007120]
synonym: "10.06-viable seed germination in oat" RELATED [GRO:0007120]
synonym: "10.06-viable seed germination in Triticeae" RELATED [GRO:0007120]
synonym: "10.06-viable seed germination in wheat" RELATED [GRO:0007120]
synonym: "10.07-seed not dormant in barley" RELATED [GRO:0007121]
synonym: "10.07-seed not dormant in oat" RELATED [GRO:0007121]
synonym: "10.07-seed not dormant in Triticeae" RELATED [GRO:0007121]
synonym: "10.07-seed not dormant in wheat" RELATED [GRO:0007121]
synonym: "10.08-secondary dormancy induced in barley" RELATED [GRO:0007122]
synonym: "10.08-secondary dormancy induced in oat" RELATED [GRO:0007122]
synonym: "10.08-secondary dormancy induced in Triticeae" RELATED [GRO:0007122]
synonym: "10.08-secondary dormancy induced in wheat" RELATED [GRO:0007122]
synonym: "10.09-secondary dormancy lost in barley" RELATED [GRO:0007123]
synonym: "10.09-secondary dormancy lost in oat" RELATED [GRO:0007123]
synonym: "10.09-secondary dormancy lost in Triticeae" RELATED [GRO:0007123]
synonym: "10.09-secondary dormancy lost in wheat" RELATED [GRO:0007123]
synonym: "D dormancy in Solanaceae" RELATED [SGN:0000053]
is_a: PO:0007033 ! whole plant growth stages

[Term]
id: PO:0007133
name: leaf production
namespace: plant_growth_and_development_stage
def: "The stage at which the leaves produced by SAM are visible above the ground in a seedling or mature plant." [Poc:curators]
comment: This stage is recommended over rosette growth or stem elongation as it is most easily observed and least ambiguous.
synonym: "leaf production in Solanaceae" RELATED [SGN:0000012]
is_a: PO:0007112 ! 1 main shoot growth

[Term]
id: PO:0007134
name: A vegetative growth
namespace: plant_growth_and_development_stage
def: "Stage of growth when vegetative structures are being produced." [Poc:curators]
synonym: "A vegetative growth in Solanaceae" RELATED [SGN:0000002]
synonym: "A-vegetative stage in rice" RELATED [GRO:0007139]
synonym: "vegetative in Arabidopsis" RELATED [TAIR:0000305]
is_a: PO:0007033 ! whole plant growth stages

[Term]
id: PO:0007135
name: 4 growth directionality
namespace: plant_growth_and_development_stage
def: "the stage involved in the directionality of expansion growth" [GR:cwt]
relationship: part_of PO:0007039 ! leaf trichome development stage

[Term]
id: PO:0007501
name: root cap formation
namespace: plant_growth_and_development_stage
def: "The stage at which the root cap becomes evident. " [GR:ap]
comment: The number and origin of root cap initials that form the root cap varies among species. The root cap initials become independent from the more internally located root meristem cells by an increase in the thickness of the cell wall that separates them
synonym: "root cap formation in crown root." RELATED []
synonym: "root cap formation in lateral root." RELATED []
synonym: "root cap formation in primary root." RELATED []
is_a: PO:0007525 ! 3 establishment of tissue systems

[Term]
id: PO:0007503
name: A2.1 root intials differntiation of primary roots
namespace: plant_growth_and_development_stage
def: "OBSOLETE. The root initials divide repeatedly and add more cells" [GR:ap]
comment: This  term has been obsoleted to keep the structure simple.
is_obsolete: true

[Term]
id: PO:0007504
name: crown root primordium formation
namespace: plant_growth_and_development_stage
def: "The stage at which the initial cells of crown root primordium are formed in  the innermost ground meristem cells by one or two periclinal divisions." [GR:ap]
comment: Crown root primordia formed endogenously opposite the collateral bundles in maize.
is_a: PO:0007505 ! 1 root primordium formation

[Term]
id: PO:0007505
name: 1 root primordium formation
namespace: plant_growth_and_development_stage
def: "The stage at which root primordium originates and develops at specific locations in embryonic and post embryonic roots." [GR:ap]
is_a: PO:0007520 ! root development stages

[Term]
id: PO:0007506
name: primary root primordium formation
namespace: plant_growth_and_development_stage
def: "The stage at which a group of cells or initials that will differentiate into the primary root become organized in the embryo ." [GR:ap]
is_a: PO:0007505 ! 1 root primordium formation

[Term]
id: PO:0007509
name: root vascular cylinder differentiation
namespace: plant_growth_and_development_stage
def: "The stage at which the root vascular cylinder becomes evident." [GR:ap]
comment: The first identifiable region in the differentiating vascular cylinder is the pericycle. In the xylem the differentiation of the tracheary elements begins in a centrifugal direction but is completed in the centripetal direction. The first phloem elements mature before the first xylem elements.
is_a: PO:0007525 ! 3 establishment of tissue systems

[Term]
id: PO:0007510
name: root emergence
namespace: plant_growth_and_development_stage
def: "The stage at which the fully formed root emerges." [GR:ap]
is_a: PO:0001031 ! 4 root elongation

[Term]
id: PO:0007511
name: lateral root primordium formation
namespace: plant_growth_and_development_stage
def: "This stage at which the transverse divisions in pericycle cells form the initials of the lateral root primordium." [GR:ap]
is_a: PO:0007505 ! 1 root primordium formation

[Term]
id: PO:0007512
name: A2 root initials differentiation stage
namespace: plant_growth_and_development_stage
def: "OBSOLETE. The root initials differentiate by cell division and cell expansion. " [GR:ap]
comment: Crown root stages are based on rice plant. This  term has been obsoleted to keep the structure simple.
is_obsolete: true

[Term]
id: PO:0007513
name: root cortex differentiation
namespace: plant_growth_and_development_stage
def: "The stage at which the root cortex becomes evident." [GR:ap]
comment: Repetitive periclinal divisions and radial enlargement of cells form the cortex layers, the innermost layers become the endodermis with the differentiation of casparian strips.
synonym: "cortex differentiation of crown root." RELATED []
synonym: "cortex differentiation of lateral root" RELATED []
synonym: "cortex differentiation of primary root." RELATED []
is_a: PO:0007525 ! 3 establishment of tissue systems

[Term]
id: PO:0007514
name: B3 crown root meristem formation
namespace: plant_growth_and_development_stage
def: "OBSOLETE. The stage at which the meristem of the crown root becomes evident." [GR:ap]
is_obsolete: true

[Term]
id: PO:0007516
name: root epidermal differentiation
namespace: plant_growth_and_development_stage
def: "The stage at which the root epidermis becomes evident." [GR:ap]
comment: Root hairs come to full development beyond the region of elongation zone, approximately at the level where the xylem begins to mature.
synonym: "epidermal differentiation of lateral root." RELATED []
synonym: "epidermal differentiation of primary root" RELATED []
synonym: "epidermial differentiation of crown root." RELATED []
is_a: PO:0007525 ! 3 establishment of tissue systems

[Term]
id: PO:0007517
name: lateral root emergence
namespace: plant_growth_and_development_stage
def: "The stage at which the lateral root emerges." [GR:ap]
comment: Starch grains can be seen in the root cap after emergence.
is_a: PO:0007510 ! root emergence

[Term]
id: PO:0007518
name: crown root emergence
namespace: plant_growth_and_development_stage
def: "The stage at which the crown root emerges." [GR:ap]
comment: Crown root stages are based on rice plant.
is_a: PO:0007510 ! root emergence

[Term]
id: PO:0007519
name: 5 root hair formation
namespace: plant_growth_and_development_stage
def: "The stage at which the root hairs becomes evident. " [GR:ap]
synonym: "Benfey's stage 3 of root development" RELATED []
is_a: PO:0007520 ! root development stages

[Term]
id: PO:0007520
name: root development stages
namespace: plant_growth_and_development_stage
alt_id: PO:0007011
def: "Stages of development of a root defined by characteristic morphological, structural, histological or other visible features. " [GR:ap]
comment: At present the stages are described for primary, lateral and crown roots and stages for adventitious root formed by wounding or hormone treatment is not described. Finer resolution of root stages has been kept in the obsolete node as they are not consistently used in the consulted literature. These terms will be reintroduced into the ontology when there is a specific user request.
synonym: "root development stage" RELATED []
is_a: PO:0007021 ! plant structure development stages

[Term]
id: PO:0007521
name: C3.1 metaxylem differentiation of root.
namespace: plant_growth_and_development_stage
def: "OBSOLETE. Differentiation begins with the enlargement and vacuolation of the tracheary elements of the metaxylem." [GR:ap]
comment: These stages are based on Arabidopsis plant. This  term has been obsoleted to keep the structure simple.
synonym: "metaxylem differentiation of crown root" RELATED []
synonym: "metaxylem differentiation of lateral root" RELATED []
synonym: "metaxylem differentiation of primary root" RELATED []
is_obsolete: true

[Term]
id: PO:0007523
name: establishment of initial cells
namespace: plant_growth_and_development_stage
def: "OBSOLETE. The root initial cells are established." [GR:ap]
is_obsolete: true

[Term]
id: PO:0007524
name: B1 primary root meristem formation
namespace: plant_growth_and_development_stage
def: "OBSOLETE. The stage at which the meristem of the primary root becomes evident." [GR:ap]
is_obsolete: true

[Term]
id: PO:0007525
name: 3 establishment of tissue systems
namespace: plant_growth_and_development_stage
def: "The stage at which distinct tissues become organized." [GR:ap]
synonym: "Benfey's stage 1 of root development" RELATED []
synonym: "cell differentiation stage of root development" RELATED []
synonym: "establishment of fundamental organization in adventitious root" RELATED []
synonym: "establishment of fundamental organization in primary root." RELATED []
synonym: "establishment of fundamental organization lateral root." RELATED []
is_a: PO:0007520 ! root development stages

[Term]
id: PO:0007526
name: F2 root hair elongation
namespace: plant_growth_and_development_stage
def: "OBSOLETE. The stage at which the root hairs are fully elongated." [GR:ap]
is_obsolete: true

[Term]
id: PO:0007527
name: 2 root meristem formation
namespace: plant_growth_and_development_stage
def: "The stage at which the root meristem becomes evident. " [GR:ap]
comment: Characteristic differences in meristem organization have been related to taxonomic groups. Terms for developmental zones formation are available in the oboslete node, and they will be reintroduced in the ontology when there is a specific user request for them.
is_a: PO:0007520 ! root development stages

[Term]
id: PO:0007528
name: A2.2 root initials differentiation of lateral roots
namespace: plant_growth_and_development_stage
def: "OBSOLETE. Radial expansion followed by subsequent periclinal divisions forms the pericycle-derived tissues." [GR:ap]
comment: This  term has been obsoleted to keep the structure simple.
is_obsolete: true

[Term]
id: PO:0007529
name: E emerged root elongation
namespace: plant_growth_and_development_stage
def: "OBSOLETE. The stage at which the emerged root starts to elongate. " [GR:ap]
synonym: "emerged crown root elongation" RELATED []
synonym: "emerged lateral root elongation" RELATED []
synonym: "emrged primary root elongation" RELATED []
is_obsolete: true

[Term]
id: PO:0007530
name: A2.3 founder cell derivatives of lateral root
namespace: plant_growth_and_development_stage
def: "OBSOLETE. Radial expansion followed by subsequent periclinal divisions forms the isodiametric founder cell tissues." [GR:ap]
comment: This  term has been obsoleted to keep the structure simple.
is_obsolete: true

[Term]
id: PO:0007531
name: F1 root hair initiation
namespace: plant_growth_and_development_stage
def: "OBSOLETE. The stage at which the roots hairs are initiated." [GR:ap]
is_obsolete: true

[Term]
id: PO:0007532
name: obsolete plant growth and development terms
namespace: plant_growth_and_development_stage
is_obsolete: true

[Term]
id: PO:0007533
name: C3.3 maturation of protoxylem elements in root.
namespace: plant_growth_and_development_stage
def: "OBSOLETE. The first protoxylem elements next to the pericycle develop secondary walls and mature." [GR:ap]
comment: This  term has been obsoleted to keep the structure simple.
synonym: "maturation of protoxylem elements in crown root" RELATED []
synonym: "maturation of protoxylem elements in lateral root" RELATED []
synonym: "maturation of protoxylem elements in primary root" RELATED []
is_obsolete: true

[Term]
id: PO:0007534
name: A2.4 root initials differentiation of crown roots
namespace: plant_growth_and_development_stage
def: "OBSOLETE. Initial cells of crown root primordium divide anticlinally and periclinally to form epidermis-endodermis initial, vascular-cylinder initial and root cap initial." [GR:ap]
comment: Crown root stages are based on rice plant. This  term has been obsoleted to keep the structure simple.
is_obsolete: true

[Term]
id: PO:0007535
name: A1 root initials formation stage
namespace: plant_growth_and_development_stage
def: "OBSOLETE. After the formation of the apical-basal axis in the young embryo, the central and basal portion give rise to the root meristem. " [GR:ap]
comment: Endogenously formed embryonic roots are exclusive to Poaceae.\nThis  term has been obsoleted to keep the structure simple.
is_obsolete: true

[Term]
id: PO:0007536
name: root primordium visible
namespace: plant_growth_and_development_stage
def: "OBSOLETE. the root primordium is visbile" [GR:ap]
is_obsolete: true

[Term]
id: PO:0007537
name: C3.2 maturation of phloem elements in root.
namespace: plant_growth_and_development_stage
def: "OBSOLETE. The first phloem elements matures." [GR:ap]
comment: This  term has been obsoleted to keep the structure simple.
synonym: "maturation phloem elements of crown root." RELATED []
synonym: "maturation phloem elements of lateral root." RELATED []
synonym: "maturation phloem elements of primary root." RELATED []
is_obsolete: true

[Term]
id: PO:0007539
name: B2 lateral root meristem formation
namespace: plant_growth_and_development_stage
def: "OBSOLETE. The stage at which the meristem of the lateral root becomes evident." [GR:ap]
is_obsolete: true

[Term]
id: PO:0007600
name: 3 floral organ development stages
namespace: plant_growth_and_development_stage
def: "Stages of development of floral organs defined by characteristic morphological, structural, histological or other visible features. " [POC:curators]
is_a: PO:0007615 ! flower development stages

[Term]
id: PO:0007601
name: 1 floral meristem visible
namespace: plant_growth_and_development_stage
def: "Stage of flower development marked by the emergence of the floral meristem on the flank of the inflorescence meristem." [POC:curators]
synonym: "stage 1 flower in Arabidopsis" RELATED []
is_a: PO:0007615 ! flower development stages

[Term]
id: PO:0007602
name: 2 floral meristem notched
namespace: plant_growth_and_development_stage
def: "Stage of floral development that begins when the floral meristem becomes demarcated from the inflorescence meristem by a slight indentation." [POC:curators]
synonym: "stage 2 flower in Arabidopsis" RELATED []
is_a: PO:0007615 ! flower development stages

[Term]
id: PO:0007603
name: calyx developmental stages
namespace: plant_growth_and_development_stage
def: "Stages of development of the calyx defined by characteristic morphological, structural, histological or other visible features." [POC:curators]
is_a: PO:0007600 ! 3 floral organ development stages

[Term]
id: PO:0007604
name: corolla developmental stages
namespace: plant_growth_and_development_stage
def: "Stages of development of the corolla defined by characteristic morphological, structural, histological or other visible features." [POC:curators]
is_a: PO:0007600 ! 3 floral organ development stages

[Term]
id: PO:0007605
name: androecium developmental stages
namespace: plant_growth_and_development_stage
def: "Stages of development of the androecium defined by characteristic morphological, structural, histological or other visible features." [POC:curators]
is_a: PO:0007600 ! 3 floral organ development stages

[Term]
id: PO:0007606
name: gynoecium developmental stages
namespace: plant_growth_and_development_stage
def: "Stages of development of the gynoecium defined by characteristic morphological, structural, histological or other visible features." [POC:curators]
is_a: PO:0007600 ! 3 floral organ development stages

[Term]
id: PO:0007607
name: sepal primordium visible
namespace: plant_growth_and_development_stage
def: "Stage of calyx development that begins when the sepal primordia arise." [POC:curators]
synonym: "stage 3 flower in Arabidopsis" RELATED []
is_a: PO:0007603 ! calyx developmental stages

[Term]
id: PO:0007608
name: petal primordium visible
namespace: plant_growth_and_development_stage
def: "Stage of corolla development that begins when the petal or petal-stamen primordia arise." [POC:curators]
synonym: "stage 5 flower in Arabidopsis" RELATED []
is_a: PO:0007604 ! corolla developmental stages

[Term]
id: PO:0007609
name: sepals 50% of final size
namespace: plant_growth_and_development_stage
def: "OBSOLETE. 50% of the absolute size of the sepals." [POC:curators]
is_obsolete: true

[Term]
id: PO:0007610
name: sepals 100% of final size
namespace: plant_growth_and_development_stage
def: "OBSOLETE. 100% of the absolute size of the sepals." [POC:curators]
is_obsolete: true

[Term]
id: PO:0007611
name: petal differentiation and expansion stage
namespace: plant_growth_and_development_stage
def: "Stage of corolla development defined by differentiation and expansion of petal." [POC:fz]
synonym: "stage 10 flower in Arabidopsis" RELATED []
synonym: "stage 12 flower in Arabidopsis" RELATED []
synonym: "stage 9 flower in Arabidopsis" RELATED []
is_a: PO:0007604 ! corolla developmental stages

[Term]
id: PO:0007612
name: fully expanded petal
namespace: plant_growth_and_development_stage
def: "Stage of corolla development when petal is fully expanded." [POC:fz]
is_a: PO:0007604 ! corolla developmental stages

[Term]
id: PO:0007613
name: stamen primordium visible
namespace: plant_growth_and_development_stage
def: "Stage of androecium development that begins when the stamens or petal-stamen primordia arise." [POC:curators]
synonym: "stage 7 flower in Arabidopsis" RELATED []
is_a: PO:0007605 ! androecium developmental stages

[Term]
id: PO:0007615
name: flower development stages
namespace: plant_growth_and_development_stage
def: "Stages of development of a flower defined by characteristic morphological, structural, histological or other visible features. " [POC:curators]
synonym: "flower development in Arabidopsis" RELATED []
is_a: PO:0007021 ! plant structure development stages

[Term]
id: PO:0007616
name: 4 anthesis
namespace: plant_growth_and_development_stage
def: "The phase of a flower when pollen is presented and/or the stigma is receptive." [APWeb:glossary]
synonym: "stage 13 flower in Arabidopsis" RELATED []
synonym: "stage 14 flower in Arabidopsis" RELATED []
synonym: "stage 15 flower in Arabidopsis" RELATED []
is_a: PO:0007615 ! flower development stages

[Term]
id: PO:0007617
name: 5 post anthesis
namespace: plant_growth_and_development_stage
def: "The phase of a flower after the pollen is presented and/or the stigma is receptive." [POC:curators]
synonym: "stage 16 flower in Arabidopsis" RELATED []
is_a: PO:0007615 ! flower development stages

[Term]
id: PO:0007618
name: carpel primordium visible
namespace: plant_growth_and_development_stage
def: "Stage of gynoecium development that begins when the carpel primordia arise." [POC:curators]
is_a: PO:0007606 ! gynoecium developmental stages

[Term]
id: PO:0007619
name: ovule developmental stages
namespace: plant_growth_and_development_stage
def: "Stages of development of the ovule defined by characteristic morphological, structural, histological or other visible features." [POC:curators]
synonym: "ovule development in Arabidopsis" RELATED []
is_a: PO:0007606 ! gynoecium developmental stages

[Term]
id: PO:0007620
name: ovule primordium visible
namespace: plant_growth_and_development_stage
def: "Stage of ovule development that begins when the ovule primordia arise." [POC:curators]
synonym: "ovule stage 1-I in Arabidopsis" RELATED []
is_a: PO:0007619 ! ovule developmental stages

[Term]
id: PO:0007621
name: megagametophyte developmental stages
namespace: plant_growth_and_development_stage
def: "Stages of development of the megagametophyte." [POC:curators]
comment: Although megaspore and megagametophyte development are normally separate, one spore producing one gametophyte, in some flowering plants a single gametophyte may be produced from two or four spores.
is_a: PO:0007619 ! ovule developmental stages

[Term]
id: PO:0007622
name: integument initiation stage
namespace: plant_growth_and_development_stage
def: "Stage of ovule development that begins when the integument primordia are visible." [POC:curators]
synonym: "ovule stage 2-II in Arabidopsis" RELATED []
synonym: "ovule stage 2-III in Arabidopsis" RELATED []
is_a: PO:0004504 ! ovule differentiation and expansion

[Term]
id: PO:0007623
name: A megaspore mother cell enlarges
namespace: plant_growth_and_development_stage
def: "The stage of megagametophyte development when the megaspore mother cell enlarges." [POC:curators]
synonym: "ovule stage 2-I in Arabidopsis" RELATED []
is_a: PO:0007621 ! megagametophyte developmental stages

[Term]
id: PO:0007624
name: B meiosis of megaspore mother cell
namespace: plant_growth_and_development_stage
def: "The stage of megagametophyte development when the megaspore mother cell undergoes meiosis." [POC:curators]
synonym: "ovule stage 2-IV in Arabidopsis" RELATED []
is_a: PO:0007621 ! megagametophyte developmental stages

[Term]
id: PO:0007625
name: C tetrad of megaspores
namespace: plant_growth_and_development_stage
def: "The product of meiosis of the megaspore mother cell." [POC:curators]
synonym: "ovule stage 2-V in Arabidopsis" RELATED []
is_a: PO:0007621 ! megagametophyte developmental stages

[Term]
id: PO:0007626
name: D megaspore degeneration
namespace: plant_growth_and_development_stage
def: "The stage of megagametophyte development when non-functional megaspores degenerate." [POC:curators]
comment: In some plants more than one megaspore contributes to the megametophyte.
synonym: "ovule stage 3-I in Arabidopsis" RELATED []
is_a: PO:0007621 ! megagametophyte developmental stages

[Term]
id: PO:0007627
name: E two nucleate megagametophyte
namespace: plant_growth_and_development_stage
def: "The stage of megagametophyte development when there are two nuclei." [POC:curators]
synonym: "ovule stage 3-II in Arabidopsis" RELATED []
is_a: PO:0007621 ! megagametophyte developmental stages

[Term]
id: PO:0007628
name: F four nucleate megagametophyte
namespace: plant_growth_and_development_stage
def: "The stage of megagametophyte development when there are four nuclei." [POC:curators]
synonym: "ovule stage 3-IV in Arabidopsis" RELATED []
is_a: PO:0007621 ! megagametophyte developmental stages

[Term]
id: PO:0007629
name: G eight nucleate megagametophyte
namespace: plant_growth_and_development_stage
def: "The stage of megagametophyte development when there are eight nuclei." [POC:curators]
comment: Some plants do not form an eight nucleate megametophyte.
synonym: "ovule stage 3-V in Arabidopsis" RELATED []
is_a: PO:0007621 ! megagametophyte developmental stages

[Term]
id: PO:0007631
name: embryo development stages
namespace: plant_growth_and_development_stage
alt_id: PO:0007020
def: "Stages of development of the embryo." [TAIR:ki]
synonym: "embryo development stage" RELATED []
synonym: "embryonic in Arabidopsis" RELATED []
is_a: PO:0001170 ! seed development stages

[Term]
id: PO:0007632
name: seed maturation stage
namespace: plant_growth_and_development_stage
def: "Stage during which the seed storage products (storage proteins, lipids and starch) are being accumulated, either in the cotyledons or in the endosperm. Also, LEA proteins are accumulated and subsequentially, desiccation tolerant state is reached at the end of this stage." [TAIR:ki]
synonym: "seed maturation in Arabidopsis" RELATED []
is_a: PO:0001170 ! seed development stages

[Term]
id: PO:0007633
name: endosperm development stages
namespace: plant_growth_and_development_stage
def: "Stages of development of the endosperm." [TAIR:ki]
is_a: PO:0001170 ! seed development stages

[Term]
id: PO:0009012
name: plant growth and development stages
namespace: plant_growth_and_development_stage
def: "The succession of changes leading from the zygote to the mature plant. " [Poc:curators]
synonym: "Arabidopsis growth" RELATED [TAIR:0000205]

[Term]
id: PO:0009075
name: plant ontology
namespace: plant_structure
def: "OBSOLETE. A controlled vocabulary to describe the various plant parts and the growth and developmental stages." [Poc:curators]
is_obsolete: true

[Term]
id: PO:0021002
name: calyx absolute size
namespace: plant_growth_and_development_stage
def: "OBSOLETE. The proportion of the absolute size reached by the calyx" [POC:curators]
is_obsolete: true

[Term]
id: PO:0021003
name: calyx relationship
namespace: plant_growth_and_development_stage
def: "OBSOLETE. The stages of development of the calyx with respect to the rest of the bud" [POC:curators]
is_obsolete: true

[Term]
id: PO:0021004
name: inflorescence initiation stage
namespace: plant_growth_and_development_stage
def: "Stage of inflorescence development marked by the formation of the inflorescence meristem on a vegetative branch." [POC:fz]
is_a: PO:0001083 ! inflorescence development stages

[Typedef]
id: part_of
name: part of

