format-version: 1.0
version: $Revision: 1.27 $
date: 20:07:2006 16:31
saved-by: Pankaj Jaiswal
auto-generated-by: DAG-Edit 1.419 rev 3
default-namespace: plant_ontology
subsetdef: Rice "Term used for rice"
subsetdef: Maize "Term used for maize"
subsetdef: Tomato "Term used for tomato"
subsetdef: Citrus "Term used for citrus"
subsetdef: Arabidopsis "Term used for Arabidopsis"
subsetdef: Poaceae "Term used for grasses"
subsetdef: reference "reference plant structure term"

[Term]
id: PO:0000001
name: embryo proper
namespace: plant_structure
def: "The body of the developing embryo attached to the maternal tissue in the ovule by filamentous suspensor." [TAIR:ki]
relationship: part_of PO:0009009 ! embryo

[Term]
id: PO:0000002
name: anther wall
namespace: plant_structure
def: "A multicellular layer with outer epidermis and an inner endothecium." [GR:pj]
subset: reference
relationship: part_of PO:0009070 ! microsporangium

[Term]
id: PO:0000003
name: whole plant
namespace: plant_structure
def: "The entire plant\, including roots\, shoots and leaves\, at any stage of its life cycle." [TAIR:ki]
comment: This term is so general that it should be avoided whenever possible.
subset: reference
is_a: PO:0009011 ! plant structure

[Term]
id: PO:0000004
name: in vitro cultured  cell, tissue and organ
namespace: plant_structure
def: "Isolated and grown plant protoplast\, cell\, tissue and organ\, involving\, as a common factor\, growth of microbe-free plant material in sterile environment\, such as sterilized nutrient medium in a test tube or petri dish." [TAIR:ki]
is_a: PO:0009011 ! plant structure

[Term]
id: PO:0000005
name: cultured cell
namespace: plant_structure
def: "In vitro grown isolated cells and small cell aggregates that proliferate while suspended in liquid sterile medium or spread on a solid agar medium." [TAIR:ki]
comment: In cell cultures\, the cells are no longer organized into tissues.
synonym: "cell suspension" []
is_a: PO:0000004 ! in vitro cultured  cell, tissue and organ
is_a: PO:0009002 ! plant cell

[Term]
id: PO:0000006
name: cultured protoplast
namespace: plant_structure
def: "In vitro isolated cells from which the entire cell wall has been enzymatically removed." [TAIR:ki]
is_a: PO:0000005 ! cultured cell

[Term]
id: PO:0000007
name: cultured leaf cell
namespace: plant_structure
def: "In vitro grown isolated cells and small cell aggregates that originated from isolated leaf protoplasts (after they re-established cell wall\, or from callus that was induced from leaf tissue)." [TAIR:ki]
is_a: PO:0000005 ! cultured cell

[Term]
id: PO:0000008
name: cultured root cell
namespace: plant_structure
def: "In vitro grown isolated cells and small cell aggregates that originated from isolated protoplasts after they re-established cell wall\, or from callus that was induced from segment of root." [TAIR:ki]
is_a: PO:0000005 ! cultured cell

[Term]
id: PO:0000009
name: cultured callus
namespace: plant_structure
def: "In vitro grown cell aggregates that originated from isolated protoplasts\, cell suspensions\, or from callus that was induced in sterile medium supplemented by plant growth regulators." [TAIR:ki]
is_a: PO:0000004 ! in vitro cultured  cell, tissue and organ
is_a: PO:0005052 ! callus

[Term]
id: PO:0000010
name: cultured embryo
namespace: plant_structure
def: "In vitro isolated and maintained mature or immature zygotic embryos\, somatic embryos or haploid embryos (derived from male gametophyte)." [TAIR:ki]
is_a: PO:0000004 ! in vitro cultured  cell, tissue and organ

[Term]
id: PO:0000011
name: somatic embryo
namespace: plant_structure
def: "An embryo arising from previously differentiated somatic cells in vitro\, rather than from fused haploid gametes\, i.e.\, zygote." [TAIR:ki]
is_a: PO:0000010 ! cultured embryo
relationship: develops_from PO:0006091 ! embryogenic callus

[Term]
id: PO:0000012
name: apical hook
namespace: plant_structure
def: "Hook-like structure which develops at the apical part of the hypocotyl in dark-grown seedlings in dicots. " [TAIR:ki]
subset: reference
synonym: "hypocotyl hook" []
relationship: develops_from PO:0020100 ! hypocotyl
relationship: part_of PO:0006341 ! primary shoot

[Term]
id: PO:0000013
name: cauline leaf
namespace: plant_structure
def: "Leaf or pairs/whorls of leaves borne on the stem. " [TAIR:ki]
comment: In Arabidopsis\, refers to the leaves that are borne on the elongated inflorescence branches.
is_a: PO:0009025 ! leaf

[Term]
id: PO:0000014
name: rosette leaf
namespace: plant_structure
def: "One of multiple leaves borne in a rosette - a group of leaves\, generally borne at the base of the plant\, that are separated by very short internodes." [TAIR:ki]
comment: n Arabidopsis\, vegetative development is characterized by the production of the rosette leaves.
is_a: PO:0009025 ! leaf

[Term]
id: PO:0000015
name: cotyledon primordium
namespace: plant_structure
def: "An organized group of cells that will differentiate into a cotyledon. " [TAIR:ki]
is_a: PO:0020030 ! cotyledon

[Term]
id: PO:0000016
name: lateral root primordium
namespace: plant_structure
def: "An organized group of cells derived from the root pericycle that will differentiate into a new root. " [TAIR:ki]
is_a: PO:0020121 ! lateral root

[Term]
id: PO:0000017
name: leaf primordium
namespace: plant_structure
def: "An organized group of cells that will differentiate into leaf that are emerging as an outgrowth in the shoot apex (flanking the meristem). " [TAIR:ki]
is_a: PO:0009025 ! leaf
relationship: part_of PO:0000037 ! shoot apex

[Term]
id: PO:0000018
name: ovule primordium
namespace: plant_structure
def: "An organized group of cells that will differentiate into ovule. " [TAIR:ki]
is_a: PO:0020003 ! ovule

[Term]
id: PO:0000019
name: gynoecium primordium
namespace: plant_structure
def: "The very first appearance of gynoecium. " [TAIR:ki]
is_a: PO:0009062 ! gynoecium

[Term]
id: PO:0000020
name: starch sheath cell
namespace: plant_structure
def: "OBSOLETE. Cells characterized by conspicuous and rather stable accumulation of starch." [ISBN:044174520]
comment: Uninformative definition
is_obsolete: true

[Term]
id: PO:0000021
name: petal primordium
namespace: plant_structure
def: "The very first appearance of a petal. " [TAIR:ki]
is_a: PO:0009032 ! petal

[Term]
id: PO:0000022
name: cuticle
namespace: plant_structure
def: "A layer of fatty material\, cutin\, rather impervious to water\, located on the outer walls of epidermal cells." [ISBN:0471245208]
is_a: PO:0004013 ! epidermal cell

[Term]
id: PO:0000023
name: casparian strip
namespace: plant_structure
def: "OBSOLETE\: A band-like wall formation within primary walls that contains suberin and lignin; typical of endodermal cells in roots\, in which it occurs in radial and transverse anticlinal walls." [ISBN:0471245208]
comment: Comment\: this term is available in the Cellular Component aspect of the Gene Ontology (GO\:0048226).
is_obsolete: true

[Term]
id: PO:0000024
name: filiform apparatus
namespace: plant_structure
def: "A complex of cell wall invaginations in a synergid cell similar to those in transfer cells." [ISBN:0471245208]
subset: reference
relationship: part_of PO:0000191 ! synergid

[Term]
id: PO:0000025
name: root tip
namespace: plant_structure
def: "The portion of the root including the meristem and root cap." [TAIR:ki]
relationship: part_of PO:0009005 ! root

[Term]
id: PO:0000026
name: primary root tip
namespace: plant_structure
def: "The portion of the primary root including the meristem and root cap." [TAIR:ki]
is_a: PO:0000025 ! root tip
relationship: part_of PO:0020127 ! primary root

[Term]
id: PO:0000027
name: lateral root tip
namespace: plant_structure
def: "The portion of the lateral root including the meristem and root cap." [TAIR:ki]
is_a: PO:0000025 ! root tip
relationship: part_of PO:0020121 ! lateral root

[Term]
id: PO:0000028
name: pollen tube tip
namespace: plant_structure
def: "Tip portion of the pollen tube that is rapidly growing." [TAIR:ki]
is_a: PO:0006345 ! pollen tube

[Term]
id: PO:0000029
name: root hair tip
namespace: plant_structure
def: "Tip portion of an outgrowth of a root epidermal cell." [TAIR:ki]
relationship: part_of PO:0000256 ! root hair

[Term]
id: PO:0000030
name: septum
namespace: plant_structure
def: "A thin partition or membrane that divides a cavity or a mass of tissue\, e.g.\, in anther\, ovary or fruit." [APWeb:Glossary]
subset: Arabidopsis
relationship: part_of PO:0009001 ! fruit
relationship: part_of PO:0009030 ! carpel
relationship: part_of PO:0009066 ! anther

[Term]
id: PO:0000031
name: lenticel
namespace: plant_structure
def: "Loosely-packed mass of cork cells occurring especially in the young stem\, bark or even leaf of a plant\, visible on the surface as a raised\, often powdery-appearing spot\, through which gaseous exchange occurs." [ISBN: 0471245208]
relationship: part_of PO:0009047 ! stem

[Term]
id: PO:0000032
name: tetrad of microspores
namespace: plant_structure
def: "A group of four haploid cells that remained joined together shortly after meiosis. Each cell will give rise to the male gametophyte." [TAIR:ki]
subset: reference
relationship: develops_from PO:0020047 ! microsporocyte

[Term]
id: PO:0000033
name: valve
namespace: plant_structure
def: "Portion of an organ that is fragmented; in capsule\, the portions into which the pericarp splits at maturity." [APWeb:Glossary]
subset: Arabidopsis
relationship: part_of PO:0009001 ! fruit

[Term]
id: PO:0000034
name: vascular system
namespace: plant_structure
def: "Total of the vascular tissues in their specific arrangement in a plant or plant organ." [ISBN:0471245208]
is_a: PO:0009007 ! tissue

[Term]
id: PO:0000035
name: cotyledon vascular system
namespace: plant_structure
def: "Vascular system of the cotyledon." [TAIR:ki]
is_a: PO:0000034 ! vascular system
relationship: part_of PO:0020030 ! cotyledon

[Term]
id: PO:0000036
name: leaf vascular system
namespace: plant_structure
def: "Vascular system of the leaf." [TAIR:ki]
is_a: PO:0000034 ! vascular system
relationship: part_of PO:0009025 ! leaf

[Term]
id: PO:0000037
name: shoot apex
namespace: plant_structure
def: "The topmost part of the shoot\, situated at the distal extremity of the shoot axis\, consists of apical meristem and the youngest leaf primordia." [TAIR:ki]
subset: reference
relationship: part_of PO:0009006 ! shoot

[Term]
id: PO:0000038
name: primary endosperm cell
namespace: plant_structure
def: "Cell produced by the fusion of sperm cell nucleus and two polar nuclei of the central cell (or diploid secondary endosperm nucleus\, in cases where two polar nuclei fuse together before double fertilization). The first cell of the endosperm\, often tripoid." [TAIR:ki]
is_a: PO:0009002 ! plant cell
relationship: part_of PO:0009089 ! endosperm

[Term]
id: PO:0000039
name: stem vascular system
namespace: plant_structure
def: "Vascular tissues in their specific arrangements in the stem" [TAIR:ki]
is_a: PO:0000034 ! vascular system
relationship: part_of PO:0009047 ! stem

[Term]
id: PO:0000040
name: adventitious root nodule
namespace: plant_structure
def: "Enlargement or swelling at position of dormant adventitious root primordium (on the stem)\, inhabited by nitrogen-fixing bacteria. " [TAIR:ki]
comment: Unlike the root nodules\, these contain functioning chloroplasts in the nodule cortex and are therefore capable of carbon fixation. Note\: stem nodule is commonly used term for this structure\, although the nodules are formed at positions of dormant adventitious root primordia.
synonym: "stem primordium" []
is_a: PO:0003023 ! root nodule
relationship: part_of PO:0000042 ! shoot borne root

[Term]
id: PO:0000041
name: epidermal cork cell
namespace: plant_structure
def: "One of the two types of short cells in the epidermis of grasses and bamboos. It is usually paired with silica cell." [TAIR:ki]
comment: Developmentally different from periderm cork cell (i.e.\, phellem)\, produced by cork cambium.\n
is_a: PO:0004718 ! short cell

[Term]
id: PO:0000042
name: shoot borne root
alt_id: PO:0003007
alt_id: PO:0020129
namespace: plant_structure
def: "Post-embryonic root developed from shoot tissue." [TAIR:ki, GR:pj]
subset: reference
synonym: "adventitious root" []
synonym: "stilt root" []
is_a: PO:0009005 ! root

[Term]
id: PO:0000043
name: crown root
namespace: plant_structure
def: "Adventitious root formed at the base of the growing stem (known as a crown)." [TAIR:ki]
subset: reference
is_a: PO:0003005 ! nodal root

[Term]
id: PO:0000044
name: prop root
namespace: plant_structure
def: "Adventitious root formed at stem nodes above the ground and growing directly into the soil." [TAIR:ki]
comment: This term is perhaps best defined functionally to prop the plant up.
subset: reference
synonym: "brace root" []
is_a: PO:0003005 ! nodal root

[Term]
id: PO:0000045
name: embryonic root
namespace: plant_structure
def: "Root that is initiated in developing embryo." [TAIR:ki]
subset: reference
is_a: PO:0009005 ! root
relationship: part_of PO:0009009 ! embryo

[Term]
id: PO:0000046
name: seminal root
namespace: plant_structure
def: "Root formed within the scutelar node of the embryo in some monocotyledonous plants." [TAIR:ki]
subset: reference
synonym: "lateral seminal root" []
synonym: "scutellar nodal root" []
synonym: "secondary root" []
is_a: PO:0000045 ! embryonic root
is_a: PO:0003005 ! nodal root

[Term]
id: PO:0000047
name: leaf lamina epidermis
namespace: plant_structure
def: "Epidermal layer of a leaf blade." [TAIR:ki]
is_a: PO:0006016 ! leaf epidermis
relationship: part_of PO:0020039 ! leaf lamina

[Term]
id: PO:0000048
name: leaf lamina vascular system
namespace: plant_structure
def: "Vascular system of the leaf lamina." [TAIR:ki]
relationship: part_of PO:0000036 ! leaf vascular system
relationship: part_of PO:0020039 ! leaf lamina

[Term]
id: PO:0000049
name: leaf lamina abaxial epidermis
namespace: plant_structure
def: "The epidermal layer of the abaxial/lower surface of the leaf blade." [TAIR:ki]
is_a: PO:0000047 ! leaf lamina epidermis

[Term]
id: PO:0000050
name: leaf lamina adaxial epidermis
namespace: plant_structure
def: "The epidermal layer of the adaxial/upper surface of the leaf blade." [TAIR:ki]
is_a: PO:0000047 ! leaf lamina epidermis

[Term]
id: PO:0000051
name: petiole epidermis
namespace: plant_structure
def: "Epidermal layer of a leaf petiole." [TAIR:ki]
is_a: PO:0006016 ! leaf epidermis
relationship: part_of PO:0020038 ! petiole

[Term]
id: PO:0000052
name: petiole vascular system
namespace: plant_structure
def: "Vascular system of the leaf petiole." [TAIR:ki]
relationship: part_of PO:0000036 ! leaf vascular system
relationship: part_of PO:0020038 ! petiole

[Term]
id: PO:0000053
name: petiole cortex
namespace: plant_structure
def: "The primary tissue located between the vascular system and the epidermis of the petiole." [TAIR:ki]
is_a: PO:0005708 ! cortex
relationship: part_of PO:0020038 ! petiole

[Term]
id: PO:0000066
name: epithem cell
namespace: plant_structure
def: "Cell of the mesophyll of a hydathode found between the xylem endings and the epidermis." [PMID:12662305, ISBN:0471245208]
comment: Proposed to be involved in the retrieval of solutes from the xylem sap.
is_a: PO:0009002 ! plant cell
relationship: part_of PO:0005660 ! hydathode

[Term]
id: PO:0000070
name: meristemoid
namespace: plant_structure
def: "A cell or a group of cells constituting an active locus of meristematic activity in a tissue composed of somewhat older\, differentiating cells." [PO:syr, ISBN:0471245208]
is_a: PO:0009002 ! plant cell

[Term]
id: PO:0000071
name: companion cell
namespace: plant_structure
def: "A specialized parenchyma cell associated with a sieve-tube member in angiosperm phloem and arising from the same mother cell as the sieve-tube member." [ISBN:0879015322]
is_a: PO:0009002 ! plant cell
relationship: part_of PO:0005043 ! secondary phloem
relationship: part_of PO:0006075 ! primary phloem

[Term]
id: PO:0000074
name: parenchyma cell
namespace: plant_structure
def: "A relatively unspecialized cell with a nucleate protoplast." [ISBN:0471245208]
is_a: PO:0009002 ! plant cell
relationship: part_of PO:0005421 ! parenchyma

[Term]
id: PO:0000075
name: collenchyma cell
namespace: plant_structure
def: "Elongated living cells with unevenly thickened nonlignified primary walls." [ISBN:0471245208]
is_a: PO:0009002 ! plant cell
relationship: part_of PO:0005423 ! collenchyma

[Term]
id: PO:0000076
name: chlorenchyma cell
namespace: plant_structure
def: "Parenchyma cell containing chloroplasts; a component of leaf mesophyll and other green parenchyma tissue." [ISBN:0471245208]
is_a: PO:0000074 ! parenchyma cell
relationship: part_of PO:0005426 ! chlorenchyma

[Term]
id: PO:0000077
name: sclerenchyma cell
namespace: plant_structure
def: "Usually dead cell variable in form and size\, with more or less thick\, often lignified\, secondary walls." [ISBN:0471245208]
is_a: PO:0009002 ! plant cell
relationship: part_of PO:0005427 ! sclerenchyma

[Term]
id: PO:0000078
name: transfer cell
namespace: plant_structure
def: "A cell with wall ingrowths (or invaginations) that increase the surface of the plasmalemma. " [ISBN:0471245208]
comment: Appears to be specialized for short-distance transfer of solutes.
is_a: PO:0009002 ! plant cell

[Term]
id: PO:0000079
name: fusiform initial
alt_id: PO:0000275
namespace: plant_structure
def: "An elongated cell with approximately wedge-shaped ends\, found in the vascular cambium\, which gives rise to the elements of the axial system in the secondary vascular tissues." [ISBN:0471245208]
synonym: "xylem initial" []
synonym: "xylem mother cell" []
is_a: PO:0000295 ! cambial initial

[Term]
id: PO:0000081
name: axial cell
namespace: plant_structure
def: "A vascular cell derived from the fusiform cambial initial and oriented with its longest diameter parallel with the main axis of stem or root." [ISBN:0471245208]
comment: These cells make up the axial system\, also known as vertical or longitudinal system.
is_a: PO:0009002 ! plant cell
relationship: develops_from PO:0000079 ! fusiform initial

[Term]
id: PO:0000082
name: ray initial
namespace: plant_structure
def: "A cell in the vascular cambium that gives rise to ray cells of the secondary xylem and secondary phloem." [ISBN:0471245208]
is_a: PO:0000295 ! cambial initial

[Term]
id: PO:0000084
name: sperm cell
alt_id: PO:0020098
namespace: plant_structure
def: "A haploid male reproductive cell (usually two in number); during double fertilization\, one fuses with the female gamete (egg cell) to produce a zygote while another fusses with the two polar nuclei of the central cell to give rise to endosperm." [TAIR:ki]
subset: reference
synonym: "sperm nucleus" []
is_a: PO:0009002 ! plant cell
relationship: develops_from PO:0020097 ! generative cell
relationship: part_of PO:0020091 ! male gametophyte

[Term]
id: PO:0000112
name: stem epidermis
namespace: plant_structure
def: "Epidermal layer of the stem." [TAIR:lr]
synonym: "culm epidermis" []
is_a: PO:0006035 ! shoot epidermis
relationship: part_of PO:0009047 ! stem

[Term]
id: PO:0000115
name: socket cell
namespace: plant_structure
def: "Cell that surrounds a trichome and provides its support." [ISBN:0471245208]
is_a: PO:0004013 ! epidermal cell
relationship: develops_from PO:0000349 ! epidermal initial

[Term]
id: PO:0000146
name: abscission zone
namespace: plant_structure
def: "Zone at base of leaf\, flower\, fruit\, or other plant part that contains an abscission (or separation) layer and a protective layer\, both involved in the abscission of the plant part." [ISBN:047124529]
synonym: "abscission layer" []
is_a: PO:0009007 ! tissue

[Term]
id: PO:0000191
name: synergid
namespace: plant_structure
def: "Cell\, usually two in number\, in the micropylar end of the embryo sac of angiosperms associated with the egg in the egg apparatus." [ISBN:047125208, TAIR:ki]
subset: reference
is_a: PO:0009002 ! plant cell
relationship: part_of PO:0020096 ! egg apparatus

[Term]
id: PO:0000198
name: free nuclear endosperm
namespace: plant_structure
def: "Endosperm in which at least the first karyokinesis is not followed by cytokinesis." [ISBN:0080374913, ISBN:0471245194]
synonym: "cenocytic endosperm" []
synonym: "coenocytic endosperm" []
synonym: "nuclear endosperm" []
is_a: PO:0009089 ! endosperm

[Term]
id: PO:0000199
name: cellular endosperm
namespace: plant_structure
def: "Endosperm in which the first karyokinesis event is accompanied by cytokinesis." [ISBN:0080374913, ISBN:0471245194]
is_a: PO:0009089 ! endosperm

[Term]
id: PO:0000200
name: micropylar endosperm
namespace: plant_structure
def: "The region of the endosperm closest to the micropyle of the seed." [TAIR:lr]
synonym: "micropylar region" []
relationship: part_of PO:0009089 ! endosperm

[Term]
id: PO:0000201
name: chalazal cyst
namespace: plant_structure
def: "The part of the endosperm nearest the chalazal region of the ovule and forming a cyst-like structure." [TAIR:lr, ISBN:047124529]
comment: Not in current literature. More like an attribute.
synonym: "chalazal endosperm cyst" []
relationship: part_of PO:0009089 ! endosperm

[Term]
id: PO:0000207
name: nectary epidermis
namespace: plant_structure
def: "The epidermal layer of the nectary." [TAIR:lr]
is_a: PO:0006035 ! shoot epidermis
relationship: part_of PO:0009035 ! nectary

[Term]
id: PO:0000223
name: stem cortex
namespace: plant_structure
def: "The primary tissue located between the vascular system and the epidermis of the stem." [GR:pj, ISBN:047124529]
is_a: PO:0005708 ! cortex
relationship: part_of PO:0009047 ! stem

[Term]
id: PO:0000224
name: central zone
namespace: plant_structure
def: "An area of densely packed cells in the shoot apex that divide infrequently." [TAIR:lr, ISBN:0521288959]
comment: Functions as a population of stem cells that replenishes the meristem.
synonym: "central initiation zone" []
relationship: part_of PO:0020148 ! shoot apical meristem

[Term]
id: PO:0000225
name: peripheral zone
namespace: plant_structure
def: "Organogenic region of the meristem\,  characterized by higher rates of cell division." [TAIR:lr, ISBN:0521288959]
synonym: "peripheral meristem" []
relationship: part_of PO:0020148 ! shoot apical meristem

[Term]
id: PO:0000226
name: rib zone
namespace: plant_structure
def: "The region of the meristem that lies below the central zone and is flanked by the peripheral zone" [ISBN:0521288959, TAIR:lr]
synonym: "file meristem" []
relationship: part_of PO:0020148 ! shoot apical meristem

[Term]
id: PO:0000229
name: floral meristem
namespace: plant_structure
def: "Meristem that gives rise to the floral organs." [GR:pj]
synonym: "floral apical meristem" []
is_a: PO:0020148 ! shoot apical meristem
relationship: part_of PO:0009049 ! inflorescence

[Term]
id: PO:0000230
name: inflorescence meristem
namespace: plant_structure
def: "Meristem that gives rise to the inflorescence." [GR:pj]
is_a: PO:0020148 ! shoot apical meristem
relationship: part_of PO:0009049 ! inflorescence

[Term]
id: PO:0000232
name: axillary bud meristem
namespace: plant_structure
def: "Meristems formed in the axil of the leaf." [TAIR:lr]
synonym: "axillary meristem" []
is_a: PO:0006079 ! shoot meristem

[Term]
id: PO:0000244
name: functional megaspore
namespace: plant_structure
def: "The megaspore(s) that forms the embryo sac." [TAIR:lr]
is_a: PO:0020019 ! megaspore

[Term]
id: PO:0000245
name: degenerate megaspore
namespace: plant_structure
def: "In monosporic and bisporic megasporogenesis\: the megaspore(s) that would not participate in megagametogenesis." [TAIR:lr]
is_a: PO:0020019 ! megaspore

[Term]
id: PO:0000252
name: endodermis
alt_id: PO:0006064
namespace: plant_structure
def: "The innermost layer of the cortex in roots and stems of seed plants. The layer of tissue forming a sheath around the vascular region and often having a casparian strip in its anticlinal walls; it may have secondary walls later." [ISBN:047124529]
synonym: "endodermoid" []
relationship: part_of PO:0005708 ! cortex

[Term]
id: PO:0000256
name: root hair
namespace: plant_structure
def: "A root epidermal cell with a simple extension that is concerned with absorption of soil solution." [ISBN:0471245208]
is_a: PO:0004013 ! epidermal cell
relationship: develops_from PO:0000262 ! trichoblast
relationship: part_of PO:0006036 ! root epidermis

[Term]
id: PO:0000258
name: root cortex
alt_id: PO:0003010
namespace: plant_structure
def: "The primary tissue located between the vascular system and the epidermis of the root." [ISBN:047125208, GR:pj]
comment: In dicots and gymnosperms\, the cortex consists of mainly parenchyma cells. In monocots sclerenchyma develops in addition to parenchyma.
is_a: PO:0005708 ! cortex
relationship: part_of PO:0009005 ! root

[Term]
id: PO:0000262
name: trichoblast
namespace: plant_structure
def: "The smaller cell produced by the asymmetric division of a root epidermal cell that gives rise to a root hair." [ISBN:0471245208]
synonym: "hair cell" []
is_a: PO:0004013 ! epidermal cell
relationship: develops_from PO:0000349 ! epidermal initial
relationship: part_of PO:0006036 ! root epidermis

[Term]
id: PO:0000263
name: atrichoblast
namespace: plant_structure
def: "A cell formed after asymmetric division of root epidermal cell that does not give rise to a root hair." [ISBN:0387987819]
synonym: "non-hair cell" []
is_a: PO:0004013 ! epidermal cell
relationship: develops_from PO:0000349 ! epidermal initial
relationship: part_of PO:0006036 ! root epidermis

[Term]
id: PO:0000272
name: protoxylem
namespace: plant_structure
def: "The first formed elements of the primary xylem." [ISBN:047125208]
relationship: part_of PO:0005849 ! primary xylem

[Term]
id: PO:0000273
name: xylem element
namespace: plant_structure
def: "A cell making up xylem tissue." [ISBN:0471245208]
is_a: PO:0000081 ! axial cell
is_a: PO:0009002 ! plant cell

[Term]
id: PO:0000274
name: xylem fiber
namespace: plant_structure
def: "A fiber in xylem." [ISBN:0471245208]
is_a: PO:0000273 ! xylem element
relationship: part_of PO:0005848 ! secondary xylem

[Term]
id: PO:0000282
name: trichome
namespace: plant_structure
def: "An outgrowth from the epidermis varying in size and complexity and including hairs\, scales\, and other structures; may be glandular." [ISBN:0471245208, TAIR:ki]
comment: In Arabidopsis\, patterning of trichome development is not random but does not appear to be lineage-based like stomata.
is_a: PO:0004013 ! epidermal cell

[Term]
id: PO:0000283
name: idioblast
namespace: plant_structure
def: "OBSOLETE. A cell in a tissue that markedly differs in form\, size\, or contents from other cells in the same tissue." [ISBN:0471245208]
comment: This term was made obsolete because its a kind of attribute for a cell type.
is_obsolete: true

[Term]
id: PO:0000284
name: subsidiary cell
alt_id: PO:0000296
namespace: plant_structure
def: "An epidermal cell associated with a stoma and at least morphologically distinguishable from the other epidermal cells." [ISBN:047124520]
synonym: "accessory cell" []
is_a: PO:0004013 ! epidermal cell
relationship: part_of PO:0002000 ! stomatal complex

[Term]
id: PO:0000289
name: sieve tube member
alt_id: PO:0000286
namespace: plant_structure
def: "One of the series of cells that make up a sieve tube; it shows a more or less pronounced differentiation between sieve plates (wide pores) and lateral sieve areas (narrow pores)." [ISBN:0471245208]
comment: Also sieve tube element and the obsolete sieve tube segment.
synonym: "sieve element" []
synonym: "sieve tube element" []
is_a: PO:0009002 ! plant cell
relationship: part_of PO:0005043 ! secondary phloem
relationship: part_of PO:0006075 ! primary phloem

[Term]
id: PO:0000290
name: tracheary element
namespace: plant_structure
def: "General term for any water conducting cell\, tracheid or vessel member." [ISBN:0471245208]
is_a: PO:0000273 ! xylem element
is_a: PO:0009002 ! plant cell
relationship: part_of PO:0005848 ! secondary xylem
relationship: part_of PO:0005849 ! primary xylem

[Term]
id: PO:0000293
name: guard cell
namespace: plant_structure
def: "One of a pair of cells flanking the stomatal pore." [ISBN:0471245208]
comment: They cause the opening and closing of the pore by changes in turgor.
is_a: PO:0004013 ! epidermal cell
relationship: develops_from PO:0000351 ! guard mother cell
relationship: part_of PO:0002000 ! stomatal complex

[Term]
id: PO:0000295
name: cambial initial
alt_id: PO:0000080
namespace: plant_structure
def: "Cell in the vascular or cork cambium which by periclinal divisions produce cells to the outside or inside of the cambial axis." [POC:curators]
synonym: "cambial cell" []
is_a: PO:0004011 ! initial cell
relationship: part_of PO:0005598 ! vascular cambium

[Term]
id: PO:0000301
name: tracheid
namespace: plant_structure
def: "In the xylem\, a dead elongated water-conducting cell in which at least the middle lamella of the end walls remains intact." [APWeb:Glossary]
is_a: PO:0000290 ! tracheary element

[Term]
id: PO:0000309
name: nectary parenchyma
namespace: plant_structure
def: "Relatively unspecialized tissue present in the nectary." [TAIR:lr]
is_a: PO:0005421 ! parenchyma

[Term]
id: PO:0000332
name: pavement cell
namespace: plant_structure
def: "Epidermal cell with characteristic sinuous anticlinal cell walls that overall give a jigsaw like appearance to the leaf epidermis." [ISBN:087694289]
is_a: PO:0004013 ! epidermal cell
relationship: develops_from PO:0000349 ! epidermal initial
relationship: part_of PO:0000049 ! leaf lamina abaxial epidermis
relationship: part_of PO:0000050 ! leaf lamina adaxial epidermis
relationship: part_of PO:0006018 ! leaf adaxial epidermis
relationship: part_of PO:0006019 ! leaf abaxial epidermis

[Term]
id: PO:0000349
name: epidermal initial
namespace: plant_structure
def: "A relatively unspecialized cell that will give rise to specialized cell types of the epidermis." [TAIR:lr]
is_a: PO:0004011 ! initial cell

[Term]
id: PO:0000351
name: guard mother cell
namespace: plant_structure
def: "Epidermal cell that divides to produce the guard cells." [ISBN:0471245208]
is_a: PO:0004013 ! epidermal cell
relationship: develops_from PO:0000070 ! meristemoid
relationship: develops_from PO:0000349 ! epidermal initial

[Term]
id: PO:0000352
name: myrosin cell
namespace: plant_structure
def: "Cell containing glucosinolates (\"mustard oil glucosides\") and myrosinases\, enzymes hydrolyzing the glucosinolates." [ISBN:0471245208]
is_a: PO:0009002 ! plant cell

[Term]
id: PO:0000353
name: passage cell
namespace: plant_structure
def: "Cell in exodermis or endodermis that remains thin walled when the associated cells develop thick secondary walls." [ISBN:0471245208]
is_a: PO:0009002 ! plant cell

[Term]
id: PO:0000355
name: fiber tracheid
namespace: plant_structure
def: "A fiber-like tracheid in the secondary xylem; commonly thick walled\, with pointed ends and bordered pits that have lenticular to slit-like apertures." [ISBN:0471245208]
is_a: PO:0000274 ! xylem fiber

[Term]
id: PO:0000372
name: metaxylem
namespace: plant_structure
def: "Part of the primary xylem that differentiates after the protoxylem and before the secondary xylem\, if any of the latter is formed." [ISBN:047125208]
relationship: part_of PO:0005849 ! primary xylem

[Term]
id: PO:0000373
name: mucilage cell
namespace: plant_structure
def: "OBSOLETE. Cell containing mucilages or gums or similar carbohydrate material characterized by the property of swelling in water." [ISBN:0471245208]
comment: Functional term
is_obsolete: true

[Term]
id: PO:0000400
name: phloem mother cell
namespace: plant_structure
def: "A cell derived from vascular cambium which is destined to differentiate into secondary phloem." [POC:curators]
comment: Phloem islands can be formed in the middle of the xylem.
is_a: PO:0000295 ! cambial initial
relationship: part_of PO:0005043 ! secondary phloem

[Term]
id: PO:0000423
name: zygote
namespace: plant_structure
def: "Diploid cell produced by the fusion of sperm cell nucleus and egg cell." [TAIR:ki]
is_a: PO:0009002 ! plant cell

[Term]
id: PO:0000431
name: megasporocyte
namespace: plant_structure
def: "A diploid (2n) cell that undergoes meiosis and produces four haploid (1n) megaspores." [ISBN:0471245208]
synonym: "MMC" []
synonym: "megaspore mother cell" []
is_a: PO:0006204 ! sporocyte
relationship: develops_from PO:0006015 ! female archesporial cell
relationship: part_of PO:0020020 ! nucellus

[Term]
id: PO:0002000
name: stomatal complex
namespace: plant_structure
def: "An opening in the epidermis of leaves and stems bordered by two guard cells and serving in gas exchange." [ISBN:0471245208]
relationship: part_of PO:0000049 ! leaf lamina abaxial epidermis
relationship: part_of PO:0000050 ! leaf lamina adaxial epidermis
relationship: part_of PO:0000051 ! petiole epidermis
relationship: part_of PO:0006018 ! leaf adaxial epidermis
relationship: part_of PO:0006019 ! leaf abaxial epidermis

[Term]
id: PO:0002001
name: papillae
namespace: plant_structure
def: "A soft protuberance on an epidermal cell of the stigma." [ISBN:0471245208]
subset: reference
relationship: part_of PO:0006061 ! stigma epidermis

[Term]
id: PO:0002002
name: basal cell
namespace: plant_structure
def: "The lowermost cell formed after the first division of the zygote." [ISBN:0471245208]
is_a: PO:0009002 ! plant cell
relationship: develops_from PO:0000423 ! zygote
relationship: part_of PO:0009009 ! embryo

[Term]
id: PO:0002003
name: vessel member
namespace: plant_structure
def: "One of the cellular components of a vessel\, a dead cell with the wall between adjacent members being variously perforated and the walls that persist variously thickened. " [ISBN:0471245208]
synonym: "vessel element" []
synonym: "vessel segment" []
is_a: PO:0000290 ! tracheary element

[Term]
id: PO:0003000
name: transition zone
namespace: plant_structure
def: "A region of the root between the meristem and the region of rapid elongation in which isodiametric growth (cell expansion) occurs." [Agricola:IND23249552, http://search.epnet.com/direct.asp?an=IND23249552&db=agr]
subset: reference
relationship: part_of PO:0009005 ! root

[Term]
id: PO:0003003
name: primary root elongation zone
namespace: plant_structure
def: "A zone of small\, densely cytoplasmic cells that are dividing and expanding in size located behind the zone of cell division in the primary root." [TAIR:ki]
is_a: PO:0020125 ! elongation zone
relationship: part_of PO:0020127 ! primary root

[Term]
id: PO:0003004
name: haustorial root
namespace: plant_structure
def: "OBSOLETE. The root of particular parasitic plants that becomes cemented to the host axis and intrudes into the tissues of the host." [http://www.botgard.ucla.edu/html/botanytextbooks/generalbotany/typesofroots/]
comment: Term is specific for parasitic plants only.
is_obsolete: true

[Term]
id: PO:0003005
name: nodal root
alt_id: PO:0003008
alt_id: PO:0003009
namespace: plant_structure
def: "Adventitious root that forms at a shoot node." [http://www.botgard.ucla.edu/html/botanytextbooks/generalbotany/typesofroots/]
subset: reference
is_a: PO:0000042 ! shoot borne root

[Term]
id: PO:0003011
name: root vascular system
namespace: plant_structure
def: "Total of the vascular tissues in their specific arrangements in the root." [TAIR:ki, ISBN:0471245208]
comment: This term was brought back from OBSOLETE node (original reason for OBSOLETE\: synonym of term stele). Since stele encompasses both\, vascular system and the pith\, in roots with pith\, vascular system and stele are not synonymous.
is_a: PO:0000034 ! vascular system
relationship: part_of PO:0020124 ! root stele

[Term]
id: PO:0003014
name: lateral root elongation zone
namespace: plant_structure
def: "The portion of the lateral root located behind the zone of cell division that includes small\, densely cytoplasmic cells that are dividing and expanding in size." [TAIR:ki]
is_a: PO:0020125 ! elongation zone
relationship: part_of PO:0020121 ! lateral root

[Term]
id: PO:0003015
name: primary root differentiation zone
namespace: plant_structure
def: "A zone of cells that are differentiating into their final form and function located behind the elongation zone of the portion of the primary root." [TAIR:ki]
is_a: PO:0020135 ! differentiation zone
relationship: part_of PO:0020127 ! primary root

[Term]
id: PO:0003016
name: lateral root differentiation zone
namespace: plant_structure
def: "The portion of the lateral root located behind the elongation zone containing cells that are differentiating into their final form and function." [TAIR:ki]
is_a: PO:0020135 ! differentiation zone
relationship: part_of PO:0020121 ! lateral root

[Term]
id: PO:0003017
name: root cap of the primary root
namespace: plant_structure
def: "A group of cells that covers the apical meristem of the primary root." [TAIR:ki]
is_a: PO:0020123 ! root cap
relationship: part_of PO:0000026 ! primary root tip

[Term]
id: PO:0003018
name: root cap of the lateral root
namespace: plant_structure
def: "A group of cells that covers the apical meristem of the lateral root." [TAIR:ki]
is_a: PO:0020123 ! root cap
relationship: part_of PO:0000027 ! lateral root tip

[Term]
id: PO:0003019
name: central root cap of the lateral root
namespace: plant_structure
def: "The central part of a root cap of a lateral root in which the cells are arranged in longitudinal files." [TAIR:ki]
is_a: PO:0020130 ! central root cap
relationship: part_of PO:0003018 ! root cap of the lateral root

[Term]
id: PO:0003020
name: lateral root cap of the lateral root
namespace: plant_structure
def: "In the lateral root\, the part of the root cap that is parallel to the sides of the axis." [TAIR:ki]
is_a: PO:0020131 ! lateral root cap
relationship: part_of PO:0003018 ! root cap of the lateral root

[Term]
id: PO:0003021
name: central root cap of the primary root
namespace: plant_structure
def: "The central part of a root cap of the primary root in which the cells are arranged in longitudinal files." [TAIR:ki]
is_a: PO:0020130 ! central root cap
relationship: part_of PO:0003017 ! root cap of the primary root

[Term]
id: PO:0003022
name: lateral root cap of the primary root
namespace: plant_structure
def: "In the primary root\, the part of the root cap that is parallel to the sides of the axis." [TAIR:ki]
is_a: PO:0020131 ! lateral root cap
relationship: part_of PO:0003017 ! root cap of the primary root

[Term]
id: PO:0003023
name: root nodule
namespace: plant_structure
def: "Enlargement or swelling on the roots of plants\, particularly in the Fabaceae\, inhabited by nitrogen-fixing bacteria." [ISBN:0471245208]
relationship: part_of PO:0009005 ! root

[Term]
id: PO:0003024
name: stolon
namespace: plant_structure
def: "A slender\, prostrate or trailing above-ground stem which produces roots and sometimes erect shoots at its nodes." [APWeb:Glossary]
subset: reference
synonym: "runner" []
is_a: PO:0009006 ! shoot

[Term]
id: PO:0004000
name: apical cell
namespace: plant_structure
def: "The uppermost cell formed after the first division of the zygote." [ISBN:0471245208]
is_a: PO:0009002 ! plant cell
relationship: develops_from PO:0000423 ! zygote
relationship: part_of PO:0009009 ! embryo

[Term]
id: PO:0004001
name: bulliform cell
namespace: plant_structure
def: "An enlarged more or less thin-walled epidermal cell present\, with other similar cells\, in longitudinal rows in leaves of monocots." [ISBN:0471245208]
comment: Also called motor cell because of its presumed participation in the mechanism of rolling and unrolling of leaves.
synonym: "motor cell" []
is_a: PO:0004013 ! epidermal cell
relationship: part_of PO:0006016 ! leaf epidermis

[Term]
id: PO:0004002
name: contact cell
namespace: plant_structure
def: "OBSOLETE. An axial parenchyma or a ray cell physiologically associated with a tracheary element. Also a cell next to a stoma." [ISBN:0471245208]
comment: Not used in current plant literature.
is_obsolete: true

[Term]
id: PO:0004003
name: phellem
alt_id: PO:0005049
namespace: plant_structure
def: "Tissue centrifugally derived from cork cambium\, nonliving at maturity\, and having suberized walls. " [ISBN:0471245208, POC:curators]
comment: Protective in function because the walls are highly impervious to water.
synonym: "cork" []
synonym: "phellem" []
is_a: PO:0009007 ! tissue
relationship: develops_from PO:0005599 ! cork cambium

[Term]
id: PO:0004004
name: epithelium cell
namespace: plant_structure
def: "OBSOLETE. A compact layer of cells\, often secretory in function\, covering a free surface or lining a cavity." [ISBN:0471245208]
comment: Functional term
is_obsolete: true

[Term]
id: PO:0004005
name: laticiferous cell
namespace: plant_structure
def: "OBSOLETE. A specialized cells or ducts resembling vessels; they form branched networks of latex-secreting cells in the phloem and other parts of plants." [http://academic.kellogg.edu/herbrandsonc/bio111/glossary/glossary.htm]
comment: Obsoleted\: Too general definition of the term. Replaced by two terms\: non-articulated laticifer cell and articulated laticifer cell.
is_obsolete: true

[Term]
id: PO:0004006
name: mesophyll cell
namespace: plant_structure
def: "A Cell that constitutes leaf mesophyll." [TAIR:ki]
is_a: PO:0000076 ! chlorenchyma cell
relationship: part_of PO:0006070 ! mesophyll

[Term]
id: PO:0004007
name: phelloid cell
namespace: plant_structure
def: "OBSOLETE.  A cell within the phellem (cork) but distinct from the cork cell in having no suberin in its walls." [ISBN:0471245208]
comment: Not used in current plant literature. Confusing definition.
is_obsolete: true

[Term]
id: PO:0004008
name: photosynthetic cell
namespace: plant_structure
def: "OBSOLETE. A chloroplast-containing cell engaged in photosynthesis." [ISBN:0471245208]
comment: Functional characterization is not part of the criteria.
is_obsolete: true

[Term]
id: PO:0004009
name: silica cell
namespace: plant_structure
def: "Cells with deposits of silica in them. One of the two types of short cells in the epidermis of grasses and bamboos. It is usually paired with epidermal cork cell." [ISBN:0471245208]
comment: One of two types of short cells in the epidermis of grasses.
is_a: PO:0004718 ! short cell

[Term]
id: PO:0004010
name: meristematic cell
namespace: plant_structure
def: "A cell synthesizing protoplasm and producing new cells by division and with only a primary cell wall." [ISBN:0471245208]
is_a: PO:0009002 ! plant cell
relationship: part_of PO:0009013 ! meristem

[Term]
id: PO:0004011
name: initial cell
namespace: plant_structure
def: "Cell in a meristem that by division gives rise to two cells one of which remains in the meristem\, the other is added to the plant body." [ISBN:0471245208]
broad_synonym: "stem cell" []
is_a: PO:0004010 ! meristematic cell

[Term]
id: PO:0004012
name: secretory cell
namespace: plant_structure
def: "OBSOLETE. Cell that produces secreted substances." [TAIR:ki]
comment: This is a functional term.
is_obsolete: true

[Term]
id: PO:0004013
name: epidermal cell
namespace: plant_structure
def: "Cell that constitutes dermal tissue." [TAIR:ki]
is_a: PO:0009002 ! plant cell
relationship: part_of PO:0005679 ! epidermis

[Term]
id: PO:0004509
name: secretory trichome
namespace: plant_structure
def: "A  trichome that secretes or sequesters a substance." [POC:curators]
is_a: PO:0000282 ! trichome
is_a: PO:0005656 ! secretory tissue

[Term]
id: PO:0004510
name: non-secretory trichome
namespace: plant_structure
def: "Trichome that does not have secretory function." [POC:curators]
is_a: PO:0000282 ! trichome

[Term]
id: PO:0004511
name: seed hair
namespace: plant_structure
def: "Trichome that develops from seed coat epidermis and is often long with putative dispersal function. " [POC:curators]
is_a: PO:0000282 ! trichome
relationship: part_of PO:0006048 ! seed coat epidermis
relationship: part_of PO:0020061 ! coma

[Term]
id: PO:0004512
name: heartwood
namespace: plant_structure
def: "The inner layers of secondary xylem that have largely ceased to function in storage and conduction and in which reserve materials have been removed or converted into heartwood substances; generally darker colored than the functioning sapwood." [POC:curators, ISBN:0471245208]
is_a: PO:0005848 ! secondary xylem

[Term]
id: PO:0004513
name: sapwood
namespace: plant_structure
def: "Outer part of the wood of stem or root containing living cells and reserves and in which conduction of water takes place. Generally lighter colored than the heartwood" [POC:curators, ISBN:0471245208]
is_a: PO:0005848 ! secondary xylem

[Term]
id: PO:0004514
name: growth ring
namespace: plant_structure
def: "A growth layer of secondary xylem or secondary phloem as seen in transection of stem or root; may be an annual ring or a false annual ring." [POC:curators, ISBN:0471245208]
is_a: PO:0005848 ! secondary xylem

[Term]
id: PO:0004515
name: early wood
namespace: plant_structure
def: "The wood formed in first part of a growth ring and characterized by a lower density and larger cells than the late wood." [POC:curators, ISBN:0471245208]
synonym: "spring wood" []
is_a: PO:0004514 ! growth ring

[Term]
id: PO:0004516
name: late wood
namespace: plant_structure
def: "The secondary xylem formed in the later part of a growth ring; denser and composed of smaller cells than the early wood. " [POC:curators]
synonym: "summer wood" []
is_a: PO:0004514 ! growth ring

[Term]
id: PO:0004517
name: growth ring boundary
namespace: plant_structure
def: "Boundary between two growth rings." [POC:curators]
is_a: PO:0004514 ! growth ring

[Term]
id: PO:0004518
name: bark
namespace: plant_structure
def: "All tissues outside the vascular cambium or the xylem; in older trees may be divided into dead outer bark and living inner bark\, which consists of secondary phloem. " [POC:curators]
is_a: PO:0009007 ! tissue
relationship: develops_from PO:0005043 ! secondary phloem

[Term]
id: PO:0004519
name: phloem fiber
namespace: plant_structure
def: "A fiber in phloem." [POC:curators]
relationship: part_of PO:0005043 ! secondary phloem

[Term]
id: PO:0004520
name: libriform fiber
namespace: plant_structure
def: "A xylem fiber commonly with thick walls and simple pits. " [POC:curators]
is_a: PO:0000274 ! xylem fiber

[Term]
id: PO:0004521
name: septate fiber
namespace: plant_structure
def: "A fiber with thin transverse walls (septa)\, which are formed after the cell develops a secondary wall thickening." [POC:curators]
is_a: PO:0000274 ! xylem fiber

[Term]
id: PO:0004522
name: outer vascular cambium
namespace: plant_structure
def: "Cambium at the outer margin of the xylem cylinder." [POC:curators]
is_a: PO:0005598 ! vascular cambium

[Term]
id: PO:0004523
name: included vascular cambium
namespace: plant_structure
def: "Cambium occurring within xylem." [POC:curators]
is_a: PO:0005598 ! vascular cambium

[Term]
id: PO:0004524
name: included phloem
namespace: plant_structure
def: "Phloem produced by included vascular cambium." [POC:curators]
relationship: part_of PO:0005043 ! secondary phloem

[Term]
id: PO:0004525
name: wood parenchyma cell
namespace: plant_structure
def: "Parenchyma cell occurring within secondary xylem." [POC:curators]
is_a: PO:0000074 ! parenchyma cell

[Term]
id: PO:0004526
name: axial wood parenchyma cell
namespace: plant_structure
def: "Parenchyma cell in the axial system of secondary xylem." [POC:curators]
is_a: PO:0004525 ! wood parenchyma cell

[Term]
id: PO:0004527
name: ray wood parenchyma cell
namespace: plant_structure
def: "Parenchyma cell of a ray in secondary xylem. " [POC:curators]
is_a: PO:0004525 ! wood parenchyma cell

[Term]
id: PO:0004528
name: upright wood ray parenchyma cell
namespace: plant_structure
def: "Ray cell in secondary xylem oriented axially (vertically in the axis) with its longest dimension." [POC:curators]
is_a: PO:0004527 ! ray wood parenchyma cell

[Term]
id: PO:0004529
name: procumbent wood ray parenchyma cell
namespace: plant_structure
def: "Ray cell within secondary xylem having its longest axis in radial direction." [POC:curators]
is_a: PO:0004527 ! ray wood parenchyma cell

[Term]
id: PO:0004530
name: tile  cell
namespace: plant_structure
def: "Empty upright ray cell of approximately the same height as the procumbent ray cell and occurring in indeterminate horizontal series usually  interspersed among the procumbent cells." [POC:curators]
is_a: PO:0004528 ! upright wood ray parenchyma cell

[Term]
id: PO:0004531
name: sheath cell
namespace: plant_structure
def: "Cell on the margin of\, and tending to form a sheath around\, the procumbent cells of a multi-seriate ray as seen in tangential section." [POC:curators]
is_a: PO:0004528 ! upright wood ray parenchyma cell

[Term]
id: PO:0004532
name: wood parenchyma
namespace: plant_structure
def: "Parenchymatous tissue occurring in the wood." [POC:curators]
is_a: PO:0005848 ! secondary xylem

[Term]
id: PO:0004533
name: axial wood parenchyma
namespace: plant_structure
def: "Parenchyma tissue in the axial system of secondary xylem." [POC:curators]
is_a: PO:0004532 ! wood parenchyma

[Term]
id: PO:0004534
name: ray wood parenchyma
namespace: plant_structure
def: "Radially oriented parenchyma tissue in secondary xylem. " [POC:curators]
is_a: PO:0004532 ! wood parenchyma

[Term]
id: PO:0004535
name: fruit placenta
namespace: plant_structure
def: "A more or less localized region within a fruit to which seeds are attached." [POC:curators]
subset: Tomato
relationship: part_of PO:0009001 ! fruit

[Term]
id: PO:0004536
name: fruit pedicel
namespace: plant_structure
def: "Basal part of the ultimate branch of the infructescence." [POC:curators]
subset: Tomato
relationship: part_of PO:0009001 ! fruit

[Term]
id: PO:0004537
name: adventitious embryo
namespace: plant_structure
def: "Embryo derived directly from nucelus cells without involving embryo sac cells." [POC:curators]
is_a: PO:0009009 ! embryo

[Term]
id: PO:0004538
name: indeterminate nodule
namespace: plant_structure
def: "Nodule characterized by a persistent meristem\, presence of vascular transfer cells\, and cell division in the inner cortex with non-dividing infected cells and bacteria. " [POC:curators, ISBN:1842460137]
comment: Nodule is persistent and may continue to grow after a physiological stress.
is_a: PO:0003023 ! root nodule

[Term]
id: PO:0004539
name: determinate nodule
namespace: plant_structure
def: "Nodule characterized by a dividing infected cells and bacteria\, vascular transfer cells absent and cell division is in the outer cortex. " [POC:curators]
comment: Nodules are not persistent.
is_a: PO:0003023 ! root nodule

[Term]
id: PO:0004540
name: fruit columella
namespace: plant_structure
def: "Central axis of the fruit." [POC:curators]
subset: Tomato
relationship: part_of PO:0009001 ! fruit

[Term]
id: PO:0004542
name: rhizome
namespace: plant_structure
def: "Underground shoot" [POC:curators]
subset: reference
is_a: PO:0009006 ! shoot

[Term]
id: PO:0004543
name: tuber
namespace: plant_structure
def: "Swollen storage shoot with determinate growth." [POC:curators]
subset: reference
is_a: PO:0009006 ! shoot

[Term]
id: PO:0004544
name: root borne shoot
namespace: plant_structure
def: "Shoot that is initiated from a root." [POC:curators]
synonym: "sucker shoot" []
is_a: PO:0009006 ! shoot

[Term]
id: PO:0004545
name: shoot borne shoot
namespace: plant_structure
def: "Shoot that is initiated from a shoot." [POC:curators]
subset: reference
synonym: "branch" []
is_a: PO:0009006 ! shoot

[Term]
id: PO:0004546
name: epicomic shoot
namespace: plant_structure
def: "Shoot developing from a trunk." [POC:curators]
is_a: PO:0004545 ! shoot borne shoot

[Term]
id: PO:0004547
name: subterranean tuber
namespace: plant_structure
def: "A swollen rhizome or a part of the rhizome with determinate growth." [POC:curator]
comment: This has nothing to do with the underground swollen storage organ of Ipomoea which is swollen.
is_a: PO:0004543 ! tuber
relationship: part_of PO:0004542 ! rhizome

[Term]
id: PO:0004548
name: aerial tuber
namespace: plant_structure
def: "An axillary shoot with a swollen stem.\n" [POC:curators]
is_a: PO:0004543 ! tuber
is_a: PO:0006343 ! axillary shoot

[Term]
id: PO:0004700
name: middle layer
namespace: plant_structure
def: "Usually a single cell layer between tapetum and endothecium which almost invariably degenerates early during angiosperm anther  development and is eventually absorbed by adjacent cells." [POC:curators]
subset: reference
relationship: develops_from PO:0006008 ! inner secondary parietal cell layer
relationship: part_of PO:0000002 ! anther wall

[Term]
id: PO:0004701
name: short shoot
namespace: plant_structure
def: "Shoot in which the internodes elongate little or at all\, bearing reproductive structures and/or leaves." [APWeb:Glossary]
synonym: "brachyblast" []
synonym: "bud spur" []
is_a: PO:0006343 ! axillary shoot

[Term]
id: PO:0004702
name: long shoot
namespace: plant_structure
def: "Shoot in which all or most of the internodes elongate." [APWeb:Glossary]
is_a: PO:0006343 ! axillary shoot

[Term]
id: PO:0004703
name: carpel primordium
namespace: plant_structure
def: "The very first appearance of a carpel. It initiates from the carpel anlagen region of the floral meristem." [POC:curators, GR:pj]
is_a: PO:0009030 ! carpel
relationship: develops_from PO:0006005 ! carpel anlagen

[Term]
id: PO:0004704
name: sepal primordium
namespace: plant_structure
def: "The very first appearance of a sepal." [POC:curators]
is_a: PO:0009031 ! sepal

[Term]
id: PO:0004705
name: stamen primordium
namespace: plant_structure
def: "The very first appearance of a stamen." [POC:curators]
is_a: PO:0009029 ! stamen

[Term]
id: PO:0004706
name: flower primordium
namespace: plant_structure
def: "The very first appearance of a flower." [POC:curators]
is_a: PO:0009046 ! flower

[Term]
id: PO:0004707
name: fruit dehiscence zone
namespace: plant_structure
def: "A narrow band of cells that extends along the entire length of the fruit. Upon fruit maturation\, cell separation within the dehiscence zone allows the valves to detach from the replum and for the seeds to be dispersed." [TAIR:ki]
subset: Arabidopsis
relationship: part_of PO:0009001 ! fruit

[Term]
id: PO:0004708
name: scutellar node
namespace: plant_structure
def: "The region in the embryo between the primary root (enclosed in the coleorhiza) and the plumule (enclosed in the coleoptile) to which the scutellum is attached." [MaizeGDB:lv]
relationship: part_of PO:0009009 ! embryo

[Term]
id: PO:0004709
name: axillary bud
namespace: plant_structure
def: "Bud formed in the axil of a leaf or shoot." [POC:curators]
subset: reference
relationship: part_of PO:0009006 ! shoot

[Term]
id: PO:0004710
name: axillary floral bud
namespace: plant_structure
def: "Bud formed in the axil of a leaf or shoot that develops into a flower." [POC:curators]
is_a: PO:0004709 ! axillary bud

[Term]
id: PO:0004711
name: axillary inflorescence bud
namespace: plant_structure
def: "Bud formed in the axil of the a leaf or shoot that develops into an inflorescence." [POC:curators]
is_a: PO:0004709 ! axillary bud

[Term]
id: PO:0004712
name: axillary vegetative bud
namespace: plant_structure
def: "Bud formed in the axil of the a leaf or shoot that develops into a long or short shoot and/or leaf(s). " [POC:curators]
is_a: PO:0004709 ! axillary bud

[Term]
id: PO:0004713
name: terminal bud
namespace: plant_structure
def: "Bud formed at the apex of shoot." [POC:curators]
subset: reference
relationship: part_of PO:0009006 ! shoot

[Term]
id: PO:0004714
name: terminal floral bud
namespace: plant_structure
def: "Bud formed at the apex of shoot that develops into a flower." [POC:curators]
is_a: PO:0004713 ! terminal bud

[Term]
id: PO:0004715
name: terminal inflorescence bud
namespace: plant_structure
def: "Bud formed at the apex of shoot that develops into an inflorescence." [POC:curators]
is_a: PO:0004713 ! terminal bud

[Term]
id: PO:0004716
name: terminal vegetative bud
namespace: plant_structure
def: "Bud formed at the apex of shoot that develops into a long or short shoot." [POC:curators]
is_a: PO:0004713 ! terminal bud

[Term]
id: PO:0004717
name: long cell
namespace: plant_structure
def: "A more or less rectangular epidermal cell in which the proximo-distal dimension is several times longer than the transverse dimension." [POC:curators]
comment: The leaf epidermis of Poaceae and Joinvilleaceae\, long cells and short cells often alternate in longitudinal rows.
is_a: PO:0004013 ! epidermal cell

[Term]
id: PO:0004718
name: short cell
namespace: plant_structure
def: "An isodiametric epidermal cell." [POC:curators]
comment: The leaf epidermis of Poaceae and Joinvilleaceae\, long cells and short cells often alternate in longitudinal rows.
is_a: PO:0004013 ! epidermal cell

[Term]
id: PO:0004719
name: hilum groove
namespace: plant_structure
def: "Longitudinal groove in the testa through the prominent hilum of the seed." [POC:curators]
synonym: "faboid split" []
relationship: part_of PO:0009010 ! seed

[Term]
id: PO:0004720
name: paraclade
namespace: plant_structure
def: "Lateral branch which ends in an inflorescence that repeats the main inflorescence." [APWeb:Glossary, ISBN:0521251346]
relationship: part_of PO:0009047 ! stem

[Term]
id: PO:0004721
name: paraclade cortex
namespace: plant_structure
def: "The primary tissue located between the vascular system and the epidermis of the paraclade." [TAIR:ki]
relationship: part_of PO:0004720 ! paraclade

[Term]
id: PO:0004722
name: pedicel cortex
namespace: plant_structure
def: "The primary tissue located between the vascular system and the epidermis of the pedicel." [TAIR:ki]
is_a: PO:0009052 ! pedicel

[Term]
id: PO:0004723
name: sepal vascular system
namespace: plant_structure
def: "Vascular system of the sepal." [TAIR:ki]
relationship: part_of PO:0009031 ! sepal

[Term]
id: PO:0004724
name: hypocotyl-root junction
namespace: plant_structure
def: "Junction point of the embryonic root and hypocotyl." [TAIR:ki]
subset: reference
relationship: part_of PO:0009006 ! shoot
relationship: part_of PO:0019018 ! embryo axis

[Term]
id: PO:0004725
name: abaxial side of leaf primordium
namespace: plant_structure
def: "The abaxial/outer side of the leaf primordium that becomes the abaxial/lower leaf blade." [TAIR:ki]
relationship: part_of PO:0000017 ! leaf primordium

[Term]
id: PO:0004726
name: adaxial side of leaf primordium
namespace: plant_structure
def: "The adaxial/inner side of the leaf primordium that becomes adaxial/upper leaf blade." [TAIR:ki]
relationship: part_of PO:0000017 ! leaf primordium

[Term]
id: PO:0005001
name: basal axillary shoot
namespace: plant_structure
def: "A branch that forms from a leaf at the very base of the shoot." [GR:ap]
synonym: "basal axillary branch" []
synonym: "tiller" []
is_a: PO:0006343 ! axillary shoot

[Term]
id: PO:0005002
name: cauline axillary shoot
namespace: plant_structure
def: "An axillary branch that forms from a leaf above the very base of the shoot." [GR:ap]
comment: The genetic distinction between cauline axillary branches and tillers may or may not be unique to the Poaceae. There are no data for other plant families.
synonym: "cauline axillary branch" []
is_a: PO:0006343 ! axillary shoot

[Term]
id: PO:0005004
name: shoot node
namespace: plant_structure
def: "The region of the shoot where the spikelet\, flower\, floret\, branch\, bud and/or leaves are attached." [GR:pj]
subset: reference
relationship: part_of PO:0009006 ! shoot

[Term]
id: PO:0005005
name: shoot internode
namespace: plant_structure
def: "The region of the shoot present between the two shoot nodes." [GR:pj]
subset: reference
relationship: part_of PO:0009006 ! shoot

[Term]
id: PO:0005006
name: articulated laticifer
namespace: plant_structure
def: "A structure consisting of long multinucleate tubes in which latex is found\, having cross walls (articulated)." [GR:pj, APWeb:Glossary]
is_a: PO:0005053 ! laticifer

[Term]
id: PO:0005007
name: non-articulated laticifer
namespace: plant_structure
def: "A structure consisting of long multinucleate tubes in which latex is found\, having no cross walls." [GR:pj, APWeb:Glossary]
is_a: PO:0005053 ! laticifer

[Term]
id: PO:0005039
name: primary thickening meristem
namespace: plant_structure
def: "A meristem derived directly from the shoot apical meristem and responsible for the primary increase in thickness of the shoot axis." [ISSN:0669014893]
comment: May appear as a distinct mantle like zone. Often found in monocotyledons
is_a: PO:0009013 ! meristem
relationship: develops_from PO:0000225 ! peripheral zone
relationship: part_of PO:0020148 ! shoot apical meristem

[Term]
id: PO:0005040
name: root pith
namespace: plant_structure
def: "Non-vascular tissue in the center of root." [ISBN:0080280307]
is_a: PO:0006109 ! pith
relationship: part_of PO:0020124 ! root stele

[Term]
id: PO:0005041
name: stem pith
namespace: plant_structure
def: "Non-vascular tissue in the center of stem." [ISBN:0080280307]
is_a: PO:0006109 ! pith
relationship: part_of PO:0009047 ! stem

[Term]
id: PO:0005043
name: secondary phloem
namespace: plant_structure
def: "The phloem tissue formed by the activity of the vascular cambium." [ISBN:0122151704]
comment: Part of the bark.
is_a: PO:0005417 ! phloem
relationship: part_of PO:0009007 ! tissue

[Term]
id: PO:0005046
name: periderm
namespace: plant_structure
def: "Secondary protective tissue that replaces the epidermis in stems and root\, rarely in other organs. " [ISBN:047124529, GR:pj]
is_a: PO:0009014 ! dermal tissue

[Term]
id: PO:0005047
name: root periderm
namespace: plant_structure
def: "Secondary protective tissue that replaces the epidermis in root." [GR:pj]
is_a: PO:0005046 ! periderm
relationship: part_of PO:0009005 ! root

[Term]
id: PO:0005048
name: stem periderm
namespace: plant_structure
def: "Secondary protective tissue that replaces the epidermis in stem." [GR:pj]
is_a: PO:0005046 ! periderm
relationship: part_of PO:0004518 ! bark
relationship: part_of PO:0009047 ! stem

[Term]
id: PO:0005050
name: phelloderm
namespace: plant_structure
def: "A tissue often resembling cortical parenchyma produced centripetally by the cork cambium." [ISBN:0080374913]
relationship: develops_from PO:0005599 ! cork cambium
relationship: part_of PO:0005048 ! stem periderm

[Term]
id: PO:0005051
name: hypodermis
namespace: plant_structure
def: "A layer or layers of cells beneath the epidermis that is distinct in appearance from adjacent tissues. It is the outermost layer or layers of cells of the cortex." [ISBN:0080374913, GR:pj]
relationship: part_of PO:0005708 ! cortex

[Term]
id: PO:0005052
name: callus
namespace: plant_structure
def: "A tissue formed as a result of wounding\, or a tissue developing in a tissue culture." [GR:pj]
is_a: PO:0005421 ! parenchyma

[Term]
id: PO:0005053
name: laticifer
namespace: plant_structure
def: "A secretory structure that produces latex." [ISBN:0080374913]
is_a: PO:0005656 ! secretory tissue

[Term]
id: PO:0005057
name: stem hypodermis
namespace: plant_structure
def: "A layer or layers of cells beneath the stem epidermis distinct in appearance from adjacent tissues." [GR:pj, ISBN:0080374913]
is_a: PO:0005051 ! hypodermis
relationship: part_of PO:0000223 ! stem cortex
relationship: part_of PO:0009047 ! stem

[Term]
id: PO:0005058
name: stem endodermis
namespace: plant_structure
def: "The innermost layer of cortex in the stem of seed plants." [GR:pj]
is_a: PO:0000252 ! endodermis
relationship: part_of PO:0000223 ! stem cortex
relationship: part_of PO:0009047 ! stem

[Term]
id: PO:0005059
name: root endodermis
namespace: plant_structure
def: "The innermost layer of the cortex in roots of  seed plants." [GR:pj]
is_a: PO:0000252 ! endodermis
relationship: part_of PO:0000258 ! root cortex

[Term]
id: PO:0005060
name: leaf endodermis
namespace: plant_structure
def: "The layer of tissue forming a sheath around the vascular region in a leaf." [GR:pj]
comment: Often found in the leaf of Gymnosperms and elsewhere.
is_a: PO:0000252 ! endodermis
relationship: part_of PO:0009025 ! leaf

[Term]
id: PO:0005349
name: schizo-lysigenous aerenchyma
namespace: plant_structure
def: "OBSOLETE. Aerenchyma\, originating by a combination of two processes\, separation and degradation of cell walls." [ISBN:0080374913, GR:pj]
comment: The term was made obsolete because schizo-lysigenous form is an attribute of regular aerenchyma.
is_obsolete: true

[Term]
id: PO:0005352
name: xylem
namespace: plant_structure
def: "vascular tissue whose principal function is the upward translocation of water and solutes." [GR:pj]
comment: See also primary xylem and secondary xylem.
is_a: PO:0009015 ! vascular tissue

[Term]
id: PO:0005360
name: aleurone layer
namespace: plant_structure
def: "The outermost endosperm tissue of the seeds\, its cells being characterized by presence of protein bodies containing seed storage proteins." [ISBN:0080374913, GR:pj]
relationship: part_of PO:0009089 ! endosperm

[Term]
id: PO:0005415
name: endosperm parenchyma
namespace: plant_structure
def: "Relatively unspecialized ground tissue present in the seed endosperm\, often devoid of intercellular spaces." [ISBN:0080374913]
is_a: PO:0005421 ! parenchyma
relationship: part_of PO:0009089 ! endosperm

[Term]
id: PO:0005417
name: phloem
namespace: plant_structure
def: "Vascular tissue whose principal function is conducting organic substances." [GR:pj]
is_a: PO:0009015 ! vascular tissue

[Term]
id: PO:0005421
name: parenchyma
namespace: plant_structure
def: "Relatively unspecialized tissue composed of polyhedral cells typically with thin\, non-lignified cellulose cell walls and nucleate living protoplasts." [GR:pj]
synonym: "parenchyma tissue" []
is_a: PO:0009007 ! tissue

[Term]
id: PO:0005423
name: collenchyma
namespace: plant_structure
def: "Living tissue composed of more or less elongated cells with thick nonlignified primary cell walls." [GR:pj]
synonym: "supporting tissue" []
is_a: PO:0009007 ! tissue

[Term]
id: PO:0005426
name: chlorenchyma
namespace: plant_structure
def: "Chloroplast-containing parenchyma tissue." [ISBN:0080374913]
synonym: "chlorenchyma tissue" []
is_a: PO:0005421 ! parenchyma

[Term]
id: PO:0005427
name: sclerenchyma
namespace: plant_structure
def: "A supporting tissue composed of fibers or sclereids." [ISBN:0080374913]
is_a: PO:0009007 ! tissue

[Term]
id: PO:0005597
name: cambium
namespace: plant_structure
def: "A lateral meristem\, the cells of which divide mostly periclinally. " [ISBN:0080374913]
is_a: PO:0020145 ! lateral meristem

[Term]
id: PO:0005598
name: vascular cambium
namespace: plant_structure
def: "A lateral meristem\, the cells of which give rise to secondary xylem and phloem\, leading to an increase in girth." [GR:pj]
is_a: PO:0005597 ! cambium

[Term]
id: PO:0005599
name: cork cambium
namespace: plant_structure
def: "Lateral meristem which produces the phellem (cork) and the phelloderm." [ISBN:0080374913]
synonym: "phellogen" []
is_a: PO:0005597 ! cambium
relationship: part_of PO:0005048 ! stem periderm

[Term]
id: PO:0005621
name: angular collenchyma
namespace: plant_structure
def: "OBSOLETE. A form of collenchyma in which the primary wall thickening is most prominent in the angles where three or more cells are joined." [GR:pj, ISBN:0080374913]
comment: The term was made obsolete because angular form is a common attribute of ordinary collenchyma.
is_obsolete: true

[Term]
id: PO:0005632
name: lacunar collenchyma
namespace: plant_structure
def: "OBSOLETE. A collenchyma characterized by intercellular spaces and cell wall thickenings facing the intercellular spaces." [GR:pj, ISBN:0080374913]
comment: The term was made obsolete because the lacunar form is an attribute of regular collenchyma.
is_obsolete: true

[Term]
id: PO:0005633
name: lamellar collenchyma
namespace: plant_structure
def: "OBSOLETE. A collenchyma in which cell wall thickenings are deposited mainly on tangential walls." [ISBN:0080374913, GR:pj]
comment: The term was made obsolete because lamellar form is an attribute of regular collenchyma.
synonym: "plate collenchyma" []
synonym: "tangential collenchyma" []
is_obsolete: true

[Term]
id: PO:0005645
name: leaf mesophyll
namespace: plant_structure
def: "The chloroplast-containing\, photosynthetic parenchymatous tissue situated between the two epidermal layers of the foliage leaf." [GR:pj, ISBN:0080374913]
synonym: "foliage leaf mesophyll" []
synonym: "leaf parenchyma" []
is_a: PO:0006070 ! mesophyll
relationship: part_of PO:0009025 ! leaf

[Term]
id: PO:0005647
name: spongy mesophyll
namespace: plant_structure
def: "Leaf mesophyll parenchyma characterized by little elongated cells\, that are not closely packed and have conspicuous intercellular spaces." [GR:pj, ISBN:0080374913]
synonym: "spongy parenchyma" []
is_a: PO:0006070 ! mesophyll
relationship: part_of PO:0005645 ! leaf mesophyll

[Term]
id: PO:0005648
name: palisade mesophyll
namespace: plant_structure
def: "parenchyma containing closely packed elongated chlorenchymatous cells oriented perpendicular to the leaf surface and which are active in photosynthesis." [ISBN:0080374913, GR:pj]
synonym: "palisade parenchyma" []
is_a: PO:0006070 ! mesophyll
relationship: part_of PO:0005645 ! leaf mesophyll

[Term]
id: PO:0005656
name: secretory tissue
namespace: plant_structure
def: "Tissues that form specialized structures producing a secretion." [ISBN:047124529, GR:pj]
comment: The synonym gland does not imply non-secretory 'glands'.
synonym: "gland" []
is_a: PO:0009007 ! tissue

[Term]
id: PO:0005660
name: hydathode
namespace: plant_structure
def: "A structural modification of vascular and non-vascular tissues\, usually in a leaf\, that permits the release of water through a pore in the epidermis." [ISBN:0080374913, GR:pj]
is_a: PO:0005656 ! secretory tissue
is_a: PO:0009015 ! vascular tissue

[Term]
id: PO:0005661
name: salt gland
namespace: plant_structure
def: "A specialized tissue where excess salt absorbed in water from the soil is concentrated\, being stores or excreted." [GR:pj]
comment: A crust of salt forms on leaves which tastes bad and the white surfaces act to reflect light. Example\, as is Mangrove vegetation
is_a: PO:0005656 ! secretory tissue

[Term]
id: PO:0005665
name: resin canal
namespace: plant_structure
def: "A duct of schizogenous origin lined with resin-secreting cells and containing resin" [ISBN:0080374913, GR:pj]
synonym: "resin duct" []
is_a: PO:0005656 ! secretory tissue

[Term]
id: PO:0005669
name: oil gland
namespace: plant_structure
def: "A gland or a cavity lined with cells that secrete oils." [GR:pj]
comment: Oil glands are schizogenous.
synonym: "oil cavity" []
is_a: PO:0005656 ! secretory tissue

[Term]
id: PO:0005679
name: epidermis
namespace: plant_structure
def: "An outermost cell layer of primary tissues of the plant\, sometimes comprised of more than one layer. " [GR:pj, ISBN:0080374913]
synonym: "epidermal layer" []
synonym: "multiseriate epidermis" []
is_a: PO:0009014 ! dermal tissue

[Term]
id: PO:0005702
name: aerenchyma
namespace: plant_structure
def: "Parenchyma tissue containing particularly large intercellular spaces of schizogenous or lysigenous origin." [ISBN:0080374913, GR:pj]
comment: As applied to an intercellular space\, originating by one or a combination of two processes\, separation and degradation of cell walls.
synonym: "aerenchyma tissue" []
is_a: PO:0005421 ! parenchyma

[Term]
id: PO:0005704
name: rhexigenous aerenchyma
namespace: plant_structure
def: "OBSOLETE. Aerenchyma originating by rupture of cells." [GR:pj, ISBN:0080374913]
comment: The term was made obsolete because rhexigenous form is an attribute of regular aerenchyma.
is_obsolete: true

[Term]
id: PO:0005706
name: lysigenous aerenchyma
namespace: plant_structure
def: "OBSOLETE. Aerenchyma originating by dissolution of cells." [GR:pj, ISBN:0080374913]
comment: The term was made obsolete because lysigenous form is an attribute of regular aerenchyma.
is_obsolete: true

[Term]
id: PO:0005708
name: cortex
namespace: plant_structure
def: "Tissue between the vascular system and the epidermis in stem and root. " [GR:pj]
is_a: PO:0009007 ! tissue

[Term]
id: PO:0005752
name: promeristem
namespace: plant_structure
def: "OBSOLETE. Meristematic tissue consisting of apical initials\, together with cells derived from them and which are still close to the initial." [GR:pj, ISBN:0080374913]
is_obsolete: true

[Term]
id: PO:0005772
name: exodermis
namespace: plant_structure
def: "The sub-epidermal layer or layers of cells of the root similar in structure and cytochemical characteristics of  the endodermis\, the outermost layer or layers of cells of the cortex." [GR:pj, ISBN:0080374913]
comment: The cell walls are thickened and contain suberin. Absent in pteridophytes\, fibrous in Phoenix and accompanied by sclerenchyma in Ananas.
synonym: "root hypodermis" []
is_a: PO:0005051 ! hypodermis
relationship: part_of PO:0000258 ! root cortex

[Term]
id: PO:0005848
name: secondary xylem
namespace: plant_structure
def: "The xylem tissue formed by the activity of the vascular cambium." [GR:pj, ISBN:0471245194]
comment: It is absent in small dicot annuals and most monocots; the \"wood\" of broad leaf angiosperm tress.
is_a: PO:0005352 ! xylem

[Term]
id: PO:0005849
name: primary xylem
namespace: plant_structure
def: "The xylem of the primary plant body. " [ISBN:0471245194, GR:pj, ISBN:0122151704]
comment: In stem or root it is differentiated behind the apical meristem.
is_a: PO:0005352 ! xylem

[Term]
id: PO:0006000
name: hull (sensu Poaceae)
namespace: plant_structure
def: "A leaf like structure often found enclosing\nthe grass fruit\, caryopsis. It is derived from the dried lemma (PO\:0009037) and palea (PO\:0009038) floral bracts found in the grass floret (PO\:0006318)." [GR:pj]
subset: Maize
subset: Poaceae
subset: Rice
relationship: develops_from PO:0009037 ! lemma
relationship: develops_from PO:0009038 ! palea
relationship: part_of PO:0006342 ! infructescence

[Term]
id: PO:0006001
name: phyllome
namespace: plant_structure
def: "A collective term for all the different types of leaves appearing on plants." [ISBN:0080374913]
subset: reference
is_a: PO:0009008 ! organ
relationship: part_of PO:0009006 ! shoot

[Term]
id: PO:0006002
name: lower glume
alt_id: PO:0006027
alt_id: PO:0006031
namespace: plant_structure
def: "The proximal/basal of the two glumes." [GR:pj]
synonym: "lower empty glume" []
synonym: "lower rudimentary glume" []
synonym: "outer empty glume" []
synonym: "outer glume" []
synonym: "outer rudimentary glume" []
is_a: PO:0009039 ! glume

[Term]
id: PO:0006003
name: scale leaf
namespace: plant_structure
def: "A reduced and more or less non-photosynthetic leaf\, often associated with a vegetatively propagating organ such as a rhizome or perennating bud." [ISBN:0080374913]
comment: Sometimes referring specifically to such leaves on a seedling.
subset: reference
synonym: "cataphyll" []
is_a: PO:0006001 ! phyllome

[Term]
id: PO:0006004
name: upper glume
alt_id: PO:0006028
alt_id: PO:0006030
namespace: plant_structure
def: "The apical/distal of the two glumes." [GR:pj]
synonym: "inner empty glume" []
synonym: "inner glume" []
synonym: "inner rudimentary glume" []
synonym: "upper empty glume" []
synonym: "upper rudimentary glume" []
is_a: PO:0009039 ! glume

[Term]
id: PO:0006005
name: carpel anlagen
namespace: plant_structure
def: "A presumptive region (carpel anlagen) on the floral meristem\, where carpel primordia would initiate." [PMID:14729915]
relationship: part_of PO:0000229 ! floral meristem

[Term]
id: PO:0006006
name: primary parietal cell layer
namespace: plant_structure
def: "The primary parietal cell and adjacent cells together form this cell layer." [PMID:2476454, GR:pj]
subset: reference
relationship: part_of PO:0000002 ! anther wall

[Term]
id: PO:0006007
name: secondary parietal cell layer
namespace: plant_structure
def: "The cells of the primary parietal cell layer undergo a periclinal division resulting in the formation of the two secondary parietal layers." [PMID:2476454, GR:pj]
subset: reference
relationship: develops_from PO:0006006 ! primary parietal cell layer
relationship: part_of PO:0000002 ! anther wall

[Term]
id: PO:0006008
name: inner secondary parietal cell layer
namespace: plant_structure
def: "One of the secondary parietal layer formed towards inner side after the cells of the primary parietal cell layer undergo a periclinal division. It divides periclinally to form the middle layer externally and the tapetum internally." [PMID:2476454, GR:pj]
is_a: PO:0006007 ! secondary parietal cell layer

[Term]
id: PO:0006009
name: outer secondary parietal cell layer
namespace: plant_structure
def: "One of the secondary parietal layer formed towards outside after the cells of the primary parietal cell layer undergo a periclinal division. It differentiates into the endothecium." [PMID:2476454, GR:pj]
is_a: PO:0006007 ! secondary parietal cell layer

[Term]
id: PO:0006010
name: primary parietal cell
namespace: plant_structure
def: "It is formed by the division of the archesporial initial." [PMID:2476454]
is_a: PO:0009002 ! plant cell
relationship: develops_from PO:0006014 ! male archesporial cell
relationship: part_of PO:0006006 ! primary parietal cell layer

[Term]
id: PO:0006011
name: lateral vein
namespace: plant_structure
def: "Unbranched second order vein of the grass leaf blade." [GR:pj]
is_a: PO:0020140 ! secondary vein

[Term]
id: PO:0006012
name: leaf collar
namespace: plant_structure
def: "A thin band of intercalary meristematic tissue at the junction of the leaf blade (lamina) and the leaf sheath found in grasses." [GR:pj, ISBN:0080374913]
relationship: part_of PO:0009025 ! leaf

[Term]
id: PO:0006013
name: juice sac
namespace: plant_structure
def: "As found in citrus the mature juice sac is a swollen sac with a slender stalk and a sac wall lined with layers of tightly arranged cells. It develops from a single cell of the endocarp. Endocarp develops from the carpellary inner epidermis." [GR:pj, web:http\://www.chineseplantscience.com/earticle_read.asp?id=12171]
subset: Citrus
synonym: "juice vesicle" []
relationship: part_of PO:0009086 ! endocarp

[Term]
id: PO:0006014
name: male archesporial cell
namespace: plant_structure
def: "It undergoes periclinal divisions\, giving rise to an inner primary sporogenous cell (PSC) layer and an outer primary parietal cell (PPC)" [PMID:10465788, GR:pj]
synonym: "anther archesporial cell" []
synonym: "male archesporial initial" []
is_a: PO:0009002 ! plant cell
relationship: part_of PO:0006089 ! anther primordium

[Term]
id: PO:0006015
name: female archesporial cell
namespace: plant_structure
def: "In the majority of flowering plants including Arabidopsis\, the female archesporial cell elongates and polarizes longitudinally\, and directly differentiates into the megasporocyte or megaspore mother cell (MMC). In some flowering plants\, it undergoes a periclinal division\, and subsequently the inner cell differentiates into the megasporocyte. " [PMID:10465788]
synonym: "female archesporial initial" []
synonym: "ovule archesporial cell" []
is_a: PO:0009002 ! plant cell
relationship: part_of PO:0000018 ! ovule primordium

[Term]
id: PO:0006016
name: leaf epidermis
namespace: plant_structure
def: "Epidermal layer of a foliage leaf." [GR:pj]
synonym: "foliage leaf epidermis" []
is_a: PO:0006035 ! shoot epidermis
relationship: part_of PO:0009025 ! leaf

[Term]
id: PO:0006017
name: helobial endosperm
namespace: plant_structure
def: "Endosperm in which the first karyokinetic event is accompanied by the formation of a horizontal wall which divides the central cell into unequal regions. The larger one is the micropylar chamber in which cytokinesis does not occur and the smaller one is the chalazal chamber." [ISBN:0080374913]
is_a: PO:0009089 ! endosperm

[Term]
id: PO:0006018
name: leaf adaxial epidermis
namespace: plant_structure
def: "The epidermal layer of adaxial/upper surface of the leaf." [ISBN:0080374913]
synonym: "upper epidermis" []
is_a: PO:0006016 ! leaf epidermis

[Term]
id: PO:0006019
name: leaf abaxial epidermis
namespace: plant_structure
def: "The epidermal layer of the abaxial/lower surface of the leaf." [ISBN:0080374913]
synonym: "lower epidermis" []
is_a: PO:0006016 ! leaf epidermis

[Term]
id: PO:0006020
name: lateral root apical meristem
alt_id: PO:0003013
namespace: plant_structure
def: "Meristem found in the apex of the lateral root." [GR:pj]
comment: This is different from root lateral meristem.
synonym: "apical meristem of lateral root" []
synonym: "lateral root meristem" []
is_a: PO:0020147 ! root apical meristem
relationship: part_of PO:0000027 ! lateral root tip

[Term]
id: PO:0006021
name: adventitious root apical meristem
namespace: plant_structure
def: "Apical meristem of the adventitious root." [GR:pj]
synonym: "crown root meristem" []
synonym: "seminal root meristem" []
is_a: PO:0020147 ! root apical meristem
relationship: part_of PO:0000042 ! shoot borne root

[Term]
id: PO:0006022
name: bundle sheath extension
namespace: plant_structure
def: "A strip of ground tissue present along the leaf veins and extending from the bundle sheath to the epidermis. It may be present on one or both sides of the vein and may consist of parenchyma or sclerenchyma." [ISBN:0080374913]
is_a: PO:0009007 ! tissue

[Term]
id: PO:0006023
name: bundle sheath
namespace: plant_structure
def: "A layer or layers of cells surrounding the vascular bundles of leaves. It may consist of parenchyma or sclerenchyma." [ISBN:0080374913]
is_a: PO:0009007 ! tissue
relationship: part_of PO:0009025 ! leaf

[Term]
id: PO:0006024
name: parenchyma sheath
namespace: plant_structure
def: "A single layered\, parenchymatous bundle sheath characterized by presence of large quantity of starch." [ISBN:0080374913]
comment: Homologous to the endodermis.
synonym: "starch sheath" []
is_a: PO:0006023 ! bundle sheath

[Term]
id: PO:0006025
name: mestome sheath
namespace: plant_structure
def: "The inner endodermal sheath of a two layered bundle sheath. The cells are smaller in diameter compared to those in outer wall (starch sheath). The cell  walls are thick and contain suberized lamellae. They are analogous to endodermis." [ISBN:0080374913]
is_a: PO:0006023 ! bundle sheath

[Term]
id: PO:0006032
name: awn
namespace: plant_structure
def: "A long bristle-like appendage found on the tip or back of various parts of the grass spikelet." [APWeb:Glossary]
subset: reference
relationship: part_of PO:0009037 ! lemma

[Term]
id: PO:0006033
name: paleal apiculus
namespace: plant_structure
def: "A short\, abrupt\, flexible point present at the apex of the palea" [GR:pj]
subset: reference
synonym: "apiculus" []
relationship: part_of PO:0009038 ! palea

[Term]
id: PO:0006034
name: leaflet margin
namespace: plant_structure
def: "The margin or edges of the leaflet." [GR:pj]
relationship: part_of PO:0020049 ! leaflet

[Term]
id: PO:0006035
name: shoot epidermis
namespace: plant_structure
def: "Outer layer of the shoot organs." [GR:pj, ISBN:047124529]
comment: Often interrupted by stomata and other structures. The shoot epidermis is different from the root epidermis in its origin\, function and structure.
is_a: PO:0005679 ! epidermis

[Term]
id: PO:0006036
name: root epidermis
alt_id: PO:0006037
namespace: plant_structure
def: "The outermost primary cell layer of the root." [ISBN:0080374913]
comment: The root epidermis is different from the shoot epidermis in its origin\, function and structure.
synonym: "epiblem" []
synonym: "rhizodermis" []
is_a: PO:0005679 ! epidermis
relationship: part_of PO:0009005 ! root

[Term]
id: PO:0006039
name: adventitious root epidermis
alt_id: PO:0006038
namespace: plant_structure
def: "The outer most cell layer of the adventitious root." [GR:pj]
synonym: "crown root epidermis" []
is_a: PO:0006036 ! root epidermis
relationship: part_of PO:0000042 ! shoot borne root

[Term]
id: PO:0006040
name: sepal epidermis
namespace: plant_structure
def: "The outermost cell layer of the sepal." [GR:pj]
is_a: PO:0006035 ! shoot epidermis
relationship: part_of PO:0009031 ! sepal

[Term]
id: PO:0006041
name: petal epidermis
namespace: plant_structure
def: "The epidermal layer of the petal." [GR:pj]
is_a: PO:0006035 ! shoot epidermis
relationship: part_of PO:0009032 ! petal

[Term]
id: PO:0006042
name: velamen
namespace: plant_structure
def: "A multiseriate epidermis found in aerial roots of some monocots. Most of its cells are dead and store water like a sponge." [ISBN:0080374913]
synonym: "velamen radicum" []
is_a: PO:0006036 ! root epidermis

[Term]
id: PO:0006043
name: integument epidermis
namespace: plant_structure
def: "The epidermis of an integument in an ovule." [GR:pj]
is_a: PO:0006035 ! shoot epidermis
relationship: part_of PO:0020021 ! integument

[Term]
id: PO:0006044
name: inner integument epidermis
namespace: plant_structure
def: "The epidermis of the inner integument in an ovule." [GR:pj]
is_a: PO:0006043 ! integument epidermis
relationship: part_of PO:0020022 ! inner integument

[Term]
id: PO:0006045
name: outer integument epidermis
namespace: plant_structure
def: "The epidermis of the outer integument in an ovule." [GR:pj]
is_a: PO:0006043 ! integument epidermis
relationship: part_of PO:0020023 ! outer integument

[Term]
id: PO:0006048
name: seed coat epidermis
namespace: plant_structure
def: "The epidermal layer of the seed coat." [GR:pj]
is_a: PO:0005679 ! epidermis
relationship: part_of PO:0009088 ! seed coat

[Term]
id: PO:0006049
name: scutellum epidermis
namespace: plant_structure
def: "The epidermal layer of the scutellum." [GR:pj]
is_a: PO:0006035 ! shoot epidermis
relationship: part_of PO:0020110 ! scutellum

[Term]
id: PO:0006050
name: exotesta
namespace: plant_structure
def: "That part of the seed coat that develops from the outer surface of the outer integument." [GR:pj]
synonym: "seed coat outer epidermis" []
is_a: PO:0006048 ! seed coat epidermis
relationship: part_of PO:0020057 ! testa

[Term]
id: PO:0006051
name: endotesta
namespace: plant_structure
def: "That part of the seed coat that develops from the inner epidermis of the outer integument." [GR:pj]
synonym: "seed coat inner epidermis" []
is_a: PO:0006048 ! seed coat epidermis
relationship: part_of PO:0020057 ! testa

[Term]
id: PO:0006052
name: petal abaxial epidermis
namespace: plant_structure
def: "The abaxial/lower epidermal cell layer of the petal." [GR:pj]
is_a: PO:0006041 ! petal epidermis

[Term]
id: PO:0006053
name: petal adaxial epidermis
namespace: plant_structure
def: "The adaxial/upper epidermal cell layer of the petal." [GR:pj]
is_a: PO:0006041 ! petal epidermis

[Term]
id: PO:0006054
name: sepal abaxial epidermis
namespace: plant_structure
def: "The abaxial/lower epidermal cell layer of the sepal." [GR:pj]
is_a: PO:0006040 ! sepal epidermis

[Term]
id: PO:0006055
name: sepal adaxial epidermis
namespace: plant_structure
def: "The adaxial/upper epidermal cell layer of the sepal." [GR:pj]
is_a: PO:0006040 ! sepal epidermis

[Term]
id: PO:0006056
name: cotyledon epidermis
namespace: plant_structure
def: "The epidermal cell layer of the cotyledon." [GR:pj]
is_a: PO:0006035 ! shoot epidermis
relationship: part_of PO:0020030 ! cotyledon

[Term]
id: PO:0006057
name: cotyledon abaxial epidermis
namespace: plant_structure
def: "The abaxial/lower epidermal cell layer of the cotyledon." [GR:pj]
is_a: PO:0006056 ! cotyledon epidermis

[Term]
id: PO:0006058
name: cotyledon adaxial epidermis
namespace: plant_structure
def: "The adaxial/upper epidermal cell layer of the cotyledon." [GR:pj]
is_a: PO:0006056 ! cotyledon epidermis

[Term]
id: PO:0006060
name: filament epidermis
namespace: plant_structure
def: "The epidermal cell layer of the stamen filament." [GR:pj]
is_a: PO:0006035 ! shoot epidermis
relationship: part_of PO:0009067 ! filament

[Term]
id: PO:0006061
name: stigma epidermis
namespace: plant_structure
def: "The epidermal cell layer of the stigma." [GR:pj, PMID:11951033]
is_a: PO:0006035 ! shoot epidermis
relationship: part_of PO:0009073 ! stigma

[Term]
id: PO:0006062
name: style epidermis
namespace: plant_structure
def: "The epidermal cell layer of the style." [GR:pj]
synonym: "transmitting tract epidermis" []
is_a: PO:0006035 ! shoot epidermis
relationship: part_of PO:0009074 ! style

[Term]
id: PO:0006063
name: ovary epidermis
namespace: plant_structure
def: "The epidermal cell layer of the ovary." [GR:pj]
is_a: PO:0006035 ! shoot epidermis
relationship: part_of PO:0009072 ! ovary

[Term]
id: PO:0006065
name: hypocotyl endodermis
namespace: plant_structure
def: "It is the innermost layer of the cortex of hypocotyl." [GR:pj]
is_a: PO:0000252 ! endodermis

[Term]
id: PO:0006066
name: petiole parenchyma
namespace: plant_structure
def: "Relatively unspecialized tissue present in the leaf petiole." [GR:pj]
is_a: PO:0005421 ! parenchyma
relationship: part_of PO:0020038 ! petiole

[Term]
id: PO:0006067
name: cambium-like transitional zone
namespace: plant_structure
def: "OBSOLETE. A cup-shaped region in the shoot apical meristem found between the central mother cell and the rib and peripheral zone. The cells of this zone are derived from the corpus intials\, but in some cases they arise also from tunica initials." [ISBN:0080374913]
comment: If found\, this zone is a temporary feature mostly in Gymnosperms.
synonym: "adaxial meristem" []
synonym: "leaf meristem" []
synonym: "ventral meristem" []
is_obsolete: true

[Term]
id: PO:0006068
name: sepal parenchyma
namespace: plant_structure
def: "Relatively unspecialized tissue present in the sepals." [GR:pj]
is_a: PO:0005421 ! parenchyma

[Term]
id: PO:0006069
name: petal parenchyma
namespace: plant_structure
def: "Relatively unspecialized tissue present in the petals." [GR:pj]
is_a: PO:0005421 ! parenchyma

[Term]
id: PO:0006070
name: mesophyll
namespace: plant_structure
def: "The chloroplast-containing\, photosynthetic parenchymatous tissue situated between the two epidermal layers of the leaf or leaf like organs." [GR:pj]
is_a: PO:0005426 ! chlorenchyma

[Term]
id: PO:0006071
name: petal mesophyll
namespace: plant_structure
def: "The chloroplast-containing\, photosynthetic parenchymatous tissue situated between the two epidermal layers of the petal." [GR:pj]
is_a: PO:0006069 ! petal parenchyma
is_a: PO:0006070 ! mesophyll

[Term]
id: PO:0006072
name: sepal mesophyll
namespace: plant_structure
def: "The chloroplast-containing\, photosynthetic parenchymatous tissue situated between the two epidermal layers of the sepal." [GR:pj]
is_a: PO:0006068 ! sepal parenchyma
is_a: PO:0006070 ! mesophyll

[Term]
id: PO:0006073
name: intercalary meristem
namespace: plant_structure
def: "Meristematic tissue separated from the apical meristem in the primary body by more or less mature tissues." [ISBN:0080374913, ISBN:0122151704]
is_a: PO:0006079 ! shoot meristem
is_a: PO:0009013 ! meristem

[Term]
id: PO:0006074
name: procambium
namespace: plant_structure
def: "A primary cambium which undergoes differentiation to form the primary vascular tissue." [ISBN:0080374913]
relationship: part_of PO:0020144 ! apical meristem

[Term]
id: PO:0006075
name: primary phloem
namespace: plant_structure
def: "The phloem of the primary plant body." [ISBN:0122151704]
comment: In stem or root it is differentiated behind the apical meristem.
is_a: PO:0005417 ! phloem

[Term]
id: PO:0006076
name: metaphloem
namespace: plant_structure
def: "Part of the primary phloem that differentiates after the protophloem and before the secondary phloem\, if any of the latter is formed." [ISBN:0471245194]
relationship: part_of PO:0006075 ! primary phloem

[Term]
id: PO:0006077
name: protophloem
namespace: plant_structure
def: "The first-formed elements of the primary phloem." [ISBN:0471245194]
relationship: part_of PO:0006075 ! primary phloem

[Term]
id: PO:0006078
name: primary vascular tissue
namespace: plant_structure
def: "OBSOLETE. The vascular tissue of the primary plant body at the embryonic stage. " [GR:pj]
comment: Redundant to sec ...
is_obsolete: true

[Term]
id: PO:0006079
name: shoot meristem
namespace: plant_structure
def: "Meristem found in a shoot." [GR:pj]
is_a: PO:0009013 ! meristem
relationship: part_of PO:0009006 ! shoot

[Term]
id: PO:0006080
name: secondary vascular tissue
namespace: plant_structure
def: "OBSOLETE. The vascular tissue derived from the vascular cambium because of the secondary growth." [GR:pj]
comment: Redundant sec phloem and xylem
is_obsolete: true

[Term]
id: PO:0006081
name: primary root apical meristem
namespace: plant_structure
def: "Meristem found in the apex of the primary root." [GR:pj]
synonym: "apical meristem of primary root" []
synonym: "embryonic root meristem" []
is_a: PO:0020147 ! root apical meristem
relationship: part_of PO:0000026 ! primary root tip
relationship: part_of PO:0020031 ! radicle

[Term]
id: PO:0006082
name: abaxial protoderm
namespace: plant_structure
def: "The outermost layer of the shoot apical meristem which gives rise to the abaxial/lower leaf epidermis. " [ISBN:0080374913, GR:pj]
is_a: PO:0006210 ! protoderm

[Term]
id: PO:0006083
name: adaxial protoderm
namespace: plant_structure
def: "The outermost layer of the shoot apical meristem which gives rise to the adaxial/upper leaf epidermis." [ISBN:0080374913, GR:pj]
is_a: PO:0006210 ! protoderm

[Term]
id: PO:0006084
name: transfusion tissue
namespace: plant_structure
def: "Tissue consisting of tracheids and parenchyma cells\, associated with the vascular bundle." [ISBN:0080374913]
comment: Found generally in gymnosperm leaves.
is_a: PO:0009007 ! tissue

[Term]
id: PO:0006085
name: root meristem
alt_id: PO:0003001
namespace: plant_structure
def: "Meristem found in a root." [GR:pj]
synonym: "meristematic zone" []
is_a: PO:0009013 ! meristem
relationship: part_of PO:0009005 ! root

[Term]
id: PO:0006086
name: accessory transfusion tissue
namespace: plant_structure
def: "OBSOLETE. The accessory tissue extending laterally into the mesophyll rather than remaining associated with the vascular bundles." [ISBN:0080374913]
comment: Not in current literature.
is_obsolete: true

[Term]
id: PO:0006087
name: proliferation tissue
namespace: plant_structure
def: "OBSOLETE. Tissue that develops from phloem parenchyma in the outer portion of the inner bark accommodating the expansion in circumference." [ISBN:0080374913]
comment: check the definition.
is_obsolete: true

[Term]
id: PO:0006088
name: primary sporogenous cell
namespace: plant_structure
def: "It is formed by the division of the male archesporial initial. After several mitotic divisions these cells differentiate into pollen mother cells." [PMID:12897248]
is_a: PO:0009002 ! plant cell
relationship: develops_from PO:0006014 ! male archesporial cell

[Term]
id: PO:0006089
name: anther primordium
namespace: plant_structure
def: "An organized group of cells that will differentiate into anther. " [GR:pj]
is_a: PO:0009066 ! anther

[Term]
id: PO:0006090
name: organogenic callus
namespace: plant_structure
def: "A type of cultured callus that has competence to form any organ such as root\, leaf\, shoot\, leafless shoot or bare stem\, etc." [POC:curators]
synonym: "meristematic callus" []
is_a: PO:0000009 ! cultured callus

[Term]
id: PO:0006091
name: embryogenic callus
namespace: plant_structure
def: "A type of cultured callus that form embryo-like structures such as somatic embryos." [POC:curators]
is_a: PO:0000009 ! cultured callus

[Term]
id: PO:0006109
name: pith
namespace: plant_structure
def: "Non-vascular tissue in the center of stem or root" [ISBN:0080280307]
is_a: PO:0009007 ! tissue

[Term]
id: PO:0006200
name: fascicular cambium
namespace: plant_structure
def: "Vascular cambium  originating from procambium within vascular bundles or fascicles." [ISBN:047124529]
is_a: PO:0005598 ! vascular cambium

[Term]
id: PO:0006201
name: interfascicular cambium
namespace: plant_structure
def: "Vascular cambium arising between vascular bundles or fascicles\, in the interfascicular parenchyma or pith." [ISBN:047124529]
is_a: PO:0005598 ! vascular cambium

[Term]
id: PO:0006202
name: interfascicular region
namespace: plant_structure
def: "Region located between vascular bundles in the stem. " [ISBN:047124529]
comment: Check for the relationship. Inapplicable for nearly all monocots.
synonym: "medullary ray" []
synonym: "pith ray" []
is_a: PO:0006109 ! pith
relationship: part_of PO:0009047 ! stem

[Term]
id: PO:0006203
name: pericycle
namespace: plant_structure
def: "Part of the tissue of the stele located between the phloem and endodermis." [ISBN:047124529]
subset: reference
is_a: PO:0009007 ! tissue
relationship: part_of PO:0020124 ! root stele

[Term]
id: PO:0006204
name: sporocyte
namespace: plant_structure
def: "A diploid (2n) cell that undergoes meiosis and produces four haploid (1n) spores." [GR:pj]
is_a: PO:0009002 ! plant cell

[Term]
id: PO:0006205
name: spongy mesophyll cell
namespace: plant_structure
def: "Irregularly-shaped\, chlorenchymatous cell\, separated by large air spaces. " [GR:pj]
comment: Usually found in the abaxial/lower part of the leaf mesophyll as in a dorsiventral leaf\, but between two palisade parenchyma layers in an isobilateral leaf.
synonym: "spongy parenchyma cell" []
is_a: PO:0004006 ! mesophyll cell
relationship: part_of PO:0005647 ! spongy mesophyll

[Term]
id: PO:0006206
name: palisade mesophyll cell
namespace: plant_structure
def: "Elongated chlorenchymatous cell oriented perpendicular to the leaf surface and which is active in photosynthesis." [GR:pj]
comment: Usually found in the adaxil/upper part of the leaf mesophyll.
synonym: "palisade parenchyma cell" []
is_a: PO:0004006 ! mesophyll cell
relationship: part_of PO:0005648 ! palisade mesophyll

[Term]
id: PO:0006207
name: exodermal passage cell
namespace: plant_structure
def: "A short cell in the dimorphic type of exodermis with cell wall that remains non-thickened." [TAIR:ki, PMID:11709575]
is_a: PO:0000353 ! passage cell
relationship: part_of PO:0005772 ! exodermis

[Term]
id: PO:0006208
name: endodermal passage cell
namespace: plant_structure
def: "Cell in the endodermal layer of the root with cell wall that remains non-thickened." [TAIR:ki]
is_a: PO:0000353 ! passage cell
relationship: part_of PO:0000252 ! endodermis

[Term]
id: PO:0006209
name: lateral root epidermis
namespace: plant_structure
def: "OBSOLETE. The outer most cell layer of the lateral roots." [GR:pj]
is_obsolete: true

[Term]
id: PO:0006210
name: protoderm
namespace: plant_structure
def: "The undifferentiated surface cell layer of the primary plant body\, which gives rise to epidermis." [ISBN:047124529, GR:pj]
comment: It may or may not arise from independent initials.  Some researchers also call it an epidermis in meristematic state.
relationship: part_of PO:0009013 ! meristem

[Term]
id: PO:0006211
name: separation layer
namespace: plant_structure
def: "Cells that develop an abnormal wall chemistry and swelling resulting in easily being pulled apart along the pectin-rich middle lamella; directly involved in the weakening process of abscission." [ISBN:0122151704]
relationship: part_of PO:0000146 ! abscission zone

[Term]
id: PO:0006212
name: protective layer
namespace: plant_structure
def: "The layer of cells in the abscission zone that have lignin and suberin depositions and are found on the axial side of the break or exposed surface of abscission." [ISBN:0122151704]
relationship: part_of PO:0000146 ! abscission zone

[Term]
id: PO:0006213
name: root aerenchyma
namespace: plant_structure
def: "Parenchyma tissue containing particularly large intercellular spaces in the tissue of roots." [GR:pj]
is_a: PO:0005702 ! aerenchyma
relationship: part_of PO:0009005 ! root

[Term]
id: PO:0006214
name: stem aerenchyma
namespace: plant_structure
def: "Parenchyma tissue containing particularly large intercellular spaces." [GR:pj]
is_a: PO:0005702 ! aerenchyma
relationship: part_of PO:0009047 ! stem

[Term]
id: PO:0006215
name: leaf aerenchyma
namespace: plant_structure
def: "Spongy parenchyma tissue containing particularly large intercellular spaces in the leaf mesophyll. " [GR:pj]
is_a: PO:0005702 ! aerenchyma
relationship: part_of PO:0009025 ! leaf

[Term]
id: PO:0006216
name: internal phloem
namespace: plant_structure
def: "Primary phloem tissue positioned internal to the primary xylem" [ISBN:0122151704]
synonym: "intraxylary phloem" []
is_a: PO:0006075 ! primary phloem

[Term]
id: PO:0006218
name: exotegmen
namespace: plant_structure
def: "That part of the seed coat that develops from the outer surface of the inner integument." [GR:pj]
is_a: PO:0006048 ! seed coat epidermis
relationship: part_of PO:0020056 ! tegmen

[Term]
id: PO:0006219
name: endotegmen
namespace: plant_structure
def: "That part of the seed coat that develops from the inner epidermis of the inner integument." [GR:pj]
is_a: PO:0006048 ! seed coat epidermis
relationship: part_of PO:0020056 ! tegmen

[Term]
id: PO:0006220
name: central endosperm
namespace: plant_structure
def: "The central region of the endosperm composed of cells that are significantly larger than those at the periphery\, especially the aleurone and sub-aleurone layers." [TAIR:ki]
comment: Also called starchy endosperm region (characteristic of some grasses).
is_a: PO:0009089 ! endosperm

[Term]
id: PO:0006221
name: articulated laticifer cell
namespace: plant_structure
def: "Latex-containing cells in which the walls between contiguous cells may partly or completely disappear." [ISBN:0471245208, TAIR:ki]
synonym: "laticiferous vessel" []
is_a: PO:0009002 ! plant cell
relationship: part_of PO:0005006 ! articulated laticifer

[Term]
id: PO:0006222
name: non-articulated laticifer cell
namespace: plant_structure
def: "Latex-containing cell that elongates indefinitely and grows intrusively between the walls of meristematic cells." [PMID:11732189]
synonym: "simple laticifer" []
is_a: PO:0009002 ! plant cell
relationship: part_of PO:0005007 ! non-articulated laticifer

[Term]
id: PO:0006300
name: obsolete plant structure
namespace: plant_structure
def: "OBSOLETE. The instances of this parent term are those anatomical terms which have become obsolete." [GR:pj]
is_obsolete: true

[Term]
id: PO:0006301
name: corpus
namespace: plant_structure
def: "OBSOLETE. Group of cells located beneath anticlinally dividing peripheral layers (tunica) and dividing in many planes. In apical shoot meristem. Such division cause the increase in the volume of shoot." [ISBN:0080374913, GR:pj]
comment: The term has been made obsolete because this concept is used in a very loose sense.
is_obsolete: true

[Term]
id: PO:0006302
name: tunica
namespace: plant_structure
def: "OBSOLETE. The outermost layer or layers in the shoot apical meristem of the Angiosperms in which the plane of division is almost anticlinal. This layer contributes to surface growth." [ISBN:047124529, GR:pj]
comment: The term has been made obsolete because this concept is used in a very loose sense.
is_obsolete: true

[Term]
id: PO:0006303
name: L1
namespace: plant_structure
def: "OBSOLETE. The outer layer of the tunica." [GR:pj]
comment: A similar term L1 meristem (PO\:0009020) occurs.
is_obsolete: true

[Term]
id: PO:0006304
name: L2
namespace: plant_structure
def: "OBSOLETE. The second layer of the tunica." [GR:pj]
comment: A similar term L2 meristem (PO\:0009021) occurs.
is_obsolete: true

[Term]
id: PO:0006305
name: L3
namespace: plant_structure
def: "OBSOLETE. The innermost layer of the tunica." [GR:pj]
comment: A similar term L3 meristem (PO\:0009022) occurs.
is_obsolete: true

[Term]
id: PO:0006306
name: shoot procambium
namespace: plant_structure
def: "A derivative of the apical meristem which undergoes differentiation to form the primary vascular tissue of a shoot." [GR:pj]
is_a: PO:0006074 ! procambium
relationship: part_of PO:0020148 ! shoot apical meristem

[Term]
id: PO:0006307
name: root procambium
namespace: plant_structure
def: "A derivative of the apical meristem which undergoes differentiation to form the primary vascular tissue of a root." [GR:pj]
is_a: PO:0006074 ! procambium
relationship: part_of PO:0006085 ! root meristem

[Term]
id: PO:0006308
name: root lateral meristem
namespace: plant_structure
def: "Meristem of the root located parallel to the sides of the axis." [ISBN:047124529]
comment: Generally causes root thickening. Not to be confused with lateral root meristem\, which is the meristem of the lateral root.
is_a: PO:0006085 ! root meristem
is_a: PO:0020145 ! lateral meristem
relationship: part_of PO:0020121 ! lateral root

[Term]
id: PO:0006309
name: tassel spikelet
namespace: plant_structure
def: "Ultimate inflorescence branch of the maize tassel." [GR:pj]
is_a: PO:0009051 ! spikelet
relationship: part_of PO:0020126 ! tassel

[Term]
id: PO:0006310
name: tassel floret
namespace: plant_structure
def: "Flowers of the spikelets of maize tassel." [GR:pj]
is_a: PO:0006318 ! floret (sensu Poaceae)
relationship: part_of PO:0006309 ! tassel spikelet

[Term]
id: PO:0006311
name: tassel sessile spikelet
namespace: plant_structure
def: "Ultimate inflorescence branch of the maize tassel without a pedicel\, developing from the spikelet pair meristem." [GR:pj]
is_a: PO:0006309 ! tassel spikelet

[Term]
id: PO:0006312
name: tassel pedicellate spikelet
namespace: plant_structure
def: "Ultimate inflorescence branch of the maize tassel with a pedicel\, developing from the spikelet pair meristem." [GR:pj]
is_a: PO:0006309 ! tassel spikelet

[Term]
id: PO:0006313
name: lower floret of pedicellate spikelet of tassel
namespace: plant_structure
def: "The lower of the two florets of the pedicellate spikelet of a maize tassel." [GR:pj]
is_a: PO:0006310 ! tassel floret
relationship: part_of PO:0006312 ! tassel pedicellate spikelet

[Term]
id: PO:0006314
name: upper floret of pedicellate spikelet of tassel
namespace: plant_structure
def: "One of the two florets placed above the lower floret on the pedicellate spikelet rachilla of a maize tassel " [GR:pj]
is_a: PO:0006310 ! tassel floret
relationship: part_of PO:0006312 ! tassel pedicellate spikelet

[Term]
id: PO:0006315
name: lower floret of sessile spikelet of tassel
namespace: plant_structure
def: "The lower of the two florets of the sessile spikelet of a maize tassel." [GR:pj]
is_a: PO:0006310 ! tassel floret
relationship: part_of PO:0006311 ! tassel sessile spikelet

[Term]
id: PO:0006316
name: upper floret of sessile spikelet of tassel
namespace: plant_structure
def: "One of the two florets placed above the lower floret on the sessile spikelet rachilla of a maize tassel." [GR:pj]
is_a: PO:0006310 ! tassel floret
relationship: part_of PO:0006311 ! tassel sessile spikelet

[Term]
id: PO:0006317
name: gynoecium of tassel floret
namespace: plant_structure
def: "Collectively the carpels of a maize tassel floret. " [GR:pj]
comment: The development of the gynoecium in the tassel floret of a normal maize plant is aborted and is present in a rudimentary state.
is_a: PO:0006357 ! gynoecium (sensu Zea)
relationship: part_of PO:0006310 ! tassel floret

[Term]
id: PO:0006318
name: floret (sensu Poaceae)
namespace: plant_structure
def: "Small flowers of the spikelets of Poaceae." [Poc:curators]
comment: It is not clear what the lemma\, palea and lodicule correspond to in conventional flowers\, therefore we are not making any assumptions of homology at the present time.
subset: reference
is_a: PO:0009082 ! floret
relationship: part_of PO:0009051 ! spikelet

[Term]
id: PO:0006319
name: spikelet pedicel
namespace: plant_structure
def: "Inflorescence branch that terminates in a spikelet." [Poc:curators]
comment: This is not a pedicel in the strict sense\, but is the ultimate naked part of the inflorescence axis.
is_a: PO:0009052 ! pedicel
relationship: part_of PO:0009051 ! spikelet

[Term]
id: PO:0006320
name: ear spikelet
namespace: plant_structure
def: "Ultimate inflorescence branch of the maize ear." [GR:pj]
is_a: PO:0009051 ! spikelet
relationship: part_of PO:0020136 ! ear (sensu Zea)

[Term]
id: PO:0006321
name: second order inflorescence branch
namespace: plant_structure
def: "Any branch forming from the primary or first order inflorescence branch." [GR:pj]
synonym: "primary branch" []
is_a: PO:0009081 ! inflorescence branch

[Term]
id: PO:0006322
name: third order inflorescence branch
namespace: plant_structure
def: "Any branch forming from the second order inflorescence branch." [GR:pj]
synonym: "secondary inflorescence branch" []
is_a: PO:0009081 ! inflorescence branch

[Term]
id: PO:0006323
name: tassel branch
namespace: plant_structure
def: "Any branch forming from the primary or higher order tassel axes." [GR:pj]
is_a: PO:0006321 ! second order inflorescence branch
relationship: part_of PO:0020126 ! tassel

[Term]
id: PO:0006324
name: central spike of tassel
namespace: plant_structure
def: "The inflorescence axis of the tassel." [GR:pj]
synonym: "tassel rachis" []
is_a: PO:0020122 ! inflorescence axis
relationship: part_of PO:0020126 ! tassel

[Term]
id: PO:0006325
name: inflorescence node
namespace: plant_structure
def: "The region of the inflorescence axis where the spikelet\, flower\, floret or the branch is attached." [GR:pj]
is_a: PO:0005004 ! shoot node
relationship: part_of PO:0020122 ! inflorescence axis

[Term]
id: PO:0006326
name: inflorescence internode
namespace: plant_structure
def: "The region of rachis present between the two nodes." [GR:pj]
is_a: PO:0005005 ! shoot internode
relationship: part_of PO:0020122 ! inflorescence axis

[Term]
id: PO:0006327
name: spikelet meristem
namespace: plant_structure
def: "Apical meristem that gives rise to the two or more florets of a grass inflorescence." [GR:pj]
is_a: PO:0000230 ! inflorescence meristem
relationship: part_of PO:0009051 ! spikelet

[Term]
id: PO:0006328
name: spikelet pair meristem
namespace: plant_structure
def: "The meristem that produces two spikelet meristems\, each of which produces two floral meristems." [GR:pj]
comment: Found in some grass inflorescences.
is_a: PO:0006327 ! spikelet meristem
relationship: part_of PO:0009049 ! inflorescence

[Term]
id: PO:0006329
name: floret meristem (sensu Poaceae)
namespace: plant_structure
def: "Meristem that gives rise to the organs of a floret of a grass plant." [GR:pj]
is_a: PO:0000229 ! floral meristem
relationship: part_of PO:0009051 ! spikelet

[Term]
id: PO:0006330
name: gynophore
namespace: plant_structure
def: "The stalk at the base of the ovary." [Poc:curators]
comment: Typically receptacular in origin.
subset: reference
relationship: part_of PO:0009062 ! gynoecium

[Term]
id: PO:0006331
name: seed raphe
namespace: plant_structure
def: "The ridge along the body of the seed formed from the part of funiculus that was adnate to the ovule." [ISBN:047124529]
relationship: develops_from PO:0020027 ! raphe
relationship: part_of PO:0009010 ! seed

[Term]
id: PO:0006332
name: seed funicle
namespace: plant_structure
def: "Remnants of the funicle from ovary where it attaches the ovule to the placenta." [GR:pj]
relationship: develops_from PO:0020006 ! funicle
relationship: part_of PO:0009010 ! seed

[Term]
id: PO:0006333
name: seed chalaza
namespace: plant_structure
def: "Remnant of the ovular chalaza which is a region in the ovule where the integuments and the nucellus merge with the funiculus. " [GR:pj]
relationship: develops_from PO:0020026 ! chalaza
relationship: part_of PO:0009010 ! seed

[Term]
id: PO:0006334
name: seed micropyle
namespace: plant_structure
def: "A pore on the seed coat which is a remnant of the ovular micropyle." [GR:pj]
relationship: develops_from PO:0020025 ! micropyle
relationship: part_of PO:0009010 ! seed

[Term]
id: PO:0006336
name: seed obturator
namespace: plant_structure
def: "An outgrowth of the seed funicle\, that forms a bridge between the seed micropyle and other tissues. It is also a remnant form of the obturator found in the ovular funicle." [GR:pj]
relationship: develops_from PO:0020029 ! obturator
relationship: part_of PO:0006332 ! seed funicle

[Term]
id: PO:0006337
name: inflorescence bract of ear
namespace: plant_structure
def: "The leaf subtending an ear of corn and acting as outer envelope of the ear." [GR:pj]
synonym: "corn husk" []
synonym: "husk leaf" []
is_a: PO:0009054 ! inflorescence bract
relationship: part_of PO:0020136 ! ear (sensu Zea)

[Term]
id: PO:0006338
name: embryonic leaf
namespace: plant_structure
def: "The first few leaves developing from the embryonic shoot apical meristem." [GR:pj]
is_a: PO:0009025 ! leaf
relationship: part_of PO:0009009 ! embryo

[Term]
id: PO:0006339
name: juvenile leaf
namespace: plant_structure
def: "Distinct from adult leaves\, being characterized by particular anatomical traits namely\, wax and trichome distribution\, presence or absence of epidermal cell types\, cell wall shape and biochemistry." [MaizeGDB:lv, GR:pj]
comment: The first juvenile leaves are e.g. the embryonic leaves found in the grass kernel (caryopsis).
is_a: PO:0009025 ! leaf

[Term]
id: PO:0006340
name: adult leaf
namespace: plant_structure
def: "Adult leaves are characterized by particular anatomical traits namely\, wax and trichome distribution\, presence or absence of epidermal cell types\, cell wall shape and biochemistry." [GR:pj, MaizeGDB:lv]
comment: The adult leaves are placed above the juvenile (oldest) leaves. However in some plants the juvenile leaves may go on to establish as adult leaves.
is_a: PO:0009025 ! leaf

[Term]
id: PO:0006341
name: primary shoot
namespace: plant_structure
def: "The shoot developing from the embryonic shoot apical meristem." [UMSL:fz]
synonym: "main stalk" []
is_a: PO:0009006 ! shoot

[Term]
id: PO:0006342
name: infructescence
namespace: plant_structure
def: "The grouping or arrangement in which fruits are borne on a plant." [GR:pj]
relationship: part_of PO:0009003 ! sporophyte

[Term]
id: PO:0006343
name: axillary shoot
namespace: plant_structure
def: "The shoot developing from the axillary bud meristem." [GR:pj]
synonym: "axillary branch" []
is_a: PO:0004545 ! shoot borne shoot

[Term]
id: PO:0006344
name: shoot lateral meristem
namespace: plant_structure
def: "Meristem of the shoot located parallel to the sides of the axis." [Poc:curators]
is_a: PO:0006079 ! shoot meristem
is_a: PO:0020145 ! lateral meristem

[Term]
id: PO:0006345
name: pollen tube
namespace: plant_structure
def: "A tubular cell extension formed by the germinating pollen grain; carries the male gametes into the ovule." [ISBN:0471245208]
subset: reference
relationship: part_of PO:0020091 ! male gametophyte

[Term]
id: PO:0006346
name: leaf intercalary meristem
namespace: plant_structure
def: "The meristematic tissue in the primary body of the leaf separated from the apical meristem by non-meristematic tissues." [GR:pj]
is_a: PO:0006073 ! intercalary meristem
relationship: part_of PO:0009025 ! leaf

[Term]
id: PO:0006347
name: stem intercalary meristem
namespace: plant_structure
def: "Meristematic tissue in the primary body of stem separated from the apical meristem by more or less mature tissues." [GR:pj]
is_a: PO:0006073 ! intercalary meristem
relationship: part_of PO:0009047 ! stem

[Term]
id: PO:0006348
name: ear pedicellate spikelet
namespace: plant_structure
def: "Ultimate pedicellate inflorescence branch of the maize ear that develops from the spikelet pair meristem." [GR:pj]
is_a: PO:0006320 ! ear spikelet

[Term]
id: PO:0006349
name: ear sessile spikelet
namespace: plant_structure
def: "Ultimate sessile inflorescence branch of the maize ear that develops from the spikelet pair meristem." [GR:pj]
is_a: PO:0006320 ! ear spikelet

[Term]
id: PO:0006350
name: upper floret of pedicellate spikelet of ear
namespace: plant_structure
def: "The uppermost of the two florets of the pedicellate spikelet rachilla of a maize ear. The upper floret on the ear usually develops into a functional one." [GR:pj]
is_a: PO:0006354 ! ear floret
relationship: part_of PO:0006348 ! ear pedicellate spikelet

[Term]
id: PO:0006351
name: lower floret of sessile spikelet of ear
namespace: plant_structure
def: "The lower of the two florets on the sessile spikelet of a maize ear." [GR:pj]
comment: This floret does not usually develop into a functional one.
is_a: PO:0006354 ! ear floret
relationship: part_of PO:0006349 ! ear sessile spikelet

[Term]
id: PO:0006352
name: upper floret of sessile spikelet of ear
namespace: plant_structure
def: "One of the two florets placed above the lower floret on the sessile spikelet rachilla of a maize ear. This floret usually develops into a functional one." [GR:pj]
is_a: PO:0006354 ! ear floret
relationship: part_of PO:0006349 ! ear sessile spikelet

[Term]
id: PO:0006353
name: lower floret of pedicellate spikelet of ear
namespace: plant_structure
def: "The lower of the two florets of the pedicellate spikelet rachilla of a maize ear." [GR:pj]
comment: The lower floret on the ear does not usually develop into a functional one.
is_a: PO:0006354 ! ear floret
relationship: part_of PO:0006348 ! ear pedicellate spikelet

[Term]
id: PO:0006354
name: ear floret
namespace: plant_structure
def: "Small flowers of the spikelets of maize ear." [GR:pj]
is_a: PO:0006318 ! floret (sensu Poaceae)
relationship: part_of PO:0006320 ! ear spikelet

[Term]
id: PO:0006355
name: androecium of ear floret
namespace: plant_structure
def: "Collectively the stamens of maize ear floret. " [GR:pj]
comment: The development of the androecium in the ear floret of a normal maize plant is aborted and is present in a rudimentary state.
is_a: PO:0006471 ! androecium (sensu Zea)
relationship: part_of PO:0006354 ! ear floret

[Term]
id: PO:0006356
name: lemma of tassel floret
namespace: plant_structure
def: "The lower of the two bracts enclosing a flower in a maize tassel floret." [GR:pj]
is_a: PO:0009037 ! lemma
relationship: part_of PO:0006310 ! tassel floret

[Term]
id: PO:0006357
name: gynoecium (sensu Zea)
namespace: plant_structure
def: "Collectively the carpels of a maize floret." [GR:pj]
is_a: PO:0006384 ! gynoecium (sensu Poaceae)

[Term]
id: PO:0006358
name: tassel spikelet pair meristem
namespace: plant_structure
def: "The meristem that produces two spikelet meristems\, each of which produces two floral meristems in a maize tassel." [GR:pj]
is_a: PO:0006328 ! spikelet pair meristem

[Term]
id: PO:0006359
name: palea of tassel floret
namespace: plant_structure
def: "In a maize tassel floret\, the upper of the two bracts enclosing a flower." [GR:pj]
is_a: PO:0009038 ! palea
relationship: part_of PO:0006310 ! tassel floret

[Term]
id: PO:0006360
name: ear spikelet pair meristem
namespace: plant_structure
def: "Apical meristem that produces two spikelet meristems\, each of which produces two floral meristems in a maize ear." [GR:pj]
is_a: PO:0006328 ! spikelet pair meristem

[Term]
id: PO:0006361
name: palea of ear floret
namespace: plant_structure
def: "In a maize ear floret\, the upper of the two bracts enclosing a flower." [GR:pj]
is_a: PO:0009038 ! palea
relationship: part_of PO:0006354 ! ear floret

[Term]
id: PO:0006362
name: embryonic shoot apical meristem
namespace: plant_structure
def: "Meristem at the apex of the embryonic axis." [GR:pj]
is_a: PO:0020148 ! shoot apical meristem
relationship: part_of PO:0019018 ! embryo axis

[Term]
id: PO:0006363
name: lemma of ear floret
namespace: plant_structure
def: "The lower of the two bracts enclosing a flower in a maize ear floret." [GR:pj]
is_a: PO:0009037 ! lemma
relationship: part_of PO:0006354 ! ear floret

[Term]
id: PO:0006365
name: gynoecium of ear floret
namespace: plant_structure
def: "Collectively the carpels of a maize ear floret." [GR:pj]
is_a: PO:0006357 ! gynoecium (sensu Zea)
relationship: part_of PO:0006354 ! ear floret

[Term]
id: PO:0006366
name: androecium of tassel floret
namespace: plant_structure
def: "Collectively the stamens of one floret of a tassel inflorescence of maize." [GR:pj]
is_a: PO:0006471 ! androecium (sensu Zea)
relationship: part_of PO:0006310 ! tassel floret

[Term]
id: PO:0006367
name: glume of ear spikelet
namespace: plant_structure
def: "A bract in the ear inflorescence of a maize plant\, subtending two florets." [GR:pj]
is_a: PO:0009039 ! glume
relationship: part_of PO:0006320 ! ear spikelet

[Term]
id: PO:0006368
name: glume of tassel spikelet
namespace: plant_structure
def: "A bract in the tassel inflorescence of a maize plant\, subtending two florets." [GR:pj]
is_a: PO:0009039 ! glume
relationship: part_of PO:0006309 ! tassel spikelet

[Term]
id: PO:0006369
name: lower glume of ear spikelet
namespace: plant_structure
def: "The proximal/basal of the two glumes in the ear spikelet." [GR:pj]
is_a: PO:0006002 ! lower glume
is_a: PO:0006367 ! glume of ear spikelet

[Term]
id: PO:0006370
name: upper glume of tassel spikelet
namespace: plant_structure
def: "The apical/distal of the two glumes in the tassel spikelet." [GR:pj]
is_a: PO:0006004 ! upper glume
is_a: PO:0006368 ! glume of tassel spikelet

[Term]
id: PO:0006371
name: upper glume of ear spikelet
namespace: plant_structure
def: "TThe apical/distal of the two glumes in the ear spikelet." [GR:pj]
is_a: PO:0006004 ! upper glume
is_a: PO:0006367 ! glume of ear spikelet

[Term]
id: PO:0006372
name: lower glume of tassel spikelet
namespace: plant_structure
def: "The proximal/basal of the two glumes in the tassel spikelet." [GR:pj]
is_a: PO:0006002 ! lower glume
is_a: PO:0006368 ! glume of tassel spikelet

[Term]
id: PO:0006373
name: ear floret meristem
namespace: plant_structure
def: "Apical shoot meristem that gives rise to the organs of a maize ear floret." [GR:pj]
is_a: PO:0006329 ! floret meristem (sensu Poaceae)
relationship: part_of PO:0006320 ! ear spikelet

[Term]
id: PO:0006374
name: tassel floret meristem
namespace: plant_structure
def: "Apical meristem that gives rise to the organs of a maize tassel floret." [GR:pj]
is_a: PO:0006329 ! floret meristem (sensu Poaceae)
relationship: part_of PO:0006309 ! tassel spikelet

[Term]
id: PO:0006375
name: ear meristem
namespace: plant_structure
def: "Apical shoot meristem that gives rise to the maize ear." [GR:pj]
is_a: PO:0000230 ! inflorescence meristem
relationship: part_of PO:0020136 ! ear (sensu Zea)

[Term]
id: PO:0006376
name: tassel meristem
namespace: plant_structure
def: "Apical meristem that gives rise to the tassel inflorescence." [GR:pj]
is_a: PO:0000230 ! inflorescence meristem
relationship: part_of PO:0020126 ! tassel

[Term]
id: PO:0006377
name: tassel spikelet meristem
namespace: plant_structure
def: "Apical meristem that gives rise to the upper and lower florets of the maize tassel spikelets. " [GR:pj]
is_a: PO:0006327 ! spikelet meristem
relationship: part_of PO:0020126 ! tassel

[Term]
id: PO:0006378
name: ear spikelet meristem
namespace: plant_structure
def: "Apical meristem that gives rise to the upper and lower florets of the maize ear spikelets." [GR:pj]
is_a: PO:0006327 ! spikelet meristem
relationship: part_of PO:0020136 ! ear (sensu Zea)

[Term]
id: PO:0006379
name: tassel spikelet rachilla
namespace: plant_structure
def: "The axis of the tassel spikelet\, above the glumes." [GR:pj]
is_a: PO:0009080 ! spikelet rachilla
relationship: part_of PO:0006309 ! tassel spikelet

[Term]
id: PO:0006380
name: ear spikelet rachilla
namespace: plant_structure
def: "The axis of the ear spikelet\, above the glumes. " [GR:pj]
is_a: PO:0009080 ! spikelet rachilla
relationship: part_of PO:0006320 ! ear spikelet

[Term]
id: PO:0006381
name: lodicule of tassel floret
namespace: plant_structure
def: "In a tassel floret\, one of two or three tiny scales or flaps of tissue outside the stamens\, possibly representing reduced perianth segments." [APWeb:Glossary, GR:pj]
is_a: PO:0009036 ! lodicule
relationship: part_of PO:0006310 ! tassel floret

[Term]
id: PO:0006382
name: lodicule of ear floret
namespace: plant_structure
def: "In a Maize ear floret\, one of two or three tiny scales or flaps of tissue outside the stamens\, possibly representing reduced perianth segments." [APWeb:Glossary, GR:pj]
is_a: PO:0009036 ! lodicule
relationship: part_of PO:0006354 ! ear floret

[Term]
id: PO:0006383
name: androecium (sensu Poaceae)
namespace: plant_structure
def: "Collectively the stamens of one grass floret." [GR:pj]
is_a: PO:0009061 ! androecium
relationship: part_of PO:0006318 ! floret (sensu Poaceae)

[Term]
id: PO:0006384
name: gynoecium (sensu Poaceae)
namespace: plant_structure
def: "Collectively the carpels of a grass floret." [GR:pj]
is_a: PO:0009062 ! gynoecium
relationship: part_of PO:0006318 ! floret (sensu Poaceae)

[Term]
id: PO:0006385
name: lower glume of pedicellate spikelet of tassel
namespace: plant_structure
def: "The proximal/basal of the two glumes in the tassel pedicellate spikelet." [GR:pj]
is_a: PO:0006372 ! lower glume of tassel spikelet
relationship: part_of PO:0006312 ! tassel pedicellate spikelet

[Term]
id: PO:0006386
name: lower glume of sessile spikelet of tassel
namespace: plant_structure
def: "The proximal/basal of the two glumes in the tassel sessile spikelet." [GR:pj]
is_a: PO:0006372 ! lower glume of tassel spikelet
relationship: part_of PO:0006311 ! tassel sessile spikelet

[Term]
id: PO:0006387
name: upper glume of sessile spikelet of tassel
namespace: plant_structure
def: "The apical/distal of the two glumes in a tassel sessile spikelet." [GR:pj]
is_a: PO:0006370 ! upper glume of tassel spikelet
relationship: part_of PO:0006311 ! tassel sessile spikelet

[Term]
id: PO:0006388
name: upper glume of pedicellate spikelet of tassel
namespace: plant_structure
def: "The apical/distal of the two glumes in a tassel pedicellate spikelet." [GR:pj]
is_a: PO:0006370 ! upper glume of tassel spikelet
relationship: part_of PO:0006312 ! tassel pedicellate spikelet

[Term]
id: PO:0006389
name: rachilla of sessile spikelet of tassel
namespace: plant_structure
def: "The axis of the tassel sessile spikelet\, above the glumes." [GR:pj]
is_a: PO:0006379 ! tassel spikelet rachilla
relationship: part_of PO:0006311 ! tassel sessile spikelet
relationship: part_of PO:0006349 ! ear sessile spikelet

[Term]
id: PO:0006390
name: rachilla of pedicellate spikelet of tassel
namespace: plant_structure
def: "The axis of the tassel pedicellate spikelet\, above the glumes." [GR:pj]
is_a: PO:0006379 ! tassel spikelet rachilla
relationship: part_of PO:0006312 ! tassel pedicellate spikelet

[Term]
id: PO:0006391
name: gynoecium of lower floret of sessile spikelet of tassel
namespace: plant_structure
def: "Collectively the carpels of a lower floret of sessile spikelet of maize tassel." [GR:pj]
comment: A non-functional or rudimentary gynoecium.
is_a: PO:0006317 ! gynoecium of tassel floret
relationship: part_of PO:0006315 ! lower floret of sessile spikelet of tassel

[Term]
id: PO:0006392
name: androecium of upper floret of sessile spikelet of tassel
namespace: plant_structure
def: "Collectively the stamens of upper floret of a sessile spikelet of tassel inflorescence of maize." [GR:pj]
is_a: PO:0006366 ! androecium of tassel floret
relationship: part_of PO:0006316 ! upper floret of sessile spikelet of tassel

[Term]
id: PO:0006393
name: androecium of lower floret of sessile spikelet of tassel
namespace: plant_structure
def: "Collectively the stamens of lower floret of a sessile spikelet of tassel inflorescence of maize." [GR:pj]
is_a: PO:0006366 ! androecium of tassel floret
relationship: part_of PO:0006315 ! lower floret of sessile spikelet of tassel

[Term]
id: PO:0006394
name: gynoecium of upper floret of sessile spikelet of tassel
namespace: plant_structure
def: "Collectively the carpels of a upper floret of sessile spikelet of maize tassel." [GR:pj]
comment: A non-functional or rudimentary gynoecium.
is_a: PO:0006317 ! gynoecium of tassel floret
relationship: part_of PO:0006316 ! upper floret of sessile spikelet of tassel

[Term]
id: PO:0006395
name: lemma of upper floret of sessile spikelet of tassel
namespace: plant_structure
def: "The lower of the two bracts enclosing a flower in a maize tassel sessile spikelet upper floret." [GR:pj]
is_a: PO:0006356 ! lemma of tassel floret
relationship: part_of PO:0006316 ! upper floret of sessile spikelet of tassel

[Term]
id: PO:0006397
name: lemma of lower floret of sessile spikelet of tassel
namespace: plant_structure
def: "The lower of the two bracts enclosing a flower in a maize tassel sessile spikelet lower floret." [GR:pj]
is_a: PO:0006356 ! lemma of tassel floret
relationship: part_of PO:0006315 ! lower floret of sessile spikelet of tassel

[Term]
id: PO:0006399
name: palea of lower floret of sessile spikelet of tassel
namespace: plant_structure
def: "The upper of the two bracts enclosing a flower in a maize tassel sessile spikelet lower floret." [GR:pj]
is_a: PO:0006359 ! palea of tassel floret
relationship: part_of PO:0006315 ! lower floret of sessile spikelet of tassel

[Term]
id: PO:0006401
name: palea of upper floret of sessile spikelet of tassel
namespace: plant_structure
def: "The upper of the two bracts enclosing a flower in a maize tassel sessile spikelet upper floret." [GR:pj]
is_a: PO:0006359 ! palea of tassel floret
relationship: part_of PO:0006316 ! upper floret of sessile spikelet of tassel

[Term]
id: PO:0006403
name: gynoecium of lower floret of pedicellate spikelet of tassel
namespace: plant_structure
def: "Collectively the carpels of a lower floret of pedicellate spikelet of maize tassel." [GR:pj]
comment: A non-functional or rudimentary gynoecium.
is_a: PO:0006317 ! gynoecium of tassel floret
relationship: part_of PO:0006313 ! lower floret of pedicellate spikelet of tassel

[Term]
id: PO:0006404
name: gynoecium of upper floret of pedicellate spikelet of tassel
namespace: plant_structure
def: "Collectively the carpels of a upper floret of pedicellate spikelet of maize tassel." [GR:pj]
comment: A non-functional or rudimentary gynoecium.
is_a: PO:0006317 ! gynoecium of tassel floret
relationship: part_of PO:0006314 ! upper floret of pedicellate spikelet of tassel

[Term]
id: PO:0006405
name: androecium of upper floret of pedicellate spikelet of tassel
namespace: plant_structure
def: "Collectively the stamens of upper floret of a pedicellate spikelet of tassel inflorescence of maize. " [GR:pj]
comment: This consitutes a functional androecium.
is_a: PO:0006366 ! androecium of tassel floret
relationship: part_of PO:0006314 ! upper floret of pedicellate spikelet of tassel

[Term]
id: PO:0006406
name: androecium of lower floret of pedicellate spikelet of tassel
namespace: plant_structure
def: "Collectively the stamens of lower floret of a pedicellate spikelet of tassel inflorescence of maize." [GR:pj]
comment: This consitutes a functional androecium.
is_a: PO:0006366 ! androecium of tassel floret
relationship: part_of PO:0006313 ! lower floret of pedicellate spikelet of tassel

[Term]
id: PO:0006407
name: lemma of lower floret of pedicellate spikelet of tassel
namespace: plant_structure
def: "The lower of the two bracts enclosing a flower in a maize tassel pedicellate spikelet lower floret." [GR:pj]
is_a: PO:0006356 ! lemma of tassel floret
relationship: part_of PO:0006313 ! lower floret of pedicellate spikelet of tassel

[Term]
id: PO:0006409
name: lemma of upper floret of pedicellate spikelet of tassel
namespace: plant_structure
def: "The lower of the two bracts enclosing a flower in a maize tassel pedicellate spikelet upper floret." [GR:pj]
is_a: PO:0006356 ! lemma of tassel floret
relationship: part_of PO:0006314 ! upper floret of pedicellate spikelet of tassel

[Term]
id: PO:0006411
name: palea of lower floret of pedicellate spikelet of tassel
namespace: plant_structure
def: "The upper of the two bracts enclosing a flower in a maize tassel pedicellate spikelet lower floret." [GR:pj]
is_a: PO:0006359 ! palea of tassel floret
relationship: part_of PO:0006313 ! lower floret of pedicellate spikelet of tassel

[Term]
id: PO:0006413
name: palea of upper floret of pedicellate spikelet of tassel
namespace: plant_structure
def: "The upper of the two bracts enclosing a flower in a maize tassel pedicellate spikelet upper floret." [GR:pj]
is_a: PO:0006359 ! palea of tassel floret
relationship: part_of PO:0006314 ! upper floret of pedicellate spikelet of tassel

[Term]
id: PO:0006415
name: pedicel of ear spikelet
namespace: plant_structure
def: "This is the ultimate branch of the pedicellate ear spikelet." [GR:pj]
is_a: PO:0006319 ! spikelet pedicel
relationship: part_of PO:0006348 ! ear pedicellate spikelet

[Term]
id: PO:0006416
name: pedicel of tassel spikelet
namespace: plant_structure
def: "This is the ultimate branch of the pedicellate tassel spikelet." [GR:pj]
is_a: PO:0006319 ! spikelet pedicel
relationship: part_of PO:0006312 ! tassel pedicellate spikelet

[Term]
id: PO:0006417
name: tassel peduncle
namespace: plant_structure
def: "The axis of a maize tassel below the lowest tassel node." [GR:pj]
is_a: PO:0009053 ! peduncle
relationship: part_of PO:0020126 ! tassel

[Term]
id: PO:0006418
name: ear peduncle
namespace: plant_structure
def: "The stalk of a maize ear below the lowest ear node." [GR:pj]
synonym: "lateral branch (sensu Zea)" []
synonym: "shank" []
is_a: PO:0009053 ! peduncle
relationship: part_of PO:0020136 ! ear (sensu Zea)

[Term]
id: PO:0006419
name: androecium of lower floret of pedicellate spikelet of ear
namespace: plant_structure
def: "Collectively the stamens of lower floret of a pedicellate spikelet of maize ear inflorescence." [GR:pj]
comment: The development of the androecium in the ear floret of a normal maize plant is aborted and is present in a rudimentary state.
is_a: PO:0006355 ! androecium of ear floret
relationship: part_of PO:0006353 ! lower floret of pedicellate spikelet of ear

[Term]
id: PO:0006420
name: androecium of lower floret of sessile spikelet of ear
namespace: plant_structure
def: "Collectively the stamens of lower floret of a sessile spikelet of maize ear inflorescence. " [GR:pj]
comment: The development of the androecium in the ear floret of a normal maize plant is aborted and is present in a rudimentary state.
is_a: PO:0006355 ! androecium of ear floret
relationship: part_of PO:0006351 ! lower floret of sessile spikelet of ear

[Term]
id: PO:0006421
name: androecium of upper floret of sessile spikelet of ear
namespace: plant_structure
def: "Collectively the stamens of upper floret of a sessile spikelet of maize ear inflorescence. " [GR:pj]
comment: The development of the androecium in the ear floret of a normal maize plant is aborted and is present in a rudimentary state.
is_a: PO:0006355 ! androecium of ear floret
relationship: part_of PO:0006352 ! upper floret of sessile spikelet of ear

[Term]
id: PO:0006422
name: androecium of upper floret of pedicellate spikelet of ear
namespace: plant_structure
def: "Collectively the stamens of upper floret of a pedicellate spikelet of maize ear inflorescence. " [GR:pj]
comment: The development of the androecium in the ear floret of a normal maize plant is aborted and is present in a rudimentary state.
is_a: PO:0006355 ! androecium of ear floret
relationship: part_of PO:0006350 ! upper floret of pedicellate spikelet of ear

[Term]
id: PO:0006423
name: gynoecium of lower floret of sessile spikelet of ear
namespace: plant_structure
def: "Collectively the carpels of a lower floret of sessile spikelet of maize ear." [GR:pj]
comment: A non-functional or rudimentary gynoecium.
is_a: PO:0006365 ! gynoecium of ear floret
relationship: part_of PO:0006351 ! lower floret of sessile spikelet of ear

[Term]
id: PO:0006424
name: gynoecium of lower floret of pedicellate spikelet of ear
namespace: plant_structure
def: "Collectively the carpels of a lower floret of pedicellate spikelet of a maize ear. " [GR:pj]
comment: A non-functional or rudimentary gynoecium.
is_a: PO:0006365 ! gynoecium of ear floret
relationship: part_of PO:0006353 ! lower floret of pedicellate spikelet of ear

[Term]
id: PO:0006425
name: gynoecium of upper floret of sessile spikelet of ear
namespace: plant_structure
def: "Collectively the carpels of a upper floret of sessile spikelet of maize ear." [GR:pj]
comment: A functional gynoecium.
is_a: PO:0006365 ! gynoecium of ear floret
relationship: part_of PO:0006352 ! upper floret of sessile spikelet of ear

[Term]
id: PO:0006426
name: gynoecium of upper floret of pedicellate spikelet of ear
namespace: plant_structure
def: "Collectively the carpels of a upper floret of pedicellate spikelet of maize ear." [GR:pj]
comment: A functional gynoecium.
is_a: PO:0006365 ! gynoecium of ear floret
relationship: part_of PO:0006350 ! upper floret of pedicellate spikelet of ear

[Term]
id: PO:0006427
name: palea of upper floret of sessile spikelet of ear
namespace: plant_structure
def: "The upper of the two bracts enclosing a flower in a maize ear sessile spikelet upper floret." [GR:pj]
is_a: PO:0006361 ! palea of ear floret
relationship: part_of PO:0006352 ! upper floret of sessile spikelet of ear

[Term]
id: PO:0006428
name: palea of lower floret of sessile spikelet of ear
namespace: plant_structure
def: "The upper of the two bracts enclosing a flower in a maize ear sessile spikelet lower floret." [GR:pj]
is_a: PO:0006361 ! palea of ear floret
relationship: part_of PO:0006351 ! lower floret of sessile spikelet of ear

[Term]
id: PO:0006429
name: palea of upper floret of pedicellate spikelet of ear
namespace: plant_structure
def: "The upper of the two bracts enclosing a flower in a maize ear pedicellate spikelet upper floret." [GR:pj]
is_a: PO:0006361 ! palea of ear floret
relationship: part_of PO:0006350 ! upper floret of pedicellate spikelet of ear

[Term]
id: PO:0006430
name: palea of lower floret of pedicellate spikelet of ear
namespace: plant_structure
def: "The upper of the two bracts enclosing a flower in a maize ear pedicellate spikelet lower floret." [GR:pj]
is_a: PO:0006361 ! palea of ear floret
relationship: part_of PO:0006353 ! lower floret of pedicellate spikelet of ear

[Term]
id: PO:0006431
name: lemma of lower floret of pedicellate spikelet of ear
namespace: plant_structure
def: "The lower of the two bracts enclosing a flower in a maize ear pedicellate spikelet lower floret." [GR:pj]
is_a: PO:0006363 ! lemma of ear floret
relationship: part_of PO:0006353 ! lower floret of pedicellate spikelet of ear

[Term]
id: PO:0006432
name: lemma of upper floret of pedicellate spikelet of ear
namespace: plant_structure
def: "The lower of the two bracts enclosing a flower in a maize ear pedicellate spikelet upper floret." [GR:pj]
is_a: PO:0006363 ! lemma of ear floret
relationship: part_of PO:0006350 ! upper floret of pedicellate spikelet of ear

[Term]
id: PO:0006433
name: lemma of lower floret of sessile spikelet of ear
namespace: plant_structure
def: "The lower of the two bracts enclosing a flower in a maize ear sessile spikelet lower floret." [GR:pj]
is_a: PO:0006363 ! lemma of ear floret
relationship: part_of PO:0006351 ! lower floret of sessile spikelet of ear

[Term]
id: PO:0006434
name: lemma of upper floret of sessile spikelet of ear
namespace: plant_structure
def: "The lower of the two bracts enclosing a flower in a maize ear sessile spikelet upper floret." [GR:pj]
is_a: PO:0006363 ! lemma of ear floret
relationship: part_of PO:0006352 ! upper floret of sessile spikelet of ear

[Term]
id: PO:0006435
name: rachilla of pedicellate spikelet of ear
namespace: plant_structure
def: "The axis of the ear pedicellate spikelet\, above the glumes." [GR:pj]
is_a: PO:0006380 ! ear spikelet rachilla
relationship: part_of PO:0006348 ! ear pedicellate spikelet

[Term]
id: PO:0006436
name: rachilla of sessile spikelet of ear
namespace: plant_structure
def: "The axis of the ear sessile spikelet\, above the glumes." [GR:pj]
is_a: PO:0006380 ! ear spikelet rachilla

[Term]
id: PO:0006437
name: lower glume of pedicellate spikelet of ear
namespace: plant_structure
def: "The proximal/basal of the two glumes in the ear pedicellate spikelet." [GR:pj]
is_a: PO:0006369 ! lower glume of ear spikelet
relationship: part_of PO:0006348 ! ear pedicellate spikelet

[Term]
id: PO:0006438
name: lower glume of sessile spikelet of ear
namespace: plant_structure
def: "The proximal/basal of the two glumes in the ear sessile spikelet." [GR:pj]
is_a: PO:0006369 ! lower glume of ear spikelet
relationship: part_of PO:0006349 ! ear sessile spikelet

[Term]
id: PO:0006439
name: upper glume of pedicellate spikelet of ear
namespace: plant_structure
def: "The apical/distal of the two glumes in the pedicellate spikelet." [GR:pj]
is_a: PO:0006371 ! upper glume of ear spikelet
relationship: part_of PO:0006348 ! ear pedicellate spikelet

[Term]
id: PO:0006440
name: upper glume of sessile spikelet of ear
namespace: plant_structure
def: "The apical/distal of the two glumes in the sessile spikelet." [GR:pj]
is_a: PO:0006371 ! upper glume of ear spikelet
relationship: part_of PO:0006349 ! ear sessile spikelet

[Term]
id: PO:0006441
name: stamen (sensu Poaceae)
namespace: plant_structure
def: "A microsporophyll\, bearing four microsporangia in a grass floret." [GR:pj]
is_a: PO:0009029 ! stamen
relationship: part_of PO:0006383 ! androecium (sensu Poaceae)

[Term]
id: PO:0006442
name: anther (sensu Poaceae)
namespace: plant_structure
def: "The pollen-bearing part of a stamen of a grass floret." [GR:pj]
is_a: PO:0009066 ! anther
relationship: part_of PO:0006441 ! stamen (sensu Poaceae)

[Term]
id: PO:0006443
name: connective (sensu Poaceae)
namespace: plant_structure
def: "The part of the stamen of a grass floret\, that connects the microsporangia/pollen sacs." [GR:pj]
is_a: PO:0009068 ! connective
relationship: part_of PO:0006442 ! anther (sensu Poaceae)

[Term]
id: PO:0006444
name: microsporangium (sensu Poaceae)
namespace: plant_structure
def: "Sporangium in the anther of a grass stamen producing microspores\, usually many in number." [GR:pj]
is_a: PO:0009070 ! microsporangium
relationship: part_of PO:0006442 ! anther (sensu Poaceae)

[Term]
id: PO:0006445
name: anther wall (sensu Poaceae)
namespace: plant_structure
def: "A multicellular layer with outer epidermis and an inner endothecium of an anther of a grass stamen." [GR:pj]
is_a: PO:0000002 ! anther wall
relationship: part_of PO:0006444 ! microsporangium (sensu Poaceae)

[Term]
id: PO:0006446
name: endothecium (sensu Poaceae)
namespace: plant_structure
def: "The hypodermis of an anther sac of a grass stamen with distinctively thickened walls and involved in its dehiscence." [GR:pj]
is_a: PO:0020002 ! endothecium
relationship: part_of PO:0006445 ! anther wall (sensu Poaceae)

[Term]
id: PO:0006447
name: exothecium (sensu Poaceae)
namespace: plant_structure
def: "The epidermis of an anther sac of a grass stamen." [GR:pj]
is_a: PO:0020004 ! exothecium
relationship: part_of PO:0006445 ! anther wall (sensu Poaceae)

[Term]
id: PO:0006448
name: placentoid (sensu Poaceae)
namespace: plant_structure
def: "An inpushing of the anther wall of a grass stamen." [GR:pj]
is_a: PO:0020005 ! placentoid
relationship: part_of PO:0006445 ! anther wall (sensu Poaceae)

[Term]
id: PO:0006449
name: stomium (sensu Poaceae)
namespace: plant_structure
def: "A fissure in the anther lobe through which the pollen is released in grasses." [GR:pj]
is_a: PO:0020101 ! stomium
relationship: part_of PO:0006445 ! anther wall (sensu Poaceae)

[Term]
id: PO:0006450
name: tapetum (sensu Poaceae)
namespace: plant_structure
def: "Innermost part of the anther wall\, involved in the nutrition of the pollen in grasses." [GR:pj]
is_a: PO:0009071 ! tapetum
relationship: part_of PO:0006445 ! anther wall (sensu Poaceae)

[Term]
id: PO:0006451
name: microsporocyte (sensu Poaceae)
namespace: plant_structure
def: "A diploid (2n) cell that undergoes meiosis and produces four haploid (1n) microspores in a grass plant." [GR:pj]
is_a: PO:0020047 ! microsporocyte
relationship: part_of PO:0006444 ! microsporangium (sensu Poaceae)

[Term]
id: PO:0006452
name: microspore (sensu Poaceae)
namespace: plant_structure
def: "The smaller\, in general\, of the two kinds of spores produced in the life cycle of a grass plant. It gives rise to the male gametophyte." [GR:pj]
is_a: PO:0020048 ! microspore
relationship: develops_from PO:0006451 ! microsporocyte (sensu Poaceae)

[Term]
id: PO:0006453
name: theca (sensu Poaceae)
namespace: plant_structure
def: "A part of the anther of a grass stamen consisting of paired sporangia that dehisce down a common slit." [GR:pj]
is_a: PO:0006444 ! microsporangium (sensu Poaceae)
is_a: PO:0009069 ! theca

[Term]
id: PO:0006454
name: filament (sensu Poaceae)
namespace: plant_structure
def: "The stalk of the stamen of a grass floret." [GR:pj]
is_a: PO:0009067 ! filament
relationship: part_of PO:0006441 ! stamen (sensu Poaceae)

[Term]
id: PO:0006455
name: carpel (sensu Poaceae)
namespace: plant_structure
def: "A megasporophyll at the center of a grass floret enclosing the ovule." [GR:pj]
is_a: PO:0009030 ! carpel
relationship: part_of PO:0006384 ! gynoecium (sensu Poaceae)

[Term]
id: PO:0006456
name: ovary (sensu Poaceae)
namespace: plant_structure
def: "The basal portion of a carpel that encloses the ovule(s) in a grass floret." [GR:pj]
is_a: PO:0009072 ! ovary
relationship: part_of PO:0006455 ! carpel (sensu Poaceae)

[Term]
id: PO:0006457
name: ovule (sensu Poaceae)
namespace: plant_structure
def: "A stalked or sessile structure in a grass carpel within which one or more megaspores are formed and later the female gametophyte or embryo sac develops." [GR:pj]
is_a: PO:0020003 ! ovule
relationship: part_of PO:0006456 ! ovary (sensu Poaceae)

[Term]
id: PO:0006458
name: chalaza (sensu Poaceae)
namespace: plant_structure
def: "Region in the grass ovule where the integuments and the nucellus merge with the funiculus." [GR:pj]
is_a: PO:0020026 ! chalaza
relationship: part_of PO:0006457 ! ovule (sensu Poaceae)

[Term]
id: PO:0006459
name: outer integumet (sensu Poaceae)
namespace: plant_structure
def: "One of the two layers of tissue that usually covers the ovule of a grass\, contiguous to the inner integument and usually involved in forming the micropyle at the apex." [GR:pj]
is_a: PO:0020023 ! outer integument
relationship: part_of PO:0006465 ! integument (sensu Poaceae)

[Term]
id: PO:0006460
name: inner integument (sensu Poaceae)
namespace: plant_structure
def: "The innermost of the two layers of tissue that cover the ovule of a grass\, contiguous to the nucellus and usually involved in forming the micropyle at the apex." [GR:pj]
is_a: PO:0020022 ! inner integument
relationship: part_of PO:0006465 ! integument (sensu Poaceae)

[Term]
id: PO:0006461
name: micropyle (sensu Poaceae)
namespace: plant_structure
def: "A small canal through the inner integument(s) at the apex of a grass ovule." [GR:pj]
is_a: PO:0020025 ! micropyle
relationship: part_of PO:0006457 ! ovule (sensu Poaceae)

[Term]
id: PO:0006462
name: nucellus (sensu Poaceae)
namespace: plant_structure
def: "Subepidermal tissue in the ovule of a grass plant surrounding the megasporocyte." [GR:pj]
is_a: PO:0020020 ! nucellus
relationship: part_of PO:0006457 ! ovule (sensu Poaceae)

[Term]
id: PO:0006463
name: megasporocyte (sensu Poaceae)
namespace: plant_structure
def: "A diploid (2n) cell that undergoes meiosis and produces four haploid (1n) megaspores in a grass plant." [GR:pj]
is_a: PO:0000431 ! megasporocyte
relationship: part_of PO:0006462 ! nucellus (sensu Poaceae)

[Term]
id: PO:0006464
name: megaspore (sensu Poaceae)
namespace: plant_structure
def: "The larger\, in general\, of the two kinds of spores produced after meiosis in the life cycle of a grass plant\, and on germination giving rise to the female gametophyte (embryo sac)." [GR:pj]
is_a: PO:0020019 ! megaspore
relationship: develops_from PO:0006463 ! megasporocyte (sensu Poaceae)

[Term]
id: PO:0006465
name: integument (sensu Poaceae)
namespace: plant_structure
def: "One of the layers of tissue that covers the ovule of a grass carpel\, enveloping the nucellus and forming the micropyle at the apex." [GR:pj]
is_a: PO:0020021 ! integument
relationship: part_of PO:0006457 ! ovule (sensu Poaceae)

[Term]
id: PO:0006466
name: funicle (sensu Poaceae)
namespace: plant_structure
def: "The stalk which attaches the ovule to the placenta in a grass carpel." [GR:pj]
is_a: PO:0020006 ! funicle
relationship: part_of PO:0006456 ! ovary (sensu Poaceae)

[Term]
id: PO:0006467
name: ovary placenta (sensu Poaceae)
namespace: plant_structure
def: "The region within an ovary to which ovules are attached in a grass carpel." [GR:pj]
is_a: PO:0020001 ! ovary placenta
relationship: part_of PO:0006456 ! ovary (sensu Poaceae)

[Term]
id: PO:0006468
name: stigma (sensu Poaceae)
namespace: plant_structure
def: "The apical part of a carpel of a grass floret on which the pollen germinates." [GR:pj]
is_a: PO:0009073 ! stigma
relationship: part_of PO:0006455 ! carpel (sensu Poaceae)

[Term]
id: PO:0006469
name: style (sensu Poaceae)
namespace: plant_structure
def: "An elongated part of a carpel between the ovary and the stigma of a grass floret\, through which the pollen tube grows." [GR:pj]
is_a: PO:0009074 ! style
relationship: part_of PO:0006455 ! carpel (sensu Poaceae)

[Term]
id: PO:0006470
name: carpel (sensu Zea)
namespace: plant_structure
def: "A megasporophyll at the center of a maize floret enclosing the ovule." [GR:pj]
is_a: PO:0006455 ! carpel (sensu Poaceae)
relationship: part_of PO:0006365 ! gynoecium of ear floret

[Term]
id: PO:0006471
name: androecium (sensu Zea)
namespace: plant_structure
def: "Collectively the stamens of one floret of a maize plant." [GR:pj]
is_a: PO:0006383 ! androecium (sensu Poaceae)

[Term]
id: PO:0006472
name: stamen (sensu Zea)
namespace: plant_structure
def: "A microsporophyll bearing four microsporangia in a maize floret." [GR:pj]
is_a: PO:0006441 ! stamen (sensu Poaceae)
relationship: part_of PO:0006366 ! androecium of tassel floret

[Term]
id: PO:0006473
name: anther (sensu Zea)
namespace: plant_structure
def: "The pollen-bearing part of a stamen of a maize floret." [GR:pj]
is_a: PO:0006442 ! anther (sensu Poaceae)
relationship: part_of PO:0006472 ! stamen (sensu Zea)

[Term]
id: PO:0006474
name: filament (sensu Zea)
namespace: plant_structure
def: "The stalk of the stamen of a maize floret." [GR:pj]
is_a: PO:0006454 ! filament (sensu Poaceae)
relationship: part_of PO:0006472 ! stamen (sensu Zea)

[Term]
id: PO:0006475
name: connective (sensu Zea)
namespace: plant_structure
def: "The part of the stamen of a maize floret\, that connects the microsporangia or pollen sacs " [GR:pj]
is_a: PO:0006443 ! connective (sensu Poaceae)
relationship: part_of PO:0006473 ! anther (sensu Zea)

[Term]
id: PO:0006476
name: microsporangium (sensu Zea)
namespace: plant_structure
def: "Sporangium in the anther of a maize stamen producing microspores\, usually many in number ." [GR:pj]
is_a: PO:0006444 ! microsporangium (sensu Poaceae)
relationship: part_of PO:0006473 ! anther (sensu Zea)

[Term]
id: PO:0006477
name: anther wall (sensu Zea)
namespace: plant_structure
def: "A multicellular layer with outer epidermis and an inner endothecium of an anther of a maize stamen." [GR:pj]
is_a: PO:0006445 ! anther wall (sensu Poaceae)
relationship: part_of PO:0006476 ! microsporangium (sensu Zea)

[Term]
id: PO:0006478
name: theca (sensu Zea)
namespace: plant_structure
def: "A part of the anther of a maize stamen consisting of paired sporangia that dehisce down a common slit." [GR:pj]
is_a: PO:0006453 ! theca (sensu Poaceae)
is_a: PO:0006476 ! microsporangium (sensu Zea)

[Term]
id: PO:0006479
name: microsporocyte (sensu Zea)
namespace: plant_structure
def: "A diploid (2n) cell that undergoes meiosis and produces four haploid (1n) microspores in a maize plant." [GR:pj]
is_a: PO:0006451 ! microsporocyte (sensu Poaceae)
relationship: part_of PO:0006476 ! microsporangium (sensu Zea)

[Term]
id: PO:0006480
name: microspore (sensu Zea)
namespace: plant_structure
def: "The smaller\, in general\, of the two kinds of spores produced in the life cycle of a maize plant. It gives rise to the male gametophyte." [GR:pj]
is_a: PO:0006452 ! microspore (sensu Poaceae)
relationship: develops_from PO:0006479 ! microsporocyte (sensu Zea)

[Term]
id: PO:0006481
name: endothecium (sensu Zea)
namespace: plant_structure
def: "The hypodermis of an anther sac of a maize stamen with distinctively thickened walls and involved in its dehiscence." [GR:pj]
is_a: PO:0006446 ! endothecium (sensu Poaceae)
relationship: part_of PO:0006477 ! anther wall (sensu Zea)

[Term]
id: PO:0006482
name: exothecium (sensu Zea)
namespace: plant_structure
def: "The epidermis of an anther sac of a maize stamen." [GR:pj]
is_a: PO:0006447 ! exothecium (sensu Poaceae)
relationship: part_of PO:0006477 ! anther wall (sensu Zea)

[Term]
id: PO:0006483
name: placentoid (sensu Zea)
namespace: plant_structure
def: "An inpushing of the anther wall of a maize stamen." [GR:pj]
is_a: PO:0006448 ! placentoid (sensu Poaceae)
relationship: part_of PO:0006477 ! anther wall (sensu Zea)

[Term]
id: PO:0006484
name: tapetum (sensu Zea)
namespace: plant_structure
def: "Innermost part of the anther wall\, involved in the nutrition of the pollen in maize." [GR:pj]
is_a: PO:0006450 ! tapetum (sensu Poaceae)
relationship: part_of PO:0006477 ! anther wall (sensu Zea)

[Term]
id: PO:0006485
name: stomium (sensu Zea)
namespace: plant_structure
def: "A fissure in the anther lobe through which the pollen is released in maize." [GR:pj]
is_a: PO:0006449 ! stomium (sensu Poaceae)
relationship: part_of PO:0006477 ! anther wall (sensu Zea)

[Term]
id: PO:0006486
name: ovary (sensu Zea)
namespace: plant_structure
def: "The basal portion of a carpel that encloses the ovule(s) in a maize floret." [GR:pj]
is_a: PO:0006456 ! ovary (sensu Poaceae)
relationship: part_of PO:0006470 ! carpel (sensu Zea)

[Term]
id: PO:0006487
name: stigma (sensu Zea)
namespace: plant_structure
def: "The apical part of a carpel of a maize floret on which the pollen germinates." [GR:pj]
is_a: PO:0006468 ! stigma (sensu Poaceae)
relationship: part_of PO:0006470 ! carpel (sensu Zea)

[Term]
id: PO:0006488
name: silk
namespace: plant_structure
def: "The style of a maize floret." [GR:pj]
synonym: "style (sensu Zea)" []
is_a: PO:0006469 ! style (sensu Poaceae)
relationship: part_of PO:0006470 ! carpel (sensu Zea)

[Term]
id: PO:0006489
name: funicle (sensu Zea)
namespace: plant_structure
def: "The stalk which attaches the ovule to the placenta in a maize carpel." [GR:pj]
is_a: PO:0006466 ! funicle (sensu Poaceae)
relationship: part_of PO:0006486 ! ovary (sensu Zea)

[Term]
id: PO:0006490
name: ovary placenta (sensu Zea)
namespace: plant_structure
def: "The region within an ovary to which ovules are attached in a maize carpel." [GR:pj]
is_a: PO:0006467 ! ovary placenta (sensu Poaceae)
relationship: part_of PO:0006486 ! ovary (sensu Zea)

[Term]
id: PO:0006491
name: ovule (sensu Zea)
namespace: plant_structure
def: "A stalked or sessile structure in a maize carpel within which one or more megaspores are formed and later the female gametophyte or embryo sac develops." [GR:pj]
is_a: PO:0006457 ! ovule (sensu Poaceae)
relationship: part_of PO:0006486 ! ovary (sensu Zea)

[Term]
id: PO:0006492
name: nucellus (sensu Zea)
namespace: plant_structure
def: "Subepidermal tissue in the ovule of a maize plant surrounding the megasporocyte." [GR:pj]
is_a: PO:0006462 ! nucellus (sensu Poaceae)
relationship: part_of PO:0006491 ! ovule (sensu Zea)

[Term]
id: PO:0006493
name: megasporocyte (sensu Zea)
namespace: plant_structure
def: "A diploid (2n) cell that undergoes meiosis and produces four haploid (1n) megaspores in a maize plant." [GR:pj]
is_a: PO:0006463 ! megasporocyte (sensu Poaceae)
relationship: part_of PO:0006492 ! nucellus (sensu Zea)

[Term]
id: PO:0006494
name: megaspore (sensu Zea)
namespace: plant_structure
def: "The larger\, in general\, of the two kinds of spores produced after meiosis in the life cycle of a maize plant\, and on germination giving rise to the female gametophyte (embryo sac)." [GR:pj]
is_a: PO:0006464 ! megaspore (sensu Poaceae)
relationship: develops_from PO:0006493 ! megasporocyte (sensu Zea)

[Term]
id: PO:0006495
name: degenerate megaspore (sensu Poaceae)
namespace: plant_structure
def: "The megaspores in a grass plant that would not participate in megagametogenesis." [GR:pj]
is_a: PO:0000245 ! degenerate megaspore
is_a: PO:0006464 ! megaspore (sensu Poaceae)

[Term]
id: PO:0006496
name: functional megaspore (sensu Poaceae)
namespace: plant_structure
def: "The megaspore that forms the embryo sac in grasses." [GR:pj]
is_a: PO:0000244 ! functional megaspore
is_a: PO:0006464 ! megaspore (sensu Poaceae)

[Term]
id: PO:0006497
name: stigma epidermis (sensu Poaceae)
namespace: plant_structure
def: "The epidermal cell layer of the grass stigma." [GR:pj]
is_a: PO:0006061 ! stigma epidermis
relationship: part_of PO:0006468 ! stigma (sensu Poaceae)

[Term]
id: PO:0006498
name: style epidermis (sensu Poaceae)
namespace: plant_structure
def: "The epidermal cell layer of the style of a grass carpel." [GR:pj]
is_a: PO:0006062 ! style epidermis
relationship: part_of PO:0006469 ! style (sensu Poaceae)

[Term]
id: PO:0006499
name: transmitting tissue (sensu Poaceae)
namespace: plant_structure
def: "Tissue in the style of a grass carpel\, through which the pollen tube grows; it connects the stigma and the inside of ovary." [GR:pj]
is_a: PO:0020102 ! transmitting tissue
relationship: part_of PO:0006469 ! style (sensu Poaceae)

[Term]
id: PO:0006500
name: ovary epidermis (sensu Poaceae)
namespace: plant_structure
def: "The epidermal cell layer of the ovary of a grass carpel." [GR:pj]
is_a: PO:0006063 ! ovary epidermis
relationship: part_of PO:0006456 ! ovary (sensu Poaceae)

[Term]
id: PO:0006501
name: leaf abscission zone
namespace: plant_structure
def: "Zone at base of the leaf that contains an abscission (or separation) layer and a protective layer\, both involved in the abscission of the leaf." [GR:pj]
is_a: PO:0000146 ! abscission zone
relationship: part_of PO:0009025 ! leaf

[Term]
id: PO:0006502
name: flower abscission zone
namespace: plant_structure
def: "Zone at base of the flower that contains an abscission (or separation) layer and a protective layer\, both involved in the abscission of the flower and its parts." [GR:pj]
is_a: PO:0000146 ! abscission zone
relationship: part_of PO:0009046 ! flower

[Term]
id: PO:0006503
name: fruit abscission zone
namespace: plant_structure
def: "Zone at base of the fruit that contains an abscission (or separation) layer and a protective layer\, both involved in the abscission of the fruit." [GR:pj]
subset: Maize
subset: Poaceae
subset: Rice
subset: Tomato
is_a: PO:0000146 ! abscission zone
relationship: part_of PO:0009001 ! fruit

[Term]
id: PO:0006504
name: leaf trichome
namespace: plant_structure
def: "Trichome on/from the epidermis of a leaf." [GR:pj]
is_a: PO:0000282 ! trichome
relationship: part_of PO:0000049 ! leaf lamina abaxial epidermis
relationship: part_of PO:0000050 ! leaf lamina adaxial epidermis
relationship: part_of PO:0006018 ! leaf adaxial epidermis
relationship: part_of PO:0006019 ! leaf abaxial epidermis

[Term]
id: PO:0006505
name: central spike of ear
namespace: plant_structure
def: "The inflorescence axis of the ear." [GR:pj]
synonym: "cob (sensu zea)" []
synonym: "ear rachis" []
is_a: PO:0020122 ! inflorescence axis
relationship: part_of PO:0020136 ! ear (sensu Zea)

[Term]
id: PO:0006506
name: chalaza (sensu Zea)
namespace: plant_structure
def: "Region in the maize ovule where the integuments and the nucellus merge with the funiculus." [GR:pj]
is_a: PO:0006458 ! chalaza (sensu Poaceae)
relationship: part_of PO:0006491 ! ovule (sensu Zea)

[Term]
id: PO:0006507
name: integument (sensu Zea)
namespace: plant_structure
def: "One of the layers of tissue that covers the ovule of a maize carpel\, enveloping the nucellus and forming the micropyle at the apex." [GR:pj]
is_a: PO:0006465 ! integument (sensu Poaceae)
relationship: part_of PO:0006491 ! ovule (sensu Zea)

[Term]
id: PO:0006508
name: integument epidermis (sensu Poaceae)
namespace: plant_structure
def: "The epidermis of an integument in a grass ovule." [GR:pj]
is_a: PO:0006043 ! integument epidermis
relationship: part_of PO:0006465 ! integument (sensu Poaceae)

[Term]
id: PO:0008001
name: fruit distal end
namespace: plant_structure
def: "The end distal from the fruit pedicel." [GR:ap "", (SGN:nm)]
subset: Tomato
synonym: "blossom end" []
relationship: part_of PO:0009001 ! fruit

[Term]
id: PO:0008002
name: fruit proximal end
namespace: plant_structure
def: "The stem end of the fruit." [GR:ap "", (SGN:nm)]
subset: Tomato
synonym: "fruit shoulders" []
relationship: part_of PO:0009001 ! fruit

[Term]
id: PO:0008003
name: fruit vascular system
namespace: plant_structure
def: "Vascular system of the fruit." [GR:ap "", (SGN:nm)]
subset: Arabidopsis
subset: Maize
subset: Poaceae
subset: Rice
subset: Tomato
is_a: PO:0000034 ! vascular system
relationship: part_of PO:0009001 ! fruit

[Term]
id: PO:0008004
name: fruit aleurone layer
namespace: plant_structure
def: "The outermost endosperm tissue of the grass caryopsis\, its cells being characterized by presence of protein bodies containing seed storage proteins." [GR:ap ""]
relationship: part_of PO:0009001 ! fruit

[Term]
id: PO:0008005
name: fruit nucellus
namespace: plant_structure
def: "Subepidermal tissue in the grass caryopsis." [GR:ap ""]
subset: Poaceae
subset: Rice
relationship: part_of PO:0009001 ! fruit

[Term]
id: PO:0008006
name: nucellar epidermis
namespace: plant_structure
def: "The morphologically distinct outer layer of the nucellus. " [GR:ap ""]
subset: Poaceae
subset: Rice
relationship: part_of PO:0008005 ! fruit nucellus

[Term]
id: PO:0008007
name: nucellar projection
namespace: plant_structure
def: "The morphologically distinct portion of the nucellus overlying the vascular strands in the grass caryopsis." [GR:ap ""]
subset: Poaceae
subset: Rice
relationship: part_of PO:0008005 ! fruit nucellus

[Term]
id: PO:0008008
name: modified aleurone
namespace: plant_structure
def: "The morphologically distinct aleurone layer located adjacent to the nucellar projection." [GR:ap ""]
subset: Poaceae
subset: Rice
relationship: part_of PO:0008004 ! fruit aleurone layer

[Term]
id: PO:0008009
name: abaxial nucellar projection
namespace: plant_structure
def: "The abaxial/lower portion of the nucellus overlying the vascular strands in the grass caryopsis." [GR:ap ""]
subset: Poaceae
subset: Rice
relationship: part_of PO:0008007 ! nucellar projection

[Term]
id: PO:0008010
name: adaxial nucellar projection
namespace: plant_structure
def: "The adaxial/upper portion of the nucellus overlying the vascular strands in the grass caryopsis." [GR:ap ""]
subset: Poaceae
subset: Rice
relationship: part_of PO:0008007 ! nucellar projection

[Term]
id: PO:0009001
name: fruit
alt_id: PO:0020067
alt_id: PO:0020068
alt_id: PO:0020069
alt_id: PO:0020070
alt_id: PO:0020071
alt_id: PO:0020072
alt_id: PO:0020073
alt_id: PO:0020074
alt_id: PO:0020076
alt_id: PO:0020077
alt_id: PO:0020078
alt_id: PO:0020079
alt_id: PO:0020080
alt_id: PO:0020082
alt_id: PO:0020083
alt_id: PO:0020087
alt_id: PO:0020107
namespace: plant_structure
def: "The seed-bearing structure in angiosperms\, formed from the ovary after flowering." [Poc:curators, APWeb:Glossary]
subset: Arabidopsis
subset: Maize
subset: Poaceae
subset: Rice
synonym: "achene" []
synonym: "berry" []
synonym: "capsule" []
synonym: "caryopsis" []
synonym: "circumcissile capsule" []
synonym: "cypsela" []
synonym: "drupe" []
synonym: "follicle" []
synonym: "grain" []
synonym: "kernel" []
synonym: "legume" []
synonym: "loculicidal capsule" []
synonym: "lomentum" []
synonym: "nut" []
synonym: "pod" []
synonym: "pome" []
synonym: "poricidal capsule" []
synonym: "schizocarp" []
synonym: "septicidal capsule" []
synonym: "septifragal capsule" []
synonym: "silicula" []
synonym: "siliqua" []
synonym: "silique" []
relationship: part_of PO:0006342 ! infructescence

[Term]
id: PO:0009002
name: plant cell
namespace: plant_structure
def: "Structural and physiological unit of a plant consisting of the cytoplasm\, protoplast and cell wall; in nonliving state\, of cell wall only\, or cell wall and some nonliving inclusions." [ISBN:0471245208, GR:pj]
subset: reference
is_a: PO:0009011 ! plant structure

[Term]
id: PO:0009003
name: sporophyte
namespace: plant_structure
def: "A plant or phase of a life cycle that bears spores formed by meiosis." [APWeb:Glossary]
subset: reference
is_a: PO:0009011 ! plant structure

[Term]
id: PO:0009004
name: gametophyte
namespace: plant_structure
def: "A haploid plant\, or phase of a plant's life cycle\, that bears gametes after mitotic events." [APWeb:Glossary]
subset: reference
is_a: PO:0009011 ! plant structure

[Term]
id: PO:0009005
name: root
alt_id: PO:0003006
namespace: plant_structure
def: "An axial system which is usually underground and more or less positively geotropic\, does not bear leaves and only rarely shoots\, is endogenous in origin\, indeterminate in growth and often with secondary thickening." [APWeb:Glossary]
comment: Commonly thought of as one of the three basic parts of the seed plant body.
subset: reference
synonym: "aerial root" []
is_a: PO:0009008 ! organ
relationship: part_of PO:0009003 ! sporophyte

[Term]
id: PO:0009006
name: shoot
namespace: plant_structure
def: "Part of the sporophyte composed of the stems and leaves\, and includes shoot apical meristems." [Poc:curators]
subset: reference
synonym: "branch" []
synonym: "crown (sensu Poaceae)" []
narrow_synonym: "tree crown" []
relationship: part_of PO:0009003 ! sporophyte

[Term]
id: PO:0009007
name: tissue
namespace: plant_structure
def: "Group of cells organized into a structural and functional unit; the component cells may be alike (simple tissue) or varied (complex tissue)." [TAIR:lr]
subset: reference
is_a: PO:0009011 ! plant structure

[Term]
id: PO:0009008
name: organ
namespace: plant_structure
def: "A natural part or structure in a plant\, capable of performing some special action (termed its function)\, which is essential to the life or well-being of the whole." [MaizeGDB:lv]
comment: All organs are represented under sporophyte.
subset: reference
is_a: PO:0009011 ! plant structure

[Term]
id: PO:0009009
name: embryo
namespace: plant_structure
def: "A young sporophyte contained within a seed." [APWeb:Glossary, GR:pj]
synonym: "germ" []
relationship: part_of PO:0009010 ! seed

[Term]
id: PO:0009010
name: seed
namespace: plant_structure
def: "A propagating organ formed in the reproductive cycle of gymnosperms and angiosperms\, derived from the ovule and enclosing an embryo." [APWeb:Glossary, GR:pj]
comment: The seed is representative of a next generation of sporophyte.
subset: Arabidopsis
subset: Citrus
subset: Maize
subset: Poaceae
subset: Rice
subset: Tomato
is_a: PO:0009003 ! sporophyte
relationship: part_of PO:0009001 ! fruit

[Term]
id: PO:0009011
name: plant structure
namespace: plant_structure
def: "Any morphological or anatomical feature of a plant." [Poc:curators]

[Term]
id: PO:0009013
name: meristem
namespace: plant_structure
def: "Regions of a plant in which cells that have retained their embryonic characteristics\, or have reverted to them secondarily\, and that divide to produce new cells that can undergo differentiation to form mature tissues\, i.e. they have a capacity for morphogenesis and growth." [APWeb:Glossary, GR:pj]
is_a: PO:0009007 ! tissue

[Term]
id: PO:0009014
name: dermal tissue
namespace: plant_structure
def: "Tissue derived from the protoderm that covers the surface of the plant body." [GR:pj, ISBN:0122151704]
is_a: PO:0009007 ! tissue

[Term]
id: PO:0009015
name: vascular tissue
namespace: plant_structure
def: "Conducting tissues made up of xylem and phloem." [APWeb:Glossary]
comment: In the stem it is often found as a stele\, surrounded by the cortex and surrounding the pith.
is_a: PO:0009007 ! tissue
relationship: part_of PO:0000034 ! vascular system

[Term]
id: PO:0009016
name: ground tissue
namespace: plant_structure
def: "OBSOLETE. Tissues other than the vascular tissues\, epidermis and the periderm." [GR:pj]
comment: Uninformative definition. Check it again.
is_obsolete: true

[Term]
id: PO:0009020
name: meristem L1
namespace: plant_structure
def: "The outermost layer of the shoot apical meristem which gives rise to the shoot epidermis." [PMID:12221985, GR:pj]
relationship: part_of PO:0020148 ! shoot apical meristem

[Term]
id: PO:0009021
name: meristem L2
namespace: plant_structure
def: "The cell layer beneath the L1 layer in the shoot meristem which gives rise to subepidermal tissue." [PMID:12221985, GR:pj]
relationship: part_of PO:0020148 ! shoot apical meristem

[Term]
id: PO:0009022
name: meristem L3
namespace: plant_structure
def: "The multicellular layer beneath the L2 layer in the shoot meristem which gives rise to internal tissues of leaf and stem." [PMID:12221985, GR:pj]
relationship: part_of PO:0020148 ! shoot apical meristem

[Term]
id: PO:0009025
name: leaf
namespace: plant_structure
def: "Commonly thought of as one of the three basic parts of the seed plant body\, a structure usually of determinate growth\, without secondary thickening\, and of superficial origin\, often flattened and photosynthetic in part\, and in the axil of which is found a bud." [APWeb:Glossary]
subset: reference
synonym: "foliage leaf" []
is_a: PO:0006001 ! phyllome

[Term]
id: PO:0009026
name: sporophyll
namespace: plant_structure
def: "A leaf-like organ on which one or more sporangia are borne." [APWeb:Glossary]
subset: reference
is_a: PO:0006001 ! phyllome

[Term]
id: PO:0009027
name: megasporophyll
namespace: plant_structure
def: "A structure upon which (or in the axil of which) one or more megasporangia are borne; in flowering plants\, a carpel." [APWeb:Glossary]
is_a: PO:0009026 ! sporophyll

[Term]
id: PO:0009028
name: microsporophyll
namespace: plant_structure
def: "A structure on which one or more microsporangia are borne; in flowering plants\, the stamen." [APWeb:Glossary]
is_a: PO:0009026 ! sporophyll

[Term]
id: PO:0009029
name: stamen
namespace: plant_structure
def: "A microsporophyll bearing one or more microsporangia." [APWeb:Glossary]
subset: reference
is_a: PO:0009028 ! microsporophyll
relationship: part_of PO:0009061 ! androecium

[Term]
id: PO:0009030
name: carpel
namespace: plant_structure
def: "A megasporophyll\, almost always at the center of a flower\, its margins more or less fused together or with other carpels to enclose the ovule(s).\n" [APWeb:Glossary]
comment: If carpels are fused\, the gynoecium is a syncarpous gynoecium\, as in Poaceae\, Brassicaceae and Solanaceae.  If carpels are free\, the gynoecium is an apocarpous gynoecium\, as in Fabaceae.
subset: reference
is_a: PO:0009027 ! megasporophyll
relationship: part_of PO:0009062 ! gynoecium

[Term]
id: PO:0009031
name: sepal
namespace: plant_structure
def: "A member of the (usually green) outer whorl of non-fertile parts surrounding the fertile organs of a flower." [APWeb:Glossary]
subset: reference
is_a: PO:0009008 ! organ
relationship: part_of PO:0009060 ! calyx

[Term]
id: PO:0009032
name: petal
namespace: plant_structure
def: "A member of the corolla\, the inner whorl of non-fertile parts surrounding the fertile organs of a flower\, usually soft and colored conspicuously." [APWeb:Glossary]
subset: reference
is_a: PO:0009008 ! organ
relationship: part_of PO:0009059 ! corolla

[Term]
id: PO:0009033
name: tepal
namespace: plant_structure
def: "A perianth segment in a flower in which there are two whorls of such segments\, but all are similar in appearance." [APWeb:Glossary]
subset: reference
relationship: part_of PO:0009058 ! perianth

[Term]
id: PO:0009034
name: floral bract
namespace: plant_structure
def: "Leaf like structure subtending a flower." [Poc:curators]
subset: reference
synonym: "chaff" []
is_a: PO:0009008 ! organ
is_a: PO:0009055 ! bract
relationship: part_of PO:0009049 ! inflorescence

[Term]
id: PO:0009035
name: nectary
namespace: plant_structure
def: "A multicellular glandular structure secreting a liquid containing organic substances especially sugars." [GR:pj]
subset: reference
is_a: PO:0005656 ! secretory tissue
relationship: part_of PO:0009006 ! shoot

[Term]
id: PO:0009036
name: lodicule
namespace: plant_structure
def: "In a grass floret\, one of two or three tiny scales or flaps of tissue outside the stamens\, possibly representing reduced perianth segments." [APWeb:Glossary]
subset: reference
relationship: part_of PO:0006318 ! floret (sensu Poaceae)

[Term]
id: PO:0009037
name: lemma
namespace: plant_structure
def: "In a grass floret\, the lower of two bracts enclosing a flower." [APWeb:Glossary, GR:pj]
subset: reference
is_a: PO:0009034 ! floral bract
relationship: part_of PO:0006318 ! floret (sensu Poaceae)

[Term]
id: PO:0009038
name: palea
namespace: plant_structure
def: "In a grass floret\, the upper of the two bracts enclosing a flower." [APWeb:Glossary, GR:pj]
comment: Possibly a prophyll/bracteole.
subset: reference
is_a: PO:0009034 ! floral bract
relationship: part_of PO:0006318 ! floret (sensu Poaceae)

[Term]
id: PO:0009039
name: glume
alt_id: PO:0006026
namespace: plant_structure
def: "A \"bract\" in the inflorescence of a grass\, sedge or similar plant." [APWeb:Glossary, GR:pj]
subset: reference
synonym: "rudimentary glume" []
is_a: PO:0009054 ! inflorescence bract
relationship: part_of PO:0009051 ! spikelet

[Term]
id: PO:0009040
name: sterile lemma
alt_id: PO:0006029
namespace: plant_structure
def: "A bract in the position of a lemma\, but not enclosing floral organs" [UMSL:tk]
comment: An undeveloped androecium or gynoecium may or may not be detectable.
subset: reference
synonym: "empty glume" []
is_a: PO:0009037 ! lemma

[Term]
id: PO:0009041
name: fertile lemma
namespace: plant_structure
def: "A lemma that encloses a functional flower\, with androecium\, gynoecium or both." [UMSL:tk]
subset: reference
is_a: PO:0009037 ! lemma

[Term]
id: PO:0009042
name: prophyll
namespace: plant_structure
def: "The first leaf or two leaves formed at the base of an axillary shoot\, often smaller and/or in a distinctively different position from those formed subsequently." [APWeb:Glossary]
subset: reference
is_a: PO:0006001 ! phyllome

[Term]
id: PO:0009043
name: bracteole
namespace: plant_structure
def: "A small leaf or leaves borne singly or in pairs on the pedicel\, the prophyll(s) of the flower-shoot (pedicel plus flower)." [APWeb:Glossary]
is_a: PO:0009042 ! prophyll
relationship: part_of PO:0009052 ! pedicel

[Term]
id: PO:0009044
name: perigynium
namespace: plant_structure
def: "Sac-like bract subtending the pistillate flower\, as in Carex." [GR:pj]
is_a: PO:0009042 ! prophyll

[Term]
id: PO:0009045
name: phyllary
namespace: plant_structure
def: "Equals inflorescence bract of an involucre\, as in Asteraceae." [APWeb:Glossary]
subset: reference
is_a: PO:0009054 ! inflorescence bract

[Term]
id: PO:0009046
name: flower
alt_id: PO:0004541
namespace: plant_structure
def: "A heterosporangiate strobilus\, typically consisting of androecium\, gynoecium\, usually surrounded by a perianth and borne on an axis or receptacle." [APWeb:Glossary, GR:pj]
comment: The characteristic reproductive structure of angiosperms.
subset: reference
synonym: "floret (sensu Asteraceae)" []
relationship: part_of PO:0009049 ! inflorescence

[Term]
id: PO:0009047
name: stem
namespace: plant_structure
def: "The axial system of plants that bears leaves and buds.\n" [APWeb:Glossary]
comment: It is usually above ground and more or less negatively geotropic\, is exogenous in origin\, often indeterminate in growth and with secondary thickening.
subset: reference
synonym: "cane" []
synonym: "culm" []
synonym: "stalk" []
synonym: "trunk" []
relationship: part_of PO:0009006 ! shoot

[Term]
id: PO:0009049
name: inflorescence
alt_id: PO:0009048
alt_id: PO:0009050
alt_id: PO:0020088
alt_id: PO:0020111
alt_id: PO:0020112
alt_id: PO:0020113
alt_id: PO:0020114
alt_id: PO:0020115
alt_id: PO:0020116
alt_id: PO:0020117
alt_id: PO:0020118
alt_id: PO:0020119
alt_id: PO:0020120
namespace: plant_structure
def: "That part of the axial system of plants above the uppermost foliage leaf/pair of foliage leaves that bears flowers." [APWeb:Glossary]
comment: Some plants have only solitary flowers\, e.g. Magnolia.
subset: reference
synonym: "catkin" []
synonym: "cob (sensu Sorghum)" []
synonym: "corymb" []
synonym: "cyme" []
synonym: "dichasium" []
synonym: "drepanium" []
synonym: "helicoid cyme" []
synonym: "monochasium" []
synonym: "panicle" []
synonym: "raceme" []
synonym: "rhipidium" []
synonym: "scorpioid cyme" []
synonym: "spike (sensu Triticeae)" []
synonym: "umbel" []
synonym: "verticillaster" []
relationship: part_of PO:0009006 ! shoot

[Term]
id: PO:0009051
name: spikelet
namespace: plant_structure
def: "Ultimate and congested inflorescence branch of the grasses." [APWeb:Glossary]
comment: It consists of one to many closely-packed flowers and associated glumes etc.
subset: reference
relationship: part_of PO:0009049 ! inflorescence

[Term]
id: PO:0009052
name: pedicel
namespace: plant_structure
def: "Basal part of the ultimate branch of the inflorescence." [APWeb:Glossary]
comment: The bracteoles are borne on the pedicel\, which terminates in a flower.
subset: reference
relationship: part_of PO:0009049 ! inflorescence

[Term]
id: PO:0009053
name: peduncle
namespace: plant_structure
def: "The stalk of an inflorescence; that part of the inflorescence below the first flower or inflorescence branch and above the last foliage leaf/pair of foliage leaves." [APWeb:Glossary]
subset: reference
synonym: "inflorescence stem " []
relationship: part_of PO:0009049 ! inflorescence

[Term]
id: PO:0009054
name: inflorescence bract
namespace: plant_structure
def: "A leaf\, modified or not\, subtending a branch of the inflorescence or borne on the inflorescence axis below any branches or flowers." [APWeb:Glossary]
subset: reference
is_a: PO:0009008 ! organ
is_a: PO:0009055 ! bract
relationship: part_of PO:0009049 ! inflorescence

[Term]
id: PO:0009055
name: bract
namespace: plant_structure
def: "A leaf\, usually different in form from the foliage leaves\, subtending a flower or inflorescence." [APWeb:Glossary]
comment: Often used to refer to what is called here floral bract.
subset: reference
synonym: "hypsophyll" []
is_a: PO:0006001 ! phyllome

[Term]
id: PO:0009056
name: floral nectary
namespace: plant_structure
def: "A multicellular glandular structure found in the flower secreting a liquid containing organic substances especially sugars." [ISBN:047124529]
subset: reference
is_a: PO:0009035 ! nectary
relationship: part_of PO:0009046 ! flower

[Term]
id: PO:0009057
name: extrafloral nectary
namespace: plant_structure
def: "A multicellular glandular structure found in places other than flower secreting a liquid containing organic substances especially sugar." [ISBN:047124529]
is_a: PO:0009035 ! nectary

[Term]
id: PO:0009058
name: perianth
namespace: plant_structure
def: "Non-fertile parts of a flower surrounding the fertile organs\, collectively the calyx and corolla of a flower\, or only a singe whorl." [APWeb:Glossary]
subset: reference
relationship: part_of PO:0009046 ! flower

[Term]
id: PO:0009059
name: corolla
namespace: plant_structure
def: "The petals of a flower collectively." [APWeb:Glossary]
subset: reference
relationship: part_of PO:0009058 ! perianth

[Term]
id: PO:0009060
name: calyx
namespace: plant_structure
def: "The sepals of one flower collectively." [APWeb:Glossary]
subset: reference
relationship: part_of PO:0009058 ! perianth

[Term]
id: PO:0009061
name: androecium
namespace: plant_structure
def: "Collectively the stamens of one flower." [APWeb:Glossary, GR:pj]
subset: reference
relationship: part_of PO:0009046 ! flower

[Term]
id: PO:0009062
name: gynoecium
namespace: plant_structure
def: "Collectively the carpels of a flower." [APWeb:Glossary, GR:pj, TAIR:lr, MaizeGDB:lv]
subset: reference
synonym: "pistil" []
relationship: part_of PO:0009046 ! flower

[Term]
id: PO:0009063
name: epicalyx
namespace: plant_structure
def: "A whorl of structures immediately outside the calyx whorl." [APWeb:Glossary]
subset: reference
relationship: part_of PO:0009046 ! flower

[Term]
id: PO:0009064
name: receptacle
namespace: plant_structure
def: "The region at end of pedicel or axis to which parts of flower are attached." [Poc:curators, APWeb:Glossary]
subset: reference
relationship: part_of PO:0009046 ! flower

[Term]
id: PO:0009065
name: hypanthium
namespace: plant_structure
def: "A cup- or tube-like structure bearing perianth and stamens on its rim\, so these arise above the base\, and often above the top\, of the ovary of a flower." [Poc:curators, APWeb:Glossary]
subset: reference
relationship: part_of PO:0009046 ! flower

[Term]
id: PO:0009066
name: anther
namespace: plant_structure
def: "The pollen-bearing part of a stamen." [APWeb:Glossary]
subset: reference
relationship: part_of PO:0009029 ! stamen

[Term]
id: PO:0009067
name: filament
namespace: plant_structure
def: "The stalk of a stamen." [GR:pj, MaizeGDB:lv]
subset: reference
relationship: part_of PO:0009029 ! stamen

[Term]
id: PO:0009068
name: connective
namespace: plant_structure
def: "The part of the stamen that connects the microsporangia/pollen sacs." [APWeb:Glossary]
subset: reference
relationship: part_of PO:0009066 ! anther

[Term]
id: PO:0009069
name: theca
namespace: plant_structure
def: "A part of the anther consisting of paired sporangia that dehisce down a common slit." [APWeb:Glossary]
subset: reference
is_a: PO:0009070 ! microsporangium

[Term]
id: PO:0009070
name: microsporangium
namespace: plant_structure
def: "Sporangium producing microspores\, usually many in number." [APWeb:Glossary]
subset: reference
synonym: "anther lobe" []
synonym: "pollen sac" []
relationship: part_of PO:0009066 ! anther

[Term]
id: PO:0009071
name: tapetum
namespace: plant_structure
def: "Innermost part of the anther wall\, involved in the nutrition of the pollen." [APWeb:Glossary, TAIR:lr]
subset: reference
relationship: develops_from PO:0006008 ! inner secondary parietal cell layer
relationship: part_of PO:0000002 ! anther wall

[Term]
id: PO:0009072
name: ovary
namespace: plant_structure
def: "The basal portion of a carpel or group of fused carpels\, that encloses the ovule(s)." [APWeb:Glossary, TAIR:lr]
subset: reference
relationship: part_of PO:0009030 ! carpel

[Term]
id: PO:0009073
name: stigma
namespace: plant_structure
def: "Part of a carpel or group of fused carpels on which the pollen germinates\, usually apical." [APWeb:Glossary, TAIR:lr]
subset: reference
relationship: part_of PO:0009030 ! carpel

[Term]
id: PO:0009074
name: style
namespace: plant_structure
def: "An elongated part of a carpel or group of fused carpels between the ovary and the stigma\, and through which the pollen tube grows." [APWeb:Glossary, TAIR:lr]
subset: reference
synonym: "silk" []
relationship: part_of PO:0009030 ! carpel

[Term]
id: PO:0009075
name: plant ontology
namespace: plant_structure
def: "OBSOLETE. A controlled vocabulary to describe the various plant parts and the growth and developmental stages." [Poc:curators]
is_obsolete: true

[Term]
id: PO:0009077
name: staminode
namespace: plant_structure
def: "Sterile stamen." [APWeb:Glossary, GR:pj]
is_a: PO:0009028 ! microsporophyll
relationship: part_of PO:0009061 ! androecium

[Term]
id: PO:0009078
name: pistillode
namespace: plant_structure
def: "A sterile pistil\, often rudimentary." [APWeb:Glossary]
subset: reference
is_a: PO:0009062 ! gynoecium

[Term]
id: PO:0009080
name: spikelet rachilla
namespace: plant_structure
def: "The axis of the spikelet\, above the glumes." [Poc:curators]
is_a: PO:0009081 ! inflorescence branch
relationship: part_of PO:0009051 ! spikelet

[Term]
id: PO:0009081
name: inflorescence branch
namespace: plant_structure
def: "Any branch forming from the primary or the higher order inflorescence axis." [Poc:curators]
synonym: "coflorescence" []
relationship: part_of PO:0009049 ! inflorescence

[Term]
id: PO:0009082
name: floret
namespace: plant_structure
def: "Small flowers\, esp. of the spikelets of Poaceae and Cyperaceae." [APWeb:Glossary]
subset: reference
is_a: PO:0009046 ! flower

[Term]
id: PO:0009083
name: reproductive structures
namespace: plant_structure
def: "OBSOLETE. Aggregation of gamete producing structures." [Poc:curators]
is_obsolete: true

[Term]
id: PO:0009084
name: pericarp
namespace: plant_structure
def: "The wall of a fruit\, developed from the ovary or carpel wall." [APWeb:Glossary, GR:pj, TAIR:lr]
subset: Arabidopsis
subset: Citrus
subset: Maize
subset: Poaceae
subset: Rice
subset: Tomato
synonym: "fruit peel" []
synonym: "fruit rind" []
relationship: part_of PO:0009001 ! fruit

[Term]
id: PO:0009085
name: epicarp
alt_id: PO:0006046
alt_id: PO:0006217
namespace: plant_structure
def: "The outer layer of the fruit wall or pericarp." [GR:pj]
subset: Citrus
subset: Tomato
synonym: "ectocarp" []
synonym: "epicarp" []
synonym: "exocarp" []
synonym: "flavedo" []
synonym: "outer epidermis of pericarp" []
synonym: "pericarp epidermis" []
relationship: part_of PO:0009084 ! pericarp

[Term]
id: PO:0009086
name: endocarp
alt_id: PO:0006047
namespace: plant_structure
def: "The innermost differentiated layer of the fruit wall or pericarp." [GR:pj]
subset: Arabidopsis
subset: Citrus
subset: Maize
subset: Poaceae
subset: Rice
subset: Tomato
synonym: "endocarp" []
synonym: "flesh (sensu Citrus)" []
synonym: "inner epidermis of pericarp" []
synonym: "pulp (sensu Citrus)" []
relationship: part_of PO:0009084 ! pericarp

[Term]
id: PO:0009087
name: mesocarp
namespace: plant_structure
def: "Middle layer of the fruit wall or pericarp." [GR:pj]
subset: Citrus
subset: Tomato
synonym: "albedo" []
relationship: part_of PO:0009084 ! pericarp

[Term]
id: PO:0009088
name: seed coat
namespace: plant_structure
def: "Covering of seed derived from ovular - mainly integumentary - tissue." [APWeb:Glossary, TAIR:lr, GR:pj]
comment: Used only when not specified more precisely; see testa\, tegmen.
relationship: part_of PO:0009010 ! seed

[Term]
id: PO:0009089
name: endosperm
namespace: plant_structure
def: "Nutritive tissue in a seed\, in angiosperms usually triploid and formed after fertilization by the fusion of one gamete with the polar nucleus\, sometimes diploid or polyploid. " [GR:pj, APWeb:Glossary]
is_a: PO:0009007 ! tissue
relationship: part_of PO:0009010 ! seed

[Term]
id: PO:0009090
name: aril
namespace: plant_structure
def: "A structure associated with and often partly or wholly covering a seed and developed from the funicle or raphe." [APWeb:Glossary]
comment: Also used more generally to refer to a similar structure derived from any part of the ovule - there has been much and sometimes acrimonious debate over the correct definition of the term\, so when used the origin of the aril should generally be given for clarity.
subset: reference
relationship: develops_from PO:0020006 ! funicle
relationship: part_of PO:0009010 ! seed

[Term]
id: PO:0009091
name: mature dispersal unit
namespace: plant_structure
def: "OBSOLETE. provisional term" [Poc:curators]
is_obsolete: true

[Term]
id: PO:0019018
name: embryo axis
namespace: plant_structure
def: "Axial part of the young sporophyte comprising the hypocotyl\, and the root meristem\, or the radicle if one is present." [ISBN:0471245208]
synonym: "hypocotyl-root axis" []
relationship: part_of PO:0009009 ! embryo

[Term]
id: PO:0019022
name: arilloid
namespace: plant_structure
def: "An outgrowth from parts of the seed other than from the funiculus or raphe." [ISBN:0080280293]
relationship: part_of PO:0009010 ! seed

[Term]
id: PO:0019023
name: strophiole
namespace: plant_structure
def: "An outgrowth occurring on the raphe." [ISBN:0080280293]
subset: reference
is_a: PO:0019022 ! arilloid
relationship: part_of PO:0020027 ! raphe

[Term]
id: PO:0019024
name: seed operculum
namespace: plant_structure
def: "A plug-like structure formed in the micropylar region of the seed coat." [ISBN:0080280293]
relationship: part_of PO:0009010 ! seed

[Term]
id: PO:0019026
name: tracheid bar
namespace: plant_structure
def: "A distinct ring-like structure\, composed of tracheid cells\, which surrounds the hilum of some taxa e.g.\, Phaseolus\, and forms a groove in the surface of the pericarp (immediately adjacent to the hilum)." [ISBN:0080280293]
relationship: part_of PO:0009010 ! seed

[Term]
id: PO:0020001
name: ovary placenta
namespace: plant_structure
def: "A more or less localized region within an ovary to which ovules are attached." [APWeb:Glossary]
subset: reference
relationship: part_of PO:0009072 ! ovary

[Term]
id: PO:0020002
name: endothecium
namespace: plant_structure
def: "The hypodermis of an anther sac with distinctively thickened walls and involved in its dehiscence\, especially when this is by slits." [APWeb:Glossary]
subset: reference
synonym: "anther sac hypodermis" []
is_a: PO:0005051 ! hypodermis
relationship: develops_from PO:0006009 ! outer secondary parietal cell layer
relationship: part_of PO:0000002 ! anther wall

[Term]
id: PO:0020003
name: ovule
namespace: plant_structure
def: "A stalked or sessile structure in a seed plant within which one or more megaspores are formed and later the female gametophyte or embryo sac develops." [APWeb:Glossary]
subset: reference
relationship: part_of PO:0009072 ! ovary

[Term]
id: PO:0020004
name: exothecium
alt_id: PO:0006059
namespace: plant_structure
def: "The epidermis of an anther sac\, sometimes with distinctively thickened walls and involved in its dehiscence\, usually only when this is poricidal." [APWeb:Glossary]
subset: reference
synonym: "anther epidermis" []
synonym: "anther sac epidermis" []
is_a: PO:0006035 ! shoot epidermis
relationship: part_of PO:0000002 ! anther wall

[Term]
id: PO:0020005
name: placentoid
namespace: plant_structure
def: "An inpushing of the anther wall." [APWeb:Glossary]
subset: reference
relationship: part_of PO:0000002 ! anther wall

[Term]
id: PO:0020006
name: funicle
namespace: plant_structure
def: "The stalk which attaches the ovule to the placenta." [APWeb:Glossary, GR:pj]
subset: reference
synonym: "funiculus" []
relationship: part_of PO:0009072 ! ovary

[Term]
id: PO:0020008
name: exine
namespace: plant_structure
def: "The outer layer of the pollen grain wall\, highly resistant to strong acids and bases\, and composed primarily of sporopollenin." [APWeb:Glossary]
subset: reference
relationship: part_of PO:0020059 ! pollen wall

[Term]
id: PO:0020009
name: ectexine
namespace: plant_structure
def: "The outer part of the exine\, which stains positively with basic fuchsin in optical microscopy and has higher electron density in conventionally prepared TEM sections." [APWeb:Glossary]
comment: Although the term endexine as originally defined (see APWeb) was more or less synonymous with nexine it no longer is because endexine is now invariably used in the sense of F?gri (see APWeb). Nexine and sexine are distinguished on purely morphological criteria\, whereas ectexine and endexine differ in their staining properties.
subset: reference
relationship: part_of PO:0020008 ! exine

[Term]
id: PO:0020010
name: endexine
namespace: plant_structure
def: "The inner part of the exine\, which stains." [APWeb:Glossary]
comment: Although the term endexine as originally defined (see APWeb) was more or less synonymous with nexine it no longer is because endexine is now invariably used in the sense of F?gri (see APWeb). Nexine and sexine are distinguished on purely morphological criteria\, whereas ectexine and endexine differ in their staining properties.
subset: reference
relationship: part_of PO:0020008 ! exine

[Term]
id: PO:0020011
name: nexine
namespace: plant_structure
def: "The inner\, non-sculptured part of the exine which lies below the sexine." [APWeb:Glossary]
comment: Although the term endexine as originally defined (see APWeb) was more or less synonymous with nexine it no longer is because endexine is now invariably used in the sense of F?gri (see APWeb). Nexine and sexine are distinguished on purely morphological criteria\, whereas ectexine and endexine differ in their staining properties.
subset: reference
relationship: part_of PO:0020008 ! exine

[Term]
id: PO:0020012
name: sexine
namespace: plant_structure
def: "The outer\, sculptured layer of the exine\, which lies above the nexine." [APWeb:Glossary]
comment: Although the term ectexine as originally defined (see APWeb) was more or less synonymous with sexine\, it no longer is because ectexine is now invariably used in the redefined sense (see APWeb). Unlike ectexine\, sexine does not include the foot layer. Sexine and nexine are distinguished on purely morphological criteria\, whereas ectexine and endexine differ in their staining properties. The two sets of terms are therefore suited for slightly different applications.  A system of sexine stratification in which sexine 1 is the innermost and sexine 5 is the outermost layer of the sexine. Comment\: Usually the sexine consists of 3 layers (sexine 1 = columellae; sexine 2 = tectum; sexine 3 = sculpture elements).
subset: reference
relationship: part_of PO:0020008 ! exine

[Term]
id: PO:0020013
name: tectum
namespace: plant_structure
def: "The layer of sexine\, which forms a roof over the columellae\, granules or other infratectal elements." [APWeb:Glossary]
subset: reference
synonym: "sexine 2" []
relationship: part_of PO:0020012 ! sexine

[Term]
id: PO:0020014
name: columella
namespace: plant_structure
def: "A rod-like element of the sexine/ectexine\, either supporting the tectum or a caput." [APWeb:Glossary]
subset: reference
synonym: "sexine 1" []
relationship: part_of PO:0020012 ! sexine

[Term]
id: PO:0020015
name: sculpture elements
namespace: plant_structure
def: "Third layer of sexine." [APWeb:Glossary]
subset: reference
synonym: "sexine 3" []
relationship: part_of PO:0020012 ! sexine

[Term]
id: PO:0020016
name: foot layer
namespace: plant_structure
def: "The inner layer of the ectexine." [APWeb:Glossary]
synonym: "nexine 1" []
relationship: part_of PO:0020009 ! ectexine

[Term]
id: PO:0020017
name: intine
namespace: plant_structure
def: "The innermost of the major layers of the pollen grain wall\, underlies the exine and borders the cytoplasm\, not acetolysis resistant and is therefore absent in conventionally prepared palynological material." [APWeb:Glossary]
subset: reference
relationship: part_of PO:0020059 ! pollen wall

[Term]
id: PO:0020018
name: germination pore
namespace: plant_structure
def: "Area through which the pollen imports the nutrition during its development\, at the time of pollen germination\, the pollen tube emerges through it." [GR:pj]
subset: reference
synonym: "pollen pore" []
relationship: part_of PO:0020059 ! pollen wall

[Term]
id: PO:0020019
name: megaspore
namespace: plant_structure
def: "The larger\, in general\, of the two kinds of spores produced after meiosis in the life cycle of a heterosporous plant\, and on germination giving rise to the female gametophyte (embryo sac)." [APWeb:Glossary]
is_a: PO:0009002 ! plant cell
relationship: develops_from PO:0000431 ! megasporocyte

[Term]
id: PO:0020020
name: nucellus
namespace: plant_structure
def: "Subepidermal tissue in the ovule surrounding the megasporocyte." [APWeb:Glossary]
subset: reference
synonym: "megasporangium" []
relationship: part_of PO:0020003 ! ovule

[Term]
id: PO:0020021
name: integument
namespace: plant_structure
def: "One of the layers of tissue that usually covers the ovule\, enveloping the nucellus and forming the micropyle at the apex." [APWeb:Glossary]
subset: reference
relationship: part_of PO:0020003 ! ovule

[Term]
id: PO:0020022
name: inner integument
namespace: plant_structure
def: "The innermost of the two layers of tissue that usually cover the ovule\, contiguous to the nucellus and usually contributing to the formation of the micropyle at the apex." [APWeb:Glossary]
is_a: PO:0020021 ! integument

[Term]
id: PO:0020023
name: outer integument
namespace: plant_structure
def: "One of the two layers of tissue that usually cover the ovule\, contiguous to the inner integument and usually involved in forming the micropyle at the apex." [APWeb:Glossary]
is_a: PO:0020021 ! integument

[Term]
id: PO:0020024
name: endothelium
namespace: plant_structure
def: "Cells of the inner epidermis of the inner (or only) integument of the ovule that are radially elongated and metabolically very active." [APWeb:Glossary]
relationship: part_of PO:0020022 ! inner integument

[Term]
id: PO:0020025
name: micropyle
namespace: plant_structure
def: "A small canal or opening through the integument(s) at the apex of an ovule." [APWeb:Glossary]
comment: In a mature seed the micropyle may remain visible as an occluded pore or may be obliterated. The micropyle originates as an opening in the integuments of an ovule through which the pollen tube usually enters the embryo sac.
subset: reference
relationship: part_of PO:0020003 ! ovule

[Term]
id: PO:0020026
name: chalaza
namespace: plant_structure
def: "Region in the ovule where the integuments and the nucellus join with the funiculus. " [ISBN:047124529]
comment: The chalaza is recognized as the region which initiates the two integuments at its flank.
subset: reference
relationship: part_of PO:0020003 ! ovule

[Term]
id: PO:0020027
name: raphe
namespace: plant_structure
def: "That part of the funiculus that is adnate to the ovule." [APWeb:Glossary, ISBN:047124529]
comment: see antiraphe.
subset: reference
relationship: part_of PO:0020003 ! ovule
relationship: part_of PO:0020006 ! funicle

[Term]
id: PO:0020028
name: antiraphe
namespace: plant_structure
def: "The region on the other side of the ovule from the raphe." [APWeb:Glossary]
comment: see raphe.
subset: reference
relationship: part_of PO:0020003 ! ovule

[Term]
id: PO:0020029
name: obturator
namespace: plant_structure
def: "An outgrowth of the funicle\, that forms a bridge between the micropyle and other tissues." [APWeb:Glossary]
comment: Most commonly arising from the funicle\, also developing from placenta\, integument\, etc.
subset: reference
relationship: develops_from PO:0020006 ! funicle

[Term]
id: PO:0020030
name: cotyledon
namespace: plant_structure
def: "A leaf or leaves formed at the first node of a sporophyte." [APWeb:Glossary, GR:pj]
subset: reference
is_a: PO:0006001 ! phyllome
relationship: part_of PO:0009009 ! embryo

[Term]
id: PO:0020031
name: radicle
namespace: plant_structure
def: "The radicle is the basal continuation of the hypocotyl in an embryo and gives rise to the root system of the adult plant; sometimes more or less abortive." [APWeb:Glossary]
subset: reference
is_a: PO:0000045 ! embryonic root
relationship: part_of PO:0019018 ! embryo axis

[Term]
id: PO:0020032
name: plumule
namespace: plant_structure
def: "The somewhat differentiated terminal bud in several embryo types above the cotyledonary node\, in which one or more internodes and leaves or scales can be discerned in a primordial stage." [APWeb:Glossary]
synonym: "embryonic shoot" []
relationship: part_of PO:0009009 ! embryo

[Term]
id: PO:0020033
name: coleoptile
namespace: plant_structure
def: "A tubular structure developed at the junction of the cotyledonary sheath with the seedling axis\, and surrounding the plumule of a monocot embryo or seedling." [APWeb:Glossary]
is_a: PO:0009025 ! leaf
relationship: part_of PO:0009009 ! embryo

[Term]
id: PO:0020034
name: coleorhiza
namespace: plant_structure
def: "Tissue surrounding the radicle in the embryo or seedling of some monocots." [APWeb:Glossary]
relationship: part_of PO:0009009 ! embryo

[Term]
id: PO:0020035
name: epicotyl
namespace: plant_structure
def: "The first internode of the stem above the hypocotyl. In literature also used for the entire embryonic axis\, consisting of several internodes\, above the cotyledonary node. " [APWeb:Glossary]
relationship: part_of PO:0009009 ! embryo

[Term]
id: PO:0020036
name: epiblast
namespace: plant_structure
def: "A flap of tissue in an embryo or seedling arising opposite to the insertion of the cotyledon/scutellum." [APWeb:Glossary]
relationship: part_of PO:0009009 ! embryo

[Term]
id: PO:0020037
name: mesocotyl
namespace: plant_structure
def: "The internode between the cotyledon or cotyledons and the leaf or leaves at the next node of a young sporophyte." [APWeb:Glossary]
relationship: part_of PO:0009009 ! embryo

[Term]
id: PO:0020038
name: petiole
namespace: plant_structure
def: "The stalk of a leaf." [APWeb:Glossary, GR:pj]
relationship: part_of PO:0009025 ! leaf

[Term]
id: PO:0020039
name: leaf lamina
namespace: plant_structure
def: "The blade of a leaf\, usually dorsiventrally flattened\, and expanded." [APWeb:Glossary]
synonym: "leaf blade" []
relationship: part_of PO:0009025 ! leaf

[Term]
id: PO:0020040
name: leaf base
namespace: plant_structure
def: "The bottom part of a leaf where it attaches to the stem." [APWeb:Glossary]
synonym: "leaf sheath base" []
relationship: part_of PO:0009025 ! leaf

[Term]
id: PO:0020041
name: stipule
namespace: plant_structure
def: "One of (usually) a pair of appendages at the bases of leaves in many broad-leaved angiosperms." [APWeb:Glossary]
comment: The term not used for monocot leaves.
relationship: part_of PO:0009025 ! leaf

[Term]
id: PO:0020042
name: simple leaf
namespace: plant_structure
def: "A leaf in which the lamina is undivided." [Poc:curators]
is_a: PO:0009025 ! leaf

[Term]
id: PO:0020043
name: compound leaf
namespace: plant_structure
def: "A leaf having two or more distinct leaflets that are evident as such from early in development." [APWeb:Glossary]
is_a: PO:0009025 ! leaf

[Term]
id: PO:0020044
name: hyperphyll
namespace: plant_structure
def: "The unifacial terete apical portion of a monocot cotyledon\, sometimes also visible on other leaves." [APWeb:Glossary]
relationship: part_of PO:0020030 ! cotyledon

[Term]
id: PO:0020045
name: pinnate leaf
namespace: plant_structure
def: "A once-compound leaf with leaflets borne along a rachis." [APWeb:Glossary]
comment: The total number of leaflets may be even or odd\, in which case the leaf is called even-pinnate or odd-pinnate respectively.
is_a: PO:0020043 ! compound leaf

[Term]
id: PO:0020046
name: palmate leaf
namespace: plant_structure
def: "A once-compound leaf divided into several leaflets which arise at the same point\, there being no rachis." [APWeb:Glossary]
is_a: PO:0020043 ! compound leaf

[Term]
id: PO:0020047
name: microsporocyte
namespace: plant_structure
def: "A diploid (2n) cell that undergoes meiosis and produces four haploid (1n) microspores." [ISBN:0878934030]
subset: reference
synonym: "PMC" []
synonym: "microspore mother cell" []
synonym: "pollen mother cell" []
is_a: PO:0006204 ! sporocyte
relationship: develops_from PO:0006088 ! primary sporogenous cell
relationship: part_of PO:0009070 ! microsporangium

[Term]
id: PO:0020048
name: microspore
namespace: plant_structure
def: "The smaller\, in general\, of the two kinds of spores produced after meiosis in the life cycle of a heterosporous plant\, and on germination giving rise to the male gametophyte." [APWeb:Glossary]
subset: reference
is_a: PO:0009002 ! plant cell
relationship: develops_from PO:0000032 ! tetrad of microspores

[Term]
id: PO:0020049
name: leaflet
namespace: plant_structure
def: "One of the ultimate segments of a compound leaf." [APWeb:Glossary]
relationship: part_of PO:0020043 ! compound leaf

[Term]
id: PO:0020050
name: petiolule
namespace: plant_structure
def: "The stalk of a leaflet." [APWeb:Glossary]
relationship: part_of PO:0020049 ! leaflet

[Term]
id: PO:0020051
name: stipel
namespace: plant_structure
def: "Stipule-like appendage(s) at the base of a leaflet (in unifoliolate or simple leaves\, found at the top of the petiole)." [APWeb:Glossary]
relationship: part_of PO:0020049 ! leaflet

[Term]
id: PO:0020052
name: megaphyll
namespace: plant_structure
def: "OBSOLETE. Literally a large leaf\, a leaf of any size whose vascular supply leaves one or more gaps as it departs from the stem vascular tissue." [APWeb:Glossary]
is_obsolete: true

[Term]
id: PO:0020053
name: microphyll
namespace: plant_structure
def: "OBSOLETE. Literally a small leaf\, a leaf of any size in which any vascular trace supplying it does not interrupt the central vascular cylinder when it departs\, i.e. there are no leaf gaps." [APWeb:Glossary]
is_obsolete: true

[Term]
id: PO:0020054
name: bud scale
namespace: plant_structure
def: "A reduced leaf surrounding a dormant bud." [UMSL:tk]
is_a: PO:0006003 ! scale leaf

[Term]
id: PO:0020055
name: leaf rachis
namespace: plant_structure
def: "That part of the main axis of a pinnate or more highly compound leaf\, that bears leaflets or divisions of the axis." [APWeb:Glossary]
relationship: part_of PO:0020043 ! compound leaf

[Term]
id: PO:0020056
name: tegmen
namespace: plant_structure
def: "That part of the seed coat that develops from the inner integument." [APWeb:Glossary, ISBN:0080374913]
relationship: part_of PO:0009088 ! seed coat

[Term]
id: PO:0020057
name: testa
namespace: plant_structure
def: "That part of the seed coat that develops from the outer integument\, or from the single integument when there is only one." [APWeb:Glossary, ISBN:0080374913]
relationship: part_of PO:0009088 ! seed coat

[Term]
id: PO:0020058
name: perisperm
alt_id: PO:0006335
namespace: plant_structure
def: "Diploid nutritive tissue in an angiospermous seed derived from nucellar tissue." [APWeb:Glossary]
synonym: "seed nucellus" []
is_a: PO:0009007 ! tissue
relationship: part_of PO:0009010 ! seed

[Term]
id: PO:0020059
name: pollen wall
namespace: plant_structure
def: "Complex wall surrounding the micrsopore." [UMSL:fz]
subset: reference
relationship: part_of PO:0020091 ! male gametophyte

[Term]
id: PO:0020060
name: caruncle
namespace: plant_structure
def: "An outgrowth from the surface of a seed\, usually near the hilum or micropyle." [APWeb:Glossary]
is_a: PO:0019022 ! arilloid

[Term]
id: PO:0020061
name: coma
namespace: plant_structure
def: "A tuft of hairs at one end of a seed." [APWeb:Glossary]
synonym: "brush" []
relationship: part_of PO:0009010 ! seed

[Term]
id: PO:0020062
name: elaiosome
namespace: plant_structure
def: "An appendage of a seed\, usually rich in oil\, attractive to animals\, especially ants." [APWeb:Glossary]
is_a: PO:0019022 ! arilloid

[Term]
id: PO:0020063
name: hilum
namespace: plant_structure
def: "The scar on a seed at the place where it was attached to its funicle." [APWeb:Glossary]
relationship: part_of PO:0009010 ! seed

[Term]
id: PO:0020064
name: dehiscent fruit
namespace: plant_structure
def: "OBSOLETE. Fruit that breaks open at maturity to release the contents." [APWeb:Glossary]
is_obsolete: true

[Term]
id: PO:0020065
name: indehiscent fruit
namespace: plant_structure
def: "OBSOLETE. Fruit that does not open at maturity." [APWeb:Glossary]
is_obsolete: true

[Term]
id: PO:0020066
name: fleshy fruit
namespace: plant_structure
def: "OBSOLETE. The fruit may be derived from monocarpellate or multicarpellate gynoecia. Their walls may consist of the pericarp or of pericarp fused with extracarpellary tissue. The outer part of the fruit wall or the entire fruit wall may become fleshy by differentiating into soft\, succulent parenchyma. Parts other than the wall such as placentae and partitions in multilocular ovaries may become fleshy." [ISBN:047124529]
is_obsolete: true

[Term]
id: PO:0020075
name: mericarp
namespace: plant_structure
def: "OBSOLETE. One segment of a fruit of a schizocarp consisting of pericarp plus seed(s)." [APWeb:Glossary]
is_obsolete: true

[Term]
id: PO:0020081
name: seed as dispersal unit
namespace: plant_structure
def: "OBSOLETE." [Poc:curators]
is_obsolete: true

[Term]
id: PO:0020084
name: pyrene
namespace: plant_structure
def: "OBSOLETE. The 'stone' or 'pit' (endocarp plus seed) of a succulent fruit." [APWeb:Glossary]
is_obsolete: true

[Term]
id: PO:0020085
name: seed and fruit wall as dispersal unit
namespace: plant_structure
def: "OBSOLETE." [Poc:curators]
is_obsolete: true

[Term]
id: PO:0020086
name: multiple fruit
namespace: plant_structure
def: "OBSOLETE. Fruit on a common axis derived from the ovaries of several flowers." [APWeb:Glossary]
is_obsolete: true

[Term]
id: PO:0020090
name: central cell
namespace: plant_structure
def: "The largest cell of the mature embryo sac. Contains two polar nuclei\, which (after double fertilization) will develop into the endosperm." [TAIR:ki]
subset: reference
is_a: PO:0009002 ! plant cell
relationship: part_of PO:0020092 ! female gametophyte

[Term]
id: PO:0020091
name: male gametophyte
alt_id: PO:0020007
namespace: plant_structure
def: "A plant body or cell lineage formed by vegetative growth of the microspore\, producing male gametes." [APWeb:Glossary]
subset: reference
synonym: "microgametophyte" []
synonym: "pollen" []
synonym: "pollen grain" []
is_a: PO:0009004 ! gametophyte

[Term]
id: PO:0020092
name: female gametophyte
namespace: plant_structure
def: "Embryo sac in flowering plants." [APWeb:Glossary]
subset: reference
synonym: "embryo sac" []
synonym: "megagametophyte" []
is_a: PO:0009004 ! gametophyte

[Term]
id: PO:0020093
name: antipodal cell
namespace: plant_structure
def: "Cell\, commonly three in number as in the eight-nucleate embryo sac\, located at the other end of the embryo sac from the female gamete. " [APWeb:Glossary]
comment: More or less persistent\, multiplicative or not.
subset: reference
is_a: PO:0009002 ! plant cell
relationship: part_of PO:0020092 ! female gametophyte

[Term]
id: PO:0020094
name: egg cell
namespace: plant_structure
def: "A non motile cell at the apex of the embryo sac immediately adjacent to the micropyle and associated with the synergid cells." [APWeb:Glossary]
subset: reference
is_a: PO:0009002 ! plant cell
relationship: part_of PO:0020096 ! egg apparatus

[Term]
id: PO:0020095
name: polar nucleus
namespace: plant_structure
def: "OBSOLETE\: Usually two nuclei in the center of the eight-nucleate embryo sac that fuse\, and subsequently fuse with one of the male gametes to produce the endosperm." [APWeb:Glossary]
comment: Comment\: this term is available in the Cellular Component aspect of the Gene Ontology (GO\:0043078).
is_obsolete: true

[Term]
id: PO:0020096
name: egg apparatus
namespace: plant_structure
def: "The egg cell and two synergids located at the micropylar end of the female gametophyte\, or the embryo sac\, in angiosperms." [TAIR:lr]
subset: reference
relationship: part_of PO:0020092 ! female gametophyte

[Term]
id: PO:0020097
name: generative cell
namespace: plant_structure
def: "A cell of the male gametophyte of angiosperms that divides to produce two male gametes or sperm cells." [APWeb:Glossary]
subset: reference
is_a: PO:0009002 ! plant cell
relationship: part_of PO:0020091 ! male gametophyte

[Term]
id: PO:0020099
name: vegetative cell
namespace: plant_structure
def: "The larger cell of the male gametophyte of angiosperms that does not divide further." [APWeb:Glossary]
subset: reference
is_a: PO:0009002 ! plant cell
relationship: part_of PO:0020091 ! male gametophyte

[Term]
id: PO:0020100
name: hypocotyl
namespace: plant_structure
def: "The part of the stem below the cotyledonary node and transitional to a root\, found in a young sporophyte." [APWeb:Glossary]
relationship: part_of PO:0019018 ! embryo axis

[Term]
id: PO:0020101
name: stomium
namespace: plant_structure
def: "A fissure or pore in the anther lobe through which the pollen is released." [GR:pj]
subset: reference
relationship: part_of PO:0000002 ! anther wall

[Term]
id: PO:0020102
name: transmitting tissue
namespace: plant_structure
def: "Tissue in the style of a carpel through which the pollen tube grows; it connects the stigma and the inside of ovary." [GR:pj, ISBN:0080374913]
subset: reference
synonym: "transmitting tract" []
is_a: PO:0009007 ! tissue
relationship: part_of PO:0009074 ! style

[Term]
id: PO:0020103
name: flag leaf
namespace: plant_structure
def: "The last mature leaf before the inflorescence in a cereal crop plant." [GR:pj]
is_a: PO:0006340 ! adult leaf

[Term]
id: PO:0020104
name: leaf sheath
namespace: plant_structure
def: "Any tubular portion of the leaf surrounding the stem\, as in the Poaceae." [GR:pj]
relationship: part_of PO:0009025 ! leaf

[Term]
id: PO:0020105
name: ligule
namespace: plant_structure
def: "A membranous or hairy appendage on the adaxial/upper surface of a leaf\, at the junction between sheath and blade\, especially in grasses" [APWeb:Glossary]
relationship: part_of PO:0009025 ! leaf

[Term]
id: PO:0020106
name: auricle
namespace: plant_structure
def: "Outgrowth at the base of a leaf blade that may wrap around the stem." [GR:pj]
relationship: part_of PO:0009025 ! leaf

[Term]
id: PO:0020108
name: suspensor
namespace: plant_structure
def: "A nearly always single file of cells at the base of the embryo derived from the basal cell." [GR:pj]
comment: It anchors the embryo in the embryo sac and pushes it into the endosperm.
relationship: part_of PO:0009009 ! embryo

[Term]
id: PO:0020109
name: hypophysis
namespace: plant_structure
def: "The uppermost cell of the suspensor from which part of the root and root cap in the embryo of angiosperms are derived." [ISBN:047124529]
is_a: PO:0009002 ! plant cell
relationship: part_of PO:0020108 ! suspensor

[Term]
id: PO:0020110
name: scutellum
namespace: plant_structure
def: "A more or less shield-shaped and absorptive portion of an embryo of grasses\, probably a modified cotyledon." [APWeb:Glossary]
synonym: "haustorial cotyledon" []
relationship: part_of PO:0009009 ! embryo

[Term]
id: PO:0020121
name: lateral root
namespace: plant_structure
def: "Root developing from the pericycle layer of the primary root." [ISBN:0122151704]
is_a: PO:0009005 ! root

[Term]
id: PO:0020122
name: inflorescence axis
namespace: plant_structure
def: "The central supporting structure around which flowers are borne." [UMSL:fz]
comment: cob (sensu Zea) is different from the cob inflorescence found in Sorghum.
synonym: "first order inflorescence branch" []
synonym: "inflorescence rachis" []
relationship: part_of PO:0009049 ! inflorescence

[Term]
id: PO:0020123
name: root cap
namespace: plant_structure
def: "A group of cells that covers the apical meristem of the root." [APWeb:Glossary]
subset: reference
relationship: part_of PO:0009005 ! root

[Term]
id: PO:0020124
name: root stele
alt_id: PO:0003012
namespace: plant_structure
def: "The central column of primary vascular tissue in the root and any tissue that it surrounds." [APWeb:Glossary]
comment: Includes the pericycle as the outermost layer of the stele
subset: reference
synonym: "root vascular cylinder" []
relationship: part_of PO:0009005 ! root

[Term]
id: PO:0020125
name: elongation zone
namespace: plant_structure
def: "The portion of the root that includes small\, densely cytoplasmic cells that are dividing and expanding in size." [GR:pj]
subset: reference
synonym: "region of cell elongation" []
synonym: "region of radial enlargement" []
relationship: part_of PO:0009005 ! root

[Term]
id: PO:0020126
name: tassel
namespace: plant_structure
def: "The functionally-staminate flowering structure that terminates the stem of a Zea mays plant." [MaizeGDB:lv]
comment: Branched inflorescence with a central axis and about 10-50 lateral branches.
subset: Maize
subset: reference
is_a: PO:0009049 ! inflorescence

[Term]
id: PO:0020127
name: primary root
alt_id: PO:0020089
namespace: plant_structure
def: "The root which develops directly from the embryonic radicle." [ISBN:0122151704]
synonym: "tap root" []
is_a: PO:0009005 ! root
relationship: develops_from PO:0020031 ! radicle

[Term]
id: PO:0020128
name: leaf margin
namespace: plant_structure
def: "The margin or edge of the lamina." [UMSL:fz]
synonym: "leaf lamina margin" []
relationship: part_of PO:0020039 ! leaf lamina

[Term]
id: PO:0020130
name: central root cap
namespace: plant_structure
def: "The central part of a root cap in which the cells are arranged in longitudinal files." [GR:pj]
synonym: "columella cells" []
relationship: part_of PO:0020123 ! root cap

[Term]
id: PO:0020131
name: lateral root cap
namespace: plant_structure
def: "The part of the root cap that is parallel to the sides of the axis." [ISBN:0122151704]
synonym: "peripheral cells" []
relationship: part_of PO:0020123 ! root cap

[Term]
id: PO:0020132
name: columella root cap cell
namespace: plant_structure
def: "Cell that constitutes the central part of the root cap\, arranged in longitudinal files." [TAIR:ki, PMID:9384380]
is_a: PO:0009002 ! plant cell
relationship: develops_from PO:0020133 ! columella root cap initial

[Term]
id: PO:0020133
name: columella root cap initial
namespace: plant_structure
def: "Cell that produces columella cells in the root cap. In direct contact with quiescent center." [TAIR:ki, ISBN:0471245208]
synonym: "columella root cap stem cell" []
is_a: PO:0004011 ! initial cell

[Term]
id: PO:0020134
name: statolith
namespace: plant_structure
def: "OBSOLETE. Solid cell inclusion of starch containing plastids occurring in root cap cells." [GR:pj]
comment: This is sub-cellular term
is_obsolete: true

[Term]
id: PO:0020135
name: differentiation zone
alt_id: PO:0003002
namespace: plant_structure
def: "The portion of the root located behind the elongation zone containing cells that are differentiating into their final form and function." [GR:pj]
subset: reference
synonym: "maturation zone" []
synonym: "specialization zone" []
relationship: part_of PO:0009005 ! root

[Term]
id: PO:0020136
name: ear (sensu Zea)
namespace: plant_structure
def: "The distal part of a lateral (axillary) branch in Zea that bears the functionally-carpellate florets in a highly contracted inflorescence." [MaizeGDB:lv]
subset: Maize
subset: reference
is_a: PO:0009049 ! inflorescence

[Term]
id: PO:0020137
name: leaf apex
namespace: plant_structure
def: "The top part of the leaf\, usually the apex of the leaf blade." [UMSL:fz]
synonym: "leaf tip" []
relationship: part_of PO:0020039 ! leaf lamina

[Term]
id: PO:0020138
name: leaf vein
namespace: plant_structure
def: "A strand of vascular tissue in the leaf blade." [APWeb:Glossary]
relationship: part_of PO:0020039 ! leaf lamina

[Term]
id: PO:0020139
name: midvein
namespace: plant_structure
def: "The central\, and usually the most prominent\, vein of a leaf or leaf-like organ." [APWeb:Glossary]
synonym: "mid rib" []
is_a: PO:0020138 ! leaf vein

[Term]
id: PO:0020140
name: secondary vein
namespace: plant_structure
def: "Second order veins in the leaf blade." [GR:pj]
synonym: "veinlet" []
is_a: PO:0020138 ! leaf vein

[Term]
id: PO:0020141
name: stem node
namespace: plant_structure
def: "The level (transverse plane) of a stem at which one or more leaves and associated axillary bud(s) arise." [APWeb:Glossary]
is_a: PO:0005004 ! shoot node
relationship: part_of PO:0009047 ! stem

[Term]
id: PO:0020142
name: stem internode
namespace: plant_structure
def: "The portion of a stem between the level of insertion of two successive leaves\, leaf pairs or leaf whorls\, or branches of an inflorescence\, i.e. between two nodes." [APWeb:Glossary]
comment: see node.
is_a: PO:0005005 ! shoot internode
relationship: part_of PO:0009047 ! stem

[Term]
id: PO:0020144
name: apical meristem
namespace: plant_structure
def: "The meristems located at the apices of the main and lateral shoots and roots." [GR:pj]
synonym: "primary meristem" []
is_a: PO:0009013 ! meristem

[Term]
id: PO:0020145
name: lateral meristem
namespace: plant_structure
def: "Cells along the stem or root that first differentiate and function as members of a mature tissue system but then again take up meristematic activity." [APWeb:Glossary]
synonym: "secondary meristem" []
is_a: PO:0009013 ! meristem

[Term]
id: PO:0020147
name: root apical meristem
namespace: plant_structure
def: "Meristem at the root apex." [UMSL:fz, GR:pj]
comment: In most cases it is involved in root elongation.
synonym: "promeristem" []
is_a: PO:0006085 ! root meristem
is_a: PO:0020144 ! apical meristem

[Term]
id: PO:0020148
name: shoot apical meristem
namespace: plant_structure
def: "Meristem formed in the apex of the shoot\, including meristems originating as axillary shoot meristems." [UMSL:fz]
synonym: "apical meristem" []
synonym: "primary shoot meristem" []
is_a: PO:0006079 ! shoot meristem
is_a: PO:0020144 ! apical meristem
relationship: part_of PO:0000037 ! shoot apex

[Term]
id: PO:0020149
name: quiescent center
namespace: plant_structure
def: "Hemispherically shaped aggregation of mitotically and metabolically inactive cells positioned behind the root cap." [ISBN:0122151704]
relationship: part_of PO:0006085 ! root meristem

[Typedef]
id: develops_from
name: develops from

[Typedef]
id: part_of
name: part of

